<?xml version="1.0" encoding="UTF-8"?>
<rdf:RDF
   xmlns:owl="http://www.w3.org/2002/07/owl#"
   xmlns:rdf="http://www.w3.org/1999/02/22-rdf-syntax-ns#"
   xmlns:rdfs="http://www.w3.org/2000/01/rdf-schema#"
   xmlns:skos="http://www.w3.org/2004/02/skos/core#"
>
  <rdf:Description rdf:about="http://isdc.gfz-potsdam.de/ontology/SPASE-allowed_values.skos.owl#Technical_Contact">
    <rdf:type rdf:resource="http://www.w3.org/2004/02/skos/core#Concept"/>
    <rdf:type rdf:resource="http://www.w3.org/2002/07/owl#NamedIndividual"/>
    <skos:prefLabel xml:lang="en">Technical Contact</skos:prefLabel>
    <skos:inScheme rdf:resource="http://isdc.gfz-potsdam.de/ontology/SPASE-allowed_values.skos.owl#Role"/>
    <skos:topConceptOf rdf:resource="http://isdc.gfz-potsdam.de/ontology/SPASE-allowed_values.skos.owl#Role"/>
    <skos:definition xml:lang="en">An individual who can provide specific information with regard to the resource or supporting
software</skos:definition>
  </rdf:Description>
  <rdf:Description rdf:about="http://isdc.gfz-potsdam.de/ontology/SPASE-allowed_values.skos.owl#Magnetosonic_Mach_Number">
    <skos:topConceptOf rdf:resource="http://isdc.gfz-potsdam.de/ontology/SPASE-allowed_values.skos.owl#Mixed_Quantity"/>
    <rdf:type rdf:resource="http://www.w3.org/2002/07/owl#NamedIndividual"/>
    <rdf:type rdf:resource="http://www.w3.org/2004/02/skos/core#Concept"/>
    <skos:prefLabel xml:lang="en">Magnetosonic Mach Number</skos:prefLabel>
    <skos:inScheme rdf:resource="http://isdc.gfz-potsdam.de/ontology/SPASE-allowed_values.skos.owl#Mixed_Quantity"/>
    <skos:definition xml:lang="en">The ratio of the velocity of fast mode waves to the Alfven velocity.</skos:definition>
  </rdf:Description>
  <rdf:Description rdf:about="http://isdc.gfz-potsdam.de/ontology/SPASE-allowed_values.skos.owl#Average_Charge_State">
    <skos:inScheme rdf:resource="http://isdc.gfz-potsdam.de/ontology/SPASE-allowed_values.skos.owl#Particle_Quantity"/>
    <rdf:type rdf:resource="http://www.w3.org/2002/07/owl#NamedIndividual"/>
    <rdf:type rdf:resource="http://www.w3.org/2004/02/skos/core#Concept"/>
    <skos:topConceptOf rdf:resource="http://isdc.gfz-potsdam.de/ontology/SPASE-allowed_values.skos.owl#Particle_Quantity"/>
    <skos:definition xml:lang="en">A measure of the composite deficit (positive) or excess (negative) of electrons with respect to
protons.</skos:definition>
    <skos:prefLabel xml:lang="en">Average Charge State</skos:prefLabel>
  </rdf:Description>
  <rdf:Description rdf:about="http://isdc.gfz-potsdam.de/ontology/SPASE-allowed_values.skos.owl#Superhalo">
    <skos:definition xml:lang="en">The part of an object or distribution surrounding some central body or distribution evident in a
second break in the distribution function (e.g., a different power law). It consists of a
population at a higher energies than for a halo.</skos:definition>
    <skos:topConceptOf rdf:resource="http://isdc.gfz-potsdam.de/ontology/SPASE-allowed_values.skos.owl#Qualifier"/>
    <skos:inScheme rdf:resource="http://isdc.gfz-potsdam.de/ontology/SPASE-allowed_values.skos.owl#Qualifier"/>
    <skos:prefLabel xml:lang="en">Superhalo</skos:prefLabel>
    <rdf:type rdf:resource="http://www.w3.org/2002/07/owl#NamedIndividual"/>
    <rdf:type rdf:resource="http://www.w3.org/2004/02/skos/core#Concept"/>
  </rdf:Description>
  <rdf:Description rdf:about="http://isdc.gfz-potsdam.de/ontology/SPASE-allowed_values.skos.owl#Binary">
    <rdf:type rdf:resource="http://www.w3.org/2002/07/owl#NamedIndividual"/>
    <rdf:type rdf:resource="http://www.w3.org/2004/02/skos/core#Concept"/>
    <skos:definition xml:lang="en">A direct representation of the bits which may be stored in memory on a computer.</skos:definition>
    <skos:topConceptOf rdf:resource="http://isdc.gfz-potsdam.de/ontology/SPASE-allowed_values.skos.owl#Format"/>
    <skos:prefLabel xml:lang="en">Binary</skos:prefLabel>
    <skos:inScheme rdf:resource="http://isdc.gfz-potsdam.de/ontology/SPASE-allowed_values.skos.owl#Format"/>
  </rdf:Description>
  <rdf:Description rdf:about="http://isdc.gfz-potsdam.de/ontology/SPASE-allowed_values.skos.owl#Akasofu_Epsilon">
    <rdf:type rdf:resource="http://www.w3.org/2002/07/owl#NamedIndividual"/>
    <skos:prefLabel xml:lang="en">Akasofu Epsilon</skos:prefLabel>
    <skos:topConceptOf rdf:resource="http://isdc.gfz-potsdam.de/ontology/SPASE-allowed_values.skos.owl#Mixed_Quantity"/>
    <skos:inScheme rdf:resource="http://isdc.gfz-potsdam.de/ontology/SPASE-allowed_values.skos.owl#Mixed_Quantity"/>
    <skos:definition xml:lang="en">A measure of the magnetopause energy flux and an indicator of the solar wind power available
for subsequent magnetospheric energization. Defined as: V*B^2*l^2sin(theta/2)^4 where B is
the IMF, l is an empirical scaling parameter equal to 7 RE, and theta = tan(BY /BZ)^-1 the IMF
clock angle.</skos:definition>
    <rdf:type rdf:resource="http://www.w3.org/2004/02/skos/core#Concept"/>
  </rdf:Description>
  <rdf:Description rdf:about="http://isdc.gfz-potsdam.de/ontology/SPASE-allowed_values.skos.owl#White_Paper">
    <skos:prefLabel xml:lang="en">White Paper</skos:prefLabel>
    <rdf:type rdf:resource="http://www.w3.org/2004/02/skos/core#Concept"/>
    <rdf:type rdf:resource="http://www.w3.org/2002/07/owl#NamedIndividual"/>
    <skos:inScheme rdf:resource="http://isdc.gfz-potsdam.de/ontology/SPASE-allowed_values.skos.owl#Document_Type"/>
    <skos:topConceptOf rdf:resource="http://isdc.gfz-potsdam.de/ontology/SPASE-allowed_values.skos.owl#Document_Type"/>
    <skos:definition xml:lang="en">An authoritative report giving information or proposals on an issue.</skos:definition>
  </rdf:Description>
  <rdf:Description rdf:about="http://isdc.gfz-potsdam.de/ontology/SPASE-allowed_values.skos.owl#Atom">
    <skos:inScheme rdf:resource="http://isdc.gfz-potsdam.de/ontology/SPASE-allowed_values.skos.owl#Particle_Type"/>
    <skos:prefLabel xml:lang="en">Atom</skos:prefLabel>
    <rdf:type rdf:resource="http://www.w3.org/2002/07/owl#NamedIndividual"/>
    <rdf:type rdf:resource="http://www.w3.org/2004/02/skos/core#Concept"/>
    <skos:topConceptOf rdf:resource="http://isdc.gfz-potsdam.de/ontology/SPASE-allowed_values.skos.owl#Particle_Type"/>
    <skos:definition xml:lang="en">Matter consisting of a nucleus surrounded by electrons which has no net charge.</skos:definition>
  </rdf:Description>
  <rdf:Description rdf:about="http://isdc.gfz-potsdam.de/ontology/SPASE-allowed_values.skos.owl#Linear">
    <skos:topConceptOf rdf:resource="http://isdc.gfz-potsdam.de/ontology/SPASE-allowed_values.skos.owl#Qualifier"/>
    <skos:definition xml:lang="en">Polarization where the E-field vector is confined to a given plane</skos:definition>
    <skos:inScheme rdf:resource="http://isdc.gfz-potsdam.de/ontology/SPASE-allowed_values.skos.owl#Qualifier"/>
    <skos:prefLabel xml:lang="en">Linear</skos:prefLabel>
    <rdf:type rdf:resource="http://www.w3.org/2002/07/owl#NamedIndividual"/>
    <rdf:type rdf:resource="http://www.w3.org/2004/02/skos/core#Concept"/>
  </rdf:Description>
  <rdf:Description rdf:about="http://isdc.gfz-potsdam.de/ontology/SPASE-allowed_values.skos.owl#Photometer">
    <skos:topConceptOf rdf:resource="http://isdc.gfz-potsdam.de/ontology/SPASE-allowed_values.skos.owl#Instrument_Type"/>
    <skos:definition xml:lang="en">An instrument which measures the strength of electromagnetic radiation within a spectral band
which can range from ultraviolet to infrared and includes the visible spectrum.</skos:definition>
    <rdf:type rdf:resource="http://www.w3.org/2004/02/skos/core#Concept"/>
    <rdf:type rdf:resource="http://www.w3.org/2002/07/owl#NamedIndividual"/>
    <skos:prefLabel xml:lang="en">Photometer</skos:prefLabel>
    <skos:inScheme rdf:resource="http://isdc.gfz-potsdam.de/ontology/SPASE-allowed_values.skos.owl#Instrument_Type"/>
  </rdf:Description>
  <rdf:Description rdf:about="http://isdc.gfz-potsdam.de/ontology/SPASE-allowed_values.skos.owl#Minimum">
    <skos:topConceptOf rdf:resource="http://isdc.gfz-potsdam.de/ontology/SPASE-allowed_values.skos.owl#Qualifier"/>
    <skos:inScheme rdf:resource="http://isdc.gfz-potsdam.de/ontology/SPASE-allowed_values.skos.owl#Qualifier"/>
    <rdf:type rdf:resource="http://www.w3.org/2002/07/owl#NamedIndividual"/>
    <rdf:type rdf:resource="http://www.w3.org/2004/02/skos/core#Concept"/>
    <skos:prefLabel xml:lang="en">Minimum</skos:prefLabel>
    <skos:definition xml:lang="en">The smallest value of a batch or sample or the lower bound of a probability distribution.</skos:definition>
  </rdf:Description>
  <rdf:Description rdf:about="http://isdc.gfz-potsdam.de/ontology/SPASE-allowed_values.skos.owl#Temporal">
    <rdf:type rdf:resource="http://www.w3.org/2004/02/skos/core#Concept"/>
    <skos:prefLabel xml:lang="en">Temporal</skos:prefLabel>
    <skos:definition xml:lang="en">Pertaining to time.</skos:definition>
    <skos:topConceptOf rdf:resource="http://isdc.gfz-potsdam.de/ontology/SPASE-allowed_values.skos.owl#Support_Quantity"/>
    <skos:inScheme rdf:resource="http://isdc.gfz-potsdam.de/ontology/SPASE-allowed_values.skos.owl#Support_Quantity"/>
    <rdf:type rdf:resource="http://www.w3.org/2002/07/owl#NamedIndividual"/>
  </rdf:Description>
  <rdf:Description rdf:about="http://isdc.gfz-potsdam.de/ontology/SPASE-allowed_values.skos.owl#CEF_2">
    <skos:topConceptOf rdf:resource="http://isdc.gfz-potsdam.de/ontology/SPASE-allowed_values.skos.owl#Format"/>
    <skos:prefLabel xml:lang="en">CEF 2</skos:prefLabel>
    <rdf:type rdf:resource="http://www.w3.org/2002/07/owl#NamedIndividual"/>
    <skos:inScheme rdf:resource="http://isdc.gfz-potsdam.de/ontology/SPASE-allowed_values.skos.owl#Format"/>
    <rdf:type rdf:resource="http://www.w3.org/2004/02/skos/core#Concept"/>
    <skos:definition xml:lang="en">Cluster Exchange Format (CEF), version 2, is a self-documenting ASCII format designed for
the exchange of data and introduced for Cluster Active Archive. Compared to version 1, the
metadata description of vectors and tensors is different.</skos:definition>
  </rdf:Description>
  <rdf:Description rdf:about="http://isdc.gfz-potsdam.de/ontology/SPASE-allowed_values.skos.owl#Bandwidth">
    <skos:definition xml:lang="en">Integration over the width a frequency band.</skos:definition>
    <skos:broader rdf:resource="http://isdc.gfz-potsdam.de/ontology/SPASE-allowed_values.skos.owl#Integral"/>
    <skos:inScheme rdf:resource="http://isdc.gfz-potsdam.de/ontology/SPASE-allowed_values.skos.owl#Qualifier"/>
    <rdf:type rdf:resource="http://www.w3.org/2002/07/owl#NamedIndividual"/>
    <rdf:type rdf:resource="http://www.w3.org/2004/02/skos/core#Concept"/>
    <skos:prefLabel xml:lang="en">Bandwidth</skos:prefLabel>
  </rdf:Description>
  <rdf:Description rdf:about="http://isdc.gfz-potsdam.de/ontology/SPASE-allowed_values.skos.owl#Principal_Investigator">
    <skos:inScheme rdf:resource="http://isdc.gfz-potsdam.de/ontology/SPASE-allowed_values.skos.owl#Role"/>
    <skos:prefLabel xml:lang="en">Principal Investigator</skos:prefLabel>
    <skos:topConceptOf rdf:resource="http://isdc.gfz-potsdam.de/ontology/SPASE-allowed_values.skos.owl#Role"/>
    <rdf:type rdf:resource="http://www.w3.org/2002/07/owl#NamedIndividual"/>
    <rdf:type rdf:resource="http://www.w3.org/2004/02/skos/core#Concept"/>
    <skos:definition xml:lang="en">An individual who is the administrative and scientific lead for an investigation.</skos:definition>
  </rdf:Description>
  <rdf:Description rdf:about="http://isdc.gfz-potsdam.de/ontology/SPASE-allowed_values.skos.owl#Flow_Velocity">
    <skos:inScheme rdf:resource="http://isdc.gfz-potsdam.de/ontology/SPASE-allowed_values.skos.owl#Particle_Quantity"/>
    <rdf:type rdf:resource="http://www.w3.org/2002/07/owl#NamedIndividual"/>
    <rdf:type rdf:resource="http://www.w3.org/2004/02/skos/core#Concept"/>
    <skos:prefLabel xml:lang="en">Flow Velocity</skos:prefLabel>
    <skos:definition xml:lang="en">The volume of matter passing through a unit area perpendicular to the direction of flow in a unit
of time.</skos:definition>
    <skos:topConceptOf rdf:resource="http://isdc.gfz-potsdam.de/ontology/SPASE-allowed_values.skos.owl#Particle_Quantity"/>
  </rdf:Description>
  <rdf:Description rdf:about="http://isdc.gfz-potsdam.de/ontology/SPASE-allowed_values.skos.owl#Team_Leader">
    <rdf:type rdf:resource="http://www.w3.org/2004/02/skos/core#Concept"/>
    <rdf:type rdf:resource="http://www.w3.org/2002/07/owl#NamedIndividual"/>
    <skos:definition xml:lang="en">An individual who is the designated leader of an investigation.</skos:definition>
    <skos:prefLabel xml:lang="en">Team Leader</skos:prefLabel>
    <skos:inScheme rdf:resource="http://isdc.gfz-potsdam.de/ontology/SPASE-allowed_values.skos.owl#Role"/>
    <skos:topConceptOf rdf:resource="http://isdc.gfz-potsdam.de/ontology/SPASE-allowed_values.skos.owl#Role"/>
  </rdf:Description>
  <rdf:Description rdf:about="http://isdc.gfz-potsdam.de/ontology/SPASE-allowed_values.skos.owl#Ion_Chamber">
    <skos:prefLabel xml:lang="en">Ion Chamber</skos:prefLabel>
    <skos:definition xml:lang="en">A device in which the collected electrical charge from ionization in a gas-filled cavity is taken
to be the proportion to some parameter (e.g. dose or exposure) of radiation field.</skos:definition>
    <skos:topConceptOf rdf:resource="http://isdc.gfz-potsdam.de/ontology/SPASE-allowed_values.skos.owl#Instrument_Type"/>
    <skos:inScheme rdf:resource="http://isdc.gfz-potsdam.de/ontology/SPASE-allowed_values.skos.owl#Instrument_Type"/>
    <rdf:type rdf:resource="http://www.w3.org/2002/07/owl#NamedIndividual"/>
    <rdf:type rdf:resource="http://www.w3.org/2004/02/skos/core#Concept"/>
  </rdf:Description>
  <rdf:Description rdf:about="http://isdc.gfz-potsdam.de/ontology/SPASE-allowed_values.skos.owl#Energy">
    <skos:inScheme rdf:resource="http://isdc.gfz-potsdam.de/ontology/SPASE-allowed_values.skos.owl#Particle_Quantity"/>
    <skos:definition xml:lang="en">The capacity for doing work as measured by the capability of doing work (potential energy) or
the conversion of this capability to motion (kinetic energy)</skos:definition>
    <skos:prefLabel xml:lang="en">Energy</skos:prefLabel>
    <skos:topConceptOf rdf:resource="http://isdc.gfz-potsdam.de/ontology/SPASE-allowed_values.skos.owl#Particle_Quantity"/>
    <rdf:type rdf:resource="http://www.w3.org/2004/02/skos/core#Concept"/>
    <rdf:type rdf:resource="http://www.w3.org/2002/07/owl#NamedIndividual"/>
  </rdf:Description>
  <rdf:Description rdf:about="http://isdc.gfz-potsdam.de/ontology/SPASE-allowed_values.skos.owl#Neutral_Particle_Detector">
    <skos:inScheme rdf:resource="http://isdc.gfz-potsdam.de/ontology/SPASE-allowed_values.skos.owl#Instrument_Type"/>
    <rdf:type rdf:resource="http://www.w3.org/2002/07/owl#NamedIndividual"/>
    <rdf:type rdf:resource="http://www.w3.org/2004/02/skos/core#Concept"/>
    <skos:prefLabel xml:lang="en">Neutral Particle Detector</skos:prefLabel>
    <skos:topConceptOf rdf:resource="http://isdc.gfz-potsdam.de/ontology/SPASE-allowed_values.skos.owl#Instrument_Type"/>
    <skos:definition xml:lang="en">An instrument which measures the quantity and properties of neutral particles. Measured
properties can include mass and plasma bulk densities.</skos:definition>
  </rdf:Description>
  <rdf:Description rdf:about="http://isdc.gfz-potsdam.de/ontology/SPASE-allowed_values.skos.owl#K-7699">
    <skos:prefLabel xml:lang="en">K-7699</skos:prefLabel>
    <rdf:type rdf:resource="http://www.w3.org/2004/02/skos/core#Concept"/>
    <rdf:type rdf:resource="http://www.w3.org/2002/07/owl#NamedIndividual"/>
    <skos:topConceptOf rdf:resource="http://isdc.gfz-potsdam.de/ontology/SPASE-allowed_values.skos.owl#Spectral_Range"/>
    <skos:inScheme rdf:resource="http://isdc.gfz-potsdam.de/ontology/SPASE-allowed_values.skos.owl#Spectral_Range"/>
    <skos:definition xml:lang="en">A spectrum with a wavelength range centred at 769.9 nm. VSO nickname: K-7699 dopplergram
with a range of 769.8 nm to 770.0 nm.</skos:definition>
  </rdf:Description>
  <rdf:Description rdf:about="http://isdc.gfz-potsdam.de/ontology/SPASE-allowed_values.skos.owl#Temperature">
    <skos:definition xml:lang="en">A measure of the kinetic energy of random motion with respect to the average. Temperature is
properly defined only for an equilibrium particle distribution (Maxwellian distribution).</skos:definition>
    <skos:topConceptOf rdf:resource="http://isdc.gfz-potsdam.de/ontology/SPASE-allowed_values.skos.owl#Particle_Quantity"/>
    <skos:prefLabel xml:lang="en">Temperature</skos:prefLabel>
    <skos:inScheme rdf:resource="http://isdc.gfz-potsdam.de/ontology/SPASE-allowed_values.skos.owl#Particle_Quantity"/>
    <rdf:type rdf:resource="http://www.w3.org/2002/07/owl#NamedIndividual"/>
    <rdf:type rdf:resource="http://www.w3.org/2004/02/skos/core#Concept"/>
  </rdf:Description>
  <rdf:Description rdf:about="http://isdc.gfz-potsdam.de/ontology/SPASE-allowed_values.skos.owl#Standard_Deviation">
    <skos:inScheme rdf:resource="http://isdc.gfz-potsdam.de/ontology/SPASE-allowed_values.skos.owl#Qualifier"/>
    <skos:prefLabel xml:lang="en">Standard Deviation</skos:prefLabel>
    <rdf:type rdf:resource="http://www.w3.org/2004/02/skos/core#Concept"/>
    <skos:definition xml:lang="en">The square root of the average of the squares of deviations about the mean of a set of data.
Standard deviation is a statistical measure of spread or variability.</skos:definition>
    <skos:topConceptOf rdf:resource="http://isdc.gfz-potsdam.de/ontology/SPASE-allowed_values.skos.owl#Qualifier"/>
    <rdf:type rdf:resource="http://www.w3.org/2002/07/owl#NamedIndividual"/>
  </rdf:Description>
  <rdf:Description rdf:about="http://isdc.gfz-potsdam.de/ontology/SPASE-allowed_values.skos.owl#Microfiche">
    <skos:broader rdf:resource="http://isdc.gfz-potsdam.de/ontology/SPASE-allowed_values.skos.owl#Hardcopy"/>
    <skos:prefLabel xml:lang="en">Microfiche</skos:prefLabel>
    <rdf:type rdf:resource="http://www.w3.org/2002/07/owl#NamedIndividual"/>
    <rdf:type rdf:resource="http://www.w3.org/2004/02/skos/core#Concept"/>
    <skos:definition xml:lang="en">A sheet of microfilm on which many pages of material have been photographed; a
magnification system is used to read the material.</skos:definition>
    <skos:inScheme rdf:resource="http://isdc.gfz-potsdam.de/ontology/SPASE-allowed_values.skos.owl#Format"/>
  </rdf:Description>
  <rdf:Description rdf:about="http://isdc.gfz-potsdam.de/ontology/SPASE-allowed_values.skos.owl#Spectral_Power_Receiver">
    <skos:topConceptOf rdf:resource="http://isdc.gfz-potsdam.de/ontology/SPASE-allowed_values.skos.owl#Instrument_Type"/>
    <skos:definition xml:lang="en">A radio receiver which determines the power spectral density of the electric or magnetic field,
or both, at one or more frequencies.</skos:definition>
    <skos:inScheme rdf:resource="http://isdc.gfz-potsdam.de/ontology/SPASE-allowed_values.skos.owl#Instrument_Type"/>
    <skos:prefLabel xml:lang="en">Spectral Power Receiver</skos:prefLabel>
    <rdf:type rdf:resource="http://www.w3.org/2004/02/skos/core#Concept"/>
    <rdf:type rdf:resource="http://www.w3.org/2002/07/owl#NamedIndividual"/>
  </rdf:Description>
  <rdf:Description rdf:about="http://isdc.gfz-potsdam.de/ontology/SPASE-allowed_values.skos.owl#Data_Producer">
    <skos:definition xml:lang="en">An individual who generated the resource and is familiar with its provenance.</skos:definition>
    <rdf:type rdf:resource="http://www.w3.org/2002/07/owl#NamedIndividual"/>
    <rdf:type rdf:resource="http://www.w3.org/2004/02/skos/core#Concept"/>
    <skos:topConceptOf rdf:resource="http://isdc.gfz-potsdam.de/ontology/SPASE-allowed_values.skos.owl#Role"/>
    <skos:inScheme rdf:resource="http://isdc.gfz-potsdam.de/ontology/SPASE-allowed_values.skos.owl#Role"/>
    <skos:prefLabel xml:lang="en">Data Producer</skos:prefLabel>
  </rdf:Description>
  <rdf:Description rdf:about="http://isdc.gfz-potsdam.de/ontology/SPASE-allowed_values.skos.owl#VOTable">
    <skos:inScheme rdf:resource="http://isdc.gfz-potsdam.de/ontology/SPASE-allowed_values.skos.owl#Format"/>
    <rdf:type rdf:resource="http://www.w3.org/2002/07/owl#NamedIndividual"/>
    <rdf:type rdf:resource="http://www.w3.org/2004/02/skos/core#Concept"/>
    <skos:topConceptOf rdf:resource="http://isdc.gfz-potsdam.de/ontology/SPASE-allowed_values.skos.owl#Format"/>
    <skos:prefLabel xml:lang="en">VOTable</skos:prefLabel>
    <skos:definition xml:lang="en">A proposed IVOA standard designed as a flexible storage and exchange format for tabular data.</skos:definition>
  </rdf:Description>
  <rdf:Description rdf:about="http://isdc.gfz-potsdam.de/ontology/SPASE-allowed_values.skos.owl#Sun">
    <rdf:type rdf:resource="http://www.w3.org/2004/02/skos/core#Concept"/>
    <skos:narrower rdf:resource="http://isdc.gfz-potsdam.de/ontology/SPASE-allowed_values.skos.owl#Transition_Region"/>
    <skos:inScheme rdf:resource="http://isdc.gfz-potsdam.de/ontology/SPASE-allowed_values.skos.owl#Observatory_Region"/>
    <rdf:type rdf:resource="http://www.w3.org/2002/07/owl#NamedIndividual"/>
    <skos:narrower rdf:resource="http://isdc.gfz-potsdam.de/ontology/SPASE-allowed_values.skos.owl#Chromosphere"/>
    <skos:topConceptOf rdf:resource="http://isdc.gfz-potsdam.de/ontology/SPASE-allowed_values.skos.owl#Observatory_Region"/>
    <skos:definition xml:lang="en">The star upon which our solar system is centered.
Allowed Values:
Chromosphere
Corona
Interior
Photosphere
Transition Region</skos:definition>
    <skos:narrower rdf:resource="http://isdc.gfz-potsdam.de/ontology/SPASE-allowed_values.skos.owl#Corona"/>
    <skos:inScheme rdf:resource="http://isdc.gfz-potsdam.de/ontology/SPASE-allowed_values.skos.owl#Observed_Region"/>
    <skos:prefLabel xml:lang="en">Sun</skos:prefLabel>
    <skos:narrower rdf:resource="http://isdc.gfz-potsdam.de/ontology/SPASE-allowed_values.skos.owl#Photosphere"/>
    <skos:narrower rdf:resource="http://isdc.gfz-potsdam.de/ontology/SPASE-allowed_values.skos.owl#Interior"/>
    <skos:topConceptOf rdf:resource="http://isdc.gfz-potsdam.de/ontology/SPASE-allowed_values.skos.owl#Observed_Region"/>
  </rdf:Description>
  <rdf:Description rdf:about="http://isdc.gfz-potsdam.de/ontology/SPASE-allowed_values.skos.owl#Channeltron">
    <skos:definition xml:lang="en">An instrument that detects electrons, ions, and UV-radiation, according to the principle of a
secondary emission multiplier. It is typically used in electron spectroscopy and mass
spectrometry.</skos:definition>
    <rdf:type rdf:resource="http://www.w3.org/2002/07/owl#NamedIndividual"/>
    <skos:topConceptOf rdf:resource="http://isdc.gfz-potsdam.de/ontology/SPASE-allowed_values.skos.owl#Instrument_Type"/>
    <skos:inScheme rdf:resource="http://isdc.gfz-potsdam.de/ontology/SPASE-allowed_values.skos.owl#Instrument_Type"/>
    <skos:prefLabel xml:lang="en">Channeltron</skos:prefLabel>
    <rdf:type rdf:resource="http://www.w3.org/2004/02/skos/core#Concept"/>
  </rdf:Description>
  <rdf:Description rdf:about="http://isdc.gfz-potsdam.de/ontology/SPASE-allowed_values.skos.owl#Energetic_Solar_Particle_Event">
    <rdf:type rdf:resource="http://www.w3.org/2004/02/skos/core#Concept"/>
    <skos:prefLabel xml:lang="en">Energetic Solar Particle Event</skos:prefLabel>
    <rdf:type rdf:resource="http://www.w3.org/2002/07/owl#NamedIndividual"/>
    <skos:inScheme rdf:resource="http://isdc.gfz-potsdam.de/ontology/SPASE-allowed_values.skos.owl#Phenomenon_Type"/>
    <skos:definition xml:lang="en">An enhancement of interplanetary fluxes of energetic ions accelerated by interplanetary shocks
and/or solar flares.</skos:definition>
    <skos:topConceptOf rdf:resource="http://isdc.gfz-potsdam.de/ontology/SPASE-allowed_values.skos.owl#Phenomenon_Type"/>
  </rdf:Description>
  <rdf:Description rdf:about="http://isdc.gfz-potsdam.de/ontology/SPASE-allowed_values.skos.owl#Electric_Field">
    <skos:topConceptOf rdf:resource="http://isdc.gfz-potsdam.de/ontology/SPASE-allowed_values.skos.owl#Measurement_Type"/>
    <rdf:type rdf:resource="http://www.w3.org/2002/07/owl#NamedIndividual"/>
    <rdf:type rdf:resource="http://www.w3.org/2004/02/skos/core#Concept"/>
    <skos:definition xml:lang="en">A region of space around a charged particle, or between two voltages within which a force is
exerted on charged objects in its vicinity. An electric field is the electric force per unit charge.</skos:definition>
    <skos:prefLabel xml:lang="en">Electric Field</skos:prefLabel>
    <skos:inScheme rdf:resource="http://isdc.gfz-potsdam.de/ontology/SPASE-allowed_values.skos.owl#Measurement_Type"/>
  </rdf:Description>
  <rdf:Description rdf:about="http://isdc.gfz-potsdam.de/ontology/SPASE-allowed_values.skos.owl#NetCDF">
    <rdf:type rdf:resource="http://www.w3.org/2002/07/owl#NamedIndividual"/>
    <skos:prefLabel xml:lang="en">NetCDF</skos:prefLabel>
    <skos:definition xml:lang="en">Unidata Program Center's Network Common Data Form (NetCDF). A self-describing portable
data format for array-oriented data access. See
&lt;http://my.unidata.ucar.edu/content/software/netcdf&gt;.</skos:definition>
    <rdf:type rdf:resource="http://www.w3.org/2004/02/skos/core#Concept"/>
    <skos:topConceptOf rdf:resource="http://isdc.gfz-potsdam.de/ontology/SPASE-allowed_values.skos.owl#Format"/>
    <skos:inScheme rdf:resource="http://isdc.gfz-potsdam.de/ontology/SPASE-allowed_values.skos.owl#Format"/>
  </rdf:Description>
  <rdf:Description rdf:about="http://isdc.gfz-potsdam.de/ontology/SPASE-allowed_values.skos.owl#Langmuir_Probe">
    <skos:topConceptOf rdf:resource="http://isdc.gfz-potsdam.de/ontology/SPASE-allowed_values.skos.owl#Instrument_Type"/>
    <skos:prefLabel xml:lang="en">Langmuir Probe</skos:prefLabel>
    <skos:definition xml:lang="en">A monopole antenna associated with an instrument. The instrument applies a potential to the
antenna which is swept to determine the voltage/current characteristic. This provides
information about the plasma surrounding the probe and spacecraft.</skos:definition>
    <skos:inScheme rdf:resource="http://isdc.gfz-potsdam.de/ontology/SPASE-allowed_values.skos.owl#Instrument_Type"/>
    <rdf:type rdf:resource="http://www.w3.org/2004/02/skos/core#Concept"/>
    <rdf:type rdf:resource="http://www.w3.org/2002/07/owl#NamedIndividual"/>
  </rdf:Description>
  <rdf:Description rdf:about="http://isdc.gfz-potsdam.de/ontology/SPASE-allowed_values.skos.owl#Heat_Flux">
    <rdf:type rdf:resource="http://www.w3.org/2004/02/skos/core#Concept"/>
    <skos:prefLabel xml:lang="en">Heat Flux</skos:prefLabel>
    <skos:topConceptOf rdf:resource="http://isdc.gfz-potsdam.de/ontology/SPASE-allowed_values.skos.owl#Particle_Quantity"/>
    <rdf:type rdf:resource="http://www.w3.org/2002/07/owl#NamedIndividual"/>
    <skos:inScheme rdf:resource="http://isdc.gfz-potsdam.de/ontology/SPASE-allowed_values.skos.owl#Particle_Quantity"/>
    <skos:definition xml:lang="en">Flow of thermal energy through a gas or plasma; typically computed as third moment of a
distribution function.</skos:definition>
  </rdf:Description>
  <rdf:Description rdf:about="http://isdc.gfz-potsdam.de/ontology/SPASE-allowed_values.skos.owl#Hardcopy">
    <skos:narrower rdf:resource="http://isdc.gfz-potsdam.de/ontology/SPASE-allowed_values.skos.owl#Photographic_Plate"/>
    <skos:narrower rdf:resource="http://isdc.gfz-potsdam.de/ontology/SPASE-allowed_values.skos.owl#Microfilm"/>
    <skos:narrower rdf:resource="http://isdc.gfz-potsdam.de/ontology/SPASE-allowed_values.skos.owl#Photograph"/>
    <skos:definition xml:lang="en">A permanent reproduction, or copy in the form of a physical object, of any media suitable for
direct use by a person.
Allowed Values:
Film
Microfiche
Microfilm
Photograph
Photographic Plate
Print</skos:definition>
    <skos:narrower rdf:resource="http://isdc.gfz-potsdam.de/ontology/SPASE-allowed_values.skos.owl#Film"/>
    <skos:narrower rdf:resource="http://isdc.gfz-potsdam.de/ontology/SPASE-allowed_values.skos.owl#Print"/>
    <skos:prefLabel xml:lang="en">Hardcopy</skos:prefLabel>
    <skos:inScheme rdf:resource="http://isdc.gfz-potsdam.de/ontology/SPASE-allowed_values.skos.owl#Format"/>
    <skos:narrower rdf:resource="http://isdc.gfz-potsdam.de/ontology/SPASE-allowed_values.skos.owl#Microfiche"/>
    <rdf:type rdf:resource="http://www.w3.org/2002/07/owl#NamedIndividual"/>
    <rdf:type rdf:resource="http://www.w3.org/2004/02/skos/core#Concept"/>
    <skos:topConceptOf rdf:resource="http://isdc.gfz-potsdam.de/ontology/SPASE-allowed_values.skos.owl#Format"/>
  </rdf:Description>
  <rdf:Description rdf:about="http://isdc.gfz-potsdam.de/ontology/SPASE-allowed_values.skos.owl#Dopplergram">
    <skos:definition xml:lang="en">A map or image depicting the spatial distribution of line-of-sight velocities of the observed
object.</skos:definition>
    <skos:prefLabel xml:lang="en">Dopplergram</skos:prefLabel>
    <rdf:type rdf:resource="http://www.w3.org/2002/07/owl#NamedIndividual"/>
    <rdf:type rdf:resource="http://www.w3.org/2004/02/skos/core#Concept"/>
    <skos:topConceptOf rdf:resource="http://isdc.gfz-potsdam.de/ontology/SPASE-allowed_values.skos.owl#Measurement_Type"/>
    <skos:inScheme rdf:resource="http://isdc.gfz-potsdam.de/ontology/SPASE-allowed_values.skos.owl#Measurement_Type"/>
  </rdf:Description>
  <rdf:Description rdf:about="http://isdc.gfz-potsdam.de/ontology/SPASE-allowed_values.skos.owl#Pluto">
    <skos:prefLabel xml:lang="en">Pluto</skos:prefLabel>
    <skos:topConceptOf rdf:resource="http://isdc.gfz-potsdam.de/ontology/SPASE-allowed_values.skos.owl#Observed_Region"/>
    <skos:inScheme rdf:resource="http://isdc.gfz-potsdam.de/ontology/SPASE-allowed_values.skos.owl#Observatory_Region"/>
    <rdf:type rdf:resource="http://www.w3.org/2004/02/skos/core#Concept"/>
    <rdf:type rdf:resource="http://www.w3.org/2002/07/owl#NamedIndividual"/>
    <skos:topConceptOf rdf:resource="http://isdc.gfz-potsdam.de/ontology/SPASE-allowed_values.skos.owl#Observatory_Region"/>
    <skos:definition xml:lang="en">The ninth (sub)planet from the sun in our solar system.</skos:definition>
    <skos:inScheme rdf:resource="http://isdc.gfz-potsdam.de/ontology/SPASE-allowed_values.skos.owl#Observed_Region"/>
  </rdf:Description>
  <rdf:Description rdf:about="http://isdc.gfz-potsdam.de/ontology/SPASE-allowed_values.skos.owl#HDF_5">
    <skos:topConceptOf rdf:resource="http://isdc.gfz-potsdam.de/ontology/SPASE-allowed_values.skos.owl#Format"/>
    <skos:prefLabel xml:lang="en">HDF 5</skos:prefLabel>
    <rdf:type rdf:resource="http://www.w3.org/2002/07/owl#NamedIndividual"/>
    <rdf:type rdf:resource="http://www.w3.org/2004/02/skos/core#Concept"/>
    <skos:inScheme rdf:resource="http://isdc.gfz-potsdam.de/ontology/SPASE-allowed_values.skos.owl#Format"/>
    <skos:definition xml:lang="en">Hierarchical Data Format, Version 5</skos:definition>
  </rdf:Description>
  <rdf:Description rdf:about="http://isdc.gfz-potsdam.de/ontology/SPASE-allowed_values.skos.owl#Strong">
    <rdf:type rdf:resource="http://www.w3.org/2004/02/skos/core#Concept"/>
    <rdf:type rdf:resource="http://www.w3.org/2002/07/owl#NamedIndividual"/>
    <skos:topConceptOf rdf:resource="http://isdc.gfz-potsdam.de/ontology/SPASE-allowed_values.skos.owl#Confidence_Rating"/>
    <skos:definition xml:lang="en">Highly likely given the available evidence. Considered in the range of 7-10 on a scale of 0-10.</skos:definition>
    <skos:inScheme rdf:resource="http://isdc.gfz-potsdam.de/ontology/SPASE-allowed_values.skos.owl#Confidence_Rating"/>
    <skos:prefLabel xml:lang="en">Strong</skos:prefLabel>
  </rdf:Description>
  <rdf:Description rdf:about="http://isdc.gfz-potsdam.de/ontology/SPASE-allowed_values.skos.owl#Uranus">
    <rdf:type rdf:resource="http://www.w3.org/2002/07/owl#NamedIndividual"/>
    <skos:definition xml:lang="en">The eighth planet from the sun in our solar system.</skos:definition>
    <skos:inScheme rdf:resource="http://isdc.gfz-potsdam.de/ontology/SPASE-allowed_values.skos.owl#Observatory_Region"/>
    <skos:topConceptOf rdf:resource="http://isdc.gfz-potsdam.de/ontology/SPASE-allowed_values.skos.owl#Observatory_Region"/>
    <skos:prefLabel xml:lang="en">Uranus</skos:prefLabel>
    <rdf:type rdf:resource="http://www.w3.org/2004/02/skos/core#Concept"/>
    <skos:inScheme rdf:resource="http://isdc.gfz-potsdam.de/ontology/SPASE-allowed_values.skos.owl#Observed_Region"/>
    <skos:topConceptOf rdf:resource="http://isdc.gfz-potsdam.de/ontology/SPASE-allowed_values.skos.owl#Observed_Region"/>
  </rdf:Description>
  <rdf:Description rdf:about="http://isdc.gfz-potsdam.de/ontology/SPASE-allowed_values.skos.owl#Spectrometer">
    <skos:prefLabel xml:lang="en">Spectrometer</skos:prefLabel>
    <skos:topConceptOf rdf:resource="http://isdc.gfz-potsdam.de/ontology/SPASE-allowed_values.skos.owl#Instrument_Type"/>
    <skos:definition xml:lang="en">An instrument that measures the component wavelengths of light (or other electromagnetic
radiation) by splitting the light up into its component wavelengths.</skos:definition>
    <skos:inScheme rdf:resource="http://isdc.gfz-potsdam.de/ontology/SPASE-allowed_values.skos.owl#Instrument_Type"/>
    <rdf:type rdf:resource="http://www.w3.org/2002/07/owl#NamedIndividual"/>
    <rdf:type rdf:resource="http://www.w3.org/2004/02/skos/core#Concept"/>
  </rdf:Description>
  <rdf:Description rdf:about="http://isdc.gfz-potsdam.de/ontology/SPASE-allowed_values.skos.owl#Active">
    <rdf:type rdf:resource="http://www.w3.org/2004/02/skos/core#Concept"/>
    <rdf:type rdf:resource="http://www.w3.org/2002/07/owl#NamedIndividual"/>
    <skos:definition xml:lang="en">Exerting an influence or producing a change or effect. An active measurement is one which
produces a transmission or excitation as a part of the measurement cycle.</skos:definition>
    <skos:inScheme rdf:resource="http://isdc.gfz-potsdam.de/ontology/SPASE-allowed_values.skos.owl#Measurement_Type"/>
    <skos:prefLabel xml:lang="en">Active</skos:prefLabel>
    <skos:broader rdf:resource="http://isdc.gfz-potsdam.de/ontology/SPASE-allowed_values.skos.owl#Waves"/>
  </rdf:Description>
  <rdf:Description rdf:about="http://isdc.gfz-potsdam.de/ontology/SPASE-allowed_values.skos.owl#Microwave">
    <skos:prefLabel xml:lang="en">Microwave</skos:prefLabel>
    <skos:inScheme rdf:resource="http://isdc.gfz-potsdam.de/ontology/SPASE-allowed_values.skos.owl#Spectral_Range"/>
    <rdf:type rdf:resource="http://www.w3.org/2002/07/owl#NamedIndividual"/>
    <rdf:type rdf:resource="http://www.w3.org/2004/02/skos/core#Concept"/>
    <skos:definition xml:lang="en">Photons with a wavelength range: 1.00x10^6 to 1.50x10^7 nm</skos:definition>
    <skos:topConceptOf rdf:resource="http://isdc.gfz-potsdam.de/ontology/SPASE-allowed_values.skos.owl#Spectral_Range"/>
  </rdf:Description>
  <rdf:Description rdf:about="http://isdc.gfz-potsdam.de/ontology/SPASE-allowed_values.skos.owl#Unlikely">
    <skos:definition xml:lang="en">Not likely given the available evidence. Considered in the range of 0 on a scale of 0-10.</skos:definition>
    <skos:topConceptOf rdf:resource="http://isdc.gfz-potsdam.de/ontology/SPASE-allowed_values.skos.owl#Confidence_Rating"/>
    <rdf:type rdf:resource="http://www.w3.org/2004/02/skos/core#Concept"/>
    <rdf:type rdf:resource="http://www.w3.org/2002/07/owl#NamedIndividual"/>
    <skos:prefLabel xml:lang="en">Unlikely</skos:prefLabel>
    <skos:inScheme rdf:resource="http://isdc.gfz-potsdam.de/ontology/SPASE-allowed_values.skos.owl#Confidence_Rating"/>
  </rdf:Description>
  <rdf:Description rdf:about="http://isdc.gfz-potsdam.de/ontology/SPASE-allowed_values.skos.owl#SHA256">
    <rdf:type rdf:resource="http://www.w3.org/2004/02/skos/core#Concept"/>
    <skos:inScheme rdf:resource="http://isdc.gfz-potsdam.de/ontology/SPASE-allowed_values.skos.owl#Hash_Function"/>
    <skos:topConceptOf rdf:resource="http://isdc.gfz-potsdam.de/ontology/SPASE-allowed_values.skos.owl#Hash_Function"/>
    <skos:prefLabel xml:lang="en">SHA256</skos:prefLabel>
    <skos:definition xml:lang="en">Secure Hash Algorithm (SHA), a 256-bit message digest algorithm developed by the NSA and
described in Federal Information Processing Standard (FIPS) publication 180-1.</skos:definition>
    <rdf:type rdf:resource="http://www.w3.org/2002/07/owl#NamedIndividual"/>
  </rdf:Description>
  <rdf:Description rdf:about="http://isdc.gfz-potsdam.de/ontology/SPASE-allowed_values.skos.owl#Inspection">
    <skos:prefLabel xml:lang="en">Inspection</skos:prefLabel>
    <rdf:type rdf:resource="http://www.w3.org/2004/02/skos/core#Concept"/>
    <rdf:type rdf:resource="http://www.w3.org/2002/07/owl#NamedIndividual"/>
    <skos:inScheme rdf:resource="http://isdc.gfz-potsdam.de/ontology/SPASE-allowed_values.skos.owl#Classification_Method"/>
    <skos:topConceptOf rdf:resource="http://isdc.gfz-potsdam.de/ontology/SPASE-allowed_values.skos.owl#Classification_Method"/>
    <skos:definition xml:lang="en">Determined by the analysis or assessment performed by a person.</skos:definition>
  </rdf:Description>
  <rdf:Description rdf:about="http://isdc.gfz-potsdam.de/ontology/SPASE-allowed_values.skos.owl#LBH_Band">
    <rdf:type rdf:resource="http://www.w3.org/2002/07/owl#NamedIndividual"/>
    <skos:inScheme rdf:resource="http://isdc.gfz-potsdam.de/ontology/SPASE-allowed_values.skos.owl#Spectral_Range"/>
    <skos:prefLabel xml:lang="en">LBH Band</skos:prefLabel>
    <rdf:type rdf:resource="http://www.w3.org/2004/02/skos/core#Concept"/>
    <skos:topConceptOf rdf:resource="http://isdc.gfz-potsdam.de/ontology/SPASE-allowed_values.skos.owl#Spectral_Range"/>
    <skos:definition xml:lang="en">Lyman-Birge-Hopfield band in the far ultraviolet range with wavelength range of 140nm to 170
nm.</skos:definition>
  </rdf:Description>
  <rdf:Description rdf:about="http://isdc.gfz-potsdam.de/ontology/SPASE-allowed_values.skos.owl#Near_Surface">
    <skos:narrower rdf:resource="http://isdc.gfz-potsdam.de/ontology/SPASE-allowed_values.skos.owl#Thermosphere"/>
    <skos:definition xml:lang="en">The gaseous and possibly ionized environment of a body extending from the surface to some
specified altitude. For the Earth, this altitude is 2000 km.
Allowed Values:
Atmosphere
Auroral Region
Equatorial Region
Ionosphere
Ionosphere.D-Region
Ionosphere.E-Region
Ionosphere.F-Region
Ionosphere.Topside
Mesosphere
Plasmasphere
Polar Cap
South Atlantic Anomaly Region
Stratosphere
Thermosphere
Troposphere</skos:definition>
    <skos:narrower rdf:resource="http://isdc.gfz-potsdam.de/ontology/SPASE-allowed_values.skos.owl#Atmosphere"/>
    <rdf:type rdf:resource="http://www.w3.org/2002/07/owl#NamedIndividual"/>
    <skos:narrower rdf:resource="http://isdc.gfz-potsdam.de/ontology/SPASE-allowed_values.skos.owl#Auroral_Region"/>
    <skos:narrower rdf:resource="http://isdc.gfz-potsdam.de/ontology/SPASE-allowed_values.skos.owl#Mesosphere"/>
    <skos:inScheme rdf:resource="http://isdc.gfz-potsdam.de/ontology/SPASE-allowed_values.skos.owl#Observed_Region"/>
    <rdf:type rdf:resource="http://www.w3.org/2004/02/skos/core#Concept"/>
    <skos:narrower rdf:resource="http://isdc.gfz-potsdam.de/ontology/SPASE-allowed_values.skos.owl#South_Atlantic_Anomaly_Region"/>
    <skos:narrower rdf:resource="http://isdc.gfz-potsdam.de/ontology/SPASE-allowed_values.skos.owl#Polar_Cap"/>
    <skos:narrower rdf:resource="http://isdc.gfz-potsdam.de/ontology/SPASE-allowed_values.skos.owl#Troposphere"/>
    <skos:inScheme rdf:resource="http://isdc.gfz-potsdam.de/ontology/SPASE-allowed_values.skos.owl#Observatory_Region"/>
    <skos:narrower rdf:resource="http://isdc.gfz-potsdam.de/ontology/SPASE-allowed_values.skos.owl#Equatorial_Region"/>
    <skos:narrower rdf:resource="http://isdc.gfz-potsdam.de/ontology/SPASE-allowed_values.skos.owl#Plasmasphere"/>
    <skos:narrower rdf:resource="http://isdc.gfz-potsdam.de/ontology/SPASE-allowed_values.skos.owl#Ionosphere"/>
    <skos:broader rdf:resource="http://isdc.gfz-potsdam.de/ontology/SPASE-allowed_values.skos.owl#Earth"/>
    <skos:prefLabel xml:lang="en">Near Surface</skos:prefLabel>
    <skos:narrower rdf:resource="http://isdc.gfz-potsdam.de/ontology/SPASE-allowed_values.skos.owl#Stratosphere"/>
  </rdf:Description>
  <rdf:Description rdf:about="http://isdc.gfz-potsdam.de/ontology/SPASE-allowed_values.skos.owl#Molecule">
    <rdf:type rdf:resource="http://www.w3.org/2002/07/owl#NamedIndividual"/>
    <skos:topConceptOf rdf:resource="http://isdc.gfz-potsdam.de/ontology/SPASE-allowed_values.skos.owl#Particle_Type"/>
    <skos:definition xml:lang="en">A group of atoms so united and combined by chemical affinity that they form a complete,
integrated whole, being the smallest portion of any particular compound that can exist in a free
state.</skos:definition>
    <skos:inScheme rdf:resource="http://isdc.gfz-potsdam.de/ontology/SPASE-allowed_values.skos.owl#Particle_Type"/>
    <skos:prefLabel xml:lang="en">Molecule</skos:prefLabel>
    <rdf:type rdf:resource="http://www.w3.org/2004/02/skos/core#Concept"/>
  </rdf:Description>
  <rdf:Description rdf:about="http://isdc.gfz-potsdam.de/ontology/SPASE-allowed_values.skos.owl#Wave_Type">
    <skos:hasTopConcept rdf:resource="http://isdc.gfz-potsdam.de/ontology/SPASE-allowed_values.skos.owl#Plasma_Waves"/>
    <skos:hasTopConcept rdf:resource="http://isdc.gfz-potsdam.de/ontology/SPASE-allowed_values.skos.owl#Hydrodynamic"/>
    <skos:hasTopConcept rdf:resource="http://isdc.gfz-potsdam.de/ontology/SPASE-allowed_values.skos.owl#MHD"/>
    <rdf:type rdf:resource="http://www.w3.org/2004/02/skos/core#ConceptScheme"/>
    <rdf:type rdf:resource="http://www.w3.org/2002/07/owl#NamedIndividual"/>
    <skos:hasTopConcept rdf:resource="http://isdc.gfz-potsdam.de/ontology/SPASE-allowed_values.skos.owl#Electromagnetic"/>
    <skos:prefLabel xml:lang="en">Wave Type</skos:prefLabel>
    <skos:hasTopConcept rdf:resource="http://isdc.gfz-potsdam.de/ontology/SPASE-allowed_values.skos.owl#Photon"/>
    <skos:hasTopConcept rdf:resource="http://isdc.gfz-potsdam.de/ontology/SPASE-allowed_values.skos.owl#Electrostatic"/>
    <skos:definition xml:lang="en">A characterization of the carrier or phenomenon of wave information observed by the
measurement.
Allowed Values:
Electromagnetic
Electrostatic
Hydrodynamic
MHD
Photon
Plasma Waves</skos:definition>
  </rdf:Description>
  <rdf:Description rdf:about="http://isdc.gfz-potsdam.de/ontology/SPASE-allowed_values.skos.owl#SR2">
    <rdf:type rdf:resource="http://www.w3.org/2002/07/owl#NamedIndividual"/>
    <rdf:type rdf:resource="http://www.w3.org/2004/02/skos/core#Concept"/>
    <skos:topConceptOf rdf:resource="http://isdc.gfz-potsdam.de/ontology/SPASE-allowed_values.skos.owl#Coordinate_System_Name"/>
    <skos:prefLabel xml:lang="en">SR2</skos:prefLabel>
    <skos:inScheme rdf:resource="http://isdc.gfz-potsdam.de/ontology/SPASE-allowed_values.skos.owl#Coordinate_System_Name"/>
    <skos:definition xml:lang="en">Spin Reference 2 - A special case of a Spacecraft (SC) coordinate system for a spinning
spacecraft. Z is parallel to the spacecraft spin vector. X is in the plane defined by Z and the
spacecraft-Sun line, positive sunward. See &lt;http://cdpp.cnes.fr/00428.pdf&gt;</skos:definition>
  </rdf:Description>
  <rdf:Description rdf:about="http://isdc.gfz-potsdam.de/ontology/SPASE-allowed_values.skos.owl#Document_Type">
    <skos:definition xml:lang="en">A characterization of the content, purpose, or style of the document.
Allowed Values:
Other
Poster
Presentation
Report
Specification
Technical Note
White Paper</skos:definition>
    <skos:prefLabel xml:lang="en">Document Type</skos:prefLabel>
    <skos:hasTopConcept rdf:resource="http://isdc.gfz-potsdam.de/ontology/SPASE-allowed_values.skos.owl#Report"/>
    <skos:hasTopConcept rdf:resource="http://isdc.gfz-potsdam.de/ontology/SPASE-allowed_values.skos.owl#SQ_Other"/>
    <skos:hasTopConcept rdf:resource="http://isdc.gfz-potsdam.de/ontology/SPASE-allowed_values.skos.owl#Technical_Note"/>
    <skos:hasTopConcept rdf:resource="http://isdc.gfz-potsdam.de/ontology/SPASE-allowed_values.skos.owl#Poster"/>
    <skos:hasTopConcept rdf:resource="http://isdc.gfz-potsdam.de/ontology/SPASE-allowed_values.skos.owl#Presentation"/>
    <rdf:type rdf:resource="http://www.w3.org/2004/02/skos/core#ConceptScheme"/>
    <skos:hasTopConcept rdf:resource="http://isdc.gfz-potsdam.de/ontology/SPASE-allowed_values.skos.owl#Specification"/>
    <rdf:type rdf:resource="http://www.w3.org/2002/07/owl#NamedIndividual"/>
    <skos:hasTopConcept rdf:resource="http://isdc.gfz-potsdam.de/ontology/SPASE-allowed_values.skos.owl#White_Paper"/>
  </rdf:Description>
  <rdf:Description rdf:about="http://isdc.gfz-potsdam.de/ontology/SPASE-allowed_values.skos.owl#JK">
    <skos:prefLabel xml:lang="en">JK</skos:prefLabel>
    <rdf:type rdf:resource="http://www.w3.org/2004/02/skos/core#Concept"/>
    <rdf:type rdf:resource="http://www.w3.org/2002/07/owl#NamedIndividual"/>
    <skos:inScheme rdf:resource="http://isdc.gfz-potsdam.de/ontology/SPASE-allowed_values.skos.owl#Qualifier"/>
    <skos:definition xml:lang="en">A measure of the length of a position or measured vector projected into the j-k (typically Y-Z)
plane of the coordinate system.</skos:definition>
    <skos:broader rdf:resource="http://isdc.gfz-potsdam.de/ontology/SPASE-allowed_values.skos.owl#Projection"/>
  </rdf:Description>
  <rdf:Description rdf:about="http://isdc.gfz-potsdam.de/ontology/SPASE-allowed_values.skos.owl#Multispectral_Imager">
    <skos:topConceptOf rdf:resource="http://isdc.gfz-potsdam.de/ontology/SPASE-allowed_values.skos.owl#Instrument_Type"/>
    <skos:prefLabel xml:lang="en">Multispectral Imager</skos:prefLabel>
    <skos:inScheme rdf:resource="http://isdc.gfz-potsdam.de/ontology/SPASE-allowed_values.skos.owl#Instrument_Type"/>
    <skos:definition xml:lang="en">An instrument which captures images at multiple spectral ranges.</skos:definition>
    <rdf:type rdf:resource="http://www.w3.org/2004/02/skos/core#Concept"/>
    <rdf:type rdf:resource="http://www.w3.org/2002/07/owl#NamedIndividual"/>
  </rdf:Description>
  <rdf:Description rdf:about="http://isdc.gfz-potsdam.de/ontology/SPASE-allowed_values.skos.owl#HTML">
    <skos:definition xml:lang="en">A text file containing structured information represented in the HyperText Mark-up Language
(HTML). See &lt;http://www.w3.org/MarkUp/&gt;.</skos:definition>
    <skos:topConceptOf rdf:resource="http://isdc.gfz-potsdam.de/ontology/SPASE-allowed_values.skos.owl#Format"/>
    <rdf:type rdf:resource="http://www.w3.org/2004/02/skos/core#Concept"/>
    <rdf:type rdf:resource="http://www.w3.org/2002/07/owl#NamedIndividual"/>
    <skos:prefLabel xml:lang="en">HTML</skos:prefLabel>
    <skos:inScheme rdf:resource="http://isdc.gfz-potsdam.de/ontology/SPASE-allowed_values.skos.owl#Format"/>
  </rdf:Description>
  <rdf:Description rdf:about="http://isdc.gfz-potsdam.de/ontology/SPASE-allowed_values.skos.owl#Source_Type">
    <skos:definition xml:lang="en">A characterization of the function or purpose of the source.
Allowed Values:
Ancillary
Browse
Data
Layout
Thumbnail</skos:definition>
    <skos:prefLabel xml:lang="en">Source Type</skos:prefLabel>
    <skos:hasTopConcept rdf:resource="http://isdc.gfz-potsdam.de/ontology/SPASE-allowed_values.skos.owl#Ancillary"/>
    <skos:hasTopConcept rdf:resource="http://isdc.gfz-potsdam.de/ontology/SPASE-allowed_values.skos.owl#Data"/>
    <skos:hasTopConcept rdf:resource="http://isdc.gfz-potsdam.de/ontology/SPASE-allowed_values.skos.owl#Browse"/>
    <skos:hasTopConcept rdf:resource="http://isdc.gfz-potsdam.de/ontology/SPASE-allowed_values.skos.owl#Thumbnail"/>
    <skos:hasTopConcept rdf:resource="http://isdc.gfz-potsdam.de/ontology/SPASE-allowed_values.skos.owl#Layout"/>
    <rdf:type rdf:resource="http://www.w3.org/2002/07/owl#NamedIndividual"/>
    <rdf:type rdf:resource="http://www.w3.org/2004/02/skos/core#ConceptScheme"/>
  </rdf:Description>
  <rdf:Description rdf:about="http://isdc.gfz-potsdam.de/ontology/SPASE-allowed_values.skos.owl#Poster">
    <rdf:type rdf:resource="http://www.w3.org/2002/07/owl#NamedIndividual"/>
    <skos:inScheme rdf:resource="http://isdc.gfz-potsdam.de/ontology/SPASE-allowed_values.skos.owl#Document_Type"/>
    <skos:definition xml:lang="en">A set of information arranged on a single page or sheet, typically in a large format.</skos:definition>
    <skos:topConceptOf rdf:resource="http://isdc.gfz-potsdam.de/ontology/SPASE-allowed_values.skos.owl#Document_Type"/>
    <skos:prefLabel xml:lang="en">Poster</skos:prefLabel>
    <rdf:type rdf:resource="http://www.w3.org/2004/02/skos/core#Concept"/>
  </rdf:Description>
  <rdf:Description rdf:about="http://isdc.gfz-potsdam.de/ontology/SPASE-allowed_values.skos.owl#Restricted">
    <skos:topConceptOf rdf:resource="http://isdc.gfz-potsdam.de/ontology/SPASE-allowed_values.skos.owl#Access_Rights"/>
    <skos:definition xml:lang="en">Access to the product is regulated and requires some form of identification.</skos:definition>
    <skos:inScheme rdf:resource="http://isdc.gfz-potsdam.de/ontology/SPASE-allowed_values.skos.owl#Access_Rights"/>
    <rdf:type rdf:resource="http://www.w3.org/2002/07/owl#NamedIndividual"/>
    <rdf:type rdf:resource="http://www.w3.org/2004/02/skos/core#Concept"/>
    <skos:prefLabel xml:lang="en">Restricted</skos:prefLabel>
  </rdf:Description>
  <rdf:Description rdf:about="http://isdc.gfz-potsdam.de/ontology/SPASE-allowed_values.skos.owl#Characteristic">
    <rdf:type rdf:resource="http://www.w3.org/2004/02/skos/core#Concept"/>
    <skos:definition xml:lang="en">A quantity which can be easily identified and measured in a given environment.</skos:definition>
    <skos:topConceptOf rdf:resource="http://isdc.gfz-potsdam.de/ontology/SPASE-allowed_values.skos.owl#Qualifier"/>
    <skos:prefLabel xml:lang="en">Characteristic</skos:prefLabel>
    <skos:inScheme rdf:resource="http://isdc.gfz-potsdam.de/ontology/SPASE-allowed_values.skos.owl#Qualifier"/>
    <rdf:type rdf:resource="http://www.w3.org/2002/07/owl#NamedIndividual"/>
  </rdf:Description>
  <rdf:Description rdf:about="http://isdc.gfz-potsdam.de/ontology/SPASE-allowed_values.skos.owl#Polar">
    <skos:prefLabel xml:lang="en">Polar</skos:prefLabel>
    <rdf:type rdf:resource="http://www.w3.org/2002/07/owl#NamedIndividual"/>
    <rdf:type rdf:resource="http://www.w3.org/2004/02/skos/core#Concept"/>
    <skos:inScheme rdf:resource="http://isdc.gfz-potsdam.de/ontology/SPASE-allowed_values.skos.owl#Observatory_Region"/>
    <skos:definition xml:lang="en">The region near the pole of a body. For a magnetosphere the polar region is the area where
magnetic field lines are open and includes the auroral zone.</skos:definition>
    <skos:broader rdf:resource="http://isdc.gfz-potsdam.de/ontology/SPASE-allowed_values.skos.owl#Magnetosphere"/>
    <skos:inScheme rdf:resource="http://isdc.gfz-potsdam.de/ontology/SPASE-allowed_values.skos.owl#Observed_Region"/>
  </rdf:Description>
  <rdf:Description rdf:about="http://isdc.gfz-potsdam.de/ontology/SPASE-allowed_values.skos.owl#Imaging_Spectrometer">
    <skos:topConceptOf rdf:resource="http://isdc.gfz-potsdam.de/ontology/SPASE-allowed_values.skos.owl#Instrument_Type"/>
    <skos:prefLabel xml:lang="en">Imaging Spectrometer</skos:prefLabel>
    <rdf:type rdf:resource="http://www.w3.org/2004/02/skos/core#Concept"/>
    <rdf:type rdf:resource="http://www.w3.org/2002/07/owl#NamedIndividual"/>
    <skos:inScheme rdf:resource="http://isdc.gfz-potsdam.de/ontology/SPASE-allowed_values.skos.owl#Instrument_Type"/>
    <skos:definition xml:lang="en">An instrument which is a multispectral scanner with a very large number of channels (64-256
channels) with very narrow band widths.</skos:definition>
  </rdf:Description>
  <rdf:Description rdf:about="http://isdc.gfz-potsdam.de/ontology/SPASE-allowed_values.skos.owl#Particle_Correlator">
    <skos:topConceptOf rdf:resource="http://isdc.gfz-potsdam.de/ontology/SPASE-allowed_values.skos.owl#Instrument_Type"/>
    <skos:prefLabel xml:lang="en">Particle Correlator</skos:prefLabel>
    <skos:inScheme rdf:resource="http://isdc.gfz-potsdam.de/ontology/SPASE-allowed_values.skos.owl#Instrument_Type"/>
    <rdf:type rdf:resource="http://www.w3.org/2002/07/owl#NamedIndividual"/>
    <rdf:type rdf:resource="http://www.w3.org/2004/02/skos/core#Concept"/>
    <skos:definition xml:lang="en">An instrument which correlates particle flux to help identify wave/particle interactions.</skos:definition>
  </rdf:Description>
  <rdf:Description rdf:about="http://isdc.gfz-potsdam.de/ontology/SPASE-allowed_values.skos.owl#GZIP">
    <rdf:type rdf:resource="http://www.w3.org/2002/07/owl#NamedIndividual"/>
    <skos:definition xml:lang="en">An open standard algorithm distributed by GHU based on LZ77 and Huffman coding. See
&lt;http://www.gnu.org/software/gzip/gzip.html&gt; or &lt;http://www.gzip.org/&gt;.</skos:definition>
    <skos:prefLabel xml:lang="en">GZIP</skos:prefLabel>
    <skos:topConceptOf rdf:resource="http://isdc.gfz-potsdam.de/ontology/SPASE-allowed_values.skos.owl#Encoding"/>
    <skos:inScheme rdf:resource="http://isdc.gfz-potsdam.de/ontology/SPASE-allowed_values.skos.owl#Encoding"/>
    <rdf:type rdf:resource="http://www.w3.org/2004/02/skos/core#Concept"/>
  </rdf:Description>
  <rdf:Description rdf:about="http://isdc.gfz-potsdam.de/ontology/SPASE-allowed_values.skos.owl#Integral">
    <skos:topConceptOf rdf:resource="http://isdc.gfz-potsdam.de/ontology/SPASE-allowed_values.skos.owl#Qualifier"/>
    <skos:definition xml:lang="en">A flux measurement in a broad range of energy and solid angle.
Allowed Values:
Area
Bandwidth
Solid Angle</skos:definition>
    <skos:prefLabel xml:lang="en">Integral</skos:prefLabel>
    <skos:inScheme rdf:resource="http://isdc.gfz-potsdam.de/ontology/SPASE-allowed_values.skos.owl#Qualifier"/>
    <skos:narrower rdf:resource="http://isdc.gfz-potsdam.de/ontology/SPASE-allowed_values.skos.owl#Bandwidth"/>
    <skos:narrower rdf:resource="http://isdc.gfz-potsdam.de/ontology/SPASE-allowed_values.skos.owl#Area"/>
    <skos:narrower rdf:resource="http://isdc.gfz-potsdam.de/ontology/SPASE-allowed_values.skos.owl#Solid_Angle"/>
    <rdf:type rdf:resource="http://www.w3.org/2004/02/skos/core#Concept"/>
    <rdf:type rdf:resource="http://www.w3.org/2002/07/owl#NamedIndividual"/>
  </rdf:Description>
  <rdf:Description rdf:about="http://isdc.gfz-potsdam.de/ontology/SPASE-allowed_values.skos.owl#Wave_Quantity">
    <skos:hasTopConcept rdf:resource="http://isdc.gfz-potsdam.de/ontology/SPASE-allowed_values.skos.owl#AC-Magnetic_Field"/>
    <rdf:type rdf:resource="http://www.w3.org/2004/02/skos/core#ConceptScheme"/>
    <skos:hasTopConcept rdf:resource="http://isdc.gfz-potsdam.de/ontology/SPASE-allowed_values.skos.owl#Gyrofrequency"/>
    <skos:hasTopConcept rdf:resource="http://isdc.gfz-potsdam.de/ontology/SPASE-allowed_values.skos.owl#Line_Depth"/>
    <skos:hasTopConcept rdf:resource="http://isdc.gfz-potsdam.de/ontology/SPASE-allowed_values.skos.owl#Plasma_Frequency"/>
    <skos:hasTopConcept rdf:resource="http://isdc.gfz-potsdam.de/ontology/SPASE-allowed_values.skos.owl#Absorption"/>
    <skos:hasTopConcept rdf:resource="http://isdc.gfz-potsdam.de/ontology/SPASE-allowed_values.skos.owl#Magnetic_Field"/>
    <skos:definition xml:lang="en">A characterization of the physical properties of a wave.
Allowed Values:
AC-Electric Field
AC-Magnetic Field
Absorption
Albedo
Doppler Frequency
Emissivity
Energy Flux
Equivalent Width
Frequency
Gyrofrequency
Intensity
Line Depth
Magnetic Field
Mode Amplitude
Plasma Frequency
Polarization
Poynting Flux
Propagation Time
Stoke's Parameters
Velocity
Wavelength</skos:definition>
    <skos:hasTopConcept rdf:resource="http://isdc.gfz-potsdam.de/ontology/SPASE-allowed_values.skos.owl#Frequency"/>
    <skos:hasTopConcept rdf:resource="http://isdc.gfz-potsdam.de/ontology/SPASE-allowed_values.skos.owl#Doppler_Frequency"/>
    <skos:hasTopConcept rdf:resource="http://isdc.gfz-potsdam.de/ontology/SPASE-allowed_values.skos.owl#Equivalent_Width"/>
    <skos:hasTopConcept rdf:resource="http://isdc.gfz-potsdam.de/ontology/SPASE-allowed_values.skos.owl#Energy_Flux"/>
    <skos:prefLabel xml:lang="en">Wave Quantity</skos:prefLabel>
    <skos:hasTopConcept rdf:resource="http://isdc.gfz-potsdam.de/ontology/SPASE-allowed_values.skos.owl#Mode_Amplitude"/>
    <skos:hasTopConcept rdf:resource="http://isdc.gfz-potsdam.de/ontology/SPASE-allowed_values.skos.owl#Albedo"/>
    <skos:hasTopConcept rdf:resource="http://isdc.gfz-potsdam.de/ontology/SPASE-allowed_values.skos.owl#Emissivity"/>
    <rdf:type rdf:resource="http://www.w3.org/2002/07/owl#NamedIndividual"/>
    <skos:hasTopConcept rdf:resource="http://isdc.gfz-potsdam.de/ontology/SPASE-allowed_values.skos.owl#Velocity"/>
    <skos:hasTopConcept rdf:resource="http://isdc.gfz-potsdam.de/ontology/SPASE-allowed_values.skos.owl#Propagation_Time"/>
    <skos:hasTopConcept rdf:resource="http://isdc.gfz-potsdam.de/ontology/SPASE-allowed_values.skos.owl#Stoke's_Parameters"/>
    <skos:hasTopConcept rdf:resource="http://isdc.gfz-potsdam.de/ontology/SPASE-allowed_values.skos.owl#Wavelength"/>
    <skos:hasTopConcept rdf:resource="http://isdc.gfz-potsdam.de/ontology/SPASE-allowed_values.skos.owl#AC-Electric_Field"/>
    <skos:hasTopConcept rdf:resource="http://isdc.gfz-potsdam.de/ontology/SPASE-allowed_values.skos.owl#Polarization"/>
    <skos:hasTopConcept rdf:resource="http://isdc.gfz-potsdam.de/ontology/SPASE-allowed_values.skos.owl#Intensity"/>
    <skos:hasTopConcept rdf:resource="http://isdc.gfz-potsdam.de/ontology/SPASE-allowed_values.skos.owl#Poynting_Flux"/>
  </rdf:Description>
  <rdf:Description rdf:about="http://isdc.gfz-potsdam.de/ontology/SPASE-allowed_values.skos.owl#Cylindrical">
    <skos:inScheme rdf:resource="http://isdc.gfz-potsdam.de/ontology/SPASE-allowed_values.skos.owl#Coordinate_Representation"/>
    <skos:prefLabel xml:lang="en">Cylindrical</skos:prefLabel>
    <rdf:type rdf:resource="http://www.w3.org/2002/07/owl#NamedIndividual"/>
    <rdf:type rdf:resource="http://www.w3.org/2004/02/skos/core#Concept"/>
    <skos:topConceptOf rdf:resource="http://isdc.gfz-potsdam.de/ontology/SPASE-allowed_values.skos.owl#Coordinate_Representation"/>
    <skos:definition xml:lang="en">A coordinate representation of a position vector or measured vector (field or flow) by its
k-component, the magnitude of its projection into the i-j plane, and the azimuthal angle of the
i-j plane projection.</skos:definition>
  </rdf:Description>
  <rdf:Description rdf:about="http://isdc.gfz-potsdam.de/ontology/SPASE-allowed_values.skos.owl#Electron_Drift_Instrument">
    <skos:definition xml:lang="en">An active experiment to measure the electron drift velocity based on sensing the displacement
of a weak beam of electrons after one gyration in the ambient magnetic field.</skos:definition>
    <skos:topConceptOf rdf:resource="http://isdc.gfz-potsdam.de/ontology/SPASE-allowed_values.skos.owl#Instrument_Type"/>
    <skos:inScheme rdf:resource="http://isdc.gfz-potsdam.de/ontology/SPASE-allowed_values.skos.owl#Instrument_Type"/>
    <rdf:type rdf:resource="http://www.w3.org/2002/07/owl#NamedIndividual"/>
    <rdf:type rdf:resource="http://www.w3.org/2004/02/skos/core#Concept"/>
    <skos:prefLabel xml:lang="en">Electron Drift Instrument</skos:prefLabel>
  </rdf:Description>
  <rdf:Description rdf:about="http://isdc.gfz-potsdam.de/ontology/SPASE-allowed_values.skos.owl#Field_Quantity">
    <rdf:type rdf:resource="http://www.w3.org/2002/07/owl#NamedIndividual"/>
    <skos:hasTopConcept rdf:resource="http://isdc.gfz-potsdam.de/ontology/SPASE-allowed_values.skos.owl#Magnetic"/>
    <skos:hasTopConcept rdf:resource="http://isdc.gfz-potsdam.de/ontology/SPASE-allowed_values.skos.owl#Electromagnetic"/>
    <skos:definition xml:lang="en">The physical attribute of the field.
Allowed Values:
Current
Electric
Electromagnetic
Gyrofrequency
Magnetic
Plasma Frequency
Potential
Poynting Flux</skos:definition>
    <skos:prefLabel xml:lang="en">Field Quantity</skos:prefLabel>
    <skos:hasTopConcept rdf:resource="http://isdc.gfz-potsdam.de/ontology/SPASE-allowed_values.skos.owl#Current"/>
    <skos:hasTopConcept rdf:resource="http://isdc.gfz-potsdam.de/ontology/SPASE-allowed_values.skos.owl#Potential"/>
    <skos:hasTopConcept rdf:resource="http://isdc.gfz-potsdam.de/ontology/SPASE-allowed_values.skos.owl#Poynting_Flux"/>
    <skos:hasTopConcept rdf:resource="http://isdc.gfz-potsdam.de/ontology/SPASE-allowed_values.skos.owl#Electric"/>
    <skos:hasTopConcept rdf:resource="http://isdc.gfz-potsdam.de/ontology/SPASE-allowed_values.skos.owl#Plasma_Frequency"/>
    <skos:hasTopConcept rdf:resource="http://isdc.gfz-potsdam.de/ontology/SPASE-allowed_values.skos.owl#Gyrofrequency"/>
    <rdf:type rdf:resource="http://www.w3.org/2004/02/skos/core#ConceptScheme"/>
  </rdf:Description>
  <rdf:Description rdf:about="http://isdc.gfz-potsdam.de/ontology/SPASE-allowed_values.skos.owl#Albedo">
    <skos:definition xml:lang="en">The ratio of reflected radiation from the surface to incident radiation upon it.</skos:definition>
    <skos:topConceptOf rdf:resource="http://isdc.gfz-potsdam.de/ontology/SPASE-allowed_values.skos.owl#Wave_Quantity"/>
    <skos:prefLabel xml:lang="en">Albedo</skos:prefLabel>
    <rdf:type rdf:resource="http://www.w3.org/2002/07/owl#NamedIndividual"/>
    <rdf:type rdf:resource="http://www.w3.org/2004/02/skos/core#Concept"/>
    <skos:inScheme rdf:resource="http://isdc.gfz-potsdam.de/ontology/SPASE-allowed_values.skos.owl#Wave_Quantity"/>
  </rdf:Description>
  <rdf:Description rdf:about="http://isdc.gfz-potsdam.de/ontology/SPASE-allowed_values.skos.owl#Weak">
    <skos:topConceptOf rdf:resource="http://isdc.gfz-potsdam.de/ontology/SPASE-allowed_values.skos.owl#Confidence_Rating"/>
    <skos:prefLabel xml:lang="en">Weak</skos:prefLabel>
    <skos:definition xml:lang="en">Slightly likely given the available evidence. Considered in the range of 1-4 on a scale of 0-10.</skos:definition>
    <skos:inScheme rdf:resource="http://isdc.gfz-potsdam.de/ontology/SPASE-allowed_values.skos.owl#Confidence_Rating"/>
    <rdf:type rdf:resource="http://www.w3.org/2002/07/owl#NamedIndividual"/>
    <rdf:type rdf:resource="http://www.w3.org/2004/02/skos/core#Concept"/>
  </rdf:Description>
  <rdf:Description rdf:about="http://isdc.gfz-potsdam.de/ontology/SPASE-allowed_values.skos.owl#Processing_Level">
    <rdf:type rdf:resource="http://www.w3.org/2002/07/owl#NamedIndividual"/>
    <rdf:type rdf:resource="http://www.w3.org/2004/02/skos/core#ConceptScheme"/>
    <skos:hasTopConcept rdf:resource="http://isdc.gfz-potsdam.de/ontology/SPASE-allowed_values.skos.owl#Calibrated"/>
    <skos:prefLabel>Processing Level</skos:prefLabel>
    <skos:hasTopConcept rdf:resource="http://isdc.gfz-potsdam.de/ontology/SPASE-allowed_values.skos.owl#Uncalibrated"/>
    <skos:definition xml:lang="en">The standard classification of the processing performed on the product.
Allowed Values:
Calibrated
Raw
Uncalibrated</skos:definition>
    <skos:hasTopConcept rdf:resource="http://isdc.gfz-potsdam.de/ontology/SPASE-allowed_values.skos.owl#Raw"/>
  </rdf:Description>
  <rdf:Description rdf:about="http://isdc.gfz-potsdam.de/ontology/SPASE-allowed_values.skos.owl#J2000">
    <skos:definition xml:lang="en">An astronomical coordinate system which uses the mean equator and equinox of Julian date
2451545.0 TT (Terrestrial Time), or January 1, 2000, noon TT. (aka J2000) to define a celestial
reference frame.</skos:definition>
    <skos:inScheme rdf:resource="http://isdc.gfz-potsdam.de/ontology/SPASE-allowed_values.skos.owl#Coordinate_System_Name"/>
    <skos:topConceptOf rdf:resource="http://isdc.gfz-potsdam.de/ontology/SPASE-allowed_values.skos.owl#Coordinate_System_Name"/>
    <skos:prefLabel xml:lang="en">J2000</skos:prefLabel>
    <rdf:type rdf:resource="http://www.w3.org/2002/07/owl#NamedIndividual"/>
    <rdf:type rdf:resource="http://www.w3.org/2004/02/skos/core#Concept"/>
  </rdf:Description>
  <rdf:Description rdf:about="http://isdc.gfz-potsdam.de/ontology/SPASE-allowed_values.skos.owl#Topside">
    <skos:broader rdf:resource="http://isdc.gfz-potsdam.de/ontology/SPASE-allowed_values.skos.owl#Ionosphere"/>
    <skos:inScheme rdf:resource="http://isdc.gfz-potsdam.de/ontology/SPASE-allowed_values.skos.owl#Observatory_Region"/>
    <skos:definition xml:lang="en">The region at the upper most areas of the ionosphere.</skos:definition>
    <rdf:type rdf:resource="http://www.w3.org/2002/07/owl#NamedIndividual"/>
    <skos:prefLabel xml:lang="en">Topside</skos:prefLabel>
    <skos:inScheme rdf:resource="http://isdc.gfz-potsdam.de/ontology/SPASE-allowed_values.skos.owl#Observed_Region"/>
    <rdf:type rdf:resource="http://www.w3.org/2004/02/skos/core#Concept"/>
  </rdf:Description>
  <rdf:Description rdf:about="http://isdc.gfz-potsdam.de/ontology/SPASE-allowed_values.skos.owl#Spectral_Range">
    <skos:hasTopConcept rdf:resource="http://isdc.gfz-potsdam.de/ontology/SPASE-allowed_values.skos.owl#Ultraviolet"/>
    <skos:hasTopConcept rdf:resource="http://isdc.gfz-potsdam.de/ontology/SPASE-allowed_values.skos.owl#X-Rays"/>
    <skos:hasTopConcept rdf:resource="http://isdc.gfz-potsdam.de/ontology/SPASE-allowed_values.skos.owl#White-Light"/>
    <skos:hasTopConcept rdf:resource="http://isdc.gfz-potsdam.de/ontology/SPASE-allowed_values.skos.owl#Radio_Frequency"/>
    <skos:hasTopConcept rdf:resource="http://isdc.gfz-potsdam.de/ontology/SPASE-allowed_values.skos.owl#Hard_X-rays"/>
    <skos:hasTopConcept rdf:resource="http://isdc.gfz-potsdam.de/ontology/SPASE-allowed_values.skos.owl#LBH_Band"/>
    <skos:hasTopConcept rdf:resource="http://isdc.gfz-potsdam.de/ontology/SPASE-allowed_values.skos.owl#Soft_X-Rays"/>
    <skos:prefLabel xml:lang="en">Spectral Range</skos:prefLabel>
    <skos:hasTopConcept rdf:resource="http://isdc.gfz-potsdam.de/ontology/SPASE-allowed_values.skos.owl#K-7699"/>
    <skos:hasTopConcept rdf:resource="http://isdc.gfz-potsdam.de/ontology/SPASE-allowed_values.skos.owl#Gamma_Rays"/>
    <skos:hasTopConcept rdf:resource="http://isdc.gfz-potsdam.de/ontology/SPASE-allowed_values.skos.owl#Infrared"/>
    <rdf:type rdf:resource="http://www.w3.org/2004/02/skos/core#ConceptScheme"/>
    <skos:hasTopConcept rdf:resource="http://isdc.gfz-potsdam.de/ontology/SPASE-allowed_values.skos.owl#Extreme_Ultraviolet"/>
    <skos:hasTopConcept rdf:resource="http://isdc.gfz-potsdam.de/ontology/SPASE-allowed_values.skos.owl#Ni-6768"/>
    <skos:hasTopConcept rdf:resource="http://isdc.gfz-potsdam.de/ontology/SPASE-allowed_values.skos.owl#H-alpha"/>
    <skos:hasTopConcept rdf:resource="http://isdc.gfz-potsdam.de/ontology/SPASE-allowed_values.skos.owl#Na-D"/>
    <skos:hasTopConcept rdf:resource="http://isdc.gfz-potsdam.de/ontology/SPASE-allowed_values.skos.owl#Ca-K"/>
    <skos:hasTopConcept rdf:resource="http://isdc.gfz-potsdam.de/ontology/SPASE-allowed_values.skos.owl#He-304"/>
    <skos:definition xml:lang="en">The general term used to describe wavelengths or frequencies within a given span of values for
those quantities.
Allowed Values:
Ca-K
Extreme Ultraviolet
Far Ultraviolet
Gamma Rays
H-alpha
Hard X-rays
He-10830
He-304
Infrared
K-7699
LBH Band
Microwave
Na-D
Ni-6768
Optical
Radio Frequency
Soft X-Rays
Ultraviolet
White-Light
X-Rays</skos:definition>
    <skos:hasTopConcept rdf:resource="http://isdc.gfz-potsdam.de/ontology/SPASE-allowed_values.skos.owl#Microwave"/>
    <skos:hasTopConcept rdf:resource="http://isdc.gfz-potsdam.de/ontology/SPASE-allowed_values.skos.owl#He-10830"/>
    <skos:hasTopConcept rdf:resource="http://isdc.gfz-potsdam.de/ontology/SPASE-allowed_values.skos.owl#Optical"/>
    <rdf:type rdf:resource="http://www.w3.org/2002/07/owl#NamedIndividual"/>
    <skos:hasTopConcept rdf:resource="http://isdc.gfz-potsdam.de/ontology/SPASE-allowed_values.skos.owl#Far_Ultraviolet"/>
  </rdf:Description>
  <rdf:Description rdf:about="http://isdc.gfz-potsdam.de/ontology/SPASE-allowed_values.skos.owl#He-10830">
    <rdf:type rdf:resource="http://www.w3.org/2004/02/skos/core#Concept"/>
    <skos:prefLabel xml:lang="en">He-10830</skos:prefLabel>
    <skos:inScheme rdf:resource="http://isdc.gfz-potsdam.de/ontology/SPASE-allowed_values.skos.owl#Spectral_Range"/>
    <skos:definition xml:lang="en">A spectrum with a wavelength range centered at 1082.9 nm. VSO nickname: He 10830 image
with a range of 1082.5 nm to 1083.3 nm.</skos:definition>
    <skos:topConceptOf rdf:resource="http://isdc.gfz-potsdam.de/ontology/SPASE-allowed_values.skos.owl#Spectral_Range"/>
    <rdf:type rdf:resource="http://www.w3.org/2002/07/owl#NamedIndividual"/>
  </rdf:Description>
  <rdf:Description rdf:about="http://isdc.gfz-potsdam.de/ontology/SPASE-allowed_values.skos.owl#Instrument_Status">
    <rdf:type rdf:resource="http://www.w3.org/2004/02/skos/core#Concept"/>
    <rdf:type rdf:resource="http://www.w3.org/2002/07/owl#NamedIndividual"/>
    <skos:definition xml:lang="en">A quantity directly related to the operation or function of an instrument.</skos:definition>
    <skos:prefLabel xml:lang="en">Instrument Status</skos:prefLabel>
    <skos:inScheme rdf:resource="http://isdc.gfz-potsdam.de/ontology/SPASE-allowed_values.skos.owl#Measurement_Type"/>
    <skos:topConceptOf rdf:resource="http://isdc.gfz-potsdam.de/ontology/SPASE-allowed_values.skos.owl#Measurement_Type"/>
  </rdf:Description>
  <rdf:Description rdf:about="http://isdc.gfz-potsdam.de/ontology/SPASE-allowed_values.skos.owl#QuickTime">
    <skos:topConceptOf rdf:resource="http://isdc.gfz-potsdam.de/ontology/SPASE-allowed_values.skos.owl#Format"/>
    <skos:definition xml:lang="en">A format for digital movies, as defined by Apple Computer. See
&lt;http://developer.apple.com/quicktime/&gt;.</skos:definition>
    <skos:prefLabel xml:lang="en">QuickTime</skos:prefLabel>
    <rdf:type rdf:resource="http://www.w3.org/2004/02/skos/core#Concept"/>
    <rdf:type rdf:resource="http://www.w3.org/2002/07/owl#NamedIndividual"/>
    <skos:inScheme rdf:resource="http://isdc.gfz-potsdam.de/ontology/SPASE-allowed_values.skos.owl#Format"/>
  </rdf:Description>
  <rdf:Description rdf:about="http://isdc.gfz-potsdam.de/ontology/SPASE-allowed_values.skos.owl#Inner">
    <skos:inScheme rdf:resource="http://isdc.gfz-potsdam.de/ontology/SPASE-allowed_values.skos.owl#Observed_Region"/>
    <skos:broader rdf:resource="http://isdc.gfz-potsdam.de/ontology/SPASE-allowed_values.skos.owl#Heliosphere"/>
    <skos:inScheme rdf:resource="http://isdc.gfz-potsdam.de/ontology/SPASE-allowed_values.skos.owl#Observatory_Region"/>
    <rdf:type rdf:resource="http://www.w3.org/2004/02/skos/core#Concept"/>
    <skos:definition xml:lang="en">The region of the heliosphere extending radially outward from the solar coronal base to just
inside 1 AU.</skos:definition>
    <rdf:type rdf:resource="http://www.w3.org/2002/07/owl#NamedIndividual"/>
    <skos:prefLabel xml:lang="en">Inner</skos:prefLabel>
  </rdf:Description>
  <rdf:Description rdf:about="http://isdc.gfz-potsdam.de/ontology/SPASE-allowed_values.skos.owl#Remote_1AU">
    <skos:definition xml:lang="en">A roughly toroidal region that includes the Earth's orbit, but exclusive of the region near the
Earth.</skos:definition>
    <rdf:type rdf:resource="http://www.w3.org/2004/02/skos/core#Concept"/>
    <skos:inScheme rdf:resource="http://isdc.gfz-potsdam.de/ontology/SPASE-allowed_values.skos.owl#Observed_Region"/>
    <rdf:type rdf:resource="http://www.w3.org/2002/07/owl#NamedIndividual"/>
    <skos:inScheme rdf:resource="http://isdc.gfz-potsdam.de/ontology/SPASE-allowed_values.skos.owl#Observatory_Region"/>
    <skos:broader rdf:resource="http://isdc.gfz-potsdam.de/ontology/SPASE-allowed_values.skos.owl#Heliosphere"/>
    <skos:prefLabel xml:lang="en">Remote 1AU</skos:prefLabel>
  </rdf:Description>
  <rdf:Description rdf:about="http://isdc.gfz-potsdam.de/ontology/SPASE-allowed_values.skos.owl#Ion">
    <rdf:type rdf:resource="http://www.w3.org/2002/07/owl#NamedIndividual"/>
    <skos:topConceptOf rdf:resource="http://isdc.gfz-potsdam.de/ontology/SPASE-allowed_values.skos.owl#Particle_Type"/>
    <skos:definition xml:lang="en">An atom that has acquired a net electric charge by gaining or losing one or more
electrons.(Note: Z&gt;2)</skos:definition>
    <skos:inScheme rdf:resource="http://isdc.gfz-potsdam.de/ontology/SPASE-allowed_values.skos.owl#Particle_Type"/>
    <skos:prefLabel xml:lang="en">Ion</skos:prefLabel>
    <rdf:type rdf:resource="http://www.w3.org/2004/02/skos/core#Concept"/>
  </rdf:Description>
  <rdf:Description rdf:about="http://isdc.gfz-potsdam.de/ontology/SPASE-allowed_values.skos.owl#SE">
    <skos:topConceptOf rdf:resource="http://isdc.gfz-potsdam.de/ontology/SPASE-allowed_values.skos.owl#Coordinate_System_Name"/>
    <skos:definition xml:lang="en">Solar Ecliptic - A heliocentric coordinate system where the Z axis is normal to the ecliptic
plane, positive northward. X axis is positive towards the first point of Aries (from Earth to Sun
at vernal equinox). Same as HAE above. See
&lt;http://nssdc.gsfc.nasa.gov/space/helios/coor_des.html&gt;.</skos:definition>
    <rdf:type rdf:resource="http://www.w3.org/2004/02/skos/core#Concept"/>
    <rdf:type rdf:resource="http://www.w3.org/2002/07/owl#NamedIndividual"/>
    <skos:inScheme rdf:resource="http://isdc.gfz-potsdam.de/ontology/SPASE-allowed_values.skos.owl#Coordinate_System_Name"/>
    <skos:prefLabel xml:lang="en">SE</skos:prefLabel>
  </rdf:Description>
  <rdf:Description rdf:about="http://isdc.gfz-potsdam.de/ontology/SPASE-allowed_values.skos.owl#Access_Rights">
    <skos:hasTopConcept rdf:resource="http://isdc.gfz-potsdam.de/ontology/SPASE-allowed_values.skos.owl#Open"/>
    <skos:prefLabel xml:lang="en">Access Rights</skos:prefLabel>
    <rdf:type rdf:resource="http://www.w3.org/2004/02/skos/core#ConceptScheme"/>
    <rdf:type rdf:resource="http://www.w3.org/2002/07/owl#NamedIndividual"/>
    <skos:hasTopConcept rdf:resource="http://isdc.gfz-potsdam.de/ontology/SPASE-allowed_values.skos.owl#Restricted"/>
    <skos:definition xml:lang="en">Permissions granted or denied by the host of a product to allow other users to access and use the
resource.
Allowed Values:
Open
Restricted</skos:definition>
  </rdf:Description>
  <rdf:Description rdf:about="http://isdc.gfz-potsdam.de/ontology/SPASE-allowed_values.skos.owl#CGM">
    <skos:prefLabel xml:lang="en">CGM</skos:prefLabel>
    <rdf:type rdf:resource="http://www.w3.org/2002/07/owl#NamedIndividual"/>
    <rdf:type rdf:resource="http://www.w3.org/2004/02/skos/core#Concept"/>
    <skos:inScheme rdf:resource="http://isdc.gfz-potsdam.de/ontology/SPASE-allowed_values.skos.owl#Coordinate_System_Name"/>
    <skos:topConceptOf rdf:resource="http://isdc.gfz-potsdam.de/ontology/SPASE-allowed_values.skos.owl#Coordinate_System_Name"/>
    <skos:definition xml:lang="en">Corrected Geomagnetic - A coordinate system from a spatial point with GEO radial distance
and geomagnetic latitude and longitude, follow the epoch-appropriate IGRF/DGRF model field
vector through to the point where the field line crosses the geomagnetic dipole equatorial plane.
Then trace the dipole magnetic field vector Earthward from that point on the equatorial plane,
in the same hemisphere as the original point, until the initial radial distance is reached.
Designate the dipole latitude and longitude at that point as the CGM latitude and longitude of
the original point. See &lt;http://nssdc.gsfc.nasa.gov/space/cgm/cgmm_des.html&gt;</skos:definition>
  </rdf:Description>
  <rdf:Description rdf:about="http://isdc.gfz-potsdam.de/ontology/SPASE-allowed_values.skos.owl#Component">
    <skos:definition xml:lang="en">Projection of a vector along one of the base axes of a coordinate system.
Allowed Values:
I
J
K</skos:definition>
    <skos:narrower rdf:resource="http://isdc.gfz-potsdam.de/ontology/SPASE-allowed_values.skos.owl#K"/>
    <rdf:type rdf:resource="http://www.w3.org/2004/02/skos/core#Concept"/>
    <rdf:type rdf:resource="http://www.w3.org/2002/07/owl#NamedIndividual"/>
    <skos:topConceptOf rdf:resource="http://isdc.gfz-potsdam.de/ontology/SPASE-allowed_values.skos.owl#Qualifier"/>
    <skos:narrower rdf:resource="http://isdc.gfz-potsdam.de/ontology/SPASE-allowed_values.skos.owl#J"/>
    <skos:prefLabel xml:lang="en">Component</skos:prefLabel>
    <skos:inScheme rdf:resource="http://isdc.gfz-potsdam.de/ontology/SPASE-allowed_values.skos.owl#Qualifier"/>
    <skos:narrower rdf:resource="http://isdc.gfz-potsdam.de/ontology/SPASE-allowed_values.skos.owl#I"/>
  </rdf:Description>
  <rdf:Description rdf:about="http://isdc.gfz-potsdam.de/ontology/SPASE-allowed_values.skos.owl#Particle_Detector">
    <skos:definition xml:lang="en">An instrument which detects particle flux!!!</skos:definition>
    <skos:topConceptOf rdf:resource="http://isdc.gfz-potsdam.de/ontology/SPASE-allowed_values.skos.owl#Instrument_Type"/>
    <rdf:type rdf:resource="http://www.w3.org/2004/02/skos/core#Concept"/>
    <rdf:type rdf:resource="http://www.w3.org/2002/07/owl#NamedIndividual"/>
    <skos:prefLabel xml:lang="en">Particle Detector</skos:prefLabel>
    <skos:inScheme rdf:resource="http://isdc.gfz-potsdam.de/ontology/SPASE-allowed_values.skos.owl#Instrument_Type"/>
  </rdf:Description>
  <rdf:Description rdf:about="http://isdc.gfz-potsdam.de/ontology/SPASE-allowed_values.skos.owl#He-304">
    <skos:prefLabel xml:lang="en">He-304</skos:prefLabel>
    <skos:definition xml:lang="en">A spectrum centered around the resonance line of ionised helium at 304 Angstrom (30.4 nm).</skos:definition>
    <skos:topConceptOf rdf:resource="http://isdc.gfz-potsdam.de/ontology/SPASE-allowed_values.skos.owl#Spectral_Range"/>
    <rdf:type rdf:resource="http://www.w3.org/2004/02/skos/core#Concept"/>
    <rdf:type rdf:resource="http://www.w3.org/2002/07/owl#NamedIndividual"/>
    <skos:inScheme rdf:resource="http://isdc.gfz-potsdam.de/ontology/SPASE-allowed_values.skos.owl#Spectral_Range"/>
  </rdf:Description>
  <rdf:Description rdf:about="http://isdc.gfz-potsdam.de/ontology/SPASE-allowed_values.skos.owl#Maximum">
    <rdf:type rdf:resource="http://www.w3.org/2002/07/owl#NamedIndividual"/>
    <skos:definition xml:lang="en">The largest value of a batch or sample or the upper bound of a probability distribution.</skos:definition>
    <skos:inScheme rdf:resource="http://isdc.gfz-potsdam.de/ontology/SPASE-allowed_values.skos.owl#Qualifier"/>
    <skos:topConceptOf rdf:resource="http://isdc.gfz-potsdam.de/ontology/SPASE-allowed_values.skos.owl#Qualifier"/>
    <skos:prefLabel xml:lang="en">Maximum</skos:prefLabel>
    <rdf:type rdf:resource="http://www.w3.org/2004/02/skos/core#Concept"/>
  </rdf:Description>
  <rdf:Description rdf:about="http://isdc.gfz-potsdam.de/ontology/SPASE-allowed_values.skos.owl#Neutral_Gas">
    <skos:inScheme rdf:resource="http://isdc.gfz-potsdam.de/ontology/SPASE-allowed_values.skos.owl#Measurement_Type"/>
    <rdf:type rdf:resource="http://www.w3.org/2004/02/skos/core#Concept"/>
    <rdf:type rdf:resource="http://www.w3.org/2002/07/owl#NamedIndividual"/>
    <skos:prefLabel xml:lang="en">Neutral Gas</skos:prefLabel>
    <skos:topConceptOf rdf:resource="http://isdc.gfz-potsdam.de/ontology/SPASE-allowed_values.skos.owl#Measurement_Type"/>
    <skos:definition xml:lang="en">Measurements of neutral atomic and molecular components of a gas.</skos:definition>
  </rdf:Description>
  <rdf:Description rdf:about="http://isdc.gfz-potsdam.de/ontology/SPASE-allowed_values.skos.owl#Far_Ultraviolet">
    <skos:topConceptOf rdf:resource="http://isdc.gfz-potsdam.de/ontology/SPASE-allowed_values.skos.owl#Spectral_Range"/>
    <skos:inScheme rdf:resource="http://isdc.gfz-potsdam.de/ontology/SPASE-allowed_values.skos.owl#Spectral_Range"/>
    <rdf:type rdf:resource="http://www.w3.org/2002/07/owl#NamedIndividual"/>
    <skos:definition xml:lang="en">A spectrum with a wavelength range of 122 nm to 200.0nm. VSO nickname: FUV image with a
range of 122.0 nm to 200 nm.</skos:definition>
    <rdf:type rdf:resource="http://www.w3.org/2004/02/skos/core#Concept"/>
    <skos:prefLabel xml:lang="en">Far Ultraviolet</skos:prefLabel>
  </rdf:Description>
  <rdf:Description rdf:about="http://isdc.gfz-potsdam.de/ontology/SPASE-allowed_values.skos.owl#Interferometer">
    <skos:prefLabel xml:lang="en">Interferometer</skos:prefLabel>
    <rdf:type rdf:resource="http://www.w3.org/2002/07/owl#NamedIndividual"/>
    <rdf:type rdf:resource="http://www.w3.org/2004/02/skos/core#Concept"/>
    <skos:inScheme rdf:resource="http://isdc.gfz-potsdam.de/ontology/SPASE-allowed_values.skos.owl#Instrument_Type"/>
    <skos:topConceptOf rdf:resource="http://isdc.gfz-potsdam.de/ontology/SPASE-allowed_values.skos.owl#Instrument_Type"/>
    <skos:definition xml:lang="en">An instrument to study the properties of two or more waves from the pattern of interference
created by their superposition.</skos:definition>
  </rdf:Description>
  <rdf:Description rdf:about="http://isdc.gfz-potsdam.de/ontology/SPASE-allowed_values.skos.owl#Trace">
    <skos:definition xml:lang="en">The sum of the elements on the main diagonal (the diagonal from the upper left to the lower
right) of a square matrix.</skos:definition>
    <skos:prefLabel xml:lang="en">Trace</skos:prefLabel>
    <skos:inScheme rdf:resource="http://isdc.gfz-potsdam.de/ontology/SPASE-allowed_values.skos.owl#Qualifier"/>
    <rdf:type rdf:resource="http://www.w3.org/2004/02/skos/core#Concept"/>
    <rdf:type rdf:resource="http://www.w3.org/2002/07/owl#NamedIndividual"/>
    <skos:topConceptOf rdf:resource="http://isdc.gfz-potsdam.de/ontology/SPASE-allowed_values.skos.owl#Qualifier"/>
  </rdf:Description>
  <rdf:Description rdf:about="http://isdc.gfz-potsdam.de/ontology/SPASE-allowed_values.skos.owl#Radio_Frequency">
    <rdf:type rdf:resource="http://www.w3.org/2002/07/owl#NamedIndividual"/>
    <skos:prefLabel xml:lang="en">Radio Frequency</skos:prefLabel>
    <skos:topConceptOf rdf:resource="http://isdc.gfz-potsdam.de/ontology/SPASE-allowed_values.skos.owl#Spectral_Range"/>
    <rdf:type rdf:resource="http://www.w3.org/2004/02/skos/core#Concept"/>
    <skos:definition xml:lang="en">Photons with a wavelength range: 100,000 to 1.00x10^11 nm</skos:definition>
    <skos:inScheme rdf:resource="http://isdc.gfz-potsdam.de/ontology/SPASE-allowed_values.skos.owl#Spectral_Range"/>
  </rdf:Description>
  <rdf:Description rdf:about="http://isdc.gfz-potsdam.de/ontology/SPASE-allowed_values.skos.owl#Alfven_Velocity">
    <skos:inScheme rdf:resource="http://isdc.gfz-potsdam.de/ontology/SPASE-allowed_values.skos.owl#Mixed_Quantity"/>
    <skos:definition xml:lang="en">Phase velocity of the Alfven wave; In SI units it is the velocity of the magnetic field divided by
the square root of the mass density times the permeability of free space (mu).</skos:definition>
    <skos:topConceptOf rdf:resource="http://isdc.gfz-potsdam.de/ontology/SPASE-allowed_values.skos.owl#Mixed_Quantity"/>
    <skos:prefLabel xml:lang="en">Alfven Velocity</skos:prefLabel>
    <rdf:type rdf:resource="http://www.w3.org/2004/02/skos/core#Concept"/>
    <rdf:type rdf:resource="http://www.w3.org/2002/07/owl#NamedIndividual"/>
  </rdf:Description>
  <rdf:Description rdf:about="http://isdc.gfz-potsdam.de/ontology/SPASE-allowed_values.skos.owl#Phase_Angle">
    <skos:definition xml:lang="en">Phase difference between two or more waves, normally expressed in degrees.</skos:definition>
    <skos:topConceptOf rdf:resource="http://isdc.gfz-potsdam.de/ontology/SPASE-allowed_values.skos.owl#Qualifier"/>
    <skos:prefLabel xml:lang="en">Phase Angle</skos:prefLabel>
    <skos:inScheme rdf:resource="http://isdc.gfz-potsdam.de/ontology/SPASE-allowed_values.skos.owl#Qualifier"/>
    <rdf:type rdf:resource="http://www.w3.org/2002/07/owl#NamedIndividual"/>
    <rdf:type rdf:resource="http://www.w3.org/2004/02/skos/core#Concept"/>
  </rdf:Description>
  <rdf:Description rdf:about="http://isdc.gfz-potsdam.de/ontology/SPASE-allowed_values.skos.owl#Role">
    <skos:hasTopConcept rdf:resource="http://isdc.gfz-potsdam.de/ontology/SPASE-allowed_values.skos.owl#Project_Scientist"/>
    <skos:hasTopConcept rdf:resource="http://isdc.gfz-potsdam.de/ontology/SPASE-allowed_values.skos.owl#Principal_Investigator"/>
    <skos:hasTopConcept rdf:resource="http://isdc.gfz-potsdam.de/ontology/SPASE-allowed_values.skos.owl#Scientist"/>
    <skos:hasTopConcept rdf:resource="http://isdc.gfz-potsdam.de/ontology/SPASE-allowed_values.skos.owl#Archive_Specialist"/>
    <skos:hasTopConcept rdf:resource="http://isdc.gfz-potsdam.de/ontology/SPASE-allowed_values.skos.owl#Team_Member"/>
    <skos:hasTopConcept rdf:resource="http://isdc.gfz-potsdam.de/ontology/SPASE-allowed_values.skos.owl#Team_Leader"/>
    <skos:hasTopConcept rdf:resource="http://isdc.gfz-potsdam.de/ontology/SPASE-allowed_values.skos.owl#Technical_Contact"/>
    <skos:hasTopConcept rdf:resource="http://isdc.gfz-potsdam.de/ontology/SPASE-allowed_values.skos.owl#Metadata_Contact"/>
    <skos:hasTopConcept rdf:resource="http://isdc.gfz-potsdam.de/ontology/SPASE-allowed_values.skos.owl#General_Contact"/>
    <skos:hasTopConcept rdf:resource="http://isdc.gfz-potsdam.de/ontology/SPASE-allowed_values.skos.owl#Contributor"/>
    <skos:prefLabel xml:lang="en">Role</skos:prefLabel>
    <skos:hasTopConcept rdf:resource="http://isdc.gfz-potsdam.de/ontology/SPASE-allowed_values.skos.owl#Publisher"/>
    <rdf:type rdf:resource="http://www.w3.org/2002/07/owl#NamedIndividual"/>
    <rdf:type rdf:resource="http://www.w3.org/2004/02/skos/core#ConceptScheme"/>
    <skos:hasTopConcept rdf:resource="http://isdc.gfz-potsdam.de/ontology/SPASE-allowed_values.skos.owl#Data_Producer"/>
    <skos:hasTopConcept rdf:resource="http://isdc.gfz-potsdam.de/ontology/SPASE-allowed_values.skos.owl#Former-PI"/>
    <skos:hasTopConcept rdf:resource="http://isdc.gfz-potsdam.de/ontology/SPASE-allowed_values.skos.owl#Co-Investigator"/>
    <skos:definition xml:lang="en">The assigned or assumed function or position of an individual.
Allowed Values:
Archive Specialist
Co-Investigator
Contributor
Data Producer
Deputy-PI
Former-PI
General Contact
Metadata Contact
Principal Investigator
Project Scientist
Publisher
Scientist
Team Leader
Team Member
Technical Contact</skos:definition>
    <skos:hasTopConcept rdf:resource="http://isdc.gfz-potsdam.de/ontology/SPASE-allowed_values.skos.owl#Deputy-PI"/>
  </rdf:Description>
  <rdf:Description rdf:about="http://isdc.gfz-potsdam.de/ontology/SPASE-allowed_values.skos.owl#Offline">
    <rdf:type rdf:resource="http://www.w3.org/2004/02/skos/core#Concept"/>
    <skos:definition xml:lang="en">Not directly accessible electronically. This includes resources which may to be moved to an
on-line status in response to a given request.</skos:definition>
    <skos:prefLabel xml:lang="en">Offline</skos:prefLabel>
    <skos:inScheme rdf:resource="http://isdc.gfz-potsdam.de/ontology/SPASE-allowed_values.skos.owl#Availability"/>
    <skos:topConceptOf rdf:resource="http://isdc.gfz-potsdam.de/ontology/SPASE-allowed_values.skos.owl#Availability"/>
    <rdf:type rdf:resource="http://www.w3.org/2002/07/owl#NamedIndividual"/>
  </rdf:Description>
  <rdf:Description rdf:about="http://isdc.gfz-potsdam.de/ontology/SPASE-allowed_values.skos.owl#Projection">
    <skos:inScheme rdf:resource="http://isdc.gfz-potsdam.de/ontology/SPASE-allowed_values.skos.owl#Qualifier"/>
    <rdf:type rdf:resource="http://www.w3.org/2002/07/owl#NamedIndividual"/>
    <skos:narrower rdf:resource="http://isdc.gfz-potsdam.de/ontology/SPASE-allowed_values.skos.owl#IJ"/>
    <skos:prefLabel xml:lang="en">Projection</skos:prefLabel>
    <skos:topConceptOf rdf:resource="http://isdc.gfz-potsdam.de/ontology/SPASE-allowed_values.skos.owl#Qualifier"/>
    <rdf:type rdf:resource="http://www.w3.org/2004/02/skos/core#Concept"/>
    <skos:narrower rdf:resource="http://isdc.gfz-potsdam.de/ontology/SPASE-allowed_values.skos.owl#JK"/>
    <skos:narrower rdf:resource="http://isdc.gfz-potsdam.de/ontology/SPASE-allowed_values.skos.owl#IK"/>
    <skos:definition xml:lang="en">A measure of the length of a position or measured vector as projected into a plane of the
coordinate system.
Allowed Values:
IJ
IK
JK</skos:definition>
  </rdf:Description>
  <rdf:Description rdf:about="http://isdc.gfz-potsdam.de/ontology/SPASE-allowed_values.skos.owl#Aurora">
    <skos:topConceptOf rdf:resource="http://isdc.gfz-potsdam.de/ontology/SPASE-allowed_values.skos.owl#Phenomenon_Type"/>
    <skos:prefLabel xml:lang="en">Aurora</skos:prefLabel>
    <skos:inScheme rdf:resource="http://isdc.gfz-potsdam.de/ontology/SPASE-allowed_values.skos.owl#Phenomenon_Type"/>
    <rdf:type rdf:resource="http://www.w3.org/2004/02/skos/core#Concept"/>
    <rdf:type rdf:resource="http://www.w3.org/2002/07/owl#NamedIndividual"/>
    <skos:definition xml:lang="en">An atmospheric phenomenon consisting of bands of light caused by charged solar particles
following the earth's magnetic lines of force.</skos:definition>
  </rdf:Description>
  <rdf:Description rdf:about="http://isdc.gfz-potsdam.de/ontology/SPASE-allowed_values.skos.owl#Plasma_Frequency">
    <skos:topConceptOf rdf:resource="http://isdc.gfz-potsdam.de/ontology/SPASE-allowed_values.skos.owl#Particle_Quantity"/>
    <skos:inScheme rdf:resource="http://isdc.gfz-potsdam.de/ontology/SPASE-allowed_values.skos.owl#Field_Quantity"/>
    <rdf:type rdf:resource="http://www.w3.org/2002/07/owl#NamedIndividual"/>
    <skos:definition xml:lang="en">A number-density-dependent characteristic frequency of a plasma.</skos:definition>
    <skos:topConceptOf rdf:resource="http://isdc.gfz-potsdam.de/ontology/SPASE-allowed_values.skos.owl#Field_Quantity"/>
    <skos:inScheme rdf:resource="http://isdc.gfz-potsdam.de/ontology/SPASE-allowed_values.skos.owl#Particle_Quantity"/>
    <rdf:type rdf:resource="http://www.w3.org/2004/02/skos/core#Concept"/>
    <skos:inScheme rdf:resource="http://isdc.gfz-potsdam.de/ontology/SPASE-allowed_values.skos.owl#Wave_Quantity"/>
    <skos:prefLabel xml:lang="en">Plasma Frequency</skos:prefLabel>
    <skos:topConceptOf rdf:resource="http://isdc.gfz-potsdam.de/ontology/SPASE-allowed_values.skos.owl#Wave_Quantity"/>
  </rdf:Description>
  <rdf:Description rdf:about="http://isdc.gfz-potsdam.de/ontology/SPASE-allowed_values.skos.owl#Plasmagram">
    <skos:inScheme rdf:resource="http://isdc.gfz-potsdam.de/ontology/SPASE-allowed_values.skos.owl#Display_Type"/>
    <rdf:type rdf:resource="http://www.w3.org/2004/02/skos/core#Concept"/>
    <rdf:type rdf:resource="http://www.w3.org/2002/07/owl#NamedIndividual"/>
    <skos:topConceptOf rdf:resource="http://isdc.gfz-potsdam.de/ontology/SPASE-allowed_values.skos.owl#Display_Type"/>
    <skos:prefLabel xml:lang="en">Plasmagram</skos:prefLabel>
    <skos:definition xml:lang="en">The characterization of signal strengths in active sounding measurements as a function of
virtual range or signal delay time and sounding frequency. A Plasmagram is also referred to as
an Ionogram.</skos:definition>
  </rdf:Description>
  <rdf:Description rdf:about="http://isdc.gfz-potsdam.de/ontology/SPASE-allowed_values.skos.owl#Part_Of">
    <rdf:type rdf:resource="http://www.w3.org/2002/07/owl#NamedIndividual"/>
    <skos:prefLabel xml:lang="en">Part Of</skos:prefLabel>
    <skos:topConceptOf rdf:resource="http://isdc.gfz-potsdam.de/ontology/SPASE-allowed_values.skos.owl#Association_Type"/>
    <skos:definition xml:lang="en">A portion of a larger resource.</skos:definition>
    <rdf:type rdf:resource="http://www.w3.org/2004/02/skos/core#Concept"/>
    <skos:inScheme rdf:resource="http://isdc.gfz-potsdam.de/ontology/SPASE-allowed_values.skos.owl#Association_Type"/>
  </rdf:Description>
  <rdf:Description rdf:about="http://isdc.gfz-potsdam.de/ontology/SPASE-allowed_values.skos.owl#JPEG">
    <rdf:type rdf:resource="http://www.w3.org/2002/07/owl#NamedIndividual"/>
    <skos:definition xml:lang="en">A binary format for still images defined by the Joint Photographic Experts Group.</skos:definition>
    <skos:topConceptOf rdf:resource="http://isdc.gfz-potsdam.de/ontology/SPASE-allowed_values.skos.owl#Format"/>
    <skos:inScheme rdf:resource="http://isdc.gfz-potsdam.de/ontology/SPASE-allowed_values.skos.owl#Format"/>
    <skos:prefLabel xml:lang="en">JPEG</skos:prefLabel>
    <rdf:type rdf:resource="http://www.w3.org/2004/02/skos/core#Concept"/>
  </rdf:Description>
  <rdf:Description rdf:about="http://isdc.gfz-potsdam.de/ontology/SPASE-allowed_values.skos.owl#Excel">
    <skos:prefLabel xml:lang="en">Excel</skos:prefLabel>
    <skos:inScheme rdf:resource="http://isdc.gfz-potsdam.de/ontology/SPASE-allowed_values.skos.owl#Format"/>
    <skos:definition xml:lang="en">A Microsoft spreadsheet format used to hold a variety of data in tables which can include
calculations.</skos:definition>
    <rdf:type rdf:resource="http://www.w3.org/2002/07/owl#NamedIndividual"/>
    <rdf:type rdf:resource="http://www.w3.org/2004/02/skos/core#Concept"/>
    <skos:topConceptOf rdf:resource="http://isdc.gfz-potsdam.de/ontology/SPASE-allowed_values.skos.owl#Format"/>
  </rdf:Description>
  <rdf:Description rdf:about="http://isdc.gfz-potsdam.de/ontology/SPASE-allowed_values.skos.owl#Transition_Region">
    <skos:prefLabel xml:lang="en">Transition Region</skos:prefLabel>
    <skos:inScheme rdf:resource="http://isdc.gfz-potsdam.de/ontology/SPASE-allowed_values.skos.owl#Observatory_Region"/>
    <rdf:type rdf:resource="http://www.w3.org/2002/07/owl#NamedIndividual"/>
    <rdf:type rdf:resource="http://www.w3.org/2004/02/skos/core#Concept"/>
    <skos:inScheme rdf:resource="http://isdc.gfz-potsdam.de/ontology/SPASE-allowed_values.skos.owl#Observed_Region"/>
    <skos:definition xml:lang="en">A very narrow (&lt;100 km) layer between the chromosphere and the corona where the
temperature rises abruptly from about 8000 to about 500,000 K.</skos:definition>
    <skos:broader rdf:resource="http://isdc.gfz-potsdam.de/ontology/SPASE-allowed_values.skos.owl#Sun"/>
  </rdf:Description>
  <rdf:Description rdf:about="http://isdc.gfz-potsdam.de/ontology/SPASE-allowed_values.skos.owl#Extreme_Ultraviolet">
    <skos:prefLabel xml:lang="en">Extreme Ultraviolet</skos:prefLabel>
    <skos:inScheme rdf:resource="http://isdc.gfz-potsdam.de/ontology/SPASE-allowed_values.skos.owl#Spectral_Range"/>
    <rdf:type rdf:resource="http://www.w3.org/2002/07/owl#NamedIndividual"/>
    <rdf:type rdf:resource="http://www.w3.org/2004/02/skos/core#Concept"/>
    <skos:topConceptOf rdf:resource="http://isdc.gfz-potsdam.de/ontology/SPASE-allowed_values.skos.owl#Spectral_Range"/>
    <skos:definition xml:lang="en">A spectrum with a wavelength range of 10.0 nm to 125.0nm. VSO nickname: EUV image with
a range of of 10.0 nm to 125.0 nm.</skos:definition>
  </rdf:Description>
  <rdf:Description rdf:about="http://isdc.gfz-potsdam.de/ontology/SPASE-allowed_values.skos.owl#K">
    <rdf:type rdf:resource="http://www.w3.org/2002/07/owl#NamedIndividual"/>
    <skos:broader rdf:resource="http://isdc.gfz-potsdam.de/ontology/SPASE-allowed_values.skos.owl#Component"/>
    <skos:prefLabel xml:lang="en">K</skos:prefLabel>
    <skos:inScheme rdf:resource="http://isdc.gfz-potsdam.de/ontology/SPASE-allowed_values.skos.owl#Qualifier"/>
    <skos:altLabel xml:lang="en">Projection of a vector along the third named axis of a coordinate system. Typically the Z axis,
but could be the N axis for an RTN coordinate system.</skos:altLabel>
    <rdf:type rdf:resource="http://www.w3.org/2004/02/skos/core#Concept"/>
  </rdf:Description>
  <rdf:Description rdf:about="http://isdc.gfz-potsdam.de/ontology/SPASE-allowed_values.skos.owl#Thermosphere">
    <skos:inScheme rdf:resource="http://isdc.gfz-potsdam.de/ontology/SPASE-allowed_values.skos.owl#Observatory_Region"/>
    <rdf:type rdf:resource="http://www.w3.org/2002/07/owl#NamedIndividual"/>
    <rdf:type rdf:resource="http://www.w3.org/2004/02/skos/core#Concept"/>
    <skos:prefLabel xml:lang="en">Thermosphere</skos:prefLabel>
    <skos:definition xml:lang="en">The layer of the atmosphere that extends from the Mesosphere to 640+ km, temperature
increasing with height.</skos:definition>
    <skos:broader rdf:resource="http://isdc.gfz-potsdam.de/ontology/SPASE-allowed_values.skos.owl#Near_Surface"/>
    <skos:inScheme rdf:resource="http://isdc.gfz-potsdam.de/ontology/SPASE-allowed_values.skos.owl#Observed_Region"/>
  </rdf:Description>
  <rdf:Description rdf:about="http://isdc.gfz-potsdam.de/ontology/SPASE-allowed_values.skos.owl#Radiance">
    <skos:topConceptOf rdf:resource="http://isdc.gfz-potsdam.de/ontology/SPASE-allowed_values.skos.owl#Measurement_Type"/>
    <rdf:type rdf:resource="http://www.w3.org/2002/07/owl#NamedIndividual"/>
    <rdf:type rdf:resource="http://www.w3.org/2004/02/skos/core#Concept"/>
    <skos:inScheme rdf:resource="http://isdc.gfz-potsdam.de/ontology/SPASE-allowed_values.skos.owl#Measurement_Type"/>
    <skos:prefLabel xml:lang="en">Radiance</skos:prefLabel>
    <skos:definition xml:lang="en">A radiometric measurement that describes the amount of electromagnetic radiation that passes
through or is emitted from a particular area, and falls within a given solid angle in a specified
direction. They are used to characterize both emission from diffuse sources and reflection from
diffuse surfaces.</skos:definition>
  </rdf:Description>
  <rdf:Description rdf:about="http://isdc.gfz-potsdam.de/ontology/SPASE-allowed_values.skos.owl#F-Region">
    <skos:broader rdf:resource="http://isdc.gfz-potsdam.de/ontology/SPASE-allowed_values.skos.owl#Ionosphere"/>
    <skos:inScheme rdf:resource="http://isdc.gfz-potsdam.de/ontology/SPASE-allowed_values.skos.owl#Observatory_Region"/>
    <rdf:type rdf:resource="http://www.w3.org/2004/02/skos/core#Concept"/>
    <rdf:type rdf:resource="http://www.w3.org/2002/07/owl#NamedIndividual"/>
    <skos:prefLabel xml:lang="en">F-Region</skos:prefLabel>
    <skos:inScheme rdf:resource="http://isdc.gfz-potsdam.de/ontology/SPASE-allowed_values.skos.owl#Observed_Region"/>
    <skos:definition xml:lang="en">A layer that contains ionized gases at a height of around 150-800 km above sea level, placing it
in the thermosphere. the F region has the highest concentration of free electrons and ions
anywhere in the atmosphere. It may be thought of as comprising two layers, the F1-and
F2-layers. One of several layers in the ionosphere. Also known as the Appleton layer.</skos:definition>
  </rdf:Description>
  <rdf:Description rdf:about="http://isdc.gfz-potsdam.de/ontology/SPASE-allowed_values.skos.owl#RTN">
    <skos:topConceptOf rdf:resource="http://isdc.gfz-potsdam.de/ontology/SPASE-allowed_values.skos.owl#Coordinate_System_Name"/>
    <skos:prefLabel xml:lang="en">RTN</skos:prefLabel>
    <skos:inScheme rdf:resource="http://isdc.gfz-potsdam.de/ontology/SPASE-allowed_values.skos.owl#Coordinate_System_Name"/>
    <rdf:type rdf:resource="http://www.w3.org/2004/02/skos/core#Concept"/>
    <rdf:type rdf:resource="http://www.w3.org/2002/07/owl#NamedIndividual"/>
    <skos:definition xml:lang="en">Radial Tangential Normal. Typically centered at a spacecraft. Used for IMF and plasma V
vectors. R (radial) axis is radially away from the Sun, T (tangential) axis is normal to the plane
formed by R and the Sun's spin vector, positive in the direction of planetary motion. N (normal)
is R x T.</skos:definition>
  </rdf:Description>
  <rdf:Description rdf:about="http://isdc.gfz-potsdam.de/ontology/SPASE-allowed_values.skos.owl#NCAR">
    <rdf:type rdf:resource="http://www.w3.org/2004/02/skos/core#Concept"/>
    <skos:inScheme rdf:resource="http://isdc.gfz-potsdam.de/ontology/SPASE-allowed_values.skos.owl#Format"/>
    <skos:definition xml:lang="en">The National Center for Atmospheric Research (NCAR) format. A complete description of that
standard is given in appendix C of the "Report on Establishment &amp; Operation of the Incoherent-
Scatter Data Base", dated August 23, 1984, obtainable from NCAR, P.O. Box 3000 Boulder,
Colorado 80307-3000.</skos:definition>
    <skos:topConceptOf rdf:resource="http://isdc.gfz-potsdam.de/ontology/SPASE-allowed_values.skos.owl#Format"/>
    <skos:prefLabel xml:lang="en">NCAR</skos:prefLabel>
    <rdf:type rdf:resource="http://www.w3.org/2002/07/owl#NamedIndividual"/>
  </rdf:Description>
  <rdf:Description rdf:about="http://isdc.gfz-potsdam.de/ontology/SPASE-allowed_values.skos.owl#Resonance_Sounder">
    <rdf:type rdf:resource="http://www.w3.org/2004/02/skos/core#Concept"/>
    <rdf:type rdf:resource="http://www.w3.org/2002/07/owl#NamedIndividual"/>
    <skos:prefLabel xml:lang="en">Resonance Sounder</skos:prefLabel>
    <skos:inScheme rdf:resource="http://isdc.gfz-potsdam.de/ontology/SPASE-allowed_values.skos.owl#Instrument_Type"/>
    <skos:definition xml:lang="en">A combination of a radio receiver and a pulsed transmitter used to study the plasma
surrounding a spacecraft by identifying resonances or cut-offs (of the wave dispersion relation),
whose frequencies are related to the ambient plasma density and magnetic field. When the
transmitter is off it is essentially a high frequency-resolution spectral power receiver.</skos:definition>
    <skos:topConceptOf rdf:resource="http://isdc.gfz-potsdam.de/ontology/SPASE-allowed_values.skos.owl#Instrument_Type"/>
  </rdf:Description>
  <rdf:Description rdf:about="http://isdc.gfz-potsdam.de/ontology/SPASE-allowed_values.skos.owl#Instrument_Mode">
    <skos:topConceptOf rdf:resource="http://isdc.gfz-potsdam.de/ontology/SPASE-allowed_values.skos.owl#Support_Quantity"/>
    <rdf:type rdf:resource="http://www.w3.org/2004/02/skos/core#Concept"/>
    <rdf:type rdf:resource="http://www.w3.org/2002/07/owl#NamedIndividual"/>
    <skos:inScheme rdf:resource="http://isdc.gfz-potsdam.de/ontology/SPASE-allowed_values.skos.owl#Support_Quantity"/>
    <skos:prefLabel xml:lang="en">Instrument Mode</skos:prefLabel>
    <skos:definition xml:lang="en">An indication of a state (mode) in which the instrument is operating. How a mode influences
the interpretation and representation of data is described in instrument related documentation.</skos:definition>
  </rdf:Description>
  <rdf:Description rdf:about="http://isdc.gfz-potsdam.de/ontology/SPASE-allowed_values.skos.owl#HEE">
    <skos:inScheme rdf:resource="http://isdc.gfz-potsdam.de/ontology/SPASE-allowed_values.skos.owl#Coordinate_System_Name"/>
    <skos:definition xml:lang="en">Heliocentric Earth Ecliptic - A coordinate system where the Z axis is normal to the ecliptic
plane, positive northward. X axis points from Sun to Earth. See Hapgood, 1992.</skos:definition>
    <rdf:type rdf:resource="http://www.w3.org/2004/02/skos/core#Concept"/>
    <rdf:type rdf:resource="http://www.w3.org/2002/07/owl#NamedIndividual"/>
    <skos:prefLabel xml:lang="en">HEE</skos:prefLabel>
    <skos:topConceptOf rdf:resource="http://isdc.gfz-potsdam.de/ontology/SPASE-allowed_values.skos.owl#Coordinate_System_Name"/>
  </rdf:Description>
  <rdf:Description rdf:about="http://isdc.gfz-potsdam.de/ontology/SPASE-allowed_values.skos.owl#IK">
    <skos:definition xml:lang="en">A measure of the length of a position or measured vector projected into the i-k (typically X-Z)
plane of the coordinate system.</skos:definition>
    <skos:broader rdf:resource="http://isdc.gfz-potsdam.de/ontology/SPASE-allowed_values.skos.owl#Projection"/>
    <skos:inScheme rdf:resource="http://isdc.gfz-potsdam.de/ontology/SPASE-allowed_values.skos.owl#Qualifier"/>
    <skos:prefLabel xml:lang="en">IK</skos:prefLabel>
    <rdf:type rdf:resource="http://www.w3.org/2004/02/skos/core#Concept"/>
    <rdf:type rdf:resource="http://www.w3.org/2002/07/owl#NamedIndividual"/>
  </rdf:Description>
  <rdf:Description rdf:about="http://isdc.gfz-potsdam.de/ontology/SPASE-allowed_values.skos.owl#Report">
    <skos:topConceptOf rdf:resource="http://isdc.gfz-potsdam.de/ontology/SPASE-allowed_values.skos.owl#Document_Type"/>
    <skos:inScheme rdf:resource="http://isdc.gfz-potsdam.de/ontology/SPASE-allowed_values.skos.owl#Document_Type"/>
    <skos:prefLabel xml:lang="en">Report</skos:prefLabel>
    <rdf:type rdf:resource="http://www.w3.org/2002/07/owl#NamedIndividual"/>
    <rdf:type rdf:resource="http://www.w3.org/2004/02/skos/core#Concept"/>
    <skos:definition xml:lang="en">A document which describes the findings of some individual or group.</skos:definition>
  </rdf:Description>
  <rdf:Description rdf:about="http://isdc.gfz-potsdam.de/ontology/SPASE-allowed_values.skos.owl#AC-Magnetic_Field">
    <rdf:type rdf:resource="http://www.w3.org/2004/02/skos/core#Concept"/>
    <rdf:type rdf:resource="http://www.w3.org/2002/07/owl#NamedIndividual"/>
    <skos:prefLabel xml:lang="en">AC-Magnetic Field</skos:prefLabel>
    <skos:definition xml:lang="en">Alternating magnetic field component of a wave.</skos:definition>
    <skos:topConceptOf rdf:resource="http://isdc.gfz-potsdam.de/ontology/SPASE-allowed_values.skos.owl#Wave_Quantity"/>
    <skos:inScheme rdf:resource="http://isdc.gfz-potsdam.de/ontology/SPASE-allowed_values.skos.owl#Wave_Quantity"/>
  </rdf:Description>
  <rdf:Description rdf:about="http://isdc.gfz-potsdam.de/ontology/SPASE-allowed_values.skos.owl#Layout">
    <skos:definition xml:lang="en">The structured arrangement of items in a collection.</skos:definition>
    <skos:topConceptOf rdf:resource="http://isdc.gfz-potsdam.de/ontology/SPASE-allowed_values.skos.owl#Source_Type"/>
    <skos:inScheme rdf:resource="http://isdc.gfz-potsdam.de/ontology/SPASE-allowed_values.skos.owl#Source_Type"/>
    <rdf:type rdf:resource="http://www.w3.org/2002/07/owl#NamedIndividual"/>
    <rdf:type rdf:resource="http://www.w3.org/2004/02/skos/core#Concept"/>
    <skos:prefLabel xml:lang="en">Layout</skos:prefLabel>
  </rdf:Description>
  <rdf:Description rdf:about="http://isdc.gfz-potsdam.de/ontology/SPASE-allowed_values.skos.owl#Positional">
    <skos:definition xml:lang="en">The specification of the location of an object or measurement within a reference coordinate
system. The position is usually expressed as a set of values corresponding to the location along
a set of orthogonal axes together with the date/time of the observation.</skos:definition>
    <skos:prefLabel xml:lang="en">Positional</skos:prefLabel>
    <skos:topConceptOf rdf:resource="http://isdc.gfz-potsdam.de/ontology/SPASE-allowed_values.skos.owl#Support_Quantity"/>
    <rdf:type rdf:resource="http://www.w3.org/2004/02/skos/core#Concept"/>
    <rdf:type rdf:resource="http://www.w3.org/2002/07/owl#NamedIndividual"/>
    <skos:inScheme rdf:resource="http://isdc.gfz-potsdam.de/ontology/SPASE-allowed_values.skos.owl#Support_Quantity"/>
  </rdf:Description>
  <rdf:Description rdf:about="http://isdc.gfz-potsdam.de/ontology/SPASE-allowed_values.skos.owl#PDF">
    <skos:inScheme rdf:resource="http://isdc.gfz-potsdam.de/ontology/SPASE-allowed_values.skos.owl#Format"/>
    <rdf:type rdf:resource="http://www.w3.org/2002/07/owl#NamedIndividual"/>
    <rdf:type rdf:resource="http://www.w3.org/2004/02/skos/core#Concept"/>
    <skos:topConceptOf rdf:resource="http://isdc.gfz-potsdam.de/ontology/SPASE-allowed_values.skos.owl#Format"/>
    <skos:prefLabel xml:lang="en">PDF</skos:prefLabel>
    <skos:definition xml:lang="en">A document expressed in the Portable Document Format (PDF) as defined by Adobe.</skos:definition>
  </rdf:Description>
  <rdf:Description rdf:about="http://isdc.gfz-potsdam.de/ontology/SPASE-allowed_values.skos.owl#SSE_L">
    <skos:prefLabel xml:lang="en">SSE_L</skos:prefLabel>
    <skos:inScheme rdf:resource="http://isdc.gfz-potsdam.de/ontology/SPASE-allowed_values.skos.owl#Coordinate_System_Name"/>
    <rdf:type rdf:resource="http://www.w3.org/2004/02/skos/core#Concept"/>
    <rdf:type rdf:resource="http://www.w3.org/2002/07/owl#NamedIndividual"/>
    <skos:definition xml:lang="en">Selenocentric Solar Ecliptic. The X axis points from the center of the Earth's moon to the sun,
the Z axis is normal to the ecliptic plane, positive northward. And the Y axis completes the
right-handed set of axes.</skos:definition>
    <skos:topConceptOf rdf:resource="http://isdc.gfz-potsdam.de/ontology/SPASE-allowed_values.skos.owl#Coordinate_System_Name"/>
  </rdf:Description>
  <rdf:Description rdf:about="http://isdc.gfz-potsdam.de/ontology/SPASE-allowed_values.skos.owl#Magnetic_Field">
    <rdf:type rdf:resource="http://www.w3.org/2004/02/skos/core#Concept"/>
    <skos:topConceptOf rdf:resource="http://isdc.gfz-potsdam.de/ontology/SPASE-allowed_values.skos.owl#Measurement_Type"/>
    <skos:inScheme rdf:resource="http://isdc.gfz-potsdam.de/ontology/SPASE-allowed_values.skos.owl#Measurement_Type"/>
    <skos:topConceptOf rdf:resource="http://isdc.gfz-potsdam.de/ontology/SPASE-allowed_values.skos.owl#Wave_Quantity"/>
    <skos:prefLabel xml:lang="en">Magnetic Field</skos:prefLabel>
    <skos:inScheme rdf:resource="http://isdc.gfz-potsdam.de/ontology/SPASE-allowed_values.skos.owl#Wave_Quantity"/>
    <skos:definition xml:lang="en">A region of space near a magnetized body where magnetic forces can be detected (as measured
by methods such as Zeeman splitting, etc.).</skos:definition>
    <rdf:type rdf:resource="http://www.w3.org/2002/07/owl#NamedIndividual"/>
  </rdf:Description>
  <rdf:Description rdf:about="http://isdc.gfz-potsdam.de/ontology/SPASE-allowed_values.skos.owl#Photosphere">
    <skos:inScheme rdf:resource="http://isdc.gfz-potsdam.de/ontology/SPASE-allowed_values.skos.owl#Observed_Region"/>
    <rdf:type rdf:resource="http://www.w3.org/2002/07/owl#NamedIndividual"/>
    <skos:broader rdf:resource="http://isdc.gfz-potsdam.de/ontology/SPASE-allowed_values.skos.owl#Sun"/>
    <rdf:type rdf:resource="http://www.w3.org/2004/02/skos/core#Concept"/>
    <skos:definition xml:lang="en">The atmospheric layer of the Sun or a star from which continuum radiation, especially optical,
is emitted to space. For the Sun, the photosphere is about 500 km thick.</skos:definition>
    <skos:prefLabel xml:lang="en">Photosphere</skos:prefLabel>
    <skos:inScheme rdf:resource="http://isdc.gfz-potsdam.de/ontology/SPASE-allowed_values.skos.owl#Observatory_Region"/>
  </rdf:Description>
  <rdf:Description rdf:about="http://isdc.gfz-potsdam.de/ontology/SPASE-allowed_values.skos.owl#MHD">
    <skos:prefLabel xml:lang="en">Hydrodynamic waves in a magnetized plasma in which the background magnetic field plays a
key role in controlling the wave propagation characteristics.</skos:prefLabel>
    <rdf:type rdf:resource="http://www.w3.org/2002/07/owl#NamedIndividual"/>
    <rdf:type rdf:resource="http://www.w3.org/2004/02/skos/core#Concept"/>
    <skos:prefLabel>MHD</skos:prefLabel>
    <skos:topConceptOf rdf:resource="http://isdc.gfz-potsdam.de/ontology/SPASE-allowed_values.skos.owl#Wave_Type"/>
    <skos:inScheme rdf:resource="http://isdc.gfz-potsdam.de/ontology/SPASE-allowed_values.skos.owl#Wave_Type"/>
  </rdf:Description>
  <rdf:Description rdf:about="http://isdc.gfz-potsdam.de/ontology/SPASE-allowed_values.skos.owl#Archive_Specialist">
    <skos:inScheme rdf:resource="http://isdc.gfz-potsdam.de/ontology/SPASE-allowed_values.skos.owl#Role"/>
    <skos:prefLabel xml:lang="en">Archive Specialist</skos:prefLabel>
    <skos:definition xml:lang="en">An individual who is an expert on a collection of resources and may also be knowledgeable of
the phenomenon and related physics represented by the resources. This includes librarians,
curators, archive scientists and other experts.</skos:definition>
    <rdf:type rdf:resource="http://www.w3.org/2002/07/owl#NamedIndividual"/>
    <rdf:type rdf:resource="http://www.w3.org/2004/02/skos/core#Concept"/>
    <skos:topConceptOf rdf:resource="http://isdc.gfz-potsdam.de/ontology/SPASE-allowed_values.skos.owl#Role"/>
  </rdf:Description>
  <rdf:Description rdf:about="http://isdc.gfz-potsdam.de/ontology/SPASE-allowed_values.skos.owl#Sector_Boundary_Crossing">
    <rdf:type rdf:resource="http://www.w3.org/2004/02/skos/core#Concept"/>
    <skos:inScheme rdf:resource="http://isdc.gfz-potsdam.de/ontology/SPASE-allowed_values.skos.owl#Phenomenon_Type"/>
    <skos:topConceptOf rdf:resource="http://isdc.gfz-potsdam.de/ontology/SPASE-allowed_values.skos.owl#Phenomenon_Type"/>
    <rdf:type rdf:resource="http://www.w3.org/2002/07/owl#NamedIndividual"/>
    <skos:prefLabel xml:lang="en">Sector Boundary Crossing</skos:prefLabel>
    <skos:definition xml:lang="en">A sector boundary crossing is a transit by a spacecraft across the heliospheric current sheet
separating the dominantly outward (away-from-the-sun) interplanetary magnetic field of one
hemisphere of the heliosphere from the dominantly inward (toward-the-sun) polarity of the
other hemisphere. Such crossings have multi-day intervals of opposite IMF dominant polarities
on either side.</skos:definition>
  </rdf:Description>
  <rdf:Description rdf:about="http://isdc.gfz-potsdam.de/ontology/SPASE-allowed_values.skos.owl#None">
    <rdf:type rdf:resource="http://www.w3.org/2004/02/skos/core#Concept"/>
    <rdf:type rdf:resource="http://www.w3.org/2002/07/owl#NamedIndividual"/>
    <skos:prefLabel xml:lang="en">None</skos:prefLabel>
    <skos:topConceptOf rdf:resource="http://isdc.gfz-potsdam.de/ontology/SPASE-allowed_values.skos.owl#Encoding"/>
    <skos:definition xml:lang="en">A lack or absence of anything.</skos:definition>
    <skos:inScheme rdf:resource="http://isdc.gfz-potsdam.de/ontology/SPASE-allowed_values.skos.owl#Encoding"/>
  </rdf:Description>
  <rdf:Description rdf:about="http://isdc.gfz-potsdam.de/ontology/SPASE-allowed_values.skos.owl#Polarization">
    <skos:definition xml:lang="en">Direction of the electric vector of an electromagnetic wave. The wave can be linearly polarized
in any direction perpendicular to the direction of travel, circularly polarized (clockwise or
counterclockwise), unpolarized, or mixtures of the above.</skos:definition>
    <rdf:type rdf:resource="http://www.w3.org/2002/07/owl#NamedIndividual"/>
    <skos:prefLabel xml:lang="en">Polarization</skos:prefLabel>
    <skos:topConceptOf rdf:resource="http://isdc.gfz-potsdam.de/ontology/SPASE-allowed_values.skos.owl#Wave_Quantity"/>
    <skos:inScheme rdf:resource="http://isdc.gfz-potsdam.de/ontology/SPASE-allowed_values.skos.owl#Wave_Quantity"/>
    <rdf:type rdf:resource="http://www.w3.org/2004/02/skos/core#Concept"/>
  </rdf:Description>
  <rdf:Description rdf:about="http://isdc.gfz-potsdam.de/ontology/SPASE-allowed_values.skos.owl#Mass_Number">
    <skos:inScheme rdf:resource="http://isdc.gfz-potsdam.de/ontology/SPASE-allowed_values.skos.owl#Particle_Quantity"/>
    <rdf:type rdf:resource="http://www.w3.org/2004/02/skos/core#Concept"/>
    <rdf:type rdf:resource="http://www.w3.org/2002/07/owl#NamedIndividual"/>
    <skos:definition xml:lang="en">The total number of protons and neutrons (together known as nucleons) in an atomic nucleus.</skos:definition>
    <skos:topConceptOf rdf:resource="http://isdc.gfz-potsdam.de/ontology/SPASE-allowed_values.skos.owl#Particle_Quantity"/>
    <skos:prefLabel xml:lang="en">Mass Number</skos:prefLabel>
  </rdf:Description>
  <rdf:Description rdf:about="http://isdc.gfz-potsdam.de/ontology/SPASE-allowed_values.skos.owl#Image_Intensity">
    <skos:topConceptOf rdf:resource="http://isdc.gfz-potsdam.de/ontology/SPASE-allowed_values.skos.owl#Measurement_Type"/>
    <rdf:type rdf:resource="http://www.w3.org/2002/07/owl#NamedIndividual"/>
    <rdf:type rdf:resource="http://www.w3.org/2004/02/skos/core#Concept"/>
    <skos:prefLabel xml:lang="en">Image Intensity</skos:prefLabel>
    <skos:definition xml:lang="en">Measurements of the two-dimensional distribution of the intensity of photons from some region
or object such as the Sun or the polar auroral regions; can be in any wavelength band, and
polarized, etc.</skos:definition>
    <skos:inScheme rdf:resource="http://isdc.gfz-potsdam.de/ontology/SPASE-allowed_values.skos.owl#Measurement_Type"/>
  </rdf:Description>
  <rdf:Description rdf:about="http://isdc.gfz-potsdam.de/ontology/SPASE-allowed_values.skos.owl#Counts">
    <skos:definition xml:lang="en">The number of detection events occurring in a detector over the detector accumulation time.</skos:definition>
    <skos:inScheme rdf:resource="http://isdc.gfz-potsdam.de/ontology/SPASE-allowed_values.skos.owl#Particle_Quantity"/>
    <skos:topConceptOf rdf:resource="http://isdc.gfz-potsdam.de/ontology/SPASE-allowed_values.skos.owl#Particle_Quantity"/>
    <skos:prefLabel xml:lang="en">Counts</skos:prefLabel>
    <rdf:type rdf:resource="http://www.w3.org/2004/02/skos/core#Concept"/>
    <rdf:type rdf:resource="http://www.w3.org/2002/07/owl#NamedIndividual"/>
  </rdf:Description>
  <rdf:Description rdf:about="http://isdc.gfz-potsdam.de/ontology/SPASE-allowed_values.skos.owl#EIT_Wave">
    <skos:topConceptOf rdf:resource="http://isdc.gfz-potsdam.de/ontology/SPASE-allowed_values.skos.owl#Phenomenon_Type"/>
    <skos:definition xml:lang="en">A wave in the corona of the Sun which produce shock waves on the Sun's chromosphere
(Moreton Waves). EIT Waves are produced by large solar flare and expand outward at about
1,000 km/s. It usually appears as a slowly moving diffuse arc of brightening in H-alpha, and
may travel for several hundred thousand km.</skos:definition>
    <rdf:type rdf:resource="http://www.w3.org/2002/07/owl#NamedIndividual"/>
    <rdf:type rdf:resource="http://www.w3.org/2004/02/skos/core#Concept"/>
    <skos:prefLabel xml:lang="en">EIT Wave</skos:prefLabel>
    <skos:inScheme rdf:resource="http://isdc.gfz-potsdam.de/ontology/SPASE-allowed_values.skos.owl#Phenomenon_Type"/>
  </rdf:Description>
  <rdf:Description rdf:about="http://isdc.gfz-potsdam.de/ontology/SPASE-allowed_values.skos.owl#Velocity">
    <skos:inScheme rdf:resource="http://isdc.gfz-potsdam.de/ontology/SPASE-allowed_values.skos.owl#Wave_Quantity"/>
    <skos:inScheme rdf:resource="http://isdc.gfz-potsdam.de/ontology/SPASE-allowed_values.skos.owl#Support_Quantity"/>
    <skos:topConceptOf rdf:resource="http://isdc.gfz-potsdam.de/ontology/SPASE-allowed_values.skos.owl#Support_Quantity"/>
    <skos:topConceptOf rdf:resource="http://isdc.gfz-potsdam.de/ontology/SPASE-allowed_values.skos.owl#Wave_Quantity"/>
    <rdf:type rdf:resource="http://www.w3.org/2002/07/owl#NamedIndividual"/>
    <skos:prefLabel xml:lang="en">Velocity</skos:prefLabel>
    <skos:topConceptOf rdf:resource="http://isdc.gfz-potsdam.de/ontology/SPASE-allowed_values.skos.owl#Particle_Quantity"/>
    <rdf:type rdf:resource="http://www.w3.org/2004/02/skos/core#Concept"/>
    <skos:definition xml:lang="en">Rate of change of position. Also used for the average velocity of a collection of particles, also
referred to as "bulk velocity".</skos:definition>
    <skos:inScheme rdf:resource="http://isdc.gfz-potsdam.de/ontology/SPASE-allowed_values.skos.owl#Particle_Quantity"/>
  </rdf:Description>
  <rdf:Description rdf:about="http://isdc.gfz-potsdam.de/ontology/SPASE-allowed_values.skos.owl#Spectrum">
    <rdf:type rdf:resource="http://www.w3.org/2004/02/skos/core#Concept"/>
    <skos:prefLabel xml:lang="en">Spectrum</skos:prefLabel>
    <skos:topConceptOf rdf:resource="http://isdc.gfz-potsdam.de/ontology/SPASE-allowed_values.skos.owl#Measurement_Type"/>
    <skos:inScheme rdf:resource="http://isdc.gfz-potsdam.de/ontology/SPASE-allowed_values.skos.owl#Measurement_Type"/>
    <skos:definition xml:lang="en">The distribution of a characteristic of a physical system or phenomenon, such as the energy
emitted by a radiant source, arranged in the order of wavelengths.</skos:definition>
    <rdf:type rdf:resource="http://www.w3.org/2002/07/owl#NamedIndividual"/>
  </rdf:Description>
  <rdf:Description rdf:about="http://isdc.gfz-potsdam.de/ontology/SPASE-allowed_values.skos.owl#H-alpha">
    <rdf:type rdf:resource="http://www.w3.org/2004/02/skos/core#Concept"/>
    <rdf:type rdf:resource="http://www.w3.org/2002/07/owl#NamedIndividual"/>
    <skos:topConceptOf rdf:resource="http://isdc.gfz-potsdam.de/ontology/SPASE-allowed_values.skos.owl#Spectral_Range"/>
    <skos:prefLabel xml:lang="en">H-alpha</skos:prefLabel>
    <skos:inScheme rdf:resource="http://isdc.gfz-potsdam.de/ontology/SPASE-allowed_values.skos.owl#Spectral_Range"/>
    <skos:definition xml:lang="en">A spectrum with a wavelength range centered at 656.3 nm. VSO nickname: H-alpha image with
a spectrum range of of 655.8 nm to 656.8 nm.</skos:definition>
  </rdf:Description>
  <rdf:Description rdf:about="http://isdc.gfz-potsdam.de/ontology/SPASE-allowed_values.skos.owl#Microchannel_Plate">
    <skos:inScheme rdf:resource="http://isdc.gfz-potsdam.de/ontology/SPASE-allowed_values.skos.owl#Instrument_Type"/>
    <rdf:type rdf:resource="http://www.w3.org/2004/02/skos/core#Concept"/>
    <rdf:type rdf:resource="http://www.w3.org/2002/07/owl#NamedIndividual"/>
    <skos:topConceptOf rdf:resource="http://isdc.gfz-potsdam.de/ontology/SPASE-allowed_values.skos.owl#Instrument_Type"/>
    <skos:prefLabel xml:lang="en">Microchannel Plate</skos:prefLabel>
    <skos:definition xml:lang="en">An instrument used for the detection of elementary particles, ions, ultraviolet rays and soft
X-rays constructed from very thin conductive glass capillaries.</skos:definition>
  </rdf:Description>
  <rdf:Description rdf:about="http://isdc.gfz-potsdam.de/ontology/SPASE-allowed_values.skos.owl#MAG">
    <skos:prefLabel xml:lang="en">MAG</skos:prefLabel>
    <skos:topConceptOf rdf:resource="http://isdc.gfz-potsdam.de/ontology/SPASE-allowed_values.skos.owl#Coordinate_System_Name"/>
    <rdf:type rdf:resource="http://www.w3.org/2002/07/owl#NamedIndividual"/>
    <rdf:type rdf:resource="http://www.w3.org/2004/02/skos/core#Concept"/>
    <skos:definition xml:lang="en">Geomagnetic - geocentric. Z axis is parallel to the geomagnetic dipole axis, positive north. X is
in the plane defined by the Z axis and the Earth's rotation axis. If N is a unit vector from the
Earth's center to the north geographic pole, the signs of the X and Y axes are given by Y = N x
Z, X = Y x Z.. See Russell, 1971, and &lt;http://cdpp.cnes.fr/00428.pdf&gt;.</skos:definition>
    <skos:inScheme rdf:resource="http://isdc.gfz-potsdam.de/ontology/SPASE-allowed_values.skos.owl#Coordinate_System_Name"/>
  </rdf:Description>
  <rdf:Description rdf:about="http://isdc.gfz-potsdam.de/ontology/SPASE-allowed_values.skos.owl#Irradiance">
    <skos:prefLabel xml:lang="en">Irradiance</skos:prefLabel>
    <rdf:type rdf:resource="http://www.w3.org/2004/02/skos/core#Concept"/>
    <rdf:type rdf:resource="http://www.w3.org/2002/07/owl#NamedIndividual"/>
    <skos:definition xml:lang="en">Irradiance - A radiometric term for the power of electromagnetic radiation at a surface, per unit
area. "Irradiance" is used when the electromagnetic radiation is incident on the surface.
Irradiance data may be reported in any units (i.e. counts/s) due to, for example, being at a
particular wavelength, or to being a not-fully-calibrated relative measurement.</skos:definition>
    <skos:inScheme rdf:resource="http://isdc.gfz-potsdam.de/ontology/SPASE-allowed_values.skos.owl#Measurement_Type"/>
    <skos:topConceptOf rdf:resource="http://isdc.gfz-potsdam.de/ontology/SPASE-allowed_values.skos.owl#Measurement_Type"/>
  </rdf:Description>
  <rdf:Description rdf:about="http://isdc.gfz-potsdam.de/ontology/SPASE-allowed_values.skos.owl#AC-Electric_Field">
    <skos:inScheme rdf:resource="http://isdc.gfz-potsdam.de/ontology/SPASE-allowed_values.skos.owl#Wave_Quantity"/>
    <skos:definition xml:lang="en">Alternating electric field component of a wave.</skos:definition>
    <rdf:type rdf:resource="http://www.w3.org/2004/02/skos/core#Concept"/>
    <skos:prefLabel xml:lang="en">AC-Electric Field</skos:prefLabel>
    <rdf:type rdf:resource="http://www.w3.org/2002/07/owl#NamedIndividual"/>
    <skos:topConceptOf rdf:resource="http://isdc.gfz-potsdam.de/ontology/SPASE-allowed_values.skos.owl#Wave_Quantity"/>
  </rdf:Description>
  <rdf:Description rdf:about="http://isdc.gfz-potsdam.de/ontology/SPASE-allowed_values.skos.owl#HGI">
    <skos:prefLabel xml:lang="en">HGI</skos:prefLabel>
    <skos:topConceptOf rdf:resource="http://isdc.gfz-potsdam.de/ontology/SPASE-allowed_values.skos.owl#Coordinate_System_Name"/>
    <skos:inScheme rdf:resource="http://isdc.gfz-potsdam.de/ontology/SPASE-allowed_values.skos.owl#Coordinate_System_Name"/>
    <skos:definition xml:lang="en">Heliographic Inertial - A heliocentric coordinate system where the Z axis is normal to the solar
equatorial plane, positive northward. X axis is along the intersection line between solar
equatorial and ecliptic planes. The X axis was positive at SE longitude of 74.367 deg on Jan 1,
1900. (See SE below.) See &lt;http://nssdc.gsfc.nasa.gov/space/helios/coor_des.html&gt;.</skos:definition>
    <rdf:type rdf:resource="http://www.w3.org/2004/02/skos/core#Concept"/>
    <rdf:type rdf:resource="http://www.w3.org/2002/07/owl#NamedIndividual"/>
  </rdf:Description>
  <rdf:Description rdf:about="http://isdc.gfz-potsdam.de/ontology/SPASE-allowed_values.skos.owl#CDF">
    <skos:definition xml:lang="en">Common Data Format (CDF). A binary storage format developed at Goddard Space Flight
Center (GSFC).</skos:definition>
    <skos:prefLabel xml:lang="en">CDF</skos:prefLabel>
    <skos:topConceptOf rdf:resource="http://isdc.gfz-potsdam.de/ontology/SPASE-allowed_values.skos.owl#Format"/>
    <rdf:type rdf:resource="http://www.w3.org/2004/02/skos/core#Concept"/>
    <rdf:type rdf:resource="http://www.w3.org/2002/07/owl#NamedIndividual"/>
    <skos:inScheme rdf:resource="http://isdc.gfz-potsdam.de/ontology/SPASE-allowed_values.skos.owl#Format"/>
  </rdf:Description>
  <rdf:Description rdf:about="http://isdc.gfz-potsdam.de/ontology/SPASE-allowed_values.skos.owl#Photon">
    <skos:inScheme rdf:resource="http://isdc.gfz-potsdam.de/ontology/SPASE-allowed_values.skos.owl#Wave_Type"/>
    <skos:topConceptOf rdf:resource="http://isdc.gfz-potsdam.de/ontology/SPASE-allowed_values.skos.owl#Wave_Type"/>
    <skos:definition xml:lang="en">Electromagnetic waves detected by techniques that utilize their corpuscular character (e.g.,
CCD, CMOS, photomultipliers).</skos:definition>
    <skos:prefLabel>Photon</skos:prefLabel>
    <rdf:type rdf:resource="http://www.w3.org/2002/07/owl#NamedIndividual"/>
    <rdf:type rdf:resource="http://www.w3.org/2004/02/skos/core#Concept"/>
  </rdf:Description>
  <rdf:Description rdf:about="http://isdc.gfz-potsdam.de/ontology/SPASE-allowed_values.skos.owl#Number_Density">
    <rdf:type rdf:resource="http://www.w3.org/2004/02/skos/core#Concept"/>
    <skos:prefLabel xml:lang="en">Number Density</skos:prefLabel>
    <skos:definition xml:lang="en">The number of particles per unit volume.</skos:definition>
    <skos:topConceptOf rdf:resource="http://isdc.gfz-potsdam.de/ontology/SPASE-allowed_values.skos.owl#Particle_Quantity"/>
    <skos:inScheme rdf:resource="http://isdc.gfz-potsdam.de/ontology/SPASE-allowed_values.skos.owl#Particle_Quantity"/>
    <rdf:type rdf:resource="http://www.w3.org/2002/07/owl#NamedIndividual"/>
  </rdf:Description>
  <rdf:Description rdf:about="http://isdc.gfz-potsdam.de/ontology/SPASE-allowed_values.skos.owl#Energetic_Particles">
    <skos:prefLabel xml:lang="en">Energetic Particles</skos:prefLabel>
    <rdf:type rdf:resource="http://www.w3.org/2004/02/skos/core#Concept"/>
    <rdf:type rdf:resource="http://www.w3.org/2002/07/owl#NamedIndividual"/>
    <skos:definition xml:lang="en">Pieces of matter that are moving very fast. Energetic particles include protons, electrons,
neutrons, neutrinos, the nuclei of atoms, and other sub-atomic particles.</skos:definition>
    <skos:inScheme rdf:resource="http://isdc.gfz-potsdam.de/ontology/SPASE-allowed_values.skos.owl#Measurement_Type"/>
    <skos:topConceptOf rdf:resource="http://isdc.gfz-potsdam.de/ontology/SPASE-allowed_values.skos.owl#Measurement_Type"/>
  </rdf:Description>
  <rdf:Description rdf:about="http://isdc.gfz-potsdam.de/ontology/SPASE-allowed_values.skos.owl#Log_Scale">
    <skos:inScheme rdf:resource="http://isdc.gfz-potsdam.de/ontology/SPASE-allowed_values.skos.owl#Scale_Type"/>
    <skos:topConceptOf rdf:resource="http://isdc.gfz-potsdam.de/ontology/SPASE-allowed_values.skos.owl#Scale_Type"/>
    <skos:definition xml:lang="en">Intervals which are spaced proportionally to the logarithms of the values being represented.</skos:definition>
    <skos:prefLabel xml:lang="en">Log Scale</skos:prefLabel>
    <rdf:type rdf:resource="http://www.w3.org/2004/02/skos/core#Concept"/>
    <rdf:type rdf:resource="http://www.w3.org/2002/07/owl#NamedIndividual"/>
  </rdf:Description>
  <rdf:Description rdf:about="http://isdc.gfz-potsdam.de/ontology/SPASE-allowed_values.skos.owl#SR">
    <skos:topConceptOf rdf:resource="http://isdc.gfz-potsdam.de/ontology/SPASE-allowed_values.skos.owl#Coordinate_System_Name"/>
    <skos:definition xml:lang="en">Spin Reference - A special case of a Spacecraft (SC) coordinate system for a spinning
spacecraft. Z is parallel to the spacecraft spin vector. X and Y rotate with the spacecraft. See
&lt;http://cdpp.cnes.fr/00428.pdf&gt;.</skos:definition>
    <rdf:type rdf:resource="http://www.w3.org/2002/07/owl#NamedIndividual"/>
    <skos:prefLabel xml:lang="en">SR</skos:prefLabel>
    <skos:inScheme rdf:resource="http://isdc.gfz-potsdam.de/ontology/SPASE-allowed_values.skos.owl#Coordinate_System_Name"/>
    <rdf:type rdf:resource="http://www.w3.org/2004/02/skos/core#Concept"/>
  </rdf:Description>
  <rdf:Description rdf:about="http://isdc.gfz-potsdam.de/ontology/SPASE-allowed_values.skos.owl#Ephemeris">
    <skos:inScheme rdf:resource="http://isdc.gfz-potsdam.de/ontology/SPASE-allowed_values.skos.owl#Measurement_Type"/>
    <skos:prefLabel xml:lang="en">Ephemeris</skos:prefLabel>
    <rdf:type rdf:resource="http://www.w3.org/2004/02/skos/core#Concept"/>
    <rdf:type rdf:resource="http://www.w3.org/2002/07/owl#NamedIndividual"/>
    <skos:topConceptOf rdf:resource="http://isdc.gfz-potsdam.de/ontology/SPASE-allowed_values.skos.owl#Measurement_Type"/>
    <skos:definition xml:lang="en">The spatial coordinates of a body as a function of time. When used as an Instrument Type it
represents the process or methods used to generate spatial coordinates.</skos:definition>
  </rdf:Description>
  <rdf:Description rdf:about="http://isdc.gfz-potsdam.de/ontology/SPASE-allowed_values.skos.owl#Field-Aligned">
    <skos:topConceptOf rdf:resource="http://isdc.gfz-potsdam.de/ontology/SPASE-allowed_values.skos.owl#Qualifier"/>
    <rdf:type rdf:resource="http://www.w3.org/2004/02/skos/core#Concept"/>
    <skos:inScheme rdf:resource="http://isdc.gfz-potsdam.de/ontology/SPASE-allowed_values.skos.owl#Qualifier"/>
    <rdf:type rdf:resource="http://www.w3.org/2002/07/owl#NamedIndividual"/>
    <skos:definition xml:lang="en">The component of a quantity which is oriented in the same direction of a field.</skos:definition>
    <skos:prefLabel xml:lang="en">Field-Aligned</skos:prefLabel>
  </rdf:Description>
  <rdf:Description rdf:about="http://isdc.gfz-potsdam.de/ontology/SPASE-allowed_values.skos.owl#Parallel">
    <skos:prefLabel xml:lang="en">Parallel</skos:prefLabel>
    <skos:topConceptOf rdf:resource="http://isdc.gfz-potsdam.de/ontology/SPASE-allowed_values.skos.owl#Qualifier"/>
    <skos:definition xml:lang="en">Having the same direction as a given direction.</skos:definition>
    <skos:inScheme rdf:resource="http://isdc.gfz-potsdam.de/ontology/SPASE-allowed_values.skos.owl#Qualifier"/>
    <rdf:type rdf:resource="http://www.w3.org/2002/07/owl#NamedIndividual"/>
    <rdf:type rdf:resource="http://www.w3.org/2004/02/skos/core#Concept"/>
  </rdf:Description>
  <rdf:Description rdf:about="http://isdc.gfz-potsdam.de/ontology/SPASE-allowed_values.skos.owl#Equatorial_Region">
    <skos:definition xml:lang="en">A region centered on the equator and limited in latitude by approximately 23 degrees north and
south of the equator.</skos:definition>
    <skos:inScheme rdf:resource="http://isdc.gfz-potsdam.de/ontology/SPASE-allowed_values.skos.owl#Observed_Region"/>
    <skos:prefLabel xml:lang="en">Equatorial Region</skos:prefLabel>
    <rdf:type rdf:resource="http://www.w3.org/2004/02/skos/core#Concept"/>
    <rdf:type rdf:resource="http://www.w3.org/2002/07/owl#NamedIndividual"/>
    <skos:broader rdf:resource="http://isdc.gfz-potsdam.de/ontology/SPASE-allowed_values.skos.owl#Near_Surface"/>
    <skos:inScheme rdf:resource="http://isdc.gfz-potsdam.de/ontology/SPASE-allowed_values.skos.owl#Observatory_Region"/>
  </rdf:Description>
  <rdf:Description rdf:about="http://isdc.gfz-potsdam.de/ontology/SPASE-allowed_values.skos.owl#Passive">
    <rdf:type rdf:resource="http://www.w3.org/2002/07/owl#NamedIndividual"/>
    <rdf:type rdf:resource="http://www.w3.org/2004/02/skos/core#Concept"/>
    <skos:broader rdf:resource="http://isdc.gfz-potsdam.de/ontology/SPASE-allowed_values.skos.owl#Waves"/>
    <skos:prefLabel xml:lang="en">Passive</skos:prefLabel>
    <skos:inScheme rdf:resource="http://isdc.gfz-potsdam.de/ontology/SPASE-allowed_values.skos.owl#Measurement_Type"/>
    <skos:definition xml:lang="en">Movement or effect produced by outside influence. A passive measurement is one which does
not produce a transmission or excitation as a part of the measurement cycle.</skos:definition>
  </rdf:Description>
  <rdf:Description rdf:about="http://isdc.gfz-potsdam.de/ontology/SPASE-allowed_values.skos.owl#Heliosheath">
    <skos:inScheme rdf:resource="http://isdc.gfz-potsdam.de/ontology/SPASE-allowed_values.skos.owl#Observed_Region"/>
    <skos:definition xml:lang="en">The region extending radially outward from the heliospheric termination shock and in which
the decelerated solar wind plasma is still significant.</skos:definition>
    <skos:broader rdf:resource="http://isdc.gfz-potsdam.de/ontology/SPASE-allowed_values.skos.owl#Heliosphere"/>
    <skos:inScheme rdf:resource="http://isdc.gfz-potsdam.de/ontology/SPASE-allowed_values.skos.owl#Observatory_Region"/>
    <rdf:type rdf:resource="http://www.w3.org/2002/07/owl#NamedIndividual"/>
    <rdf:type rdf:resource="http://www.w3.org/2004/02/skos/core#Concept"/>
    <skos:prefLabel xml:lang="en">Heliosheath</skos:prefLabel>
  </rdf:Description>
  <rdf:Description rdf:about="http://isdc.gfz-potsdam.de/ontology/SPASE-allowed_values.skos.owl#Flow_Speed">
    <skos:prefLabel xml:lang="en">Flow Speed</skos:prefLabel>
    <skos:definition xml:lang="en">The rate at which particles or energy is passing through a unit area in a unit time.</skos:definition>
    <rdf:type rdf:resource="http://www.w3.org/2002/07/owl#NamedIndividual"/>
    <rdf:type rdf:resource="http://www.w3.org/2004/02/skos/core#Concept"/>
    <skos:topConceptOf rdf:resource="http://isdc.gfz-potsdam.de/ontology/SPASE-allowed_values.skos.owl#Particle_Quantity"/>
    <skos:inScheme rdf:resource="http://isdc.gfz-potsdam.de/ontology/SPASE-allowed_values.skos.owl#Particle_Quantity"/>
  </rdf:Description>
  <rdf:Description rdf:about="http://isdc.gfz-potsdam.de/ontology/SPASE-allowed_values.skos.owl#Magnetotail">
    <skos:inScheme rdf:resource="http://isdc.gfz-potsdam.de/ontology/SPASE-allowed_values.skos.owl#Observed_Region"/>
    <skos:definition xml:lang="en">The region on the night side of the body where the magnetic filed is stretched backwards by the
force of the solar wind. For Earth, the magnetotail begins at a night-side radial distance of 10
Re (X &gt; -10Re).</skos:definition>
    <skos:broader rdf:resource="http://isdc.gfz-potsdam.de/ontology/SPASE-allowed_values.skos.owl#Magnetosphere"/>
    <rdf:type rdf:resource="http://www.w3.org/2004/02/skos/core#Concept"/>
    <rdf:type rdf:resource="http://www.w3.org/2002/07/owl#NamedIndividual"/>
    <skos:inScheme rdf:resource="http://isdc.gfz-potsdam.de/ontology/SPASE-allowed_values.skos.owl#Observatory_Region"/>
    <skos:prefLabel xml:lang="en">Magnetotail</skos:prefLabel>
  </rdf:Description>
  <rdf:Description rdf:about="http://isdc.gfz-potsdam.de/ontology/SPASE-allowed_values.skos.owl#Mesosphere">
    <skos:inScheme rdf:resource="http://isdc.gfz-potsdam.de/ontology/SPASE-allowed_values.skos.owl#Observed_Region"/>
    <skos:definition xml:lang="en">The layer of the atmosphere that extends from the Stratosphere to a range of 80 km to 85 km,
temperature decreasing with height.</skos:definition>
    <skos:prefLabel xml:lang="en">Mesosphere</skos:prefLabel>
    <skos:broader rdf:resource="http://isdc.gfz-potsdam.de/ontology/SPASE-allowed_values.skos.owl#Near_Surface"/>
    <skos:inScheme rdf:resource="http://isdc.gfz-potsdam.de/ontology/SPASE-allowed_values.skos.owl#Observatory_Region"/>
    <rdf:type rdf:resource="http://www.w3.org/2004/02/skos/core#Concept"/>
    <rdf:type rdf:resource="http://www.w3.org/2002/07/owl#NamedIndividual"/>
  </rdf:Description>
  <rdf:Description rdf:about="http://isdc.gfz-potsdam.de/ontology/SPASE-allowed_values.skos.owl#Online">
    <skos:inScheme rdf:resource="http://isdc.gfz-potsdam.de/ontology/SPASE-allowed_values.skos.owl#Availability"/>
    <rdf:type rdf:resource="http://www.w3.org/2002/07/owl#NamedIndividual"/>
    <rdf:type rdf:resource="http://www.w3.org/2004/02/skos/core#Concept"/>
    <skos:prefLabel xml:lang="en">Online</skos:prefLabel>
    <skos:definition xml:lang="en">Directly accessible electronically.</skos:definition>
    <skos:topConceptOf rdf:resource="http://isdc.gfz-potsdam.de/ontology/SPASE-allowed_values.skos.owl#Availability"/>
  </rdf:Description>
  <rdf:Description rdf:about="http://isdc.gfz-potsdam.de/ontology/SPASE-allowed_values.skos.owl#Stream_Interaction_Region">
    <skos:prefLabel xml:lang="en">Stream Interaction Region</skos:prefLabel>
    <skos:topConceptOf rdf:resource="http://isdc.gfz-potsdam.de/ontology/SPASE-allowed_values.skos.owl#Phenomenon_Type"/>
    <rdf:type rdf:resource="http://www.w3.org/2002/07/owl#NamedIndividual"/>
    <rdf:type rdf:resource="http://www.w3.org/2004/02/skos/core#Concept"/>
    <skos:inScheme rdf:resource="http://isdc.gfz-potsdam.de/ontology/SPASE-allowed_values.skos.owl#Phenomenon_Type"/>
    <skos:definition xml:lang="en">The region (SIR) where two solar wind streams, typically having differing characteristics and
solar sources, abut up against (and possibly partially interpenetrate) each other.</skos:definition>
  </rdf:Description>
  <rdf:Description rdf:about="http://isdc.gfz-potsdam.de/ontology/SPASE-allowed_values.skos.owl#Raw">
    <skos:inScheme rdf:resource="http://isdc.gfz-potsdam.de/ontology/SPASE-allowed_values.skos.owl#Processing_Level"/>
    <rdf:type rdf:resource="http://www.w3.org/2002/07/owl#NamedIndividual"/>
    <skos:definition xml:lang="en">Data in its original state with no processing to account for calibration!!!</skos:definition>
    <rdf:type rdf:resource="http://www.w3.org/2004/02/skos/core#Concept"/>
    <skos:topConceptOf rdf:resource="http://isdc.gfz-potsdam.de/ontology/SPASE-allowed_values.skos.owl#Processing_Level"/>
    <skos:prefLabel xml:lang="en">Raw</skos:prefLabel>
  </rdf:Description>
  <rdf:Description rdf:about="http://isdc.gfz-potsdam.de/ontology/SPASE-allowed_values.skos.owl#Ancillary">
    <skos:topConceptOf rdf:resource="http://isdc.gfz-potsdam.de/ontology/SPASE-allowed_values.skos.owl#Source_Type"/>
    <rdf:type rdf:resource="http://www.w3.org/2004/02/skos/core#Concept"/>
    <rdf:type rdf:resource="http://www.w3.org/2002/07/owl#NamedIndividual"/>
    <skos:definition xml:lang="en">A complementary item which can be subordinate, subsidiary, auxiliary, supplementary to the
primary item.</skos:definition>
    <skos:inScheme rdf:resource="http://isdc.gfz-potsdam.de/ontology/SPASE-allowed_values.skos.owl#Source_Type"/>
    <skos:prefLabel xml:lang="en">Ancillary</skos:prefLabel>
  </rdf:Description>
  <rdf:Description rdf:about="http://isdc.gfz-potsdam.de/ontology/SPASE-allowed_values.skos.owl#Coronal_Hole">
    <skos:prefLabel xml:lang="en">Coronal Hole</skos:prefLabel>
    <rdf:type rdf:resource="http://www.w3.org/2004/02/skos/core#Concept"/>
    <rdf:type rdf:resource="http://www.w3.org/2002/07/owl#NamedIndividual"/>
    <skos:inScheme rdf:resource="http://isdc.gfz-potsdam.de/ontology/SPASE-allowed_values.skos.owl#Phenomenon_Type"/>
    <skos:definition xml:lang="en">An extended region of the corona, exceptionally low in density and associated with unipolar
photospheric regions. A coronal hole can be an "open" magnetic field in the corona and
(perhaps) inner heliosphere which has a faster than average outflow (wind); A region of lower
than "quiet" ion and electron density in the corona; or a region of lower peak electron
temperature in the corona than in the "quiet" corona.</skos:definition>
    <skos:topConceptOf rdf:resource="http://isdc.gfz-potsdam.de/ontology/SPASE-allowed_values.skos.owl#Phenomenon_Type"/>
  </rdf:Description>
  <rdf:Description rdf:about="http://isdc.gfz-potsdam.de/ontology/SPASE-allowed_values.skos.owl#Electrostatic_Analyser">
    <rdf:type rdf:resource="http://www.w3.org/2002/07/owl#NamedIndividual"/>
    <rdf:type rdf:resource="http://www.w3.org/2004/02/skos/core#Concept"/>
    <skos:prefLabel xml:lang="en">Electrostatic Analyser</skos:prefLabel>
    <skos:definition xml:lang="en">An instrument which uses charged plates to analyze the mass, charge and kinetic energies of
charged particles which enter the instrument.</skos:definition>
    <skos:topConceptOf rdf:resource="http://isdc.gfz-potsdam.de/ontology/SPASE-allowed_values.skos.owl#Instrument_Type"/>
    <skos:inScheme rdf:resource="http://isdc.gfz-potsdam.de/ontology/SPASE-allowed_values.skos.owl#Instrument_Type"/>
  </rdf:Description>
  <rdf:Description rdf:about="http://isdc.gfz-potsdam.de/ontology/SPASE-allowed_values.skos.owl#HPC">
    <skos:prefLabel xml:lang="en">HPC</skos:prefLabel>
    <skos:inScheme rdf:resource="http://isdc.gfz-potsdam.de/ontology/SPASE-allowed_values.skos.owl#Coordinate_System_Name"/>
    <rdf:type rdf:resource="http://www.w3.org/2004/02/skos/core#Concept"/>
    <rdf:type rdf:resource="http://www.w3.org/2002/07/owl#NamedIndividual"/>
    <skos:definition xml:lang="en">Helioprojective Cartesian = A 3-D orthonormal (left-handed) coordinate system that is
primarily intended to specify with two dimensions a point on the solar disk. The Z axis points
from the observer to the center of the solar disk. The Y axis lies in the plane defined by the
solar spin vector and the Z axis, positive northward. The X axis is perpendicular to the Y and Z
axes, positive toward solar west. Given as the distance between the observer and the center of
the solar disk, the standard representation of an (x,y) point on the solar disk is via the point's
longitude angle [arctan (x/d)] and latitude angle [arctan y/d].</skos:definition>
    <skos:topConceptOf rdf:resource="http://isdc.gfz-potsdam.de/ontology/SPASE-allowed_values.skos.owl#Coordinate_System_Name"/>
  </rdf:Description>
  <rdf:Description rdf:about="http://isdc.gfz-potsdam.de/ontology/SPASE-allowed_values.skos.owl#Fluence">
    <skos:prefLabel xml:lang="en">Fluence</skos:prefLabel>
    <skos:topConceptOf rdf:resource="http://isdc.gfz-potsdam.de/ontology/SPASE-allowed_values.skos.owl#Particle_Quantity"/>
    <skos:inScheme rdf:resource="http://isdc.gfz-potsdam.de/ontology/SPASE-allowed_values.skos.owl#Particle_Quantity"/>
    <rdf:type rdf:resource="http://www.w3.org/2002/07/owl#NamedIndividual"/>
    <rdf:type rdf:resource="http://www.w3.org/2004/02/skos/core#Concept"/>
    <skos:definition xml:lang="en">The time integral of a flux. A fluence does not have any "per unit time" in its units.</skos:definition>
  </rdf:Description>
  <rdf:Description rdf:about="http://isdc.gfz-potsdam.de/ontology/SPASE-allowed_values.skos.owl#Proportional_Counter">
    <rdf:type rdf:resource="http://www.w3.org/2002/07/owl#NamedIndividual"/>
    <rdf:type rdf:resource="http://www.w3.org/2004/02/skos/core#Concept"/>
    <skos:prefLabel xml:lang="en">Proportional Counter</skos:prefLabel>
    <skos:topConceptOf rdf:resource="http://isdc.gfz-potsdam.de/ontology/SPASE-allowed_values.skos.owl#Instrument_Type"/>
    <skos:definition xml:lang="en">An instrument which measures energy of ionization radiation based on interactions with a gas.</skos:definition>
    <skos:inScheme rdf:resource="http://isdc.gfz-potsdam.de/ontology/SPASE-allowed_values.skos.owl#Instrument_Type"/>
  </rdf:Description>
  <rdf:Description rdf:about="http://isdc.gfz-potsdam.de/ontology/SPASE-allowed_values.skos.owl#D-Region">
    <skos:inScheme rdf:resource="http://isdc.gfz-potsdam.de/ontology/SPASE-allowed_values.skos.owl#Observatory_Region"/>
    <rdf:type rdf:resource="http://www.w3.org/2002/07/owl#NamedIndividual"/>
    <rdf:type rdf:resource="http://www.w3.org/2004/02/skos/core#Concept"/>
    <skos:inScheme rdf:resource="http://isdc.gfz-potsdam.de/ontology/SPASE-allowed_values.skos.owl#Observed_Region"/>
    <skos:broader rdf:resource="http://isdc.gfz-potsdam.de/ontology/SPASE-allowed_values.skos.owl#Ionosphere"/>
    <skos:definition xml:lang="en">The layer of the ionosphere that exists approximately 50 to 95 km above the surface of the
Earth. One of several layers in the ionosphere.</skos:definition>
    <skos:prefLabel xml:lang="en">D-Region</skos:prefLabel>
  </rdf:Description>
  <rdf:Description rdf:about="http://isdc.gfz-potsdam.de/ontology/SPASE-allowed_values.skos.owl#Line_Depth">
    <skos:definition xml:lang="en">The measure of the amount of absorption below the continuum (depth) in a particular
wavelength or frequency in an absorption spectrum.</skos:definition>
    <skos:inScheme rdf:resource="http://isdc.gfz-potsdam.de/ontology/SPASE-allowed_values.skos.owl#Wave_Quantity"/>
    <skos:prefLabel xml:lang="en">Line Depth</skos:prefLabel>
    <skos:topConceptOf rdf:resource="http://isdc.gfz-potsdam.de/ontology/SPASE-allowed_values.skos.owl#Wave_Quantity"/>
    <rdf:type rdf:resource="http://www.w3.org/2002/07/owl#NamedIndividual"/>
    <rdf:type rdf:resource="http://www.w3.org/2004/02/skos/core#Concept"/>
  </rdf:Description>
  <rdf:Description rdf:about="http://isdc.gfz-potsdam.de/ontology/SPASE-allowed_values.skos.owl#Spherical">
    <skos:inScheme rdf:resource="http://isdc.gfz-potsdam.de/ontology/SPASE-allowed_values.skos.owl#Coordinate_Representation"/>
    <rdf:type rdf:resource="http://www.w3.org/2002/07/owl#NamedIndividual"/>
    <skos:prefLabel xml:lang="en">Spherical</skos:prefLabel>
    <rdf:type rdf:resource="http://www.w3.org/2004/02/skos/core#Concept"/>
    <skos:topConceptOf rdf:resource="http://isdc.gfz-potsdam.de/ontology/SPASE-allowed_values.skos.owl#Coordinate_Representation"/>
    <skos:definition xml:lang="en">A coordinate representation of a position vector or of a measured vector by its magnitude and
two direction angles. The angles are relative to the base axes of the coordinate system used.
Typically the angles are phi [azimuth angle, =arctan (j/i)] and theta, where theta may be a polar
angle, arctan {[SQRT(i^2+j^2)]/k}, or an elevation angle, arctan [k/SQRT (i^2+j^2)].</skos:definition>
  </rdf:Description>
  <rdf:Description rdf:about="http://isdc.gfz-potsdam.de/ontology/SPASE-allowed_values.skos.owl#Faraday_Cup">
    <skos:topConceptOf rdf:resource="http://isdc.gfz-potsdam.de/ontology/SPASE-allowed_values.skos.owl#Instrument_Type"/>
    <skos:inScheme rdf:resource="http://isdc.gfz-potsdam.de/ontology/SPASE-allowed_values.skos.owl#Instrument_Type"/>
    <rdf:type rdf:resource="http://www.w3.org/2004/02/skos/core#Concept"/>
    <rdf:type rdf:resource="http://www.w3.org/2002/07/owl#NamedIndividual"/>
    <skos:prefLabel xml:lang="en">Faraday Cup</skos:prefLabel>
    <skos:definition xml:lang="en">An instrument consisting of an electrode from which electrical current is measured while a
charged particle beam (electrons or ions) impinges on it. Used to determine energy spectrum
and sometimes ion composition of the impinging particles.</skos:definition>
  </rdf:Description>
  <rdf:Description rdf:about="http://isdc.gfz-potsdam.de/ontology/SPASE-allowed_values.skos.owl#Area">
    <rdf:type rdf:resource="http://www.w3.org/2002/07/owl#NamedIndividual"/>
    <rdf:type rdf:resource="http://www.w3.org/2004/02/skos/core#Concept"/>
    <skos:broader rdf:resource="http://isdc.gfz-potsdam.de/ontology/SPASE-allowed_values.skos.owl#Integral"/>
    <skos:definition xml:lang="en">Integration over the extent of a planar region, or of the surface of a solid.</skos:definition>
    <skos:prefLabel xml:lang="en">Area</skos:prefLabel>
    <skos:inScheme rdf:resource="http://isdc.gfz-potsdam.de/ontology/SPASE-allowed_values.skos.owl#Qualifier"/>
  </rdf:Description>
  <rdf:Description rdf:about="http://isdc.gfz-potsdam.de/ontology/SPASE-allowed_values.skos.owl#Wavelength">
    <skos:definition xml:lang="en">The peak-to-peak distance over one wave period.</skos:definition>
    <skos:topConceptOf rdf:resource="http://isdc.gfz-potsdam.de/ontology/SPASE-allowed_values.skos.owl#Wave_Quantity"/>
    <rdf:type rdf:resource="http://www.w3.org/2002/07/owl#NamedIndividual"/>
    <rdf:type rdf:resource="http://www.w3.org/2004/02/skos/core#Concept"/>
    <skos:inScheme rdf:resource="http://isdc.gfz-potsdam.de/ontology/SPASE-allowed_values.skos.owl#Wave_Quantity"/>
    <skos:prefLabel xml:lang="en">Wavelength</skos:prefLabel>
  </rdf:Description>
  <rdf:Description rdf:about="http://isdc.gfz-potsdam.de/ontology/SPASE-allowed_values.skos.owl#Encoding">
    <skos:hasTopConcept rdf:resource="http://isdc.gfz-potsdam.de/ontology/SPASE-allowed_values.skos.owl#S3_BUCKET"/>
    <skos:prefLabel xml:lang="en">Encoding</skos:prefLabel>
    <skos:hasTopConcept rdf:resource="http://isdc.gfz-potsdam.de/ontology/SPASE-allowed_values.skos.owl#GZIP"/>
    <skos:hasTopConcept rdf:resource="http://isdc.gfz-potsdam.de/ontology/SPASE-allowed_values.skos.owl#BZIP2"/>
    <skos:hasTopConcept rdf:resource="http://isdc.gfz-potsdam.de/ontology/SPASE-allowed_values.skos.owl#ZIP"/>
    <rdf:type rdf:resource="http://www.w3.org/2004/02/skos/core#ConceptScheme"/>
    <rdf:type rdf:resource="http://www.w3.org/2002/07/owl#NamedIndividual"/>
    <skos:hasTopConcept rdf:resource="http://isdc.gfz-potsdam.de/ontology/SPASE-allowed_values.skos.owl#None"/>
    <skos:definition xml:lang="en">A set of unambiguous rules that establishes the representation of information within a file.
Allowed Values:
ASCII
BZIP2
Base64
GZIP
None
S3_BUCKET
TAR
Unicode
ZIP</skos:definition>
    <skos:hasTopConcept rdf:resource="http://isdc.gfz-potsdam.de/ontology/SPASE-allowed_values.skos.owl#TAR"/>
    <skos:hasTopConcept rdf:resource="http://isdc.gfz-potsdam.de/ontology/SPASE-allowed_values.skos.owl#Base64"/>
  </rdf:Description>
  <rdf:Description rdf:about="http://isdc.gfz-potsdam.de/ontology/SPASE-allowed_values.skos.owl#Microfilm">
    <skos:prefLabel xml:lang="en">Microfilm</skos:prefLabel>
    <skos:inScheme rdf:resource="http://isdc.gfz-potsdam.de/ontology/SPASE-allowed_values.skos.owl#Format"/>
    <skos:broader rdf:resource="http://isdc.gfz-potsdam.de/ontology/SPASE-allowed_values.skos.owl#Hardcopy"/>
    <rdf:type rdf:resource="http://www.w3.org/2004/02/skos/core#Concept"/>
    <rdf:type rdf:resource="http://www.w3.org/2002/07/owl#NamedIndividual"/>
    <skos:definition xml:lang="en">Film rolls on which materials are photographed at greatly reduced size; a magnification system
is used to read the material.</skos:definition>
  </rdf:Description>
  <rdf:Description rdf:about="http://isdc.gfz-potsdam.de/ontology/SPASE-allowed_values.skos.owl#Interior">
    <skos:inScheme rdf:resource="http://isdc.gfz-potsdam.de/ontology/SPASE-allowed_values.skos.owl#Observed_Region"/>
    <skos:definition xml:lang="en">The region inside the body which is not visible from outside the body.</skos:definition>
    <skos:broader rdf:resource="http://isdc.gfz-potsdam.de/ontology/SPASE-allowed_values.skos.owl#Sun"/>
    <skos:prefLabel xml:lang="en">Interior</skos:prefLabel>
    <skos:inScheme rdf:resource="http://isdc.gfz-potsdam.de/ontology/SPASE-allowed_values.skos.owl#Observatory_Region"/>
    <rdf:type rdf:resource="http://www.w3.org/2002/07/owl#NamedIndividual"/>
    <rdf:type rdf:resource="http://www.w3.org/2004/02/skos/core#Concept"/>
  </rdf:Description>
  <rdf:Description rdf:about="http://isdc.gfz-potsdam.de/ontology/SPASE-allowed_values.skos.owl#Unspecified">
    <skos:inScheme rdf:resource="http://isdc.gfz-potsdam.de/ontology/SPASE-allowed_values.skos.owl#Instrument_Type"/>
    <rdf:type rdf:resource="http://www.w3.org/2004/02/skos/core#Concept"/>
    <rdf:type rdf:resource="http://www.w3.org/2002/07/owl#NamedIndividual"/>
    <skos:prefLabel xml:lang="en">Unspecified</skos:prefLabel>
    <skos:topConceptOf rdf:resource="http://isdc.gfz-potsdam.de/ontology/SPASE-allowed_values.skos.owl#Instrument_Type"/>
    <skos:definition xml:lang="en">A value which is not provided.</skos:definition>
  </rdf:Description>
  <rdf:Description rdf:about="http://isdc.gfz-potsdam.de/ontology/SPASE-allowed_values.skos.owl#Observatory_Region">
    <skos:hasTopConcept rdf:resource="http://isdc.gfz-potsdam.de/ontology/SPASE-allowed_values.skos.owl#Saturn"/>
    <skos:hasTopConcept rdf:resource="http://isdc.gfz-potsdam.de/ontology/SPASE-allowed_values.skos.owl#Venus"/>
    <skos:inScheme rdf:resource="http://isdc.gfz-potsdam.de/ontology/SPASE-allowed_values.skos.owl#Observatory_Region"/>
    <skos:hasTopConcept rdf:resource="http://isdc.gfz-potsdam.de/ontology/SPASE-allowed_values.skos.owl#Neptune"/>
    <rdf:type rdf:resource="http://www.w3.org/2002/07/owl#NamedIndividual"/>
    <skos:hasTopConcept rdf:resource="http://isdc.gfz-potsdam.de/ontology/SPASE-allowed_values.skos.owl#Jupiter"/>
    <skos:hasTopConcept rdf:resource="http://isdc.gfz-potsdam.de/ontology/SPASE-allowed_values.skos.owl#Uranus"/>
    <skos:hasTopConcept rdf:resource="http://isdc.gfz-potsdam.de/ontology/SPASE-allowed_values.skos.owl#Sun"/>
    <skos:hasTopConcept rdf:resource="http://isdc.gfz-potsdam.de/ontology/SPASE-allowed_values.skos.owl#Interstellar"/>
    <rdf:type rdf:resource="http://www.w3.org/2004/02/skos/core#ConceptScheme"/>
    <skos:hasTopConcept rdf:resource="http://isdc.gfz-potsdam.de/ontology/SPASE-allowed_values.skos.owl#Mars"/>
    <skos:hasTopConcept rdf:resource="http://isdc.gfz-potsdam.de/ontology/SPASE-allowed_values.skos.owl#Earth"/>
    <skos:hasTopConcept rdf:resource="http://isdc.gfz-potsdam.de/ontology/SPASE-allowed_values.skos.owl#Asteroid"/>
    <skos:prefLabel xml:lang="en">Observatory Region</skos:prefLabel>
    <skos:hasTopConcept rdf:resource="http://isdc.gfz-potsdam.de/ontology/SPASE-allowed_values.skos.owl#Heliosphere"/>
    <skos:definition xml:lang="en">A spatial location distinguished by certain natural features or physical characteristics where an
observatory is located.
Allowed Values:
Asteroid
Comet
Earth
Earth.Magnetosheath
Earth.Magnetosphere
Earth.Magnetosphere.Magnetotail
Earth.Magnetosphere.Main
Earth.Magnetosphere.Polar
Earth.Magnetosphere.Radiation Belt
Earth.Near Surface
Earth.Near Surface.Atmosphere
Earth.Near Surface.Auroral Region
Earth.Near Surface.Equatorial Region
Earth.Near Surface.Ionosphere
Earth.Near Surface.Ionosphere.D-Region
Earth.Near Surface.Ionosphere.E-Region
Earth.Near Surface.Ionosphere.F-Region
Earth.Near Surface.Ionosphere.Topside
Earth.Near Surface.Mesosphere
Earth.Near Surface.Plasmasphere
Earth.Near Surface.Polar Cap
Earth.Near Surface.South Atlantic Anomaly Region
Earth.Near Surface.Stratosphere
Earth.Near Surface.Thermosphere
Earth.Near Surface.Troposphere
Earth.Surface
Heliosphere
Heliosphere.Heliosheath
Heliosphere.Inner
Heliosphere.Near Earth
Heliosphere.Outer
Heliosphere.Remote 1AU
Interstellar
Jupiter
Mars
Mercury
Neptune
Pluto
Saturn
Sun
Sun.Chromosphere
Sun.Corona
Sun.Interior
Sun.Photosphere
Sun.Transition Region
Uranus
Venus</skos:definition>
    <skos:hasTopConcept rdf:resource="http://isdc.gfz-potsdam.de/ontology/SPASE-allowed_values.skos.owl#Pluto"/>
    <skos:hasTopConcept rdf:resource="http://isdc.gfz-potsdam.de/ontology/SPASE-allowed_values.skos.owl#Comet"/>
    <skos:hasTopConcept rdf:resource="http://isdc.gfz-potsdam.de/ontology/SPASE-allowed_values.skos.owl#Mercury"/>
  </rdf:Description>
  <rdf:Description rdf:about="http://isdc.gfz-potsdam.de/ontology/SPASE-allowed_values.skos.owl#Near_Earth">
    <skos:broader rdf:resource="http://isdc.gfz-potsdam.de/ontology/SPASE-allowed_values.skos.owl#Heliosphere"/>
    <skos:inScheme rdf:resource="http://isdc.gfz-potsdam.de/ontology/SPASE-allowed_values.skos.owl#Observatory_Region"/>
    <rdf:type rdf:resource="http://www.w3.org/2002/07/owl#NamedIndividual"/>
    <rdf:type rdf:resource="http://www.w3.org/2004/02/skos/core#Concept"/>
    <skos:prefLabel xml:lang="en">Near Earth</skos:prefLabel>
    <skos:inScheme rdf:resource="http://isdc.gfz-potsdam.de/ontology/SPASE-allowed_values.skos.owl#Observed_Region"/>
    <skos:definition xml:lang="en">The heliospheric region near the Earth which extends to and includes the area near the L1 and
L2 Lagrange point.</skos:definition>
  </rdf:Description>
  <rdf:Description rdf:about="http://isdc.gfz-potsdam.de/ontology/SPASE-allowed_values.skos.owl#Specification">
    <skos:topConceptOf rdf:resource="http://isdc.gfz-potsdam.de/ontology/SPASE-allowed_values.skos.owl#Document_Type"/>
    <skos:definition xml:lang="en">A detailed description of the requirements and other aspects of an object or component that may
be used to develop an implementation.</skos:definition>
    <skos:inScheme rdf:resource="http://isdc.gfz-potsdam.de/ontology/SPASE-allowed_values.skos.owl#Document_Type"/>
    <skos:prefLabel xml:lang="en">Specification</skos:prefLabel>
    <rdf:type rdf:resource="http://www.w3.org/2002/07/owl#NamedIndividual"/>
    <rdf:type rdf:resource="http://www.w3.org/2004/02/skos/core#Concept"/>
  </rdf:Description>
  <rdf:Description rdf:about="http://isdc.gfz-potsdam.de/ontology/SPASE-allowed_values.skos.owl#Wave_Form">
    <rdf:type rdf:resource="http://www.w3.org/2002/07/owl#NamedIndividual"/>
    <rdf:type rdf:resource="http://www.w3.org/2004/02/skos/core#Concept"/>
    <skos:definition xml:lang="en">Spatial or temporal variations of wave amplitude over wave-period timescales.</skos:definition>
    <skos:topConceptOf rdf:resource="http://isdc.gfz-potsdam.de/ontology/SPASE-allowed_values.skos.owl#Display_Type"/>
    <skos:prefLabel xml:lang="en">Wave Form</skos:prefLabel>
    <skos:inScheme rdf:resource="http://isdc.gfz-potsdam.de/ontology/SPASE-allowed_values.skos.owl#Display_Type"/>
  </rdf:Description>
  <rdf:Description rdf:about="http://isdc.gfz-potsdam.de/ontology/SPASE-allowed_values.skos.owl#Radiometer">
    <skos:definition xml:lang="en">An instrument for detecting or measuring radiant energy. Radiometers are commonly limited to
infrared radiation.</skos:definition>
    <skos:inScheme rdf:resource="http://isdc.gfz-potsdam.de/ontology/SPASE-allowed_values.skos.owl#Instrument_Type"/>
    <rdf:type rdf:resource="http://www.w3.org/2004/02/skos/core#Concept"/>
    <rdf:type rdf:resource="http://www.w3.org/2002/07/owl#NamedIndividual"/>
    <skos:topConceptOf rdf:resource="http://isdc.gfz-potsdam.de/ontology/SPASE-allowed_values.skos.owl#Instrument_Type"/>
    <skos:prefLabel xml:lang="en">Radiometer</skos:prefLabel>
  </rdf:Description>
  <rdf:Description rdf:about="http://isdc.gfz-potsdam.de/ontology/SPASE-allowed_values.skos.owl#Display_Type">
    <skos:hasTopConcept rdf:resource="http://isdc.gfz-potsdam.de/ontology/SPASE-allowed_values.skos.owl#Image"/>
    <rdf:type rdf:resource="http://www.w3.org/2004/02/skos/core#ConceptScheme"/>
    <rdf:type rdf:resource="http://www.w3.org/2002/07/owl#NamedIndividual"/>
    <skos:prefLabel xml:lang="en">Display Type</skos:prefLabel>
    <skos:hasTopConcept rdf:resource="http://isdc.gfz-potsdam.de/ontology/SPASE-allowed_values.skos.owl#Spectrogram"/>
    <skos:definition xml:lang="en">The general styling or type of plot that is suitable for the variable.
Allowed Values:
Image
Plasmagram
Spectrogram
Stack Plot
Time Series
Wave Form</skos:definition>
    <skos:hasTopConcept rdf:resource="http://isdc.gfz-potsdam.de/ontology/SPASE-allowed_values.skos.owl#Stack_Plot"/>
    <skos:hasTopConcept rdf:resource="http://isdc.gfz-potsdam.de/ontology/SPASE-allowed_values.skos.owl#Time_Series"/>
    <skos:hasTopConcept rdf:resource="http://isdc.gfz-potsdam.de/ontology/SPASE-allowed_values.skos.owl#Wave_Form"/>
    <skos:hasTopConcept rdf:resource="http://isdc.gfz-potsdam.de/ontology/SPASE-allowed_values.skos.owl#Plasmagram"/>
  </rdf:Description>
  <rdf:Description rdf:about="http://isdc.gfz-potsdam.de/ontology/SPASE-allowed_values.skos.owl#Aerosol">
    <rdf:type rdf:resource="http://www.w3.org/2004/02/skos/core#Concept"/>
    <skos:inScheme rdf:resource="http://isdc.gfz-potsdam.de/ontology/SPASE-allowed_values.skos.owl#Particle_Type"/>
    <skos:prefLabel xml:lang="en">Aerosol</skos:prefLabel>
    <rdf:type rdf:resource="http://www.w3.org/2002/07/owl#NamedIndividual"/>
    <skos:topConceptOf rdf:resource="http://isdc.gfz-potsdam.de/ontology/SPASE-allowed_values.skos.owl#Particle_Type"/>
    <skos:definition xml:lang="en">A suspension of fine solid or liquid particles in a gas.</skos:definition>
  </rdf:Description>
  <rdf:Description rdf:about="http://isdc.gfz-potsdam.de/ontology/SPASE-allowed_values.skos.owl#Jupiter">
    <rdf:type rdf:resource="http://www.w3.org/2002/07/owl#NamedIndividual"/>
    <rdf:type rdf:resource="http://www.w3.org/2004/02/skos/core#Concept"/>
    <skos:topConceptOf rdf:resource="http://isdc.gfz-potsdam.de/ontology/SPASE-allowed_values.skos.owl#Observed_Region"/>
    <skos:definition xml:lang="en">The fifth planet from the sun in our solar system.</skos:definition>
    <skos:prefLabel xml:lang="en">Jupiter</skos:prefLabel>
    <skos:inScheme rdf:resource="http://isdc.gfz-potsdam.de/ontology/SPASE-allowed_values.skos.owl#Observed_Region"/>
    <skos:topConceptOf rdf:resource="http://isdc.gfz-potsdam.de/ontology/SPASE-allowed_values.skos.owl#Observatory_Region"/>
    <skos:inScheme rdf:resource="http://isdc.gfz-potsdam.de/ontology/SPASE-allowed_values.skos.owl#Observatory_Region"/>
  </rdf:Description>
  <rdf:Description rdf:about="http://isdc.gfz-potsdam.de/ontology/SPASE-allowed_values.skos.owl#Quadrispherical_Analyser">
    <skos:topConceptOf rdf:resource="http://isdc.gfz-potsdam.de/ontology/SPASE-allowed_values.skos.owl#Instrument_Type"/>
    <skos:definition xml:lang="en">An instrument used for the 3-D detection of plasma, energetic electrons and ions, and for
positive-ion composition measurements.</skos:definition>
    <skos:inScheme rdf:resource="http://isdc.gfz-potsdam.de/ontology/SPASE-allowed_values.skos.owl#Instrument_Type"/>
    <rdf:type rdf:resource="http://www.w3.org/2002/07/owl#NamedIndividual"/>
    <rdf:type rdf:resource="http://www.w3.org/2004/02/skos/core#Concept"/>
    <skos:prefLabel xml:lang="en">Quadrispherical Analyser</skos:prefLabel>
  </rdf:Description>
  <rdf:Description rdf:about="http://isdc.gfz-potsdam.de/ontology/SPASE-allowed_values.skos.owl#Outer">
    <skos:broader rdf:resource="http://isdc.gfz-potsdam.de/ontology/SPASE-allowed_values.skos.owl#Heliosphere"/>
    <skos:inScheme rdf:resource="http://isdc.gfz-potsdam.de/ontology/SPASE-allowed_values.skos.owl#Observatory_Region"/>
    <rdf:type rdf:resource="http://www.w3.org/2002/07/owl#NamedIndividual"/>
    <rdf:type rdf:resource="http://www.w3.org/2004/02/skos/core#Concept"/>
    <skos:inScheme rdf:resource="http://isdc.gfz-potsdam.de/ontology/SPASE-allowed_values.skos.owl#Observed_Region"/>
    <skos:prefLabel xml:lang="en">Outer</skos:prefLabel>
    <skos:definition xml:lang="en">The region of the heliosphere extending radially outward from just outside 1 AU to the
heliospheric termination shock.</skos:definition>
  </rdf:Description>
  <rdf:Description rdf:about="http://isdc.gfz-potsdam.de/ontology/SPASE-allowed_values.skos.owl#Corona">
    <skos:broader rdf:resource="http://isdc.gfz-potsdam.de/ontology/SPASE-allowed_values.skos.owl#Sun"/>
    <rdf:type rdf:resource="http://www.w3.org/2004/02/skos/core#Concept"/>
    <skos:inScheme rdf:resource="http://isdc.gfz-potsdam.de/ontology/SPASE-allowed_values.skos.owl#Observed_Region"/>
    <rdf:type rdf:resource="http://www.w3.org/2002/07/owl#NamedIndividual"/>
    <skos:definition xml:lang="en">The outermost atmospheric region of the Sun or a star, characterized by ionization temperatures
above 10^5 K. The solar corona starts at about 2100 km above the photosphere; there is no
generally defined upper limit.</skos:definition>
    <skos:prefLabel xml:lang="en">Corona</skos:prefLabel>
    <skos:inScheme rdf:resource="http://isdc.gfz-potsdam.de/ontology/SPASE-allowed_values.skos.owl#Observatory_Region"/>
  </rdf:Description>
  <rdf:Description rdf:about="http://isdc.gfz-potsdam.de/ontology/SPASE-allowed_values.skos.owl#TIFF">
    <skos:definition xml:lang="en">A binary format for still pictures. Tagged Image Format File (TIFF). Originally developed by
Aldus and now controlled by Adobe.</skos:definition>
    <skos:prefLabel xml:lang="en">TIFF</skos:prefLabel>
    <rdf:type rdf:resource="http://www.w3.org/2002/07/owl#NamedIndividual"/>
    <skos:topConceptOf rdf:resource="http://isdc.gfz-potsdam.de/ontology/SPASE-allowed_values.skos.owl#Format"/>
    <rdf:type rdf:resource="http://www.w3.org/2004/02/skos/core#Concept"/>
    <skos:inScheme rdf:resource="http://isdc.gfz-potsdam.de/ontology/SPASE-allowed_values.skos.owl#Format"/>
  </rdf:Description>
  <rdf:Description rdf:about="http://isdc.gfz-potsdam.de/ontology/SPASE-allowed_values.skos.owl#Coordinate_System_Name">
    <skos:hasTopConcept rdf:resource="http://isdc.gfz-potsdam.de/ontology/SPASE-allowed_values.skos.owl#HPR"/>
    <skos:hasTopConcept rdf:resource="http://isdc.gfz-potsdam.de/ontology/SPASE-allowed_values.skos.owl#HPC"/>
    <skos:hasTopConcept rdf:resource="http://isdc.gfz-potsdam.de/ontology/SPASE-allowed_values.skos.owl#J2000"/>
    <skos:hasTopConcept rdf:resource="http://isdc.gfz-potsdam.de/ontology/SPASE-allowed_values.skos.owl#HGI"/>
    <skos:hasTopConcept rdf:resource="http://isdc.gfz-potsdam.de/ontology/SPASE-allowed_values.skos.owl#SSE"/>
    <skos:hasTopConcept rdf:resource="http://isdc.gfz-potsdam.de/ontology/SPASE-allowed_values.skos.owl#LGM"/>
    <skos:hasTopConcept rdf:resource="http://isdc.gfz-potsdam.de/ontology/SPASE-allowed_values.skos.owl#HEEQ"/>
    <skos:hasTopConcept rdf:resource="http://isdc.gfz-potsdam.de/ontology/SPASE-allowed_values.skos.owl#CGM"/>
    <skos:hasTopConcept rdf:resource="http://isdc.gfz-potsdam.de/ontology/SPASE-allowed_values.skos.owl#RTN"/>
    <rdf:type rdf:resource="http://www.w3.org/2002/07/owl#NamedIndividual"/>
    <skos:hasTopConcept rdf:resource="http://isdc.gfz-potsdam.de/ontology/SPASE-allowed_values.skos.owl#SR2"/>
    <skos:hasTopConcept rdf:resource="http://isdc.gfz-potsdam.de/ontology/SPASE-allowed_values.skos.owl#SE"/>
    <skos:hasTopConcept rdf:resource="http://isdc.gfz-potsdam.de/ontology/SPASE-allowed_values.skos.owl#SR"/>
    <skos:hasTopConcept rdf:resource="http://isdc.gfz-potsdam.de/ontology/SPASE-allowed_values.skos.owl#GSM"/>
    <skos:hasTopConcept rdf:resource="http://isdc.gfz-potsdam.de/ontology/SPASE-allowed_values.skos.owl#SC"/>
    <skos:hasTopConcept rdf:resource="http://isdc.gfz-potsdam.de/ontology/SPASE-allowed_values.skos.owl#HEE"/>
    <skos:hasTopConcept rdf:resource="http://isdc.gfz-potsdam.de/ontology/SPASE-allowed_values.skos.owl#GEI"/>
    <skos:hasTopConcept rdf:resource="http://isdc.gfz-potsdam.de/ontology/SPASE-allowed_values.skos.owl#Spacecraft_Orbit_Plane"/>
    <skos:hasTopConcept rdf:resource="http://isdc.gfz-potsdam.de/ontology/SPASE-allowed_values.skos.owl#SSE_L"/>
    <skos:hasTopConcept rdf:resource="http://isdc.gfz-potsdam.de/ontology/SPASE-allowed_values.skos.owl#GEO"/>
    <skos:hasTopConcept rdf:resource="http://isdc.gfz-potsdam.de/ontology/SPASE-allowed_values.skos.owl#GSE"/>
    <skos:prefLabel xml:lang="en">Coordinate System Name</skos:prefLabel>
    <skos:hasTopConcept rdf:resource="http://isdc.gfz-potsdam.de/ontology/SPASE-allowed_values.skos.owl#HCR"/>
    <skos:hasTopConcept rdf:resource="http://isdc.gfz-potsdam.de/ontology/SPASE-allowed_values.skos.owl#HAE"/>
    <rdf:type rdf:resource="http://www.w3.org/2004/02/skos/core#ConceptScheme"/>
    <skos:hasTopConcept rdf:resource="http://isdc.gfz-potsdam.de/ontology/SPASE-allowed_values.skos.owl#DM"/>
    <skos:hasTopConcept rdf:resource="http://isdc.gfz-potsdam.de/ontology/SPASE-allowed_values.skos.owl#Carrington"/>
    <skos:hasTopConcept rdf:resource="http://isdc.gfz-potsdam.de/ontology/SPASE-allowed_values.skos.owl#HG"/>
    <skos:hasTopConcept rdf:resource="http://isdc.gfz-potsdam.de/ontology/SPASE-allowed_values.skos.owl#WGS84"/>
    <skos:hasTopConcept rdf:resource="http://isdc.gfz-potsdam.de/ontology/SPASE-allowed_values.skos.owl#MFA"/>
    <skos:hasTopConcept rdf:resource="http://isdc.gfz-potsdam.de/ontology/SPASE-allowed_values.skos.owl#HCC"/>
    <skos:hasTopConcept rdf:resource="http://isdc.gfz-potsdam.de/ontology/SPASE-allowed_values.skos.owl#SM"/>
    <skos:hasTopConcept rdf:resource="http://isdc.gfz-potsdam.de/ontology/SPASE-allowed_values.skos.owl#MAG"/>
    <skos:hasTopConcept rdf:resource="http://isdc.gfz-potsdam.de/ontology/SPASE-allowed_values.skos.owl#HCI"/>
    <skos:hasTopConcept rdf:resource="http://isdc.gfz-potsdam.de/ontology/SPASE-allowed_values.skos.owl#GSEQ"/>
    <skos:definition xml:lang="en">Identifies the coordinate system in which the position, direction or observation has been
-39-
SPASE Data Model
expressed.
Allowed Values:
CGM
Carrington
DM
GEI
GEO
GSE
GSEQ
GSM
HAE
HCC
HCI
HCR
HEE
HEEQ
HG
HGI
HPC
HPR
J2000
LGM
MAG
MFA
RTN
SC
SE
SM
SR
SR2
SSE
SSE_L
Spacecraft Orbit Plane
WGS84</skos:definition>
  </rdf:Description>
  <rdf:Description rdf:about="http://isdc.gfz-potsdam.de/ontology/SPASE-allowed_values.skos.owl#Format">
    <skos:hasTopConcept rdf:resource="http://isdc.gfz-potsdam.de/ontology/SPASE-allowed_values.skos.owl#MATLAB_7"/>
    <skos:hasTopConcept rdf:resource="http://isdc.gfz-potsdam.de/ontology/SPASE-allowed_values.skos.owl#IDFS"/>
    <skos:hasTopConcept rdf:resource="http://isdc.gfz-potsdam.de/ontology/SPASE-allowed_values.skos.owl#HDF_4"/>
    <skos:hasTopConcept rdf:resource="http://isdc.gfz-potsdam.de/ontology/SPASE-allowed_values.skos.owl#Hardcopy"/>
    <rdf:type rdf:resource="http://www.w3.org/2002/07/owl#NamedIndividual"/>
    <skos:hasTopConcept rdf:resource="http://isdc.gfz-potsdam.de/ontology/SPASE-allowed_values.skos.owl#CEF_1"/>
    <rdf:type rdf:resource="http://www.w3.org/2004/02/skos/core#ConceptScheme"/>
    <skos:hasTopConcept rdf:resource="http://isdc.gfz-potsdam.de/ontology/SPASE-allowed_values.skos.owl#VOTable"/>
    <skos:hasTopConcept rdf:resource="http://isdc.gfz-potsdam.de/ontology/SPASE-allowed_values.skos.owl#CEF"/>
    <skos:hasTopConcept rdf:resource="http://isdc.gfz-potsdam.de/ontology/SPASE-allowed_values.skos.owl#Excel"/>
    <skos:hasTopConcept rdf:resource="http://isdc.gfz-potsdam.de/ontology/SPASE-allowed_values.skos.owl#CDF"/>
    <skos:hasTopConcept rdf:resource="http://isdc.gfz-potsdam.de/ontology/SPASE-allowed_values.skos.owl#QuickTime"/>
    <skos:hasTopConcept rdf:resource="http://isdc.gfz-potsdam.de/ontology/SPASE-allowed_values.skos.owl#UDF"/>
    <skos:hasTopConcept rdf:resource="http://isdc.gfz-potsdam.de/ontology/SPASE-allowed_values.skos.owl#PNG"/>
    <skos:hasTopConcept rdf:resource="http://isdc.gfz-potsdam.de/ontology/SPASE-allowed_values.skos.owl#NetCDF"/>
    <skos:hasTopConcept rdf:resource="http://isdc.gfz-potsdam.de/ontology/SPASE-allowed_values.skos.owl#PDF"/>
    <skos:hasTopConcept rdf:resource="http://isdc.gfz-potsdam.de/ontology/SPASE-allowed_values.skos.owl#FITS"/>
    <skos:hasTopConcept rdf:resource="http://isdc.gfz-potsdam.de/ontology/SPASE-allowed_values.skos.owl#MATLAB_4"/>
    <skos:hasTopConcept rdf:resource="http://isdc.gfz-potsdam.de/ontology/SPASE-allowed_values.skos.owl#JPEG"/>
    <skos:hasTopConcept rdf:resource="http://isdc.gfz-potsdam.de/ontology/SPASE-allowed_values.skos.owl#HDF_5"/>
    <skos:hasTopConcept rdf:resource="http://isdc.gfz-potsdam.de/ontology/SPASE-allowed_values.skos.owl#Postscript"/>
    <skos:hasTopConcept rdf:resource="http://isdc.gfz-potsdam.de/ontology/SPASE-allowed_values.skos.owl#HTML"/>
    <skos:hasTopConcept rdf:resource="http://isdc.gfz-potsdam.de/ontology/SPASE-allowed_values.skos.owl#Binary"/>
    <skos:prefLabel xml:lang="en">Format</skos:prefLabel>
    <skos:hasTopConcept rdf:resource="http://isdc.gfz-potsdam.de/ontology/SPASE-allowed_values.skos.owl#HDF"/>
    <skos:hasTopConcept rdf:resource="http://isdc.gfz-potsdam.de/ontology/SPASE-allowed_values.skos.owl#CEF_2"/>
    <skos:hasTopConcept rdf:resource="http://isdc.gfz-potsdam.de/ontology/SPASE-allowed_values.skos.owl#AVI"/>
    <skos:hasTopConcept rdf:resource="http://isdc.gfz-potsdam.de/ontology/SPASE-allowed_values.skos.owl#XML"/>
    <skos:definition xml:lang="en">The organization of data according to preset specifications. The value is selected from a list of
accepted names for known, well documented formats.
Allowed Values:
AVI
Binary
CDF
CEF
CEF 1
CEF 2
Excel
FITS
GIF
HDF
HDF 4
HDF 5
HTML
Hardcopy
Hardcopy.Film
Hardcopy.Microfiche
Hardcopy.Microfilm
Hardcopy.Photograph
Hardcopy.Photographic Plate
Hardcopy.Print
IDFS
IDL
JPEG
MATLAB_4
MATLAB_6
MATLAB_7
MPEG
NCAR
NetCDF
PDF
PNG
Postscript
QuickTime
TIFF
Text
Text.ASCII
Text.Unicode
UDF
VOTable
XML</skos:definition>
    <skos:hasTopConcept rdf:resource="http://isdc.gfz-potsdam.de/ontology/SPASE-allowed_values.skos.owl#Text"/>
    <skos:hasTopConcept rdf:resource="http://isdc.gfz-potsdam.de/ontology/SPASE-allowed_values.skos.owl#MATLAB_6"/>
    <skos:hasTopConcept rdf:resource="http://isdc.gfz-potsdam.de/ontology/SPASE-allowed_values.skos.owl#NCAR"/>
    <skos:hasTopConcept rdf:resource="http://isdc.gfz-potsdam.de/ontology/SPASE-allowed_values.skos.owl#GIF"/>
    <skos:hasTopConcept rdf:resource="http://isdc.gfz-potsdam.de/ontology/SPASE-allowed_values.skos.owl#TIFF"/>
    <skos:hasTopConcept rdf:resource="http://isdc.gfz-potsdam.de/ontology/SPASE-allowed_values.skos.owl#IDL"/>
    <skos:hasTopConcept rdf:resource="http://isdc.gfz-potsdam.de/ontology/SPASE-allowed_values.skos.owl#MPEG"/>
  </rdf:Description>
  <rdf:Description rdf:about="http://isdc.gfz-potsdam.de/ontology/SPASE-allowed_values.skos.owl#CEF_1">
    <rdf:type rdf:resource="http://www.w3.org/2004/02/skos/core#Concept"/>
    <skos:prefLabel xml:lang="en">CEF 1</skos:prefLabel>
    <skos:definition xml:lang="en">Cluster Exchange Format (CEF), version 1, is a self-documenting ASCII format designed for
the exchange of data. The metadata contains information compatible with the ISTP
recommendations for CDF.</skos:definition>
    <skos:inScheme rdf:resource="http://isdc.gfz-potsdam.de/ontology/SPASE-allowed_values.skos.owl#Format"/>
    <skos:topConceptOf rdf:resource="http://isdc.gfz-potsdam.de/ontology/SPASE-allowed_values.skos.owl#Format"/>
    <rdf:type rdf:resource="http://www.w3.org/2002/07/owl#NamedIndividual"/>
  </rdf:Description>
  <rdf:Description rdf:about="http://isdc.gfz-potsdam.de/ontology/SPASE-allowed_values.skos.owl#Mars">
    <skos:topConceptOf rdf:resource="http://isdc.gfz-potsdam.de/ontology/SPASE-allowed_values.skos.owl#Observatory_Region"/>
    <skos:prefLabel xml:lang="en">Mars</skos:prefLabel>
    <skos:definition xml:lang="en">The forth planet from the sun in our solar system.</skos:definition>
    <rdf:type rdf:resource="http://www.w3.org/2004/02/skos/core#Concept"/>
    <skos:inScheme rdf:resource="http://isdc.gfz-potsdam.de/ontology/SPASE-allowed_values.skos.owl#Observed_Region"/>
    <rdf:type rdf:resource="http://www.w3.org/2002/07/owl#NamedIndividual"/>
    <skos:topConceptOf rdf:resource="http://isdc.gfz-potsdam.de/ontology/SPASE-allowed_values.skos.owl#Observed_Region"/>
    <skos:inScheme rdf:resource="http://isdc.gfz-potsdam.de/ontology/SPASE-allowed_values.skos.owl#Observatory_Region"/>
  </rdf:Description>
  <rdf:Description rdf:about="http://isdc.gfz-potsdam.de/ontology/SPASE-allowed_values.skos.owl#Alpha_Particle">
    <rdf:type rdf:resource="http://www.w3.org/2002/07/owl#NamedIndividual"/>
    <rdf:type rdf:resource="http://www.w3.org/2004/02/skos/core#Concept"/>
    <skos:topConceptOf rdf:resource="http://isdc.gfz-potsdam.de/ontology/SPASE-allowed_values.skos.owl#Particle_Type"/>
    <skos:prefLabel xml:lang="en">Alpha Particle</skos:prefLabel>
    <skos:definition xml:lang="en">A positively charged nuclear particle that consists of two protons and two neutrons.</skos:definition>
    <skos:inScheme rdf:resource="http://isdc.gfz-potsdam.de/ontology/SPASE-allowed_values.skos.owl#Particle_Type"/>
  </rdf:Description>
  <rdf:Description rdf:about="http://isdc.gfz-potsdam.de/ontology/SPASE-allowed_values.skos.owl#Ion_Drift">
    <skos:definition xml:lang="en">A device which measures the current produced by the displacement of ambient ions on a grid,
thereby allowing the determination of the ion trajectory and velocity.</skos:definition>
    <skos:inScheme rdf:resource="http://isdc.gfz-potsdam.de/ontology/SPASE-allowed_values.skos.owl#Instrument_Type"/>
    <rdf:type rdf:resource="http://www.w3.org/2004/02/skos/core#Concept"/>
    <rdf:type rdf:resource="http://www.w3.org/2002/07/owl#NamedIndividual"/>
    <skos:topConceptOf rdf:resource="http://isdc.gfz-potsdam.de/ontology/SPASE-allowed_values.skos.owl#Instrument_Type"/>
    <skos:prefLabel xml:lang="en">Ion Drift</skos:prefLabel>
  </rdf:Description>
  <rdf:Description rdf:about="http://isdc.gfz-potsdam.de/ontology/SPASE-allowed_values.skos.owl#Troposphere">
    <rdf:type rdf:resource="http://www.w3.org/2002/07/owl#NamedIndividual"/>
    <skos:definition xml:lang="en">The lowest layer of the atmosphere which begins at the surface and extends to between 7 km
(4.4 mi) at the poles and 17 km (10.6 mi) at the equator, with some variation due to weather
factors.</skos:definition>
    <skos:prefLabel xml:lang="en">Troposphere</skos:prefLabel>
    <skos:inScheme rdf:resource="http://isdc.gfz-potsdam.de/ontology/SPASE-allowed_values.skos.owl#Observatory_Region"/>
    <skos:inScheme rdf:resource="http://isdc.gfz-potsdam.de/ontology/SPASE-allowed_values.skos.owl#Observed_Region"/>
    <skos:broader rdf:resource="http://isdc.gfz-potsdam.de/ontology/SPASE-allowed_values.skos.owl#Near_Surface"/>
    <rdf:type rdf:resource="http://www.w3.org/2004/02/skos/core#Concept"/>
  </rdf:Description>
  <rdf:Description rdf:about="http://isdc.gfz-potsdam.de/ontology/SPASE-allowed_values.skos.owl#Substorm">
    <rdf:type rdf:resource="http://www.w3.org/2002/07/owl#NamedIndividual"/>
    <skos:prefLabel xml:lang="en">Substorm</skos:prefLabel>
    <skos:definition xml:lang="en">A process by which plasma in the magnetotail becomes energized at a fast rate.</skos:definition>
    <skos:inScheme rdf:resource="http://isdc.gfz-potsdam.de/ontology/SPASE-allowed_values.skos.owl#Phenomenon_Type"/>
    <skos:topConceptOf rdf:resource="http://isdc.gfz-potsdam.de/ontology/SPASE-allowed_values.skos.owl#Phenomenon_Type"/>
    <rdf:type rdf:resource="http://www.w3.org/2004/02/skos/core#Concept"/>
  </rdf:Description>
  <rdf:Description rdf:about="http://isdc.gfz-potsdam.de/ontology/SPASE-allowed_values.skos.owl#HAE">
    <skos:definition xml:lang="en">Heliocentric Aries Ecliptic - A coordinate system where the Z axis is normal to the ecliptic
plane, positive northward. X axis is positive towards the first point of Aries (from Earth to Sun
at vernal equinox). Same as SE below. See Hapgood, 1992.</skos:definition>
    <skos:inScheme rdf:resource="http://isdc.gfz-potsdam.de/ontology/SPASE-allowed_values.skos.owl#Coordinate_System_Name"/>
    <skos:topConceptOf rdf:resource="http://isdc.gfz-potsdam.de/ontology/SPASE-allowed_values.skos.owl#Coordinate_System_Name"/>
    <skos:prefLabel xml:lang="en">HAE</skos:prefLabel>
    <rdf:type rdf:resource="http://www.w3.org/2002/07/owl#NamedIndividual"/>
    <rdf:type rdf:resource="http://www.w3.org/2004/02/skos/core#Concept"/>
  </rdf:Description>
  <rdf:Description rdf:about="http://isdc.gfz-potsdam.de/ontology/SPASE-allowed_values.skos.owl#Hydrodynamic">
    <rdf:type rdf:resource="http://www.w3.org/2002/07/owl#NamedIndividual"/>
    <skos:topConceptOf rdf:resource="http://isdc.gfz-potsdam.de/ontology/SPASE-allowed_values.skos.owl#Wave_Type"/>
    <skos:prefLabel>Hydrodynamic</skos:prefLabel>
    <skos:inScheme rdf:resource="http://isdc.gfz-potsdam.de/ontology/SPASE-allowed_values.skos.owl#Wave_Type"/>
    <skos:definition xml:lang="en">Periodic or quasi-periodic oscillations of fluid quantities.</skos:definition>
    <rdf:type rdf:resource="http://www.w3.org/2004/02/skos/core#Concept"/>
  </rdf:Description>
  <rdf:Description rdf:about="http://isdc.gfz-potsdam.de/ontology/SPASE-allowed_values.skos.owl#Waveform_Receiver">
    <skos:definition xml:lang="en">A radio receiver which outputs the value of one or more components of the electric and/or
magnetic field as a function of time.</skos:definition>
    <rdf:type rdf:resource="http://www.w3.org/2004/02/skos/core#Concept"/>
    <rdf:type rdf:resource="http://www.w3.org/2002/07/owl#NamedIndividual"/>
    <skos:prefLabel xml:lang="en">Waveform Receiver</skos:prefLabel>
    <skos:inScheme rdf:resource="http://isdc.gfz-potsdam.de/ontology/SPASE-allowed_values.skos.owl#Instrument_Type"/>
    <skos:topConceptOf rdf:resource="http://isdc.gfz-potsdam.de/ontology/SPASE-allowed_values.skos.owl#Instrument_Type"/>
  </rdf:Description>
  <rdf:Description rdf:about="http://isdc.gfz-potsdam.de/ontology/SPASE-allowed_values.skos.owl#X-Rays">
    <skos:definition xml:lang="en">Photons with a wavelength range: 0.001 &lt;= x &lt; 10 nm</skos:definition>
    <skos:topConceptOf rdf:resource="http://isdc.gfz-potsdam.de/ontology/SPASE-allowed_values.skos.owl#Spectral_Range"/>
    <skos:inScheme rdf:resource="http://isdc.gfz-potsdam.de/ontology/SPASE-allowed_values.skos.owl#Spectral_Range"/>
    <rdf:type rdf:resource="http://www.w3.org/2002/07/owl#NamedIndividual"/>
    <rdf:type rdf:resource="http://www.w3.org/2004/02/skos/core#Concept"/>
    <skos:prefLabel xml:lang="en">X-Rays</skos:prefLabel>
  </rdf:Description>
  <rdf:Description rdf:about="http://isdc.gfz-potsdam.de/ontology/SPASE-allowed_values.skos.owl#J">
    <skos:definition xml:lang="en">Projection of a vector along the second named axis of a coordinate system. Typically the Y
axis, but could be the T axis for an RTN coordinate system.</skos:definition>
    <skos:broader rdf:resource="http://isdc.gfz-potsdam.de/ontology/SPASE-allowed_values.skos.owl#Component"/>
    <skos:inScheme rdf:resource="http://isdc.gfz-potsdam.de/ontology/SPASE-allowed_values.skos.owl#Qualifier"/>
    <rdf:type rdf:resource="http://www.w3.org/2002/07/owl#NamedIndividual"/>
    <rdf:type rdf:resource="http://www.w3.org/2004/02/skos/core#Concept"/>
    <skos:prefLabel xml:lang="en">J</skos:prefLabel>
  </rdf:Description>
  <rdf:Description rdf:about="http://isdc.gfz-potsdam.de/ontology/SPASE-allowed_values.skos.owl#Radar">
    <rdf:type rdf:resource="http://www.w3.org/2004/02/skos/core#Concept"/>
    <skos:definition xml:lang="en">An instrument that uses directional properties of returned power to infer spatial and/or other
characteristics of a remote object.</skos:definition>
    <skos:topConceptOf rdf:resource="http://isdc.gfz-potsdam.de/ontology/SPASE-allowed_values.skos.owl#Instrument_Type"/>
    <skos:prefLabel xml:lang="en">Radar</skos:prefLabel>
    <skos:inScheme rdf:resource="http://isdc.gfz-potsdam.de/ontology/SPASE-allowed_values.skos.owl#Instrument_Type"/>
    <rdf:type rdf:resource="http://www.w3.org/2002/07/owl#NamedIndividual"/>
  </rdf:Description>
  <rdf:Description rdf:about="http://isdc.gfz-potsdam.de/ontology/SPASE-allowed_values.skos.owl#Observed_By">
    <skos:prefLabel xml:lang="en">Observed By</skos:prefLabel>
    <skos:definition xml:lang="en">Detected or originating from another resource.</skos:definition>
    <rdf:type rdf:resource="http://www.w3.org/2002/07/owl#NamedIndividual"/>
    <rdf:type rdf:resource="http://www.w3.org/2004/02/skos/core#Concept"/>
    <skos:topConceptOf rdf:resource="http://isdc.gfz-potsdam.de/ontology/SPASE-allowed_values.skos.owl#Association_Type"/>
    <skos:inScheme rdf:resource="http://isdc.gfz-potsdam.de/ontology/SPASE-allowed_values.skos.owl#Association_Type"/>
  </rdf:Description>
  <rdf:Description rdf:about="http://isdc.gfz-potsdam.de/ontology/SPASE-allowed_values.skos.owl#Perturbation">
    <skos:inScheme rdf:resource="http://isdc.gfz-potsdam.de/ontology/SPASE-allowed_values.skos.owl#Qualifier"/>
    <skos:definition xml:lang="en">Variations in the state of a system.</skos:definition>
    <skos:topConceptOf rdf:resource="http://isdc.gfz-potsdam.de/ontology/SPASE-allowed_values.skos.owl#Qualifier"/>
    <rdf:type rdf:resource="http://www.w3.org/2004/02/skos/core#Concept"/>
    <rdf:type rdf:resource="http://www.w3.org/2002/07/owl#NamedIndividual"/>
    <skos:prefLabel xml:lang="en">Perturbation</skos:prefLabel>
  </rdf:Description>
  <rdf:Description rdf:about="http://isdc.gfz-potsdam.de/ontology/SPASE-allowed_values.skos.owl#Revision_Of">
    <skos:topConceptOf rdf:resource="http://isdc.gfz-potsdam.de/ontology/SPASE-allowed_values.skos.owl#Association_Type"/>
    <skos:definition xml:lang="en">A modified version of a resource instance.</skos:definition>
    <skos:inScheme rdf:resource="http://isdc.gfz-potsdam.de/ontology/SPASE-allowed_values.skos.owl#Association_Type"/>
    <rdf:type rdf:resource="http://www.w3.org/2004/02/skos/core#Concept"/>
    <rdf:type rdf:resource="http://www.w3.org/2002/07/owl#NamedIndividual"/>
    <skos:prefLabel xml:lang="en">Revision Of</skos:prefLabel>
  </rdf:Description>
  <rdf:Description rdf:about="http://isdc.gfz-potsdam.de/ontology/SPASE-allowed_values.skos.owl#Cross_Spectrum">
    <rdf:type rdf:resource="http://www.w3.org/2002/07/owl#NamedIndividual"/>
    <rdf:type rdf:resource="http://www.w3.org/2004/02/skos/core#Concept"/>
    <skos:definition xml:lang="en">The Fourier transform of the cross correlation of two physical or empirical observations.</skos:definition>
    <skos:prefLabel xml:lang="en">Cross Spectrum</skos:prefLabel>
    <skos:topConceptOf rdf:resource="http://isdc.gfz-potsdam.de/ontology/SPASE-allowed_values.skos.owl#Qualifier"/>
    <skos:inScheme rdf:resource="http://isdc.gfz-potsdam.de/ontology/SPASE-allowed_values.skos.owl#Qualifier"/>
  </rdf:Description>
  <rdf:Description rdf:about="http://isdc.gfz-potsdam.de/ontology/SPASE-allowed_values.skos.owl#Plasma_Beta">
    <skos:inScheme rdf:resource="http://isdc.gfz-potsdam.de/ontology/SPASE-allowed_values.skos.owl#Mixed_Quantity"/>
    <rdf:type rdf:resource="http://www.w3.org/2002/07/owl#NamedIndividual"/>
    <rdf:type rdf:resource="http://www.w3.org/2004/02/skos/core#Concept"/>
    <skos:definition xml:lang="en">The ratio of the plasma pressure (nkT) to the magnetic pressure (B^2/2mu0) of the
SUM(nkT)/(B^2/2mu0).</skos:definition>
    <skos:prefLabel xml:lang="en">Plasma Beta</skos:prefLabel>
    <skos:topConceptOf rdf:resource="http://isdc.gfz-potsdam.de/ontology/SPASE-allowed_values.skos.owl#Mixed_Quantity"/>
  </rdf:Description>
  <rdf:Description rdf:about="http://isdc.gfz-potsdam.de/ontology/SPASE-allowed_values.skos.owl#SM">
    <skos:inScheme rdf:resource="http://isdc.gfz-potsdam.de/ontology/SPASE-allowed_values.skos.owl#Coordinate_System_Name"/>
    <rdf:type rdf:resource="http://www.w3.org/2004/02/skos/core#Concept"/>
    <skos:topConceptOf rdf:resource="http://isdc.gfz-potsdam.de/ontology/SPASE-allowed_values.skos.owl#Coordinate_System_Name"/>
    <rdf:type rdf:resource="http://www.w3.org/2002/07/owl#NamedIndividual"/>
    <skos:definition xml:lang="en">Solar Magnetic - A geocentric coordinate system where the Z axis is northward along Earth's
dipole axis, X axis is in plane of z axis and Earth-Sun line, positive sunward. See Russell, 1971.</skos:definition>
    <skos:prefLabel xml:lang="en">SM</skos:prefLabel>
  </rdf:Description>
  <rdf:Description rdf:about="http://isdc.gfz-potsdam.de/ontology/SPASE-allowed_values.skos.owl#Column">
    <skos:inScheme rdf:resource="http://isdc.gfz-potsdam.de/ontology/SPASE-allowed_values.skos.owl#Qualifier"/>
    <skos:definition xml:lang="en">A two-dimensional measure of a quantity. The column is the area over which the quantity is
measured.</skos:definition>
    <rdf:type rdf:resource="http://www.w3.org/2004/02/skos/core#Concept"/>
    <skos:prefLabel xml:lang="en">Column</skos:prefLabel>
    <rdf:type rdf:resource="http://www.w3.org/2002/07/owl#NamedIndividual"/>
    <skos:topConceptOf rdf:resource="http://isdc.gfz-potsdam.de/ontology/SPASE-allowed_values.skos.owl#Qualifier"/>
  </rdf:Description>
  <rdf:Description rdf:about="http://isdc.gfz-potsdam.de/ontology/SPASE-allowed_values.skos.owl#Count_Rate">
    <skos:inScheme rdf:resource="http://isdc.gfz-potsdam.de/ontology/SPASE-allowed_values.skos.owl#Particle_Quantity"/>
    <rdf:type rdf:resource="http://www.w3.org/2004/02/skos/core#Concept"/>
    <rdf:type rdf:resource="http://www.w3.org/2002/07/owl#NamedIndividual"/>
    <skos:prefLabel xml:lang="en">Count Rate</skos:prefLabel>
    <skos:topConceptOf rdf:resource="http://isdc.gfz-potsdam.de/ontology/SPASE-allowed_values.skos.owl#Particle_Quantity"/>
    <skos:definition xml:lang="en">The number of events per unit time.</skos:definition>
  </rdf:Description>
  <rdf:Description rdf:about="http://isdc.gfz-potsdam.de/ontology/SPASE-allowed_values.skos.owl#Electrostatic">
    <skos:topConceptOf rdf:resource="http://isdc.gfz-potsdam.de/ontology/SPASE-allowed_values.skos.owl#Wave_Type"/>
    <rdf:type rdf:resource="http://www.w3.org/2004/02/skos/core#Concept"/>
    <rdf:type rdf:resource="http://www.w3.org/2002/07/owl#NamedIndividual"/>
    <skos:definition xml:lang="en">Collective longitudinal electric-field and plasma oscillations trapped within a body of plasma.</skos:definition>
    <skos:inScheme rdf:resource="http://isdc.gfz-potsdam.de/ontology/SPASE-allowed_values.skos.owl#Wave_Type"/>
    <skos:prefLabel>Electrostatic</skos:prefLabel>
  </rdf:Description>
  <rdf:Description rdf:about="http://isdc.gfz-potsdam.de/ontology/SPASE-allowed_values.skos.owl#Stratosphere">
    <skos:definition xml:lang="en">The layer of the atmosphere that extends from the troposphere to about 30 km, temperature
increases with height. The stratosphere contains the ozone layer.</skos:definition>
    <skos:inScheme rdf:resource="http://isdc.gfz-potsdam.de/ontology/SPASE-allowed_values.skos.owl#Observed_Region"/>
    <skos:broader rdf:resource="http://isdc.gfz-potsdam.de/ontology/SPASE-allowed_values.skos.owl#Near_Surface"/>
    <skos:inScheme rdf:resource="http://isdc.gfz-potsdam.de/ontology/SPASE-allowed_values.skos.owl#Observatory_Region"/>
    <rdf:type rdf:resource="http://www.w3.org/2004/02/skos/core#Concept"/>
    <rdf:type rdf:resource="http://www.w3.org/2002/07/owl#NamedIndividual"/>
    <skos:prefLabel xml:lang="en">Stratosphere</skos:prefLabel>
  </rdf:Description>
  <rdf:Description rdf:about="http://isdc.gfz-potsdam.de/ontology/SPASE-allowed_values.skos.owl#Phase">
    <rdf:type rdf:resource="http://www.w3.org/2002/07/owl#NamedIndividual"/>
    <skos:prefLabel xml:lang="en">Phase</skos:prefLabel>
    <skos:inScheme rdf:resource="http://isdc.gfz-potsdam.de/ontology/SPASE-allowed_values.skos.owl#Qualifier"/>
    <rdf:type rdf:resource="http://www.w3.org/2004/02/skos/core#Concept"/>
    <skos:topConceptOf rdf:resource="http://isdc.gfz-potsdam.de/ontology/SPASE-allowed_values.skos.owl#Qualifier"/>
    <skos:definition xml:lang="en">A point or portion in a recurring series of changes.</skos:definition>
  </rdf:Description>
  <rdf:Description rdf:about="http://isdc.gfz-potsdam.de/ontology/SPASE-allowed_values.skos.owl#Data">
    <skos:prefLabel xml:lang="en">Data</skos:prefLabel>
    <rdf:type rdf:resource="http://www.w3.org/2002/07/owl#NamedIndividual"/>
    <skos:topConceptOf rdf:resource="http://isdc.gfz-potsdam.de/ontology/SPASE-allowed_values.skos.owl#Source_Type"/>
    <rdf:type rdf:resource="http://www.w3.org/2004/02/skos/core#Concept"/>
    <skos:inScheme rdf:resource="http://isdc.gfz-potsdam.de/ontology/SPASE-allowed_values.skos.owl#Source_Type"/>
    <skos:definition xml:lang="en">A collection of organized information, usually the results of experience, observation or
experiment, or a set of premises. This may consist of numbers, words, or images, particularly as
measurements or observations of a set of variables.</skos:definition>
  </rdf:Description>
  <rdf:Description rdf:about="http://isdc.gfz-potsdam.de/ontology/SPASE-allowed_values.skos.owl#Direction_Angle">
    <rdf:type rdf:resource="http://www.w3.org/2004/02/skos/core#Concept"/>
    <skos:narrower rdf:resource="http://isdc.gfz-potsdam.de/ontology/SPASE-allowed_values.skos.owl#Elevation_Angle"/>
    <skos:topConceptOf rdf:resource="http://isdc.gfz-potsdam.de/ontology/SPASE-allowed_values.skos.owl#Qualifier"/>
    <skos:narrower rdf:resource="http://isdc.gfz-potsdam.de/ontology/SPASE-allowed_values.skos.owl#Polar_Angle"/>
    <skos:inScheme rdf:resource="http://isdc.gfz-potsdam.de/ontology/SPASE-allowed_values.skos.owl#Qualifier"/>
    <skos:definition xml:lang="en">The angle between a position vector or measured vector (or one of its projections onto a plane)
and one of the base axes of the coordinate system.
Allowed Values:
Azimuth Angle
Elevation Angle
Polar Angle</skos:definition>
    <skos:prefLabel xml:lang="en">Direction Angle</skos:prefLabel>
    <skos:narrower rdf:resource="http://isdc.gfz-potsdam.de/ontology/SPASE-allowed_values.skos.owl#Azimuth_Angle"/>
    <rdf:type rdf:resource="http://www.w3.org/2002/07/owl#NamedIndividual"/>
  </rdf:Description>
  <rdf:Description rdf:about="http://isdc.gfz-potsdam.de/ontology/SPASE-allowed_values.skos.owl#Electric">
    <rdf:type rdf:resource="http://www.w3.org/2002/07/owl#NamedIndividual"/>
    <rdf:type rdf:resource="http://www.w3.org/2004/02/skos/core#Concept"/>
    <skos:definition xml:lang="en">The physical attribute that exerts an electrical force.</skos:definition>
    <skos:inScheme rdf:resource="http://isdc.gfz-potsdam.de/ontology/SPASE-allowed_values.skos.owl#Field_Quantity"/>
    <skos:topConceptOf rdf:resource="http://isdc.gfz-potsdam.de/ontology/SPASE-allowed_values.skos.owl#Field_Quantity"/>
    <skos:prefLabel xml:lang="en">Electric</skos:prefLabel>
  </rdf:Description>
  <rdf:Description rdf:about="http://isdc.gfz-potsdam.de/ontology/SPASE-allowed_values.skos.owl#GEO">
    <rdf:type rdf:resource="http://www.w3.org/2002/07/owl#NamedIndividual"/>
    <skos:topConceptOf rdf:resource="http://isdc.gfz-potsdam.de/ontology/SPASE-allowed_values.skos.owl#Coordinate_System_Name"/>
    <skos:inScheme rdf:resource="http://isdc.gfz-potsdam.de/ontology/SPASE-allowed_values.skos.owl#Coordinate_System_Name"/>
    <skos:definition xml:lang="en">Geographic - geocentric corotating - A coordinate system where the Z axis is along Earth's spin
vector, positive northward. X axis lies in Greenwich meridian, positive towards Greenwich. See
Russell, 1971.</skos:definition>
    <skos:prefLabel xml:lang="en">GEO</skos:prefLabel>
    <rdf:type rdf:resource="http://www.w3.org/2004/02/skos/core#Concept"/>
  </rdf:Description>
  <rdf:Description rdf:about="http://isdc.gfz-potsdam.de/ontology/SPASE-allowed_values.skos.owl#Vector">
    <skos:topConceptOf rdf:resource="http://isdc.gfz-potsdam.de/ontology/SPASE-allowed_values.skos.owl#Qualifier"/>
    <rdf:type rdf:resource="http://www.w3.org/2004/02/skos/core#Concept"/>
    <rdf:type rdf:resource="http://www.w3.org/2002/07/owl#NamedIndividual"/>
    <skos:definition xml:lang="en">A set of parameter values each along some independent variable (e.g., components of a field in
three orthogonal spatial directions; atmospheric temperature values at several altitudes, or at a
given latitude and longitude;).</skos:definition>
    <skos:prefLabel xml:lang="en">Vector</skos:prefLabel>
    <skos:inScheme rdf:resource="http://isdc.gfz-potsdam.de/ontology/SPASE-allowed_values.skos.owl#Qualifier"/>
  </rdf:Description>
  <rdf:Description rdf:about="http://isdc.gfz-potsdam.de/ontology/SPASE-allowed_values.skos.owl#Anomaly">
    <skos:topConceptOf rdf:resource="http://isdc.gfz-potsdam.de/ontology/SPASE-allowed_values.skos.owl#Annotation_Type"/>
    <skos:prefLabel xml:lang="en">Anomaly</skos:prefLabel>
    <rdf:type rdf:resource="http://www.w3.org/2004/02/skos/core#Concept"/>
    <skos:definition xml:lang="en">An interval where measurements or observations may be adversely affected.</skos:definition>
    <rdf:type rdf:resource="http://www.w3.org/2002/07/owl#NamedIndividual"/>
    <skos:inScheme rdf:resource="http://isdc.gfz-potsdam.de/ontology/SPASE-allowed_values.skos.owl#Annotation_Type"/>
  </rdf:Description>
  <rdf:Description rdf:about="http://isdc.gfz-potsdam.de/ontology/SPASE-allowed_values.skos.owl#Poynting_Flux">
    <skos:inScheme rdf:resource="http://isdc.gfz-potsdam.de/ontology/SPASE-allowed_values.skos.owl#Wave_Quantity"/>
    <skos:prefLabel xml:lang="en">Poynting Flux</skos:prefLabel>
    <skos:definition xml:lang="en">Electromagnetic energy flux transported by a wave characterized as the rate of energy transport
per unit area per steradian.</skos:definition>
    <rdf:type rdf:resource="http://www.w3.org/2004/02/skos/core#Concept"/>
    <rdf:type rdf:resource="http://www.w3.org/2002/07/owl#NamedIndividual"/>
    <skos:topConceptOf rdf:resource="http://isdc.gfz-potsdam.de/ontology/SPASE-allowed_values.skos.owl#Wave_Quantity"/>
    <skos:inScheme rdf:resource="http://isdc.gfz-potsdam.de/ontology/SPASE-allowed_values.skos.owl#Field_Quantity"/>
    <skos:topConceptOf rdf:resource="http://isdc.gfz-potsdam.de/ontology/SPASE-allowed_values.skos.owl#Field_Quantity"/>
  </rdf:Description>
  <rdf:Description rdf:about="http://isdc.gfz-potsdam.de/ontology/SPASE-allowed_values.skos.owl#Team_Member">
    <skos:prefLabel xml:lang="en">Team Member</skos:prefLabel>
    <skos:definition xml:lang="en">An individual who is a major participant in an investigation.</skos:definition>
    <skos:inScheme rdf:resource="http://isdc.gfz-potsdam.de/ontology/SPASE-allowed_values.skos.owl#Role"/>
    <skos:topConceptOf rdf:resource="http://isdc.gfz-potsdam.de/ontology/SPASE-allowed_values.skos.owl#Role"/>
    <rdf:type rdf:resource="http://www.w3.org/2002/07/owl#NamedIndividual"/>
    <rdf:type rdf:resource="http://www.w3.org/2004/02/skos/core#Concept"/>
  </rdf:Description>
  <rdf:Description rdf:about="http://isdc.gfz-potsdam.de/ontology/SPASE-allowed_values.skos.owl#Support_Quantity">
    <skos:hasTopConcept rdf:resource="http://isdc.gfz-potsdam.de/ontology/SPASE-allowed_values.skos.owl#Temporal"/>
    <skos:hasTopConcept rdf:resource="http://isdc.gfz-potsdam.de/ontology/SPASE-allowed_values.skos.owl#Positional"/>
    <skos:hasTopConcept rdf:resource="http://isdc.gfz-potsdam.de/ontology/SPASE-allowed_values.skos.owl#Instrument_Mode"/>
    <skos:hasTopConcept rdf:resource="http://isdc.gfz-potsdam.de/ontology/SPASE-allowed_values.skos.owl#Velocity"/>
    <skos:definition xml:lang="en">A characterization of the support information.
Allowed Values:
Instrument Mode
Other
Positional
Temporal
Velocity</skos:definition>
    <skos:hasTopConcept rdf:resource="http://isdc.gfz-potsdam.de/ontology/SPASE-allowed_values.skos.owl#SQ_Other"/>
    <rdf:type rdf:resource="http://www.w3.org/2002/07/owl#NamedIndividual"/>
    <rdf:type rdf:resource="http://www.w3.org/2004/02/skos/core#ConceptScheme"/>
    <skos:prefLabel xml:lang="en">Support Quantity</skos:prefLabel>
  </rdf:Description>
  <rdf:Description rdf:about="http://isdc.gfz-potsdam.de/ontology/SPASE-allowed_values.skos.owl#Calibrated">
    <rdf:type rdf:resource="http://www.w3.org/2002/07/owl#NamedIndividual"/>
    <rdf:type rdf:resource="http://www.w3.org/2004/02/skos/core#Concept"/>
    <skos:topConceptOf rdf:resource="http://isdc.gfz-potsdam.de/ontology/SPASE-allowed_values.skos.owl#Processing_Level"/>
    <skos:prefLabel xml:lang="en">Calibrated</skos:prefLabel>
    <skos:inScheme rdf:resource="http://isdc.gfz-potsdam.de/ontology/SPASE-allowed_values.skos.owl#Processing_Level"/>
    <skos:definition xml:lang="en">Data wherein sensor outputs have been convolved with instrument response function, often
irreversibly, to yield data in physical units.</skos:definition>
  </rdf:Description>
  <rdf:Description rdf:about="http://isdc.gfz-potsdam.de/ontology/SPASE-allowed_values.skos.owl#Magnetic_Cloud">
    <skos:inScheme rdf:resource="http://isdc.gfz-potsdam.de/ontology/SPASE-allowed_values.skos.owl#Phenomenon_Type"/>
    <skos:topConceptOf rdf:resource="http://isdc.gfz-potsdam.de/ontology/SPASE-allowed_values.skos.owl#Phenomenon_Type"/>
    <skos:prefLabel xml:lang="en">Magnetic Cloud</skos:prefLabel>
    <rdf:type rdf:resource="http://www.w3.org/2002/07/owl#NamedIndividual"/>
    <rdf:type rdf:resource="http://www.w3.org/2004/02/skos/core#Concept"/>
    <skos:definition xml:lang="en">A transient event observed in the solar wind characterized as a region of enhanced magnetic
field strength, smooth rotation of the magnetic field vector and low proton density and
temperature.</skos:definition>
  </rdf:Description>
  <rdf:Description rdf:about="http://isdc.gfz-potsdam.de/ontology/SPASE-allowed_values.skos.owl#Availability">
    <skos:prefLabel xml:lang="en">Availability</skos:prefLabel>
    <rdf:type rdf:resource="http://www.w3.org/2004/02/skos/core#ConceptScheme"/>
    <skos:hasTopConcept rdf:resource="http://isdc.gfz-potsdam.de/ontology/SPASE-allowed_values.skos.owl#Online"/>
    <rdf:type rdf:resource="http://www.w3.org/2002/07/owl#NamedIndividual"/>
    <skos:hasTopConcept rdf:resource="http://isdc.gfz-potsdam.de/ontology/SPASE-allowed_values.skos.owl#Offline"/>
    <skos:definition xml:lang="en">An indication of the method or service which may be used to access the resource.
Allowed Values:
Offline
Online</skos:definition>
  </rdf:Description>
  <rdf:Description rdf:about="http://isdc.gfz-potsdam.de/ontology/SPASE-allowed_values.skos.owl#Charge_State">
    <skos:inScheme rdf:resource="http://isdc.gfz-potsdam.de/ontology/SPASE-allowed_values.skos.owl#Particle_Quantity"/>
    <skos:prefLabel xml:lang="en">Charge State</skos:prefLabel>
    <rdf:type rdf:resource="http://www.w3.org/2004/02/skos/core#Concept"/>
    <rdf:type rdf:resource="http://www.w3.org/2002/07/owl#NamedIndividual"/>
    <skos:topConceptOf rdf:resource="http://isdc.gfz-potsdam.de/ontology/SPASE-allowed_values.skos.owl#Particle_Quantity"/>
    <skos:definition xml:lang="en">Charge of a fully or partially stripped ion, in units of the charge of a proton. Charge state of a
bare proton = 1.</skos:definition>
  </rdf:Description>
  <rdf:Description rdf:about="http://isdc.gfz-potsdam.de/ontology/SPASE-allowed_values.skos.owl#Alfven_Mach_Number">
    <skos:inScheme rdf:resource="http://isdc.gfz-potsdam.de/ontology/SPASE-allowed_values.skos.owl#Mixed_Quantity"/>
    <rdf:type rdf:resource="http://www.w3.org/2002/07/owl#NamedIndividual"/>
    <rdf:type rdf:resource="http://www.w3.org/2004/02/skos/core#Concept"/>
    <skos:definition xml:lang="en">The ratio of the bulk flow speed to the Alfven speed.</skos:definition>
    <skos:prefLabel xml:lang="en">Alfven Mach Number</skos:prefLabel>
    <skos:topConceptOf rdf:resource="http://isdc.gfz-potsdam.de/ontology/SPASE-allowed_values.skos.owl#Mixed_Quantity"/>
  </rdf:Description>
  <rdf:Description rdf:about="http://isdc.gfz-potsdam.de/ontology/SPASE-allowed_values.skos.owl#Electron">
    <skos:definition xml:lang="en">An elementary particle consisting of a charge of negative electricity equal to about 1.602 x
10^(-19) Coulomb and having a mass when at rest of about 9.109534 x 10^(-28) gram.</skos:definition>
    <rdf:type rdf:resource="http://www.w3.org/2004/02/skos/core#Concept"/>
    <skos:inScheme rdf:resource="http://isdc.gfz-potsdam.de/ontology/SPASE-allowed_values.skos.owl#Particle_Type"/>
    <rdf:type rdf:resource="http://www.w3.org/2002/07/owl#NamedIndividual"/>
    <skos:prefLabel xml:lang="en">Electron</skos:prefLabel>
    <skos:topConceptOf rdf:resource="http://isdc.gfz-potsdam.de/ontology/SPASE-allowed_values.skos.owl#Particle_Type"/>
  </rdf:Description>
  <rdf:Description rdf:about="http://isdc.gfz-potsdam.de/ontology/SPASE-allowed_values.skos.owl#Former-PI">
    <skos:topConceptOf rdf:resource="http://isdc.gfz-potsdam.de/ontology/SPASE-allowed_values.skos.owl#Role"/>
    <skos:definition xml:lang="en">An individual who had served as the administrative and scientific lead for an investigation, but
no longer assumes that role.</skos:definition>
    <skos:prefLabel xml:lang="en">Former-PI</skos:prefLabel>
    <skos:inScheme rdf:resource="http://isdc.gfz-potsdam.de/ontology/SPASE-allowed_values.skos.owl#Role"/>
    <rdf:type rdf:resource="http://www.w3.org/2004/02/skos/core#Concept"/>
    <rdf:type rdf:resource="http://www.w3.org/2002/07/owl#NamedIndividual"/>
  </rdf:Description>
  <rdf:Description rdf:about="http://isdc.gfz-potsdam.de/ontology/SPASE-allowed_values.skos.owl#Polar_Cap">
    <rdf:type rdf:resource="http://www.w3.org/2002/07/owl#NamedIndividual"/>
    <skos:prefLabel xml:lang="en">Polar Cap</skos:prefLabel>
    <skos:inScheme rdf:resource="http://isdc.gfz-potsdam.de/ontology/SPASE-allowed_values.skos.owl#Observatory_Region"/>
    <skos:inScheme rdf:resource="http://isdc.gfz-potsdam.de/ontology/SPASE-allowed_values.skos.owl#Observed_Region"/>
    <skos:broader rdf:resource="http://isdc.gfz-potsdam.de/ontology/SPASE-allowed_values.skos.owl#Near_Surface"/>
    <skos:definition xml:lang="en">The areas of the globe surrounding the poles and consisting of the region north of 60 degrees
north latitude an the region south of 60 degrees south latitude.</skos:definition>
    <rdf:type rdf:resource="http://www.w3.org/2004/02/skos/core#Concept"/>
  </rdf:Description>
  <rdf:Description rdf:about="http://isdc.gfz-potsdam.de/ontology/SPASE-allowed_values.skos.owl#Gyrofrequency">
    <skos:inScheme rdf:resource="http://isdc.gfz-potsdam.de/ontology/SPASE-allowed_values.skos.owl#Field_Quantity"/>
    <skos:prefLabel xml:lang="en">Gyrofrequency</skos:prefLabel>
    <skos:topConceptOf rdf:resource="http://isdc.gfz-potsdam.de/ontology/SPASE-allowed_values.skos.owl#Particle_Quantity"/>
    <rdf:type rdf:resource="http://www.w3.org/2002/07/owl#NamedIndividual"/>
    <rdf:type rdf:resource="http://www.w3.org/2004/02/skos/core#Concept"/>
    <skos:definition>The number of gyrations around a magnetic guiding center (field line) a charged particle makes
per unit time due to the Lorentz force.</skos:definition>
    <skos:topConceptOf rdf:resource="http://isdc.gfz-potsdam.de/ontology/SPASE-allowed_values.skos.owl#Wave_Quantity"/>
    <skos:inScheme rdf:resource="http://isdc.gfz-potsdam.de/ontology/SPASE-allowed_values.skos.owl#Particle_Quantity"/>
    <skos:topConceptOf rdf:resource="http://isdc.gfz-potsdam.de/ontology/SPASE-allowed_values.skos.owl#Field_Quantity"/>
    <skos:inScheme rdf:resource="http://isdc.gfz-potsdam.de/ontology/SPASE-allowed_values.skos.owl#Wave_Quantity"/>
  </rdf:Description>
  <rdf:Description rdf:about="http://isdc.gfz-potsdam.de/ontology/SPASE-allowed_values.skos.owl#SHA1">
    <rdf:type rdf:resource="http://www.w3.org/2004/02/skos/core#Concept"/>
    <rdf:type rdf:resource="http://www.w3.org/2002/07/owl#NamedIndividual"/>
    <skos:prefLabel xml:lang="en">SHA1</skos:prefLabel>
    <skos:definition xml:lang="en">Secure Hash Algorithm (SHA), a 160-bit message digest algorithm developed by the NSA and
described in Federal Information Processing Standard (FIPS) publication 180-1.</skos:definition>
    <skos:topConceptOf rdf:resource="http://isdc.gfz-potsdam.de/ontology/SPASE-allowed_values.skos.owl#Hash_Function"/>
    <skos:inScheme rdf:resource="http://isdc.gfz-potsdam.de/ontology/SPASE-allowed_values.skos.owl#Hash_Function"/>
  </rdf:Description>
  <rdf:Description rdf:about="http://isdc.gfz-potsdam.de/ontology/SPASE-allowed_values.skos.owl#Coronal_Mass_Ejection">
    <skos:definition xml:lang="en">A solar event (CME) that involves a burst of plasma ejected into the interplanetary medium.
CME's may be observed remotely relatively near the sun or in situ in the interplanetary
medium. The latter type of observations are often referred to as Interplanetary CME's (ICME's).</skos:definition>
    <skos:inScheme rdf:resource="http://isdc.gfz-potsdam.de/ontology/SPASE-allowed_values.skos.owl#Phenomenon_Type"/>
    <skos:topConceptOf rdf:resource="http://isdc.gfz-potsdam.de/ontology/SPASE-allowed_values.skos.owl#Phenomenon_Type"/>
    <skos:prefLabel xml:lang="en">Coronal Mass Ejection</skos:prefLabel>
    <rdf:type rdf:resource="http://www.w3.org/2002/07/owl#NamedIndividual"/>
    <rdf:type rdf:resource="http://www.w3.org/2004/02/skos/core#Concept"/>
  </rdf:Description>
  <rdf:Description rdf:about="http://isdc.gfz-potsdam.de/ontology/SPASE-allowed_values.skos.owl#Equivalent_Width">
    <rdf:type rdf:resource="http://www.w3.org/2004/02/skos/core#Concept"/>
    <skos:prefLabel xml:lang="en">Equivalent Width</skos:prefLabel>
    <skos:topConceptOf rdf:resource="http://isdc.gfz-potsdam.de/ontology/SPASE-allowed_values.skos.owl#Wave_Quantity"/>
    <skos:inScheme rdf:resource="http://isdc.gfz-potsdam.de/ontology/SPASE-allowed_values.skos.owl#Wave_Quantity"/>
    <skos:definition xml:lang="en">The spectral width of a total absorption line having the amount of absorbed radiant energy
being equivalent to that in an observed absorption line.</skos:definition>
    <rdf:type rdf:resource="http://www.w3.org/2002/07/owl#NamedIndividual"/>
  </rdf:Description>
  <rdf:Description rdf:about="http://isdc.gfz-potsdam.de/ontology/SPASE-allowed_values.skos.owl#Confidence_Rating">
    <skos:hasTopConcept rdf:resource="http://isdc.gfz-potsdam.de/ontology/SPASE-allowed_values.skos.owl#Strong"/>
    <rdf:type rdf:resource="http://www.w3.org/2002/07/owl#NamedIndividual"/>
    <skos:prefLabel xml:lang="en">Confidence Rating</skos:prefLabel>
    <skos:hasTopConcept rdf:resource="http://isdc.gfz-potsdam.de/ontology/SPASE-allowed_values.skos.owl#Probable"/>
    <skos:definition xml:lang="en">A classification of the certainty of an assertion.
Allowed Values:
Probable
Strong
Unlikely
Weak</skos:definition>
    <skos:hasTopConcept rdf:resource="http://isdc.gfz-potsdam.de/ontology/SPASE-allowed_values.skos.owl#Weak"/>
    <skos:hasTopConcept rdf:resource="http://isdc.gfz-potsdam.de/ontology/SPASE-allowed_values.skos.owl#Unlikely"/>
    <rdf:type rdf:resource="http://www.w3.org/2004/02/skos/core#ConceptScheme"/>
  </rdf:Description>
  <rdf:Description rdf:about="http://isdc.gfz-potsdam.de/ontology/SPASE-allowed_values.skos.owl#Magnetic">
    <skos:prefLabel xml:lang="en">Magnetic</skos:prefLabel>
    <skos:inScheme rdf:resource="http://isdc.gfz-potsdam.de/ontology/SPASE-allowed_values.skos.owl#Field_Quantity"/>
    <skos:topConceptOf rdf:resource="http://isdc.gfz-potsdam.de/ontology/SPASE-allowed_values.skos.owl#Field_Quantity"/>
    <skos:definition xml:lang="en">The physical attribute attributed to a magnet or its equivalent.</skos:definition>
    <rdf:type rdf:resource="http://www.w3.org/2004/02/skos/core#Concept"/>
    <rdf:type rdf:resource="http://www.w3.org/2002/07/owl#NamedIndividual"/>
  </rdf:Description>
  <rdf:Description rdf:about="http://isdc.gfz-potsdam.de/ontology/SPASE-allowed_values.skos.owl#Active_Region">
    <skos:definition xml:lang="en">A localized, transient volume of the solar atmosphere in which PLAGEs, SUNSPOTS,
FACULAe, FLAREs, etc. may be observed.</skos:definition>
    <rdf:type rdf:resource="http://www.w3.org/2004/02/skos/core#Concept"/>
    <skos:topConceptOf rdf:resource="http://isdc.gfz-potsdam.de/ontology/SPASE-allowed_values.skos.owl#Phenomenon_Type"/>
    <skos:prefLabel xml:lang="en">Active Region</skos:prefLabel>
    <rdf:type rdf:resource="http://www.w3.org/2002/07/owl#NamedIndividual"/>
    <skos:inScheme rdf:resource="http://isdc.gfz-potsdam.de/ontology/SPASE-allowed_values.skos.owl#Phenomenon_Type"/>
  </rdf:Description>
  <rdf:Description rdf:about="http://isdc.gfz-potsdam.de/ontology/SPASE-allowed_values.skos.owl#Energy_Density">
    <skos:definition xml:lang="en">The amount of energy per unit volume.</skos:definition>
    <skos:inScheme rdf:resource="http://isdc.gfz-potsdam.de/ontology/SPASE-allowed_values.skos.owl#Particle_Quantity"/>
    <rdf:type rdf:resource="http://www.w3.org/2002/07/owl#NamedIndividual"/>
    <skos:prefLabel xml:lang="en">Energy Density</skos:prefLabel>
    <rdf:type rdf:resource="http://www.w3.org/2004/02/skos/core#Concept"/>
    <skos:topConceptOf rdf:resource="http://isdc.gfz-potsdam.de/ontology/SPASE-allowed_values.skos.owl#Particle_Quantity"/>
  </rdf:Description>
  <rdf:Description rdf:about="http://isdc.gfz-potsdam.de/ontology/SPASE-allowed_values.skos.owl#Sonic_Mach_Number">
    <rdf:type rdf:resource="http://www.w3.org/2002/07/owl#NamedIndividual"/>
    <skos:inScheme rdf:resource="http://isdc.gfz-potsdam.de/ontology/SPASE-allowed_values.skos.owl#Particle_Quantity"/>
    <skos:prefLabel xml:lang="en">Sonic Mach Number</skos:prefLabel>
    <skos:topConceptOf rdf:resource="http://isdc.gfz-potsdam.de/ontology/SPASE-allowed_values.skos.owl#Particle_Quantity"/>
    <skos:definition xml:lang="en">The ratio of the bulk flow speed to the speed of sound in the medium.</skos:definition>
    <rdf:type rdf:resource="http://www.w3.org/2004/02/skos/core#Concept"/>
  </rdf:Description>
  <rdf:Description rdf:about="http://isdc.gfz-potsdam.de/ontology/SPASE-allowed_values.skos.owl#Halo">
    <rdf:type rdf:resource="http://www.w3.org/2004/02/skos/core#Concept"/>
    <skos:definition xml:lang="en">The part of an object or distribution surrounding some central body or distribution. For
example, the particles above the core energies that show enhancements above the thermal
population. Typically, a "power law tail" shows a break from the core Maxwellian at a
particular energy.</skos:definition>
    <skos:topConceptOf rdf:resource="http://isdc.gfz-potsdam.de/ontology/SPASE-allowed_values.skos.owl#Qualifier"/>
    <skos:prefLabel xml:lang="en">Halo</skos:prefLabel>
    <skos:inScheme rdf:resource="http://isdc.gfz-potsdam.de/ontology/SPASE-allowed_values.skos.owl#Qualifier"/>
    <rdf:type rdf:resource="http://www.w3.org/2002/07/owl#NamedIndividual"/>
  </rdf:Description>
  <rdf:Description rdf:about="http://isdc.gfz-potsdam.de/ontology/SPASE-allowed_values.skos.owl#Image">
    <skos:definition xml:lang="en">A two-dimensional representation of data with values at each element of the array related to an
intensity or a color.</skos:definition>
    <skos:topConceptOf rdf:resource="http://isdc.gfz-potsdam.de/ontology/SPASE-allowed_values.skos.owl#Display_Type"/>
    <skos:prefLabel xml:lang="en">Image</skos:prefLabel>
    <skos:inScheme rdf:resource="http://isdc.gfz-potsdam.de/ontology/SPASE-allowed_values.skos.owl#Display_Type"/>
    <rdf:type rdf:resource="http://www.w3.org/2002/07/owl#NamedIndividual"/>
    <rdf:type rdf:resource="http://www.w3.org/2004/02/skos/core#Concept"/>
  </rdf:Description>
  <rdf:Description rdf:about="http://isdc.gfz-potsdam.de/ontology/SPASE-allowed_values.skos.owl#Film">
    <skos:prefLabel xml:lang="en">Film</skos:prefLabel>
    <skos:broader rdf:resource="http://isdc.gfz-potsdam.de/ontology/SPASE-allowed_values.skos.owl#Hardcopy"/>
    <rdf:type rdf:resource="http://www.w3.org/2004/02/skos/core#Concept"/>
    <rdf:type rdf:resource="http://www.w3.org/2002/07/owl#NamedIndividual"/>
    <skos:inScheme rdf:resource="http://isdc.gfz-potsdam.de/ontology/SPASE-allowed_values.skos.owl#Format"/>
    <skos:definition xml:lang="en">An image recording medium on which usually a "negative" analog image is registered. A
"positive" image can be recovered or reproduced from film, which is usually made of flexible
materials for ease of storage and transportation.</skos:definition>
  </rdf:Description>
  <rdf:Description rdf:about="http://isdc.gfz-potsdam.de/ontology/SPASE-allowed_values.skos.owl#Neutron">
    <skos:topConceptOf rdf:resource="http://isdc.gfz-potsdam.de/ontology/SPASE-allowed_values.skos.owl#Particle_Type"/>
    <rdf:type rdf:resource="http://www.w3.org/2002/07/owl#NamedIndividual"/>
    <skos:definition xml:lang="en">Neutron</skos:definition>
    <rdf:type rdf:resource="http://www.w3.org/2004/02/skos/core#Concept"/>
    <skos:definition xml:lang="en">An elementary particle that has no net charge and is a constituent of atomic nuclei, and that has
a mass slightly large than a proton (1.673 x 10^(-24) gram.).</skos:definition>
    <skos:inScheme rdf:resource="http://isdc.gfz-potsdam.de/ontology/SPASE-allowed_values.skos.owl#Particle_Type"/>
  </rdf:Description>
  <rdf:Description rdf:about="http://isdc.gfz-potsdam.de/ontology/SPASE-allowed_values.skos.owl#Deviation">
    <skos:topConceptOf rdf:resource="http://isdc.gfz-potsdam.de/ontology/SPASE-allowed_values.skos.owl#Qualifier"/>
    <skos:definition xml:lang="en">The difference between an observed value and the expected value of a quantity.</skos:definition>
    <skos:inScheme rdf:resource="http://isdc.gfz-potsdam.de/ontology/SPASE-allowed_values.skos.owl#Qualifier"/>
    <rdf:type rdf:resource="http://www.w3.org/2002/07/owl#NamedIndividual"/>
    <rdf:type rdf:resource="http://www.w3.org/2004/02/skos/core#Concept"/>
    <skos:prefLabel xml:lang="en">Deviation</skos:prefLabel>
  </rdf:Description>
  <rdf:Description rdf:about="http://isdc.gfz-potsdam.de/ontology/SPASE-allowed_values.skos.owl#MFA">
    <skos:topConceptOf rdf:resource="http://isdc.gfz-potsdam.de/ontology/SPASE-allowed_values.skos.owl#Coordinate_System_Name"/>
    <skos:prefLabel xml:lang="en">MFA</skos:prefLabel>
    <rdf:type rdf:resource="http://www.w3.org/2004/02/skos/core#Concept"/>
    <skos:inScheme rdf:resource="http://isdc.gfz-potsdam.de/ontology/SPASE-allowed_values.skos.owl#Coordinate_System_Name"/>
    <skos:definition xml:lang="en">Magnetic Field Aligned - A coordinate system spacecraft-centered system with Z in the
direction of the ambient magnetic field vector. X is in the plane defined by Z and the
spacecraft-Sun line, positive sunward. See &lt;http://cdpp.cnes.fr/00428.pdf&gt;.</skos:definition>
    <rdf:type rdf:resource="http://www.w3.org/2002/07/owl#NamedIndividual"/>
  </rdf:Description>
  <rdf:Description rdf:about="http://isdc.gfz-potsdam.de/ontology/SPASE-allowed_values.skos.owl#Peak">
    <rdf:type rdf:resource="http://www.w3.org/2002/07/owl#NamedIndividual"/>
    <skos:inScheme rdf:resource="http://isdc.gfz-potsdam.de/ontology/SPASE-allowed_values.skos.owl#Qualifier"/>
    <skos:prefLabel xml:lang="en">Peak</skos:prefLabel>
    <skos:topConceptOf rdf:resource="http://isdc.gfz-potsdam.de/ontology/SPASE-allowed_values.skos.owl#Qualifier"/>
    <skos:definition xml:lang="en">The maximum value for the quantity in question, over a period of time which is usually equal to
the cadence.</skos:definition>
    <rdf:type rdf:resource="http://www.w3.org/2004/02/skos/core#Concept"/>
  </rdf:Description>
  <rdf:Description rdf:about="http://isdc.gfz-potsdam.de/ontology/SPASE-allowed_values.skos.owl#Solid_Angle">
    <skos:prefLabel xml:lang="en">Solid Angle</skos:prefLabel>
    <rdf:type rdf:resource="http://www.w3.org/2002/07/owl#NamedIndividual"/>
    <rdf:type rdf:resource="http://www.w3.org/2004/02/skos/core#Concept"/>
    <skos:inScheme rdf:resource="http://isdc.gfz-potsdam.de/ontology/SPASE-allowed_values.skos.owl#Qualifier"/>
    <skos:definition xml:lang="en">Integration over the angle in three-dimensional space that an object subtends at a point.</skos:definition>
    <skos:broader rdf:resource="http://isdc.gfz-potsdam.de/ontology/SPASE-allowed_values.skos.owl#Integral"/>
  </rdf:Description>
  <rdf:Description rdf:about="http://isdc.gfz-potsdam.de/ontology/SPASE-allowed_values.skos.owl#LGM">
    <rdf:type rdf:resource="http://www.w3.org/2002/07/owl#NamedIndividual"/>
    <rdf:type rdf:resource="http://www.w3.org/2004/02/skos/core#Concept"/>
    <skos:topConceptOf rdf:resource="http://isdc.gfz-potsdam.de/ontology/SPASE-allowed_values.skos.owl#Coordinate_System_Name"/>
    <skos:inScheme rdf:resource="http://isdc.gfz-potsdam.de/ontology/SPASE-allowed_values.skos.owl#Coordinate_System_Name"/>
    <skos:prefLabel xml:lang="en">LGM</skos:prefLabel>
    <skos:definition xml:lang="en">Local Geomagnetic - A coordinate system used mainly for Earth surface or near Earth surface
magnetic field data. X axis northward from observation point in a geographic meridian. Z axis
downward towards Earth's center. In this system, H (total horizontal component) = SQRT
(Bx^2 + By^2) and D (declination angle) = arctan (By/Bx).</skos:definition>
  </rdf:Description>
  <rdf:Description rdf:about="http://isdc.gfz-potsdam.de/ontology/SPASE-allowed_values.skos.owl#Plasmasphere">
    <skos:inScheme rdf:resource="http://isdc.gfz-potsdam.de/ontology/SPASE-allowed_values.skos.owl#Observed_Region"/>
    <skos:broader rdf:resource="http://isdc.gfz-potsdam.de/ontology/SPASE-allowed_values.skos.owl#Near_Surface"/>
    <skos:inScheme rdf:resource="http://isdc.gfz-potsdam.de/ontology/SPASE-allowed_values.skos.owl#Observatory_Region"/>
    <skos:prefLabel xml:lang="en">Plasmasphere</skos:prefLabel>
    <rdf:type rdf:resource="http://www.w3.org/2002/07/owl#NamedIndividual"/>
    <rdf:type rdf:resource="http://www.w3.org/2004/02/skos/core#Concept"/>
    <skos:definition xml:lang="en">A region of the magnetosphere consisting of low energy (cool) plasma. It is located above the
ionosphere. The outer boundary of the plasmasphere is known as the plasmapause, which is
defined by an order of magnitude drop in plasma density.</skos:definition>
  </rdf:Description>
  <rdf:Description rdf:about="http://isdc.gfz-potsdam.de/ontology/SPASE-allowed_values.skos.owl#South_Atlantic_Anomaly_Region">
    <rdf:type rdf:resource="http://www.w3.org/2002/07/owl#NamedIndividual"/>
    <skos:definition xml:lang="en">The region where the Earth's inner van Allen radiation belt makes its closest approach to the
planet's surface. The result is that, for a given altitude, the radiation intensity is higher over this
region than elsewhere.</skos:definition>
    <skos:inScheme rdf:resource="http://isdc.gfz-potsdam.de/ontology/SPASE-allowed_values.skos.owl#Observatory_Region"/>
    <skos:inScheme rdf:resource="http://isdc.gfz-potsdam.de/ontology/SPASE-allowed_values.skos.owl#Observed_Region"/>
    <skos:prefLabel xml:lang="en">South Atlantic Anomaly Region</skos:prefLabel>
    <skos:broader rdf:resource="http://isdc.gfz-potsdam.de/ontology/SPASE-allowed_values.skos.owl#Near_Surface"/>
    <rdf:type rdf:resource="http://www.w3.org/2004/02/skos/core#Concept"/>
  </rdf:Description>
  <rdf:Description rdf:about="http://isdc.gfz-potsdam.de/ontology/SPASE-allowed_values.skos.owl#Imager">
    <rdf:type rdf:resource="http://www.w3.org/2004/02/skos/core#Concept"/>
    <skos:definition xml:lang="en">An instrument which samples the radiation from an area at one or more spectral ranges emitted
or reflected by an object.</skos:definition>
    <skos:topConceptOf rdf:resource="http://isdc.gfz-potsdam.de/ontology/SPASE-allowed_values.skos.owl#Instrument_Type"/>
    <skos:prefLabel xml:lang="en">Imager</skos:prefLabel>
    <skos:inScheme rdf:resource="http://isdc.gfz-potsdam.de/ontology/SPASE-allowed_values.skos.owl#Instrument_Type"/>
    <rdf:type rdf:resource="http://www.w3.org/2002/07/owl#NamedIndividual"/>
  </rdf:Description>
  <rdf:Description rdf:about="http://isdc.gfz-potsdam.de/ontology/SPASE-allowed_values.skos.owl#Activity_Index">
    <skos:inScheme rdf:resource="http://isdc.gfz-potsdam.de/ontology/SPASE-allowed_values.skos.owl#Measurement_Type"/>
    <rdf:type rdf:resource="http://www.w3.org/2004/02/skos/core#Concept"/>
    <rdf:type rdf:resource="http://www.w3.org/2002/07/owl#NamedIndividual"/>
    <skos:definition xml:lang="en">An indication, derived from one or more measurements, of the level of activity of an object or SPASE Data Model region, such as sunspot number, F10.7 flux, Dst, or the Polar Cap Indices.</skos:definition>
    <skos:topConceptOf rdf:resource="http://isdc.gfz-potsdam.de/ontology/SPASE-allowed_values.skos.owl#Measurement_Type"/>
    <skos:prefLabel xml:lang="en">Activity Index</skos:prefLabel>
  </rdf:Description>
  <rdf:Description rdf:about="http://isdc.gfz-potsdam.de/ontology/SPASE-allowed_values.skos.owl#GEI">
    <skos:inScheme rdf:resource="http://isdc.gfz-potsdam.de/ontology/SPASE-allowed_values.skos.owl#Coordinate_System_Name"/>
    <skos:prefLabel xml:lang="en">GEI</skos:prefLabel>
    <skos:topConceptOf rdf:resource="http://isdc.gfz-potsdam.de/ontology/SPASE-allowed_values.skos.owl#Coordinate_System_Name"/>
    <skos:definition xml:lang="en">Geocentric Equatorial Inertial - A coordinate system where the Z axis is along Earth's spin
vector, positive northward. X axis points towards the first point of Aries (from the Earth
towards the Sun at the vernal equinox). See Russell, 1971.</skos:definition>
    <rdf:type rdf:resource="http://www.w3.org/2002/07/owl#NamedIndividual"/>
    <rdf:type rdf:resource="http://www.w3.org/2004/02/skos/core#Concept"/>
  </rdf:Description>
  <rdf:Description rdf:about="http://isdc.gfz-potsdam.de/ontology/SPASE-allowed_values.skos.owl#Ion_Composition">
    <skos:topConceptOf rdf:resource="http://isdc.gfz-potsdam.de/ontology/SPASE-allowed_values.skos.owl#Measurement_Type"/>
    <rdf:type rdf:resource="http://www.w3.org/2002/07/owl#NamedIndividual"/>
    <rdf:type rdf:resource="http://www.w3.org/2004/02/skos/core#Concept"/>
    <skos:inScheme rdf:resource="http://isdc.gfz-potsdam.de/ontology/SPASE-allowed_values.skos.owl#Measurement_Type"/>
    <skos:prefLabel xml:lang="en">Ion Composition</skos:prefLabel>
    <skos:definition xml:lang="en">In situ measurements of the relative flux or density of electrically charged particles in the space
environment. May give simple fluxes, but full distribution functions are sometimes measured.</skos:definition>
  </rdf:Description>
  <rdf:Description rdf:about="http://isdc.gfz-potsdam.de/ontology/SPASE-allowed_values.skos.owl#Anisotropy">
    <skos:inScheme rdf:resource="http://isdc.gfz-potsdam.de/ontology/SPASE-allowed_values.skos.owl#Qualifier"/>
    <rdf:type rdf:resource="http://www.w3.org/2002/07/owl#NamedIndividual"/>
    <rdf:type rdf:resource="http://www.w3.org/2004/02/skos/core#Concept"/>
    <skos:prefLabel xml:lang="en">Anisotropy</skos:prefLabel>
    <skos:definition xml:lang="en">Direction-dependent property.</skos:definition>
    <skos:topConceptOf rdf:resource="http://isdc.gfz-potsdam.de/ontology/SPASE-allowed_values.skos.owl#Qualifier"/>
  </rdf:Description>
  <rdf:Description rdf:about="http://isdc.gfz-potsdam.de/ontology/SPASE-allowed_values.skos.owl#Energetic_Particle_Instrument">
    <rdf:type rdf:resource="http://www.w3.org/2004/02/skos/core#Concept"/>
    <skos:definition xml:lang="en">An instrument that measures fluxes of charged particles as a function of time, direction of
motion, mass, charge and/or species.</skos:definition>
    <skos:topConceptOf rdf:resource="http://isdc.gfz-potsdam.de/ontology/SPASE-allowed_values.skos.owl#Instrument_Type"/>
    <skos:prefLabel xml:lang="en">Energetic Particle Instrument</skos:prefLabel>
    <skos:inScheme rdf:resource="http://isdc.gfz-potsdam.de/ontology/SPASE-allowed_values.skos.owl#Instrument_Type"/>
    <rdf:type rdf:resource="http://www.w3.org/2002/07/owl#NamedIndividual"/>
  </rdf:Description>
  <rdf:Description rdf:about="http://isdc.gfz-potsdam.de/ontology/SPASE-allowed_values.skos.owl#Antenna">
    <skos:topConceptOf rdf:resource="http://isdc.gfz-potsdam.de/ontology/SPASE-allowed_values.skos.owl#Instrument_Type"/>
    <skos:inScheme rdf:resource="http://isdc.gfz-potsdam.de/ontology/SPASE-allowed_values.skos.owl#Instrument_Type"/>
    <rdf:type rdf:resource="http://www.w3.org/2002/07/owl#NamedIndividual"/>
    <rdf:type rdf:resource="http://www.w3.org/2004/02/skos/core#Concept"/>
    <skos:prefLabel xml:lang="en">Antenna</skos:prefLabel>
    <skos:definition xml:lang="en">A sensor used to measure electric potential.</skos:definition>
  </rdf:Description>
  <rdf:Description rdf:about="http://isdc.gfz-potsdam.de/ontology/SPASE-allowed_values.skos.owl#Core">
    <skos:definition xml:lang="en">The central or main part of an object or calculated distribution. For example, the part of a
distribution of particles at low energies that is a thermal (Maxwellian) population.</skos:definition>
    <skos:topConceptOf rdf:resource="http://isdc.gfz-potsdam.de/ontology/SPASE-allowed_values.skos.owl#Qualifier"/>
    <skos:inScheme rdf:resource="http://isdc.gfz-potsdam.de/ontology/SPASE-allowed_values.skos.owl#Qualifier"/>
    <rdf:type rdf:resource="http://www.w3.org/2002/07/owl#NamedIndividual"/>
    <rdf:type rdf:resource="http://www.w3.org/2004/02/skos/core#Concept"/>
    <skos:prefLabel xml:lang="en">Core</skos:prefLabel>
  </rdf:Description>
  <rdf:Description rdf:about="http://isdc.gfz-potsdam.de/ontology/SPASE-allowed_values.skos.owl#HDF">
    <skos:topConceptOf rdf:resource="http://isdc.gfz-potsdam.de/ontology/SPASE-allowed_values.skos.owl#Format"/>
    <skos:definition xml:lang="en">Hierarchical Data Format</skos:definition>
    <skos:inScheme rdf:resource="http://isdc.gfz-potsdam.de/ontology/SPASE-allowed_values.skos.owl#Format"/>
    <rdf:type rdf:resource="http://www.w3.org/2002/07/owl#NamedIndividual"/>
    <skos:prefLabel xml:lang="en">HDF</skos:prefLabel>
    <rdf:type rdf:resource="http://www.w3.org/2004/02/skos/core#Concept"/>
  </rdf:Description>
  <rdf:Description rdf:about="http://isdc.gfz-potsdam.de/ontology/SPASE-allowed_values.skos.owl#Arrival_Direction">
    <rdf:type rdf:resource="http://www.w3.org/2002/07/owl#NamedIndividual"/>
    <skos:definition xml:lang="en">An angular measure of the direction from which an energetic particle or photon was incident on
a detector. The angles may be measured in any coordinate system.</skos:definition>
    <skos:inScheme rdf:resource="http://isdc.gfz-potsdam.de/ontology/SPASE-allowed_values.skos.owl#Particle_Quantity"/>
    <skos:prefLabel xml:lang="en">Arrival Direction</skos:prefLabel>
    <skos:topConceptOf rdf:resource="http://isdc.gfz-potsdam.de/ontology/SPASE-allowed_values.skos.owl#Particle_Quantity"/>
    <rdf:type rdf:resource="http://www.w3.org/2004/02/skos/core#Concept"/>
  </rdf:Description>
  <rdf:Description rdf:about="http://isdc.gfz-potsdam.de/ontology/SPASE-allowed_values.skos.owl#Horizontal">
    <skos:definition xml:lang="en">Parallel to or in the plane of the horizon or a base line.</skos:definition>
    <skos:inScheme rdf:resource="http://isdc.gfz-potsdam.de/ontology/SPASE-allowed_values.skos.owl#Rendering_Axis"/>
    <skos:prefLabel xml:lang="en">Horizontal</skos:prefLabel>
    <skos:topConceptOf rdf:resource="http://isdc.gfz-potsdam.de/ontology/SPASE-allowed_values.skos.owl#Rendering_Axis"/>
    <rdf:type rdf:resource="http://www.w3.org/2002/07/owl#NamedIndividual"/>
    <rdf:type rdf:resource="http://www.w3.org/2004/02/skos/core#Concept"/>
  </rdf:Description>
  <rdf:Description rdf:about="http://isdc.gfz-potsdam.de/ontology/SPASE-allowed_values.skos.owl#Number_Flux">
    <skos:inScheme rdf:resource="http://isdc.gfz-potsdam.de/ontology/SPASE-allowed_values.skos.owl#Particle_Quantity"/>
    <rdf:type rdf:resource="http://www.w3.org/2002/07/owl#NamedIndividual"/>
    <rdf:type rdf:resource="http://www.w3.org/2004/02/skos/core#Concept"/>
    <skos:definition xml:lang="en">The number of particles passing a unit area in unit time, possibly also per unit energy (or
equivalent) and/or per unit look direction.</skos:definition>
    <skos:topConceptOf rdf:resource="http://isdc.gfz-potsdam.de/ontology/SPASE-allowed_values.skos.owl#Particle_Quantity"/>
    <skos:prefLabel xml:lang="en">Number Flux</skos:prefLabel>
  </rdf:Description>
  <rdf:Description rdf:about="http://isdc.gfz-potsdam.de/ontology/SPASE-allowed_values.skos.owl#Contributor">
    <skos:prefLabel xml:lang="en">Contributor</skos:prefLabel>
    <rdf:type rdf:resource="http://www.w3.org/2004/02/skos/core#Concept"/>
    <rdf:type rdf:resource="http://www.w3.org/2002/07/owl#NamedIndividual"/>
    <skos:definition xml:lang="en">An entity responsible for making contributions to the content of the resource.</skos:definition>
    <skos:inScheme rdf:resource="http://isdc.gfz-potsdam.de/ontology/SPASE-allowed_values.skos.owl#Role"/>
    <skos:topConceptOf rdf:resource="http://isdc.gfz-potsdam.de/ontology/SPASE-allowed_values.skos.owl#Role"/>
  </rdf:Description>
  <rdf:Description rdf:about="http://isdc.gfz-potsdam.de/ontology/SPASE-allowed_values.skos.owl#Auroral_Region">
    <rdf:type rdf:resource="http://www.w3.org/2004/02/skos/core#Concept"/>
    <skos:definition xml:lang="en">The region in the atmospheric where electrically-charged particles bombarding the upper
atmosphere of a planet in the presence of a magnetic field produce an optical phenomenon.</skos:definition>
    <skos:prefLabel xml:lang="en">Auroral Region</skos:prefLabel>
    <skos:broader rdf:resource="http://isdc.gfz-potsdam.de/ontology/SPASE-allowed_values.skos.owl#Near_Surface"/>
    <rdf:type rdf:resource="http://www.w3.org/2002/07/owl#NamedIndividual"/>
    <skos:inScheme rdf:resource="http://isdc.gfz-potsdam.de/ontology/SPASE-allowed_values.skos.owl#Observatory_Region"/>
    <skos:inScheme rdf:resource="http://isdc.gfz-potsdam.de/ontology/SPASE-allowed_values.skos.owl#Observed_Region"/>
  </rdf:Description>
  <rdf:Description rdf:about="http://isdc.gfz-potsdam.de/ontology/SPASE-allowed_values.skos.owl#S3_BUCKET">
    <skos:prefLabel xml:lang="en">S3_BUCKET</skos:prefLabel>
    <skos:definition xml:lang="en">A container of objects that comply with the Amazon Simple Storage Service (S3)
specifications. A bucket has a unique, user-assigned key (name). A bucket can contain any
number of objects with an aggregate size of 5 gigabytes. A bucket may be accompanied by up
to 2 kilobytes of metadata.</skos:definition>
    <rdf:type rdf:resource="http://www.w3.org/2002/07/owl#NamedIndividual"/>
    <rdf:type rdf:resource="http://www.w3.org/2004/02/skos/core#Concept"/>
    <skos:topConceptOf rdf:resource="http://isdc.gfz-potsdam.de/ontology/SPASE-allowed_values.skos.owl#Encoding"/>
    <skos:inScheme rdf:resource="http://isdc.gfz-potsdam.de/ontology/SPASE-allowed_values.skos.owl#Encoding"/>
  </rdf:Description>
  <rdf:Description rdf:about="http://isdc.gfz-potsdam.de/ontology/SPASE-allowed_values.skos.owl#GSE">
    <skos:inScheme rdf:resource="http://isdc.gfz-potsdam.de/ontology/SPASE-allowed_values.skos.owl#Coordinate_System_Name"/>
    <skos:topConceptOf rdf:resource="http://isdc.gfz-potsdam.de/ontology/SPASE-allowed_values.skos.owl#Coordinate_System_Name"/>
    <skos:definition xml:lang="en">Geocentric Solar Ecliptic - A coordinate system where the X axis is from Earth to Sun. Z axis is
normal to the ecliptic, positive northward. See Russell, 1971.</skos:definition>
    <skos:prefLabel xml:lang="en">GSE</skos:prefLabel>
    <rdf:type rdf:resource="http://www.w3.org/2002/07/owl#NamedIndividual"/>
    <rdf:type rdf:resource="http://www.w3.org/2004/02/skos/core#Concept"/>
  </rdf:Description>
  <rdf:Description rdf:about="http://isdc.gfz-potsdam.de/ontology/SPASE-allowed_values.skos.owl#Mixed_Quantity">
    <rdf:type rdf:resource="http://www.w3.org/2002/07/owl#NamedIndividual"/>
    <rdf:type rdf:resource="http://www.w3.org/2004/02/skos/core#ConceptScheme"/>
    <skos:hasTopConcept rdf:resource="http://isdc.gfz-potsdam.de/ontology/SPASE-allowed_values.skos.owl#Alfven_Velocity"/>
    <skos:definition xml:lang="en">A characterization of the combined attributes of a quantity.
Allowed Values:
Akasofu Epsilon
Alfven Mach Number
Alfven Velocity
Frequency-To-Gyrofrequency Ratio
Magnetosonic Mach Number
Other
Plasma Beta
Total Pressure
V Cross B</skos:definition>
    <skos:hasTopConcept rdf:resource="http://isdc.gfz-potsdam.de/ontology/SPASE-allowed_values.skos.owl#Akasofu_Epsilon"/>
    <skos:hasTopConcept rdf:resource="http://isdc.gfz-potsdam.de/ontology/SPASE-allowed_values.skos.owl#Total_Pressure"/>
    <skos:hasTopConcept rdf:resource="http://isdc.gfz-potsdam.de/ontology/SPASE-allowed_values.skos.owl#Alfven_Mach_Number"/>
    <skos:hasTopConcept rdf:resource="http://isdc.gfz-potsdam.de/ontology/SPASE-allowed_values.skos.owl#Frequency-To-Gyrofrequency_Ratio"/>
    <skos:hasTopConcept rdf:resource="http://isdc.gfz-potsdam.de/ontology/SPASE-allowed_values.skos.owl#V_Cross_B"/>
    <skos:prefLabel xml:lang="en">Mixed Quantity</skos:prefLabel>
    <skos:hasTopConcept rdf:resource="http://isdc.gfz-potsdam.de/ontology/SPASE-allowed_values.skos.owl#Magnetosonic_Mach_Number"/>
    <skos:hasTopConcept rdf:resource="http://isdc.gfz-potsdam.de/ontology/SPASE-allowed_values.skos.owl#Plasma_Beta"/>
    <skos:hasTopConcept rdf:resource="http://isdc.gfz-potsdam.de/ontology/SPASE-allowed_values.skos.owl#SQ_Other"/>
  </rdf:Description>
  <rdf:Description rdf:about="http://isdc.gfz-potsdam.de/ontology/SPASE-allowed_values.skos.owl#Flux_Feedback">
    <skos:inScheme rdf:resource="http://isdc.gfz-potsdam.de/ontology/SPASE-allowed_values.skos.owl#Instrument_Type"/>
    <rdf:type rdf:resource="http://www.w3.org/2004/02/skos/core#Concept"/>
    <rdf:type rdf:resource="http://www.w3.org/2002/07/owl#NamedIndividual"/>
    <skos:definition xml:lang="en">A search coil whose bandwidth and signal/noise ratio are increased by the application of
negative feedback at the sensor (flux) level by driving a collocated coil with a signal from the
preamplifier.</skos:definition>
    <skos:topConceptOf rdf:resource="http://isdc.gfz-potsdam.de/ontology/SPASE-allowed_values.skos.owl#Instrument_Type"/>
    <skos:prefLabel xml:lang="en">Flux Feedback</skos:prefLabel>
  </rdf:Description>
  <rdf:Description rdf:about="http://isdc.gfz-potsdam.de/ontology/SPASE-allowed_values.skos.owl#ASCII">
    <rdf:type rdf:resource="http://www.w3.org/2002/07/owl#NamedIndividual"/>
    <skos:prefLabel xml:lang="en">ASCII</skos:prefLabel>
    <skos:inScheme rdf:resource="http://isdc.gfz-potsdam.de/ontology/SPASE-allowed_values.skos.owl#Format"/>
    <skos:definition xml:lang="en">A sequence of characters that adheres to American Standard Code for Information Interchange
(ASCII) which is an 7-bit character-coding scheme.</skos:definition>
    <skos:inScheme rdf:resource="http://isdc.gfz-potsdam.de/ontology/SPASE-allowed_values.skos.owl#Encoding"/>
    <skos:broader rdf:resource="http://isdc.gfz-potsdam.de/ontology/SPASE-allowed_values.skos.owl#Text"/>
    <rdf:type rdf:resource="http://www.w3.org/2004/02/skos/core#Concept"/>
  </rdf:Description>
  <rdf:Description rdf:about="http://isdc.gfz-potsdam.de/ontology/SPASE-allowed_values.skos.owl#Frequency-To-Gyrofrequency_Ratio">
    <rdf:type rdf:resource="http://www.w3.org/2004/02/skos/core#Concept"/>
    <rdf:type rdf:resource="http://www.w3.org/2002/07/owl#NamedIndividual"/>
    <skos:prefLabel xml:lang="en">Frequency-To-Gyrofrequency Ratio</skos:prefLabel>
    <skos:inScheme rdf:resource="http://isdc.gfz-potsdam.de/ontology/SPASE-allowed_values.skos.owl#Mixed_Quantity"/>
    <skos:topConceptOf rdf:resource="http://isdc.gfz-potsdam.de/ontology/SPASE-allowed_values.skos.owl#Mixed_Quantity"/>
    <skos:definition xml:lang="en">The ratio of the characteristic frequency of a medium to gyrofrequency of a particle.</skos:definition>
  </rdf:Description>
  <rdf:Description rdf:about="http://isdc.gfz-potsdam.de/ontology/SPASE-allowed_values.skos.owl#Uncertainty">
    <skos:topConceptOf rdf:resource="http://isdc.gfz-potsdam.de/ontology/SPASE-allowed_values.skos.owl#Qualifier"/>
    <skos:definition xml:lang="en">A statistically defined discrepancy between a measured quantity and the true value of that
quantity that cannot be corrected by calculation or calibration.</skos:definition>
    <skos:prefLabel xml:lang="en">Uncertainty</skos:prefLabel>
    <rdf:type rdf:resource="http://www.w3.org/2002/07/owl#NamedIndividual"/>
    <rdf:type rdf:resource="http://www.w3.org/2004/02/skos/core#Concept"/>
    <skos:inScheme rdf:resource="http://isdc.gfz-potsdam.de/ontology/SPASE-allowed_values.skos.owl#Qualifier"/>
  </rdf:Description>
  <rdf:Description rdf:about="http://isdc.gfz-potsdam.de/ontology/SPASE-allowed_values.skos.owl#Pseudo">
    <skos:prefLabel xml:lang="en">Pseudo</skos:prefLabel>
    <skos:inScheme rdf:resource="http://isdc.gfz-potsdam.de/ontology/SPASE-allowed_values.skos.owl#Qualifier"/>
    <skos:topConceptOf rdf:resource="http://isdc.gfz-potsdam.de/ontology/SPASE-allowed_values.skos.owl#Qualifier"/>
    <rdf:type rdf:resource="http://www.w3.org/2004/02/skos/core#Concept"/>
    <skos:definition xml:lang="en">Similar to or having the appearance of something else. Can be used to indicate an estimation or
approximation of a particular quantity.</skos:definition>
    <rdf:type rdf:resource="http://www.w3.org/2002/07/owl#NamedIndividual"/>
  </rdf:Description>
  <rdf:Description rdf:about="http://isdc.gfz-potsdam.de/ontology/SPASE-allowed_values.skos.owl#Group">
    <skos:definition xml:lang="en">An assemblage of values that a certain relation or common characteristic.</skos:definition>
    <skos:topConceptOf rdf:resource="http://isdc.gfz-potsdam.de/ontology/SPASE-allowed_values.skos.owl#Qualifier"/>
    <skos:prefLabel xml:lang="en">Group</skos:prefLabel>
    <skos:inScheme rdf:resource="http://isdc.gfz-potsdam.de/ontology/SPASE-allowed_values.skos.owl#Qualifier"/>
    <rdf:type rdf:resource="http://www.w3.org/2002/07/owl#NamedIndividual"/>
    <rdf:type rdf:resource="http://www.w3.org/2004/02/skos/core#Concept"/>
  </rdf:Description>
  <rdf:Description rdf:about="http://isdc.gfz-potsdam.de/ontology/SPASE-allowed_values.skos.owl#Chromosphere">
    <skos:inScheme rdf:resource="http://isdc.gfz-potsdam.de/ontology/SPASE-allowed_values.skos.owl#Observatory_Region"/>
    <skos:broader rdf:resource="http://isdc.gfz-potsdam.de/ontology/SPASE-allowed_values.skos.owl#Sun"/>
    <skos:inScheme rdf:resource="http://isdc.gfz-potsdam.de/ontology/SPASE-allowed_values.skos.owl#Observed_Region"/>
    <rdf:type rdf:resource="http://www.w3.org/2004/02/skos/core#Concept"/>
    <rdf:type rdf:resource="http://www.w3.org/2002/07/owl#NamedIndividual"/>
    <skos:prefLabel xml:lang="en">Chromosphere</skos:prefLabel>
    <skos:definition xml:lang="en">The region of the Sun's (or a star's) atmosphere above the temperature minimum and below the
Transition Region. The solar chromosphere is approximately 400 km to 2100 km above the
photosphere, and characterized by temperatures from 4500 - 28000 K.</skos:definition>
  </rdf:Description>
  <rdf:Description rdf:about="http://isdc.gfz-potsdam.de/ontology/SPASE-allowed_values.skos.owl#Particle_Radius">
    <skos:topConceptOf rdf:resource="http://isdc.gfz-potsdam.de/ontology/SPASE-allowed_values.skos.owl#Particle_Quantity"/>
    <skos:prefLabel xml:lang="en">Particle Radius</skos:prefLabel>
    <rdf:type rdf:resource="http://www.w3.org/2002/07/owl#NamedIndividual"/>
    <skos:inScheme rdf:resource="http://isdc.gfz-potsdam.de/ontology/SPASE-allowed_values.skos.owl#Particle_Quantity"/>
    <skos:definition xml:lang="en">The mean radius for a Gaussian distribution of particles with an axial ratio of 2 and a
distribution width that varies as 0.5 radius. A value of zero means no cloud was detected.</skos:definition>
    <rdf:type rdf:resource="http://www.w3.org/2004/02/skos/core#Concept"/>
  </rdf:Description>
  <rdf:Description rdf:about="http://isdc.gfz-potsdam.de/ontology/SPASE-allowed_values.skos.owl#Metadata_Contact">
    <skos:prefLabel xml:lang="en">Metadata Contact</skos:prefLabel>
    <rdf:type rdf:resource="http://www.w3.org/2002/07/owl#NamedIndividual"/>
    <rdf:type rdf:resource="http://www.w3.org/2004/02/skos/core#Concept"/>
    <skos:topConceptOf rdf:resource="http://isdc.gfz-potsdam.de/ontology/SPASE-allowed_values.skos.owl#Role"/>
    <skos:inScheme rdf:resource="http://isdc.gfz-potsdam.de/ontology/SPASE-allowed_values.skos.owl#Role"/>
    <skos:definition xml:lang="en">An individual who can affect a change in the metadata describing a resource.</skos:definition>
  </rdf:Description>
  <rdf:Description rdf:about="http://isdc.gfz-potsdam.de/ontology/SPASE-allowed_values.skos.owl#Geiger-Mueller_Tube">
    <skos:definition xml:lang="en">An instrument which measures density of ionizing radiation based on interactions with a gas.</skos:definition>
    <skos:inScheme rdf:resource="http://isdc.gfz-potsdam.de/ontology/SPASE-allowed_values.skos.owl#Instrument_Type"/>
    <rdf:type rdf:resource="http://www.w3.org/2004/02/skos/core#Concept"/>
    <rdf:type rdf:resource="http://www.w3.org/2002/07/owl#NamedIndividual"/>
    <skos:topConceptOf rdf:resource="http://isdc.gfz-potsdam.de/ontology/SPASE-allowed_values.skos.owl#Instrument_Type"/>
    <skos:prefLabel xml:lang="en">Geiger-Mueller Tube</skos:prefLabel>
  </rdf:Description>
  <rdf:Description rdf:about="http://isdc.gfz-potsdam.de/ontology/SPASE-allowed_values.skos.owl#Scalar">
    <skos:inScheme rdf:resource="http://isdc.gfz-potsdam.de/ontology/SPASE-allowed_values.skos.owl#Qualifier"/>
    <skos:definition xml:lang="en">A quantity that is completely specified by its magnitude and has no direction.</skos:definition>
    <skos:topConceptOf rdf:resource="http://isdc.gfz-potsdam.de/ontology/SPASE-allowed_values.skos.owl#Qualifier"/>
    <rdf:type rdf:resource="http://www.w3.org/2002/07/owl#NamedIndividual"/>
    <rdf:type rdf:resource="http://www.w3.org/2004/02/skos/core#Concept"/>
    <skos:prefLabel xml:lang="en">Scalar</skos:prefLabel>
  </rdf:Description>
  <rdf:Description rdf:about="http://isdc.gfz-potsdam.de/ontology/SPASE-allowed_values.skos.owl">
    <owl:imports rdf:resource="http://www.w3.org/2004/02/skos/core"/>
    <rdf:type rdf:resource="http://www.w3.org/2002/07/owl#Ontology"/>
  </rdf:Description>
  <rdf:Description rdf:about="http://isdc.gfz-potsdam.de/ontology/SPASE-allowed_values.skos.owl#AVI">
    <skos:topConceptOf rdf:resource="http://isdc.gfz-potsdam.de/ontology/SPASE-allowed_values.skos.owl#Format"/>
    <skos:prefLabel xml:lang="en">AVI</skos:prefLabel>
    <rdf:type rdf:resource="http://www.w3.org/2002/07/owl#NamedIndividual"/>
    <skos:definition xml:lang="en">Audio Video Interleave (AVI) a digital format for movies that conforms to the Microsoft
Windows Resource Interchange File Format (RIFF).</skos:definition>
    <rdf:type rdf:resource="http://www.w3.org/2004/02/skos/core#Concept"/>
    <skos:inScheme rdf:resource="http://isdc.gfz-potsdam.de/ontology/SPASE-allowed_values.skos.owl#Format"/>
  </rdf:Description>
  <rdf:Description rdf:about="http://isdc.gfz-potsdam.de/ontology/SPASE-allowed_values.skos.owl#Thermal_Plasma">
    <skos:prefLabel xml:lang="en">Thermal Plasma</skos:prefLabel>
    <rdf:type rdf:resource="http://www.w3.org/2004/02/skos/core#Concept"/>
    <rdf:type rdf:resource="http://www.w3.org/2002/07/owl#NamedIndividual"/>
    <skos:topConceptOf rdf:resource="http://isdc.gfz-potsdam.de/ontology/SPASE-allowed_values.skos.owl#Measurement_Type"/>
    <skos:inScheme rdf:resource="http://isdc.gfz-potsdam.de/ontology/SPASE-allowed_values.skos.owl#Measurement_Type"/>
    <skos:definition xml:lang="en">Measurements of the plasma in the energy regime where the most of the plasma occurs. May be
the basic fluxes in the form of distribution functions or the derived bulk parameters (density,
flow velocity, etc.).</skos:definition>
  </rdf:Description>
  <rdf:Description rdf:about="http://isdc.gfz-potsdam.de/ontology/SPASE-allowed_values.skos.owl#BZIP2">
    <skos:inScheme rdf:resource="http://isdc.gfz-potsdam.de/ontology/SPASE-allowed_values.skos.owl#Encoding"/>
    <skos:prefLabel xml:lang="en">BZIP2</skos:prefLabel>
    <skos:topConceptOf rdf:resource="http://isdc.gfz-potsdam.de/ontology/SPASE-allowed_values.skos.owl#Encoding"/>
    <rdf:type rdf:resource="http://www.w3.org/2004/02/skos/core#Concept"/>
    <rdf:type rdf:resource="http://www.w3.org/2002/07/owl#NamedIndividual"/>
    <skos:definition xml:lang="en">An open standard algorithm by Julian Seward using Burrows-Wheeler block sorting and
Huffman coding. See &lt;http://www.bzip.org/&gt;</skos:definition>
  </rdf:Description>
  <rdf:Description rdf:about="http://isdc.gfz-potsdam.de/ontology/SPASE-allowed_values.skos.owl#Open">
    <rdf:type rdf:resource="http://www.w3.org/2002/07/owl#NamedIndividual"/>
    <skos:inScheme rdf:resource="http://isdc.gfz-potsdam.de/ontology/SPASE-allowed_values.skos.owl#Access_Rights"/>
    <skos:prefLabel xml:lang="en">Open</skos:prefLabel>
    <skos:topConceptOf rdf:resource="http://isdc.gfz-potsdam.de/ontology/SPASE-allowed_values.skos.owl#Access_Rights"/>
    <skos:definition xml:lang="en">Access is granted to everyone.</skos:definition>
    <rdf:type rdf:resource="http://www.w3.org/2004/02/skos/core#Concept"/>
  </rdf:Description>
  <rdf:Description rdf:about="http://isdc.gfz-potsdam.de/ontology/SPASE-allowed_values.skos.owl#Fit">
    <rdf:type rdf:resource="http://www.w3.org/2004/02/skos/core#Concept"/>
    <skos:prefLabel xml:lang="en">Fit</skos:prefLabel>
    <rdf:type rdf:resource="http://www.w3.org/2002/07/owl#NamedIndividual"/>
    <skos:inScheme rdf:resource="http://isdc.gfz-potsdam.de/ontology/SPASE-allowed_values.skos.owl#Qualifier"/>
    <skos:definition xml:lang="en">Values that make an model agree with the data.</skos:definition>
    <skos:topConceptOf rdf:resource="http://isdc.gfz-potsdam.de/ontology/SPASE-allowed_values.skos.owl#Qualifier"/>
  </rdf:Description>
  <rdf:Description rdf:about="http://isdc.gfz-potsdam.de/ontology/SPASE-allowed_values.skos.owl#Dust_Detector">
    <skos:prefLabel xml:lang="en">Dust Detector</skos:prefLabel>
    <skos:topConceptOf rdf:resource="http://isdc.gfz-potsdam.de/ontology/SPASE-allowed_values.skos.owl#Instrument_Type"/>
    <rdf:type rdf:resource="http://www.w3.org/2004/02/skos/core#Concept"/>
    <rdf:type rdf:resource="http://www.w3.org/2002/07/owl#NamedIndividual"/>
    <skos:definition xml:lang="en">An instrument which determines the mass and speed of ambient dust particles.</skos:definition>
    <skos:inScheme rdf:resource="http://isdc.gfz-potsdam.de/ontology/SPASE-allowed_values.skos.owl#Instrument_Type"/>
  </rdf:Description>
  <rdf:Description rdf:about="http://isdc.gfz-potsdam.de/ontology/SPASE-allowed_values.skos.owl#Measurement_Type">
    <skos:hasTopConcept rdf:resource="http://isdc.gfz-potsdam.de/ontology/SPASE-allowed_values.skos.owl#Dust"/>
    <skos:hasTopConcept rdf:resource="http://isdc.gfz-potsdam.de/ontology/SPASE-allowed_values.skos.owl#Ion_Composition"/>
    <rdf:type rdf:resource="http://www.w3.org/2004/02/skos/core#ConceptScheme"/>
    <skos:hasTopConcept rdf:resource="http://isdc.gfz-potsdam.de/ontology/SPASE-allowed_values.skos.owl#Magnetogram"/>
    <skos:hasTopConcept rdf:resource="http://isdc.gfz-potsdam.de/ontology/SPASE-allowed_values.skos.owl#Instrument_Status"/>
    <skos:hasTopConcept rdf:resource="http://isdc.gfz-potsdam.de/ontology/SPASE-allowed_values.skos.owl#Image_Intensity"/>
    <skos:hasTopConcept rdf:resource="http://isdc.gfz-potsdam.de/ontology/SPASE-allowed_values.skos.owl#Neutral_Atom_Images"/>
    <skos:hasTopConcept rdf:resource="http://isdc.gfz-potsdam.de/ontology/SPASE-allowed_values.skos.owl#Waves"/>
    <skos:hasTopConcept rdf:resource="http://isdc.gfz-potsdam.de/ontology/SPASE-allowed_values.skos.owl#Magnetic_Field"/>
    <skos:hasTopConcept rdf:resource="http://isdc.gfz-potsdam.de/ontology/SPASE-allowed_values.skos.owl#Irradiance"/>
    <skos:hasTopConcept rdf:resource="http://isdc.gfz-potsdam.de/ontology/SPASE-allowed_values.skos.owl#Ephemeris"/>
    <skos:hasTopConcept rdf:resource="http://isdc.gfz-potsdam.de/ontology/SPASE-allowed_values.skos.owl#Activity_Index"/>
    <rdf:type rdf:resource="http://www.w3.org/2002/07/owl#NamedIndividual"/>
    <skos:hasTopConcept rdf:resource="http://isdc.gfz-potsdam.de/ontology/SPASE-allowed_values.skos.owl#Electric_Field"/>
    <skos:hasTopConcept rdf:resource="http://isdc.gfz-potsdam.de/ontology/SPASE-allowed_values.skos.owl#Spectrum"/>
    <skos:hasTopConcept rdf:resource="http://isdc.gfz-potsdam.de/ontology/SPASE-allowed_values.skos.owl#Thermal_Plasma"/>
    <skos:hasTopConcept rdf:resource="http://isdc.gfz-potsdam.de/ontology/SPASE-allowed_values.skos.owl#Neutral_Gas"/>
    <skos:hasTopConcept rdf:resource="http://isdc.gfz-potsdam.de/ontology/SPASE-allowed_values.skos.owl#Profile"/>
    <skos:prefLabel xml:lang="en">Measurement Type</skos:prefLabel>
    <skos:hasTopConcept rdf:resource="http://isdc.gfz-potsdam.de/ontology/SPASE-allowed_values.skos.owl#Radiance"/>
    <skos:hasTopConcept rdf:resource="http://isdc.gfz-potsdam.de/ontology/SPASE-allowed_values.skos.owl#Energetic_Particles"/>
    <skos:definition xml:lang="en">A characterization of the quantitative assessment of a phenomenon.
Allowed Values:
Activity Index
Dopplergram
Dust
Electric Field
Energetic Particles
Ephemeris
Image Intensity
Instrument Status
Ion Composition
Irradiance
Magnetic Field
Magnetogram
Neutral Atom Images
Neutral Gas
Profile
Radiance
Spectrum
Thermal Plasma
Waves
Waves.Active
Waves.Passive</skos:definition>
    <skos:hasTopConcept rdf:resource="http://isdc.gfz-potsdam.de/ontology/SPASE-allowed_values.skos.owl#Dopplergram"/>
  </rdf:Description>
  <rdf:Description rdf:about="http://isdc.gfz-potsdam.de/ontology/SPASE-allowed_values.skos.owl#Ca-K">
    <skos:inScheme rdf:resource="http://isdc.gfz-potsdam.de/ontology/SPASE-allowed_values.skos.owl#Spectral_Range"/>
    <skos:definition xml:lang="en">A spectrum with a wavelength of range centered near 393.5 nm. VSO nickname: Ca-K image
with range of 391.9 nm to 395.2 nm.</skos:definition>
    <rdf:type rdf:resource="http://www.w3.org/2004/02/skos/core#Concept"/>
    <rdf:type rdf:resource="http://www.w3.org/2002/07/owl#NamedIndividual"/>
    <skos:prefLabel xml:lang="en">Ca-K</skos:prefLabel>
    <skos:topConceptOf rdf:resource="http://isdc.gfz-potsdam.de/ontology/SPASE-allowed_values.skos.owl#Spectral_Range"/>
  </rdf:Description>
  <rdf:Description rdf:about="http://isdc.gfz-potsdam.de/ontology/SPASE-allowed_values.skos.owl#Pressure">
    <skos:inScheme rdf:resource="http://isdc.gfz-potsdam.de/ontology/SPASE-allowed_values.skos.owl#Particle_Quantity"/>
    <rdf:type rdf:resource="http://www.w3.org/2002/07/owl#NamedIndividual"/>
    <rdf:type rdf:resource="http://www.w3.org/2004/02/skos/core#Concept"/>
    <skos:definition xml:lang="en">The force per unit area exerted by a particle distribution or field.</skos:definition>
    <skos:prefLabel xml:lang="en">Pressure</skos:prefLabel>
    <skos:topConceptOf rdf:resource="http://isdc.gfz-potsdam.de/ontology/SPASE-allowed_values.skos.owl#Particle_Quantity"/>
  </rdf:Description>
  <rdf:Description rdf:about="http://isdc.gfz-potsdam.de/ontology/SPASE-allowed_values.skos.owl#Cartesian">
    <skos:topConceptOf rdf:resource="http://isdc.gfz-potsdam.de/ontology/SPASE-allowed_values.skos.owl#Coordinate_Representation"/>
    <skos:inScheme rdf:resource="http://isdc.gfz-potsdam.de/ontology/SPASE-allowed_values.skos.owl#Coordinate_Representation"/>
    <skos:prefLabel xml:lang="en">Cartesian</skos:prefLabel>
    <rdf:type rdf:resource="http://www.w3.org/2004/02/skos/core#Concept"/>
    <rdf:type rdf:resource="http://www.w3.org/2002/07/owl#NamedIndividual"/>
    <skos:definition xml:lang="en">A representation in which a position vector or a measured vector (e.g., field or flow) is
specified by its components along the base axes of the coordinate system.</skos:definition>
  </rdf:Description>
  <rdf:Description rdf:about="http://isdc.gfz-potsdam.de/ontology/SPASE-allowed_values.skos.owl#HPR">
    <skos:inScheme rdf:resource="http://isdc.gfz-potsdam.de/ontology/SPASE-allowed_values.skos.owl#Coordinate_System_Name"/>
    <skos:prefLabel xml:lang="en">HPR</skos:prefLabel>
    <skos:topConceptOf rdf:resource="http://isdc.gfz-potsdam.de/ontology/SPASE-allowed_values.skos.owl#Coordinate_System_Name"/>
    <rdf:type rdf:resource="http://www.w3.org/2002/07/owl#NamedIndividual"/>
    <rdf:type rdf:resource="http://www.w3.org/2004/02/skos/core#Concept"/>
    <skos:definition xml:lang="en">Helioprojective Radial - A 3-D orthonormal (left-handed) coordinate system that is primarily
intended to specify with two dimensions a point on the solar disk. The Z axis points from the
observer to the center of the solar disk. The Y axis lies in the plane defined by the solar spin
vector and the Z axis, positive northward. The X axis is perpendicular to the Y and Z axes,
positive toward solar west. Given as the distance between the observer and the center of the
solar disk, the standard representation for this system of an (x,y) point on the solar disk is via
the point's latitude angle theta {= arctan [SQRT(x**2 + y**2)]/d]} or equivalent declination
parameter delta (= theta - 90 deg), and its phase angle psi as measured counter- clockwise from
the +Y axis [psi = arctan (-y/x)].</skos:definition>
  </rdf:Description>
  <rdf:Description rdf:about="http://isdc.gfz-potsdam.de/ontology/SPASE-allowed_values.skos.owl#Neutral_Atom_Images">
    <skos:definition xml:lang="en">Measurements of neutral atom fluxes as a function of look direction; often related to remote
energetic charged particles that lose their charge through charge-exchange and then reach the
detector on a line-of-sight trajectory.</skos:definition>
    <rdf:type rdf:resource="http://www.w3.org/2002/07/owl#NamedIndividual"/>
    <skos:inScheme rdf:resource="http://isdc.gfz-potsdam.de/ontology/SPASE-allowed_values.skos.owl#Measurement_Type"/>
    <skos:topConceptOf rdf:resource="http://isdc.gfz-potsdam.de/ontology/SPASE-allowed_values.skos.owl#Measurement_Type"/>
    <rdf:type rdf:resource="http://www.w3.org/2004/02/skos/core#Concept"/>
    <skos:prefLabel xml:lang="en">Neutral Atom Images</skos:prefLabel>
  </rdf:Description>
  <rdf:Description rdf:about="http://isdc.gfz-potsdam.de/ontology/SPASE-allowed_values.skos.owl#Particle_Type">
    <skos:hasTopConcept rdf:resource="http://isdc.gfz-potsdam.de/ontology/SPASE-allowed_values.skos.owl#Dust"/>
    <skos:definition xml:lang="en">A characterization of the kind of particle observed by the measurement.
Allowed Values:
Aerosol
Alpha Particle
Atom
Dust
Electron
Ion
Molecule
Neutron
Proton</skos:definition>
    <skos:hasTopConcept rdf:resource="http://isdc.gfz-potsdam.de/ontology/SPASE-allowed_values.skos.owl#Electron"/>
    <skos:hasTopConcept rdf:resource="http://isdc.gfz-potsdam.de/ontology/SPASE-allowed_values.skos.owl#Aerosol"/>
    <skos:hasTopConcept rdf:resource="http://isdc.gfz-potsdam.de/ontology/SPASE-allowed_values.skos.owl#Atom"/>
    <skos:prefLabel xml:lang="en">Particle Type</skos:prefLabel>
    <skos:hasTopConcept rdf:resource="http://isdc.gfz-potsdam.de/ontology/SPASE-allowed_values.skos.owl#Proton"/>
    <rdf:type rdf:resource="http://www.w3.org/2002/07/owl#NamedIndividual"/>
    <skos:hasTopConcept rdf:resource="http://isdc.gfz-potsdam.de/ontology/SPASE-allowed_values.skos.owl#Alpha_Particle"/>
    <rdf:type rdf:resource="http://www.w3.org/2004/02/skos/core#ConceptScheme"/>
    <skos:hasTopConcept rdf:resource="http://isdc.gfz-potsdam.de/ontology/SPASE-allowed_values.skos.owl#Molecule"/>
    <skos:hasTopConcept rdf:resource="http://isdc.gfz-potsdam.de/ontology/SPASE-allowed_values.skos.owl#Ion"/>
    <skos:hasTopConcept rdf:resource="http://isdc.gfz-potsdam.de/ontology/SPASE-allowed_values.skos.owl#Neutron"/>
  </rdf:Description>
  <rdf:Description rdf:about="http://isdc.gfz-potsdam.de/ontology/SPASE-allowed_values.skos.owl#Fourier_Transform_Spectrograph">
    <skos:inScheme rdf:resource="http://isdc.gfz-potsdam.de/ontology/SPASE-allowed_values.skos.owl#Instrument_Type"/>
    <skos:definition xml:lang="en">An instrument that determines the spectra of a radiative source, using time-domain
measurements and a Fourier transform.</skos:definition>
    <rdf:type rdf:resource="http://www.w3.org/2002/07/owl#NamedIndividual"/>
    <rdf:type rdf:resource="http://www.w3.org/2004/02/skos/core#Concept"/>
    <skos:prefLabel xml:lang="en">Fourier Transform Spectrograph</skos:prefLabel>
    <skos:topConceptOf rdf:resource="http://isdc.gfz-potsdam.de/ontology/SPASE-allowed_values.skos.owl#Instrument_Type"/>
  </rdf:Description>
  <rdf:Description rdf:about="http://isdc.gfz-potsdam.de/ontology/SPASE-allowed_values.skos.owl#Line_Of_Sight">
    <skos:prefLabel xml:lang="en">Line Of Sight</skos:prefLabel>
    <rdf:type rdf:resource="http://www.w3.org/2004/02/skos/core#Concept"/>
    <skos:inScheme rdf:resource="http://isdc.gfz-potsdam.de/ontology/SPASE-allowed_values.skos.owl#Qualifier"/>
    <skos:definition xml:lang="en">The line of sight is the line that connects the observer with the observed object. This expression
is often used with measurements of Doppler velocity and magnetic field in magnetograms,
where only the component of the vector field directed along the line of sight is measured.</skos:definition>
    <rdf:type rdf:resource="http://www.w3.org/2002/07/owl#NamedIndividual"/>
    <skos:topConceptOf rdf:resource="http://isdc.gfz-potsdam.de/ontology/SPASE-allowed_values.skos.owl#Qualifier"/>
  </rdf:Description>
  <rdf:Description rdf:about="http://isdc.gfz-potsdam.de/ontology/SPASE-allowed_values.skos.owl#ZIP">
    <skos:inScheme rdf:resource="http://isdc.gfz-potsdam.de/ontology/SPASE-allowed_values.skos.owl#Encoding"/>
    <skos:topConceptOf rdf:resource="http://isdc.gfz-potsdam.de/ontology/SPASE-allowed_values.skos.owl#Encoding"/>
    <rdf:type rdf:resource="http://www.w3.org/2002/07/owl#NamedIndividual"/>
    <rdf:type rdf:resource="http://www.w3.org/2004/02/skos/core#Concept"/>
    <skos:definition xml:lang="en">An open standard for compression which is a variation of the LZW method and was originally
used in the PKZIP utility.</skos:definition>
    <skos:prefLabel xml:lang="en">ZIP</skos:prefLabel>
  </rdf:Description>
  <rdf:Description rdf:about="http://isdc.gfz-potsdam.de/ontology/SPASE-allowed_values.skos.owl#Tensor">
    <skos:inScheme rdf:resource="http://isdc.gfz-potsdam.de/ontology/SPASE-allowed_values.skos.owl#Qualifier"/>
    <rdf:type rdf:resource="http://www.w3.org/2002/07/owl#NamedIndividual"/>
    <skos:prefLabel xml:lang="en">Tensor</skos:prefLabel>
    <skos:definition xml:lang="en">A generalized linear "quantity" or "geometrical entity" that can be expressed as a
multi-dimensional array relative to a choice of basis of the particular space on which it is
defined.</skos:definition>
    <rdf:type rdf:resource="http://www.w3.org/2004/02/skos/core#Concept"/>
    <skos:topConceptOf rdf:resource="http://isdc.gfz-potsdam.de/ontology/SPASE-allowed_values.skos.owl#Qualifier"/>
  </rdf:Description>
  <rdf:Description rdf:about="http://isdc.gfz-potsdam.de/ontology/SPASE-allowed_values.skos.owl#Sounder">
    <skos:definition xml:lang="en">An instrument which measures the radiances from an object. A sounder may measure radiances
at multiple spectral ranges.</skos:definition>
    <rdf:type rdf:resource="http://www.w3.org/2004/02/skos/core#Concept"/>
    <skos:inScheme rdf:resource="http://isdc.gfz-potsdam.de/ontology/SPASE-allowed_values.skos.owl#Instrument_Type"/>
    <rdf:type rdf:resource="http://www.w3.org/2002/07/owl#NamedIndividual"/>
    <skos:topConceptOf rdf:resource="http://isdc.gfz-potsdam.de/ontology/SPASE-allowed_values.skos.owl#Instrument_Type"/>
  </rdf:Description>
  <rdf:Description rdf:about="http://isdc.gfz-potsdam.de/ontology/SPASE-allowed_values.skos.owl#MATLAB_6">
    <skos:prefLabel xml:lang="en">MATLAB_6</skos:prefLabel>
    <skos:definition xml:lang="en">MATLAB Workspace save set, version 6. MAT-files are double-precision, binary, MATLAB
format files. MATLAB is a proprietary product of The MathWorks.</skos:definition>
    <skos:inScheme rdf:resource="http://isdc.gfz-potsdam.de/ontology/SPASE-allowed_values.skos.owl#Format"/>
    <rdf:type rdf:resource="http://www.w3.org/2002/07/owl#NamedIndividual"/>
    <rdf:type rdf:resource="http://www.w3.org/2004/02/skos/core#Concept"/>
    <skos:topConceptOf rdf:resource="http://isdc.gfz-potsdam.de/ontology/SPASE-allowed_values.skos.owl#Format"/>
  </rdf:Description>
  <rdf:Description rdf:about="http://isdc.gfz-potsdam.de/ontology/SPASE-allowed_values.skos.owl#Hash_Function">
    <rdf:type rdf:resource="http://www.w3.org/2004/02/skos/core#ConceptScheme"/>
    <rdf:type rdf:resource="http://www.w3.org/2002/07/owl#NamedIndividual"/>
    <skos:prefLabel xml:lang="en">Hash Function</skos:prefLabel>
    <skos:hasTopConcept rdf:resource="http://isdc.gfz-potsdam.de/ontology/SPASE-allowed_values.skos.owl#MD5"/>
    <skos:definition xml:lang="en">A function or algorithm that converts a digital data object into a hash value. Typically the hash
value is small and concise when compared to the digital data object.
Allowed Values:
MD5
SHA1
SHA256</skos:definition>
    <skos:hasTopConcept rdf:resource="http://isdc.gfz-potsdam.de/ontology/SPASE-allowed_values.skos.owl#SHA1"/>
    <skos:hasTopConcept rdf:resource="http://isdc.gfz-potsdam.de/ontology/SPASE-allowed_values.skos.owl#SHA256"/>
  </rdf:Description>
  <rdf:Description rdf:about="http://isdc.gfz-potsdam.de/ontology/SPASE-allowed_values.skos.owl#IJ">
    <skos:prefLabel xml:lang="en">IJ</skos:prefLabel>
    <skos:inScheme rdf:resource="http://isdc.gfz-potsdam.de/ontology/SPASE-allowed_values.skos.owl#Qualifier"/>
    <skos:broader rdf:resource="http://isdc.gfz-potsdam.de/ontology/SPASE-allowed_values.skos.owl#Projection"/>
    <rdf:type rdf:resource="http://www.w3.org/2002/07/owl#NamedIndividual"/>
    <rdf:type rdf:resource="http://www.w3.org/2004/02/skos/core#Concept"/>
    <skos:definition xml:lang="en">A measure of the length of a position or measured vector projected into the i-j (typically X-Y)
plane of the coordinate system.</skos:definition>
  </rdf:Description>
  <rdf:Description rdf:about="http://isdc.gfz-potsdam.de/ontology/SPASE-allowed_values.skos.owl#I">
    <skos:broader rdf:resource="http://isdc.gfz-potsdam.de/ontology/SPASE-allowed_values.skos.owl#Component"/>
    <skos:prefLabel xml:lang="en">I</skos:prefLabel>
    <rdf:type rdf:resource="http://www.w3.org/2004/02/skos/core#Concept"/>
    <rdf:type rdf:resource="http://www.w3.org/2002/07/owl#NamedIndividual"/>
    <skos:definition xml:lang="en">Projection of a vector along the first named axis of a coordinate system. Typically the X axis,
but could be the R axis for an RTN coordinate system.</skos:definition>
    <skos:inScheme rdf:resource="http://isdc.gfz-potsdam.de/ontology/SPASE-allowed_values.skos.owl#Qualifier"/>
  </rdf:Description>
  <rdf:Description rdf:about="http://isdc.gfz-potsdam.de/ontology/SPASE-allowed_values.skos.owl#Thermal_Speed">
    <rdf:type rdf:resource="http://www.w3.org/2002/07/owl#NamedIndividual"/>
    <skos:prefLabel xml:lang="en">Thermal Speed</skos:prefLabel>
    <skos:inScheme rdf:resource="http://isdc.gfz-potsdam.de/ontology/SPASE-allowed_values.skos.owl#Particle_Quantity"/>
    <skos:definition xml:lang="en">For a Maxwellian distribution, the difference between the mean speed and the speed within
which ~69% (one sigma) of all the members of the speed distribution occur.</skos:definition>
    <skos:topConceptOf rdf:resource="http://isdc.gfz-potsdam.de/ontology/SPASE-allowed_values.skos.owl#Particle_Quantity"/>
    <rdf:type rdf:resource="http://www.w3.org/2004/02/skos/core#Concept"/>
  </rdf:Description>
  <rdf:Description rdf:about="http://isdc.gfz-potsdam.de/ontology/SPASE-allowed_values.skos.owl#Sound_Speed">
    <skos:topConceptOf rdf:resource="http://isdc.gfz-potsdam.de/ontology/SPASE-allowed_values.skos.owl#Particle_Quantity"/>
    <skos:definition xml:lang="en">The speed at which sound travels through a medium.</skos:definition>
    <skos:inScheme rdf:resource="http://isdc.gfz-potsdam.de/ontology/SPASE-allowed_values.skos.owl#Particle_Quantity"/>
    <rdf:type rdf:resource="http://www.w3.org/2002/07/owl#NamedIndividual"/>
    <rdf:type rdf:resource="http://www.w3.org/2004/02/skos/core#Concept"/>
    <skos:prefLabel xml:lang="en">Sound Speed</skos:prefLabel>
  </rdf:Description>
  <rdf:Description rdf:about="http://isdc.gfz-potsdam.de/ontology/SPASE-allowed_values.skos.owl#Waves">
    <rdf:type rdf:resource="http://www.w3.org/2002/07/owl#NamedIndividual"/>
    <skos:definition xml:lang="en">Data resulting from observations of wave experiments and natural wave phenomena. Wave
experiments are typically active and natural wave phenomena are passive. Examples of wave
experiments include coherent/incoherent scatter radars, radio soundings, VLF propagation
studies, ionospheric scintillation of beacon satellite signals, etc. Examples of natural wave
phenomena include micropulsations, mesospheric gravity waves, auroral/plasmaspheric hiss,
Langmuir waves, AKR, Jovian decametric radiation, solar radio bursts, etc.
Allowed Values:
Active
Passive</skos:definition>
    <skos:prefLabel xml:lang="en">Waves</skos:prefLabel>
    <rdf:type rdf:resource="http://www.w3.org/2004/02/skos/core#Concept"/>
    <skos:topConceptOf rdf:resource="http://isdc.gfz-potsdam.de/ontology/SPASE-allowed_values.skos.owl#Measurement_Type"/>
    <skos:inScheme rdf:resource="http://isdc.gfz-potsdam.de/ontology/SPASE-allowed_values.skos.owl#Measurement_Type"/>
    <skos:narrower rdf:resource="http://isdc.gfz-potsdam.de/ontology/SPASE-allowed_values.skos.owl#Passive"/>
    <skos:narrower rdf:resource="http://isdc.gfz-potsdam.de/ontology/SPASE-allowed_values.skos.owl#Active"/>
  </rdf:Description>
  <rdf:Description rdf:about="http://isdc.gfz-potsdam.de/ontology/SPASE-allowed_values.skos.owl#CEF">
    <skos:inScheme rdf:resource="http://isdc.gfz-potsdam.de/ontology/SPASE-allowed_values.skos.owl#Format"/>
    <rdf:type rdf:resource="http://www.w3.org/2004/02/skos/core#Concept"/>
    <rdf:type rdf:resource="http://www.w3.org/2002/07/owl#NamedIndividual"/>
    <skos:prefLabel xml:lang="en">CEF</skos:prefLabel>
    <skos:topConceptOf rdf:resource="http://isdc.gfz-potsdam.de/ontology/SPASE-allowed_values.skos.owl#Format"/>
    <skos:definition xml:lang="en">Cluster Exchange Format (CEF) is a self-documenting ASCII format designed for the exchange
of data. There are two versions of CEF which are not totally compatible.</skos:definition>
  </rdf:Description>
  <rdf:Description rdf:about="http://isdc.gfz-potsdam.de/ontology/SPASE-allowed_values.skos.owl#Project_Scientist">
    <skos:prefLabel xml:lang="en">Project Scientist</skos:prefLabel>
    <rdf:type rdf:resource="http://www.w3.org/2002/07/owl#NamedIndividual"/>
    <rdf:type rdf:resource="http://www.w3.org/2004/02/skos/core#Concept"/>
    <skos:topConceptOf rdf:resource="http://isdc.gfz-potsdam.de/ontology/SPASE-allowed_values.skos.owl#Role"/>
    <skos:inScheme rdf:resource="http://isdc.gfz-potsdam.de/ontology/SPASE-allowed_values.skos.owl#Role"/>
    <skos:definition xml:lang="en">An individual who is an expert in the phenomenon and related physics explored by the project.
A project scientist may also have a managerial role within the project.</skos:definition>
  </rdf:Description>
  <rdf:Description rdf:about="http://isdc.gfz-potsdam.de/ontology/SPASE-allowed_values.skos.owl#TAR">
    <skos:inScheme rdf:resource="http://isdc.gfz-potsdam.de/ontology/SPASE-allowed_values.skos.owl#Encoding"/>
    <skos:topConceptOf rdf:resource="http://isdc.gfz-potsdam.de/ontology/SPASE-allowed_values.skos.owl#Encoding"/>
    <skos:prefLabel xml:lang="en">TAR</skos:prefLabel>
    <rdf:type rdf:resource="http://www.w3.org/2004/02/skos/core#Concept"/>
    <rdf:type rdf:resource="http://www.w3.org/2002/07/owl#NamedIndividual"/>
    <skos:definition xml:lang="en">A file format used to collate collections of files into one larger file, for distribution or archiving,
while preserving file system information such as user and group permissions, dates, and
directory structures. The format was standardized by POSIX.1-1988 and later POSIX.1-2001.</skos:definition>
  </rdf:Description>
  <rdf:Description rdf:about="http://isdc.gfz-potsdam.de/ontology/SPASE-allowed_values.skos.owl#Electromagnetic">
    <skos:inScheme rdf:resource="http://isdc.gfz-potsdam.de/ontology/SPASE-allowed_values.skos.owl#Field_Quantity"/>
    <skos:inScheme rdf:resource="http://isdc.gfz-potsdam.de/ontology/SPASE-allowed_values.skos.owl#Wave_Type"/>
    <skos:prefLabel xml:lang="en">Electromagnetic</skos:prefLabel>
    <rdf:type rdf:resource="http://www.w3.org/2002/07/owl#NamedIndividual"/>
    <rdf:type rdf:resource="http://www.w3.org/2004/02/skos/core#Concept"/>
    <skos:definition xml:lang="en">Electric and magnetic field variations in time and space that propagate through a medium or a
vacuum with the wave's propagation, electric field, and magnetic field vectors forming an
orthogonal triad. Waves in this category are detected by having their field quantities measured.</skos:definition>
    <skos:topConceptOf rdf:resource="http://isdc.gfz-potsdam.de/ontology/SPASE-allowed_values.skos.owl#Wave_Type"/>
    <skos:topConceptOf rdf:resource="http://isdc.gfz-potsdam.de/ontology/SPASE-allowed_values.skos.owl#Field_Quantity"/>
  </rdf:Description>
  <rdf:Description rdf:about="http://isdc.gfz-potsdam.de/ontology/SPASE-allowed_values.skos.owl#Probable">
    <rdf:type rdf:resource="http://www.w3.org/2002/07/owl#NamedIndividual"/>
    <skos:prefLabel xml:lang="en">Probable</skos:prefLabel>
    <skos:definition xml:lang="en">Likely given the available evidence. Considered in the range of 4-7 on a scale of 0-10.</skos:definition>
    <skos:topConceptOf rdf:resource="http://isdc.gfz-potsdam.de/ontology/SPASE-allowed_values.skos.owl#Confidence_Rating"/>
    <skos:inScheme rdf:resource="http://isdc.gfz-potsdam.de/ontology/SPASE-allowed_values.skos.owl#Confidence_Rating"/>
    <rdf:type rdf:resource="http://www.w3.org/2004/02/skos/core#Concept"/>
  </rdf:Description>
  <rdf:Description rdf:about="http://isdc.gfz-potsdam.de/ontology/SPASE-allowed_values.skos.owl#Base64">
    <skos:inScheme rdf:resource="http://isdc.gfz-potsdam.de/ontology/SPASE-allowed_values.skos.owl#Encoding"/>
    <skos:topConceptOf rdf:resource="http://isdc.gfz-potsdam.de/ontology/SPASE-allowed_values.skos.owl#Encoding"/>
    <skos:definition xml:lang="en">A data encoding scheme whereby binary-encoded data is converted to printable ASCII
characters. It is defined as a MIME content transfer encoding for use in Internet e-mail. The
only characters used are the upper- and lower-case Roman alphabet characters (A-Z, a-z), the
numerals (0-9), and the "+" and "/" symbols, with the "=" symbol as a special suffix (padding)
code.</skos:definition>
    <rdf:type rdf:resource="http://www.w3.org/2002/07/owl#NamedIndividual"/>
    <rdf:type rdf:resource="http://www.w3.org/2004/02/skos/core#Concept"/>
    <skos:prefLabel xml:lang="en">Base64</skos:prefLabel>
  </rdf:Description>
  <rdf:Description rdf:about="http://isdc.gfz-potsdam.de/ontology/SPASE-allowed_values.skos.owl#Association_Type">
    <skos:hasTopConcept rdf:resource="http://isdc.gfz-potsdam.de/ontology/SPASE-allowed_values.skos.owl#Revision_Of"/>
    <rdf:type rdf:resource="http://www.w3.org/2004/02/skos/core#ConceptScheme"/>
    <skos:hasTopConcept rdf:resource="http://isdc.gfz-potsdam.de/ontology/SPASE-allowed_values.skos.owl#Derived_From"/>
    <skos:hasTopConcept rdf:resource="http://isdc.gfz-potsdam.de/ontology/SPASE-allowed_values.skos.owl#Child_Event_Of"/>
    <skos:hasTopConcept rdf:resource="http://isdc.gfz-potsdam.de/ontology/SPASE-allowed_values.skos.owl#Part_Of"/>
    <skos:hasTopConcept rdf:resource="http://isdc.gfz-potsdam.de/ontology/SPASE-allowed_values.skos.owl#Observed_By"/>
    <rdf:type rdf:resource="http://www.w3.org/2002/07/owl#NamedIndividual"/>
    <skos:definition xml:lang="en">A characterization of the role or purpose of an associated resource.
Allowed Values:
Child Event Of
Derived From
Observed By
Other
Part Of
Revision Of</skos:definition>
    <skos:prefLabel xml:lang="en">Association Type</skos:prefLabel>
    <skos:hasTopConcept rdf:resource="http://isdc.gfz-potsdam.de/ontology/SPASE-allowed_values.skos.owl#SQ_Other"/>
  </rdf:Description>
  <rdf:Description rdf:about="http://isdc.gfz-potsdam.de/ontology/SPASE-allowed_values.skos.owl#Perpendicular">
    <rdf:type rdf:resource="http://www.w3.org/2002/07/owl#NamedIndividual"/>
    <rdf:type rdf:resource="http://www.w3.org/2004/02/skos/core#Concept"/>
    <skos:prefLabel xml:lang="en">Perpendicular</skos:prefLabel>
    <skos:topConceptOf rdf:resource="http://isdc.gfz-potsdam.de/ontology/SPASE-allowed_values.skos.owl#Qualifier"/>
    <skos:definition xml:lang="en">At right angles to a given direction.</skos:definition>
    <skos:inScheme rdf:resource="http://isdc.gfz-potsdam.de/ontology/SPASE-allowed_values.skos.owl#Qualifier"/>
  </rdf:Description>
  <rdf:Description rdf:about="http://isdc.gfz-potsdam.de/ontology/SPASE-allowed_values.skos.owl#Phenomenon_Type">
    <skos:hasTopConcept rdf:resource="http://isdc.gfz-potsdam.de/ontology/SPASE-allowed_values.skos.owl#Geomagnetic_Storm"/>
    <rdf:type rdf:resource="http://www.w3.org/2004/02/skos/core#ConceptScheme"/>
    <skos:hasTopConcept rdf:resource="http://isdc.gfz-potsdam.de/ontology/SPASE-allowed_values.skos.owl#Magnetopause_Crossing"/>
    <skos:hasTopConcept rdf:resource="http://isdc.gfz-potsdam.de/ontology/SPASE-allowed_values.skos.owl#Aurora"/>
    <skos:hasTopConcept rdf:resource="http://isdc.gfz-potsdam.de/ontology/SPASE-allowed_values.skos.owl#Magnetic_Cloud"/>
    <skos:hasTopConcept rdf:resource="http://isdc.gfz-potsdam.de/ontology/SPASE-allowed_values.skos.owl#Coronal_Hole"/>
    <skos:hasTopConcept rdf:resource="http://isdc.gfz-potsdam.de/ontology/SPASE-allowed_values.skos.owl#Bow_Shock_Crossing"/>
    <skos:definition xml:lang="en">The characteristics or categorization of an event type.
Allowed Values:
Active Region
Aurora
Bow Shock Crossing
Coronal Hole
Coronal Mass Ejection
EIT Wave
Energetic Solar Particle Event
Forbush Decrease
Geomagnetic Storm
Interplanetary Shock
Magnetic Cloud
Magnetopause Crossing
Radio Burst
Sector Boundary Crossing
Solar Flare
Solar Wind Extreme
Stream Interaction Region
Substorm</skos:definition>
    <skos:hasTopConcept rdf:resource="http://isdc.gfz-potsdam.de/ontology/SPASE-allowed_values.skos.owl#EIT_Wave"/>
    <skos:hasTopConcept rdf:resource="http://isdc.gfz-potsdam.de/ontology/SPASE-allowed_values.skos.owl#Forbush_Decrease"/>
    <skos:prefLabel xml:lang="en">Phenomenon Type</skos:prefLabel>
    <skos:hasTopConcept rdf:resource="http://isdc.gfz-potsdam.de/ontology/SPASE-allowed_values.skos.owl#Active_Region"/>
    <skos:hasTopConcept rdf:resource="http://isdc.gfz-potsdam.de/ontology/SPASE-allowed_values.skos.owl#Substorm"/>
    <rdf:type rdf:resource="http://www.w3.org/2002/07/owl#NamedIndividual"/>
    <skos:hasTopConcept rdf:resource="http://isdc.gfz-potsdam.de/ontology/SPASE-allowed_values.skos.owl#Solar_Wind_Extreme"/>
    <skos:hasTopConcept rdf:resource="http://isdc.gfz-potsdam.de/ontology/SPASE-allowed_values.skos.owl#Sector_Boundary_Crossing"/>
    <skos:hasTopConcept rdf:resource="http://isdc.gfz-potsdam.de/ontology/SPASE-allowed_values.skos.owl#Coronal_Mass_Ejection"/>
    <skos:hasTopConcept rdf:resource="http://isdc.gfz-potsdam.de/ontology/SPASE-allowed_values.skos.owl#Radio_Burst"/>
    <skos:hasTopConcept rdf:resource="http://isdc.gfz-potsdam.de/ontology/SPASE-allowed_values.skos.owl#Stream_Interaction_Region"/>
    <skos:hasTopConcept rdf:resource="http://isdc.gfz-potsdam.de/ontology/SPASE-allowed_values.skos.owl#Solar_Flare"/>
    <skos:hasTopConcept rdf:resource="http://isdc.gfz-potsdam.de/ontology/SPASE-allowed_values.skos.owl#Interplanetary_Shock"/>
    <skos:hasTopConcept rdf:resource="http://isdc.gfz-potsdam.de/ontology/SPASE-allowed_values.skos.owl#Energetic_Solar_Particle_Event"/>
  </rdf:Description>
  <rdf:Description rdf:about="http://isdc.gfz-potsdam.de/ontology/SPASE-allowed_values.skos.owl#Stoke's_Parameters">
    <skos:inScheme rdf:resource="http://isdc.gfz-potsdam.de/ontology/SPASE-allowed_values.skos.owl#Qualifier"/>
    <skos:topConceptOf rdf:resource="http://isdc.gfz-potsdam.de/ontology/SPASE-allowed_values.skos.owl#Qualifier"/>
    <skos:definition xml:lang="en">A set of four parameters (usually called I,Q, U and V) which describe the polarization state of
an electromagnetic wave propagating through space.</skos:definition>
    <skos:topConceptOf rdf:resource="http://isdc.gfz-potsdam.de/ontology/SPASE-allowed_values.skos.owl#Wave_Quantity"/>
    <rdf:type rdf:resource="http://www.w3.org/2004/02/skos/core#Concept"/>
    <rdf:type rdf:resource="http://www.w3.org/2002/07/owl#NamedIndividual"/>
    <skos:prefLabel xml:lang="en">Stoke's Parameters</skos:prefLabel>
    <skos:inScheme rdf:resource="http://isdc.gfz-potsdam.de/ontology/SPASE-allowed_values.skos.owl#Wave_Quantity"/>
  </rdf:Description>
  <rdf:Description rdf:about="http://isdc.gfz-potsdam.de/ontology/SPASE-allowed_values.skos.owl#Riometer">
    <rdf:type rdf:resource="http://www.w3.org/2002/07/owl#NamedIndividual"/>
    <skos:inScheme rdf:resource="http://isdc.gfz-potsdam.de/ontology/SPASE-allowed_values.skos.owl#Instrument_Type"/>
    <skos:definition xml:lang="en">An instrument which measure the signal strength in various directions of the galactic radio
signals. Variations in these signals are influenced by solar flare activity and geomagnetic storm
and substorm processes.</skos:definition>
    <skos:prefLabel xml:lang="en">Riometer</skos:prefLabel>
    <skos:topConceptOf rdf:resource="http://isdc.gfz-potsdam.de/ontology/SPASE-allowed_values.skos.owl#Instrument_Type"/>
    <rdf:type rdf:resource="http://www.w3.org/2004/02/skos/core#Concept"/>
  </rdf:Description>
  <rdf:Description rdf:about="http://isdc.gfz-potsdam.de/ontology/SPASE-allowed_values.skos.owl#Differential">
    <skos:definition xml:lang="en">A measurement within a narrow range of energy and/or solid angle.</skos:definition>
    <skos:prefLabel xml:lang="en">Differential</skos:prefLabel>
    <skos:inScheme rdf:resource="http://isdc.gfz-potsdam.de/ontology/SPASE-allowed_values.skos.owl#Qualifier"/>
    <rdf:type rdf:resource="http://www.w3.org/2002/07/owl#NamedIndividual"/>
    <rdf:type rdf:resource="http://www.w3.org/2004/02/skos/core#Concept"/>
    <skos:topConceptOf rdf:resource="http://isdc.gfz-potsdam.de/ontology/SPASE-allowed_values.skos.owl#Qualifier"/>
  </rdf:Description>
  <rdf:Description rdf:about="http://isdc.gfz-potsdam.de/ontology/SPASE-allowed_values.skos.owl#Forbush_Decrease">
    <rdf:type rdf:resource="http://www.w3.org/2004/02/skos/core#Concept"/>
    <skos:inScheme rdf:resource="http://isdc.gfz-potsdam.de/ontology/SPASE-allowed_values.skos.owl#Phenomenon_Type"/>
    <skos:topConceptOf rdf:resource="http://isdc.gfz-potsdam.de/ontology/SPASE-allowed_values.skos.owl#Phenomenon_Type"/>
    <skos:prefLabel xml:lang="en">Forbush Decrease</skos:prefLabel>
    <skos:definition xml:lang="en">A rapid decrease in the observed galactic cosmic ray intensity following the passage of an
outwardly convecting interplanetary magnetic field disturbance, such as those associated with
large CME's, that sweep some galactic cosmic rays away from Earth.</skos:definition>
    <rdf:type rdf:resource="http://www.w3.org/2002/07/owl#NamedIndividual"/>
  </rdf:Description>
  <rdf:Description rdf:about="http://isdc.gfz-potsdam.de/ontology/SPASE-allowed_values.skos.owl#Long_Wire">
    <skos:topConceptOf rdf:resource="http://isdc.gfz-potsdam.de/ontology/SPASE-allowed_values.skos.owl#Instrument_Type"/>
    <skos:definition xml:lang="en">A dipole antenna whose active (sensor) elements are two wires deployed in the equatorial plane
on opposite sides of a spinning spacecraft, and whose length is several times greater than the
spacecraft diameter.</skos:definition>
    <rdf:type rdf:resource="http://www.w3.org/2004/02/skos/core#Concept"/>
    <rdf:type rdf:resource="http://www.w3.org/2002/07/owl#NamedIndividual"/>
    <skos:prefLabel xml:lang="en">Long Wire</skos:prefLabel>
    <skos:inScheme rdf:resource="http://isdc.gfz-potsdam.de/ontology/SPASE-allowed_values.skos.owl#Instrument_Type"/>
  </rdf:Description>
  <rdf:Description rdf:about="http://isdc.gfz-potsdam.de/ontology/SPASE-allowed_values.skos.owl#Hard_X-rays">
    <rdf:type rdf:resource="http://www.w3.org/2002/07/owl#NamedIndividual"/>
    <rdf:type rdf:resource="http://www.w3.org/2004/02/skos/core#Concept"/>
    <skos:inScheme rdf:resource="http://isdc.gfz-potsdam.de/ontology/SPASE-allowed_values.skos.owl#Spectral_Range"/>
    <skos:definition xml:lang="en">Photons with a wavelength range: 0.001 to 0.1 nm and an energy range of 12 keV to 120 keV.</skos:definition>
    <skos:topConceptOf rdf:resource="http://isdc.gfz-potsdam.de/ontology/SPASE-allowed_values.skos.owl#Spectral_Range"/>
    <skos:prefLabel xml:lang="en">Hard X-rays</skos:prefLabel>
  </rdf:Description>
  <rdf:Description rdf:about="http://isdc.gfz-potsdam.de/ontology/SPASE-allowed_values.skos.owl#General_Contact">
    <skos:topConceptOf rdf:resource="http://isdc.gfz-potsdam.de/ontology/SPASE-allowed_values.skos.owl#Role"/>
    <skos:prefLabel xml:lang="en">General Contact</skos:prefLabel>
    <skos:inScheme rdf:resource="http://isdc.gfz-potsdam.de/ontology/SPASE-allowed_values.skos.owl#Role"/>
    <skos:definition xml:lang="en">An individual who can provide information on a range of subjects or who can direct you to a
domain expert.</skos:definition>
    <rdf:type rdf:resource="http://www.w3.org/2004/02/skos/core#Concept"/>
    <rdf:type rdf:resource="http://www.w3.org/2002/07/owl#NamedIndividual"/>
  </rdf:Description>
  <rdf:Description rdf:about="http://isdc.gfz-potsdam.de/ontology/SPASE-allowed_values.skos.owl#Scale_Type">
    <skos:prefLabel xml:lang="en">Scale Type</skos:prefLabel>
    <skos:definition xml:lang="en">The scaling to apply to an axis. If this attribute is not present, linear scale should be assumed.
Allowed Values:
Linear Scale
Log Scale</skos:definition>
    <skos:hasTopConcept rdf:resource="http://isdc.gfz-potsdam.de/ontology/SPASE-allowed_values.skos.owl#Linear_Scale"/>
    <rdf:type rdf:resource="http://www.w3.org/2004/02/skos/core#ConceptScheme"/>
    <rdf:type rdf:resource="http://www.w3.org/2002/07/owl#NamedIndividual"/>
    <skos:hasTopConcept rdf:resource="http://isdc.gfz-potsdam.de/ontology/SPASE-allowed_values.skos.owl#Log_Scale"/>
  </rdf:Description>
  <rdf:Description rdf:about="http://isdc.gfz-potsdam.de/ontology/SPASE-allowed_values.skos.owl#Total">
    <skos:topConceptOf rdf:resource="http://isdc.gfz-potsdam.de/ontology/SPASE-allowed_values.skos.owl#Qualifier"/>
    <skos:inScheme rdf:resource="http://isdc.gfz-potsdam.de/ontology/SPASE-allowed_values.skos.owl#Qualifier"/>
    <skos:definition xml:lang="en">The summation of quantities over all possible species.</skos:definition>
    <skos:prefLabel xml:lang="en">Total</skos:prefLabel>
    <rdf:type rdf:resource="http://www.w3.org/2002/07/owl#NamedIndividual"/>
    <rdf:type rdf:resource="http://www.w3.org/2004/02/skos/core#Concept"/>
  </rdf:Description>
  <rdf:Description rdf:about="http://isdc.gfz-potsdam.de/ontology/SPASE-allowed_values.skos.owl#Ionosphere">
    <skos:narrower rdf:resource="http://isdc.gfz-potsdam.de/ontology/SPASE-allowed_values.skos.owl#D-Region"/>
    <skos:inScheme rdf:resource="http://isdc.gfz-potsdam.de/ontology/SPASE-allowed_values.skos.owl#Observatory_Region"/>
    <rdf:type rdf:resource="http://www.w3.org/2002/07/owl#NamedIndividual"/>
    <skos:definition xml:lang="en">The charged or ionized gases surrounding a body that are nominally bound to the body by
virtue of the gravitational attraction.
Allowed Values:
D-Region
E-Region
F-Region
Topside</skos:definition>
    <skos:broader rdf:resource="http://isdc.gfz-potsdam.de/ontology/SPASE-allowed_values.skos.owl#Near_Surface"/>
    <skos:inScheme rdf:resource="http://isdc.gfz-potsdam.de/ontology/SPASE-allowed_values.skos.owl#Observed_Region"/>
    <skos:prefLabel xml:lang="en">Ionosphere</skos:prefLabel>
    <skos:narrower rdf:resource="http://isdc.gfz-potsdam.de/ontology/SPASE-allowed_values.skos.owl#Topside"/>
    <skos:narrower rdf:resource="http://isdc.gfz-potsdam.de/ontology/SPASE-allowed_values.skos.owl#F-Region"/>
    <rdf:type rdf:resource="http://www.w3.org/2004/02/skos/core#Concept"/>
    <skos:narrower rdf:resource="http://isdc.gfz-potsdam.de/ontology/SPASE-allowed_values.skos.owl#E-Region"/>
  </rdf:Description>
  <rdf:Description rdf:about="http://isdc.gfz-potsdam.de/ontology/SPASE-allowed_values.skos.owl#Co-Investigator">
    <skos:topConceptOf rdf:resource="http://isdc.gfz-potsdam.de/ontology/SPASE-allowed_values.skos.owl#Role"/>
    <skos:inScheme rdf:resource="http://isdc.gfz-potsdam.de/ontology/SPASE-allowed_values.skos.owl#Role"/>
    <skos:prefLabel xml:lang="en">Co-Investigator</skos:prefLabel>
    <skos:definition xml:lang="en">An individual who is a scientific peer and major participant in an investigation.</skos:definition>
    <rdf:type rdf:resource="http://www.w3.org/2004/02/skos/core#Concept"/>
    <rdf:type rdf:resource="http://www.w3.org/2002/07/owl#NamedIndividual"/>
  </rdf:Description>
  <rdf:Description rdf:about="http://isdc.gfz-potsdam.de/ontology/SPASE-allowed_values.skos.owl#Dust">
    <skos:inScheme rdf:resource="http://isdc.gfz-potsdam.de/ontology/SPASE-allowed_values.skos.owl#Measurement_Type"/>
    <skos:topConceptOf rdf:resource="http://isdc.gfz-potsdam.de/ontology/SPASE-allowed_values.skos.owl#Measurement_Type"/>
    <skos:definition xml:lang="en">Free microscopic particles of solid material.</skos:definition>
    <rdf:type rdf:resource="http://www.w3.org/2004/02/skos/core#Concept"/>
    <rdf:type rdf:resource="http://www.w3.org/2002/07/owl#NamedIndividual"/>
    <skos:inScheme rdf:resource="http://isdc.gfz-potsdam.de/ontology/SPASE-allowed_values.skos.owl#Particle_Type"/>
    <skos:prefLabel xml:lang="en">Dust</skos:prefLabel>
    <skos:topConceptOf rdf:resource="http://isdc.gfz-potsdam.de/ontology/SPASE-allowed_values.skos.owl#Particle_Type"/>
  </rdf:Description>
  <rdf:Description rdf:about="http://isdc.gfz-potsdam.de/ontology/SPASE-allowed_values.skos.owl#V_Cross_B">
    <skos:definition xml:lang="en">The cross product of the charge velocity (V) and the magnetic field (B). It is the electric field
exerted on a point charge by a magnetic field.</skos:definition>
    <skos:prefLabel xml:lang="en">V Cross B</skos:prefLabel>
    <skos:inScheme rdf:resource="http://isdc.gfz-potsdam.de/ontology/SPASE-allowed_values.skos.owl#Mixed_Quantity"/>
    <rdf:type rdf:resource="http://www.w3.org/2002/07/owl#NamedIndividual"/>
    <rdf:type rdf:resource="http://www.w3.org/2004/02/skos/core#Concept"/>
    <skos:topConceptOf rdf:resource="http://isdc.gfz-potsdam.de/ontology/SPASE-allowed_values.skos.owl#Mixed_Quantity"/>
  </rdf:Description>
  <rdf:Description rdf:about="http://isdc.gfz-potsdam.de/ontology/SPASE-allowed_values.skos.owl#Child_Event_Of">
    <skos:prefLabel xml:lang="en">Child Event Of</skos:prefLabel>
    <skos:inScheme rdf:resource="http://isdc.gfz-potsdam.de/ontology/SPASE-allowed_values.skos.owl#Association_Type"/>
    <skos:topConceptOf rdf:resource="http://isdc.gfz-potsdam.de/ontology/SPASE-allowed_values.skos.owl#Association_Type"/>
    <skos:definition xml:lang="en">A descendant or caused by another resource.</skos:definition>
    <rdf:type rdf:resource="http://www.w3.org/2004/02/skos/core#Concept"/>
    <rdf:type rdf:resource="http://www.w3.org/2002/07/owl#NamedIndividual"/>
  </rdf:Description>
  <rdf:Description rdf:about="http://isdc.gfz-potsdam.de/ontology/SPASE-allowed_values.skos.owl#Phase-Space_Density">
    <rdf:type rdf:resource="http://www.w3.org/2004/02/skos/core#Concept"/>
    <skos:definition xml:lang="en">The number of particles per unit volume in the six-dimensional space of position and velocity.</skos:definition>
    <skos:inScheme rdf:resource="http://isdc.gfz-potsdam.de/ontology/SPASE-allowed_values.skos.owl#Particle_Quantity"/>
    <skos:prefLabel xml:lang="en">Phase-Space Density</skos:prefLabel>
    <rdf:type rdf:resource="http://www.w3.org/2002/07/owl#NamedIndividual"/>
    <skos:topConceptOf rdf:resource="http://isdc.gfz-potsdam.de/ontology/SPASE-allowed_values.skos.owl#Particle_Quantity"/>
  </rdf:Description>
  <rdf:Description rdf:about="http://isdc.gfz-potsdam.de/ontology/SPASE-allowed_values.skos.owl#Azimuth_Angle">
    <rdf:type rdf:resource="http://www.w3.org/2004/02/skos/core#Concept"/>
    <skos:broader rdf:resource="http://isdc.gfz-potsdam.de/ontology/SPASE-allowed_values.skos.owl#Direction_Angle"/>
    <skos:inScheme rdf:resource="http://isdc.gfz-potsdam.de/ontology/SPASE-allowed_values.skos.owl#Qualifier"/>
    <rdf:type rdf:resource="http://www.w3.org/2002/07/owl#NamedIndividual"/>
    <skos:definition xml:lang="en">The angle between the projection into the i-j plane of a position or measured vector and the
i-axis of the coordinate system. Mathematically defined as arctan(j/i).</skos:definition>
    <skos:prefLabel xml:lang="en">Azimuth Angle</skos:prefLabel>
  </rdf:Description>
  <rdf:Description rdf:about="http://isdc.gfz-potsdam.de/ontology/SPASE-allowed_values.skos.owl#Automatic">
    <skos:prefLabel xml:lang="en">Automatic</skos:prefLabel>
    <skos:topConceptOf rdf:resource="http://isdc.gfz-potsdam.de/ontology/SPASE-allowed_values.skos.owl#Classification_Method"/>
    <skos:definition xml:lang="en">Determined by the analysis or assessment performed by a program or server.</skos:definition>
    <skos:inScheme rdf:resource="http://isdc.gfz-potsdam.de/ontology/SPASE-allowed_values.skos.owl#Classification_Method"/>
    <rdf:type rdf:resource="http://www.w3.org/2004/02/skos/core#Concept"/>
    <rdf:type rdf:resource="http://www.w3.org/2002/07/owl#NamedIndividual"/>
  </rdf:Description>
  <rdf:Description rdf:about="http://isdc.gfz-potsdam.de/ontology/SPASE-allowed_values.skos.owl#HG">
    <rdf:type rdf:resource="http://www.w3.org/2004/02/skos/core#Concept"/>
    <skos:prefLabel xml:lang="en">HG</skos:prefLabel>
    <skos:topConceptOf rdf:resource="http://isdc.gfz-potsdam.de/ontology/SPASE-allowed_values.skos.owl#Coordinate_System_Name"/>
    <skos:definition xml:lang="en">Heliographic - A heliocentric rotating coordinate system where the Z axis is normal to the solar
equatorial plane, positive northward. X, Y axes rotate with a 25.38 day period. The zero
longitude (X axis) is defined as the longitude that passed through the ascending node of the
solar equator on the ecliptic plane on 1 January, 1854 at 12 UT. See
&lt;http://nssdc.gsfc.nasa.gov/space/helios/coor_des.html&gt;.</skos:definition>
    <skos:inScheme rdf:resource="http://isdc.gfz-potsdam.de/ontology/SPASE-allowed_values.skos.owl#Coordinate_System_Name"/>
    <rdf:type rdf:resource="http://www.w3.org/2002/07/owl#NamedIndividual"/>
  </rdf:Description>
  <rdf:Description rdf:about="http://isdc.gfz-potsdam.de/ontology/SPASE-allowed_values.skos.owl#SC">
    <skos:inScheme rdf:resource="http://isdc.gfz-potsdam.de/ontology/SPASE-allowed_values.skos.owl#Coordinate_System_Name"/>
    <skos:prefLabel xml:lang="en">SC</skos:prefLabel>
    <rdf:type rdf:resource="http://www.w3.org/2002/07/owl#NamedIndividual"/>
    <skos:definition xml:lang="en">Spacecraft - A coordinate system defined by the spacecraft geometry and/or spin. Often has Z
axis parallel to spacecraft spin vector. X and Y axes may or may not corotate with the
spacecraft. See SR and SR2 below.</skos:definition>
    <skos:topConceptOf rdf:resource="http://isdc.gfz-potsdam.de/ontology/SPASE-allowed_values.skos.owl#Coordinate_System_Name"/>
    <rdf:type rdf:resource="http://www.w3.org/2004/02/skos/core#Concept"/>
  </rdf:Description>
  <rdf:Description rdf:about="http://isdc.gfz-potsdam.de/ontology/SPASE-allowed_values.skos.owl#GSEQ">
    <rdf:type rdf:resource="http://www.w3.org/2004/02/skos/core#Concept"/>
    <rdf:type rdf:resource="http://www.w3.org/2002/07/owl#NamedIndividual"/>
    <skos:inScheme rdf:resource="http://isdc.gfz-potsdam.de/ontology/SPASE-allowed_values.skos.owl#Coordinate_System_Name"/>
    <skos:definition xml:lang="en">Geocentric Solar Equatorial - A coordinate system where the X axis is from Earth to Sun. Y
axis is parallel to solar equatorial plane. Z axis is positive northward. See Russell, 1971.</skos:definition>
    <skos:topConceptOf rdf:resource="http://isdc.gfz-potsdam.de/ontology/SPASE-allowed_values.skos.owl#Coordinate_System_Name"/>
    <skos:prefLabel xml:lang="en">GSEQ</skos:prefLabel>
  </rdf:Description>
  <rdf:Description rdf:about="http://isdc.gfz-potsdam.de/ontology/SPASE-allowed_values.skos.owl#IDL">
    <skos:prefLabel xml:lang="en">IDL</skos:prefLabel>
    <skos:definition xml:lang="en">Interactive Data Language (IDL) save set. IDL is a proprietary format.</skos:definition>
    <skos:inScheme rdf:resource="http://isdc.gfz-potsdam.de/ontology/SPASE-allowed_values.skos.owl#Format"/>
    <rdf:type rdf:resource="http://www.w3.org/2002/07/owl#NamedIndividual"/>
    <rdf:type rdf:resource="http://www.w3.org/2004/02/skos/core#Concept"/>
    <skos:topConceptOf rdf:resource="http://isdc.gfz-potsdam.de/ontology/SPASE-allowed_values.skos.owl#Format"/>
  </rdf:Description>
  <rdf:Description rdf:about="http://isdc.gfz-potsdam.de/ontology/SPASE-allowed_values.skos.owl#Elevation_Angle">
    <rdf:type rdf:resource="http://www.w3.org/2002/07/owl#NamedIndividual"/>
    <rdf:type rdf:resource="http://www.w3.org/2004/02/skos/core#Concept"/>
    <skos:broader rdf:resource="http://isdc.gfz-potsdam.de/ontology/SPASE-allowed_values.skos.owl#Direction_Angle"/>
    <skos:prefLabel xml:lang="en">Elevation Angle</skos:prefLabel>
    <skos:definition xml:lang="en">The angle between the position or measured vector and the i-j plane of the coordinate system.
Mathematically defined as arctan(k/SQRT(i^2+j^2)).</skos:definition>
    <skos:inScheme rdf:resource="http://isdc.gfz-potsdam.de/ontology/SPASE-allowed_values.skos.owl#Qualifier"/>
  </rdf:Description>
  <rdf:Description rdf:about="http://isdc.gfz-potsdam.de/ontology/SPASE-allowed_values.skos.owl#Doppler_Frequency">
    <skos:inScheme rdf:resource="http://isdc.gfz-potsdam.de/ontology/SPASE-allowed_values.skos.owl#Wave_Quantity"/>
    <skos:prefLabel xml:lang="en">Doppler Frequency</skos:prefLabel>
    <skos:definition xml:lang="en">Change in the frequency of a propagating wave due to motion of the source, the observer, the
reflector, or the propagation medium.</skos:definition>
    <skos:topConceptOf rdf:resource="http://isdc.gfz-potsdam.de/ontology/SPASE-allowed_values.skos.owl#Wave_Quantity"/>
    <rdf:type rdf:resource="http://www.w3.org/2002/07/owl#NamedIndividual"/>
    <rdf:type rdf:resource="http://www.w3.org/2004/02/skos/core#Concept"/>
  </rdf:Description>
  <rdf:Description rdf:about="http://isdc.gfz-potsdam.de/ontology/SPASE-allowed_values.skos.owl#MPEG">
    <skos:inScheme rdf:resource="http://isdc.gfz-potsdam.de/ontology/SPASE-allowed_values.skos.owl#Format"/>
    <skos:prefLabel xml:lang="en">MPEG</skos:prefLabel>
    <skos:definition xml:lang="en">A digital format for movies defined by the Motion Picture Experts Group.</skos:definition>
    <rdf:type rdf:resource="http://www.w3.org/2004/02/skos/core#Concept"/>
    <rdf:type rdf:resource="http://www.w3.org/2002/07/owl#NamedIndividual"/>
    <skos:topConceptOf rdf:resource="http://isdc.gfz-potsdam.de/ontology/SPASE-allowed_values.skos.owl#Format"/>
  </rdf:Description>
  <rdf:Description rdf:about="http://isdc.gfz-potsdam.de/ontology/SPASE-allowed_values.skos.owl#Mass">
    <skos:prefLabel xml:lang="en">Mass</skos:prefLabel>
    <rdf:type rdf:resource="http://www.w3.org/2004/02/skos/core#Concept"/>
    <rdf:type rdf:resource="http://www.w3.org/2002/07/owl#NamedIndividual"/>
    <skos:inScheme rdf:resource="http://isdc.gfz-potsdam.de/ontology/SPASE-allowed_values.skos.owl#Particle_Quantity"/>
    <skos:topConceptOf rdf:resource="http://isdc.gfz-potsdam.de/ontology/SPASE-allowed_values.skos.owl#Particle_Quantity"/>
    <skos:definition xml:lang="en">The measure of inertia (mass) of individual objects (e.g., aerosols).</skos:definition>
  </rdf:Description>
  <rdf:Description rdf:about="http://isdc.gfz-potsdam.de/ontology/SPASE-allowed_values.skos.owl#Text">
    <rdf:type rdf:resource="http://www.w3.org/2002/07/owl#NamedIndividual"/>
    <skos:narrower rdf:resource="http://isdc.gfz-potsdam.de/ontology/SPASE-allowed_values.skos.owl#ASCII"/>
    <skos:prefLabel xml:lang="en">Text</skos:prefLabel>
    <rdf:type rdf:resource="http://www.w3.org/2004/02/skos/core#Concept"/>
    <skos:narrower rdf:resource="http://isdc.gfz-potsdam.de/ontology/SPASE-allowed_values.skos.owl#Unicode"/>
    <skos:inScheme rdf:resource="http://isdc.gfz-potsdam.de/ontology/SPASE-allowed_values.skos.owl#Format"/>
    <skos:topConceptOf rdf:resource="http://isdc.gfz-potsdam.de/ontology/SPASE-allowed_values.skos.owl#Format"/>
    <skos:definition xml:lang="en">A sequence of characters which may have an imposed structure or organization.
Allowed Values:
ASCII
Unicode</skos:definition>
  </rdf:Description>
  <rdf:Description rdf:about="http://isdc.gfz-potsdam.de/ontology/SPASE-allowed_values.skos.owl#Emissivity">
    <skos:topConceptOf rdf:resource="http://isdc.gfz-potsdam.de/ontology/SPASE-allowed_values.skos.owl#Wave_Quantity"/>
    <skos:definition xml:lang="en">The energy emitted spontaneously per unit bandwidth (typically frequency) per unit time per
unit mass of source. Emissivity is usually integrated over all directions/solid angles.</skos:definition>
    <rdf:type rdf:resource="http://www.w3.org/2002/07/owl#NamedIndividual"/>
    <rdf:type rdf:resource="http://www.w3.org/2004/02/skos/core#Concept"/>
    <skos:prefLabel xml:lang="en">Emissivity</skos:prefLabel>
    <skos:inScheme rdf:resource="http://isdc.gfz-potsdam.de/ontology/SPASE-allowed_values.skos.owl#Wave_Quantity"/>
  </rdf:Description>
  <rdf:Description rdf:about="http://isdc.gfz-potsdam.de/ontology/SPASE-allowed_values.skos.owl#Inferred">
    <skos:topConceptOf rdf:resource="http://isdc.gfz-potsdam.de/ontology/SPASE-allowed_values.skos.owl#Classification_Method"/>
    <skos:inScheme rdf:resource="http://isdc.gfz-potsdam.de/ontology/SPASE-allowed_values.skos.owl#Classification_Method"/>
    <skos:prefLabel xml:lang="en">Inferred</skos:prefLabel>
    <skos:definition xml:lang="en">Determined by the analysis of other information or resources.</skos:definition>
    <rdf:type rdf:resource="http://www.w3.org/2004/02/skos/core#Concept"/>
    <rdf:type rdf:resource="http://www.w3.org/2002/07/owl#NamedIndividual"/>
  </rdf:Description>
  <rdf:Description rdf:about="http://isdc.gfz-potsdam.de/ontology/SPASE-allowed_values.skos.owl#Interplanetary_Shock">
    <skos:prefLabel xml:lang="en">Interplanetary Shock</skos:prefLabel>
    <skos:topConceptOf rdf:resource="http://isdc.gfz-potsdam.de/ontology/SPASE-allowed_values.skos.owl#Phenomenon_Type"/>
    <skos:definition xml:lang="en">A shock propagating generally anti-sunward through the slower solar wind, often seen in front
of CME-associated plasma clouds.</skos:definition>
    <rdf:type rdf:resource="http://www.w3.org/2002/07/owl#NamedIndividual"/>
    <rdf:type rdf:resource="http://www.w3.org/2004/02/skos/core#Concept"/>
    <skos:inScheme rdf:resource="http://isdc.gfz-potsdam.de/ontology/SPASE-allowed_values.skos.owl#Phenomenon_Type"/>
  </rdf:Description>
  <rdf:Description rdf:about="http://isdc.gfz-potsdam.de/ontology/SPASE-allowed_values.skos.owl#Asteroid">
    <skos:prefLabel xml:lang="en">Asteroid</skos:prefLabel>
    <skos:inScheme rdf:resource="http://isdc.gfz-potsdam.de/ontology/SPASE-allowed_values.skos.owl#Observed_Region"/>
    <rdf:type rdf:resource="http://www.w3.org/2004/02/skos/core#Concept"/>
    <rdf:type rdf:resource="http://www.w3.org/2002/07/owl#NamedIndividual"/>
    <skos:topConceptOf rdf:resource="http://isdc.gfz-potsdam.de/ontology/SPASE-allowed_values.skos.owl#Observed_Region"/>
    <skos:inScheme rdf:resource="http://isdc.gfz-potsdam.de/ontology/SPASE-allowed_values.skos.owl#Observatory_Region"/>
    <skos:topConceptOf rdf:resource="http://isdc.gfz-potsdam.de/ontology/SPASE-allowed_values.skos.owl#Observatory_Region"/>
    <skos:definition xml:lang="en">A small extraterrestrial body consisting mostly of rock and metal that is in orbit around the sun.</skos:definition>
  </rdf:Description>
  <rdf:Description rdf:about="http://isdc.gfz-potsdam.de/ontology/SPASE-allowed_values.skos.owl#Mass_Spectrometer">
    <skos:topConceptOf rdf:resource="http://isdc.gfz-potsdam.de/ontology/SPASE-allowed_values.skos.owl#Instrument_Type"/>
    <skos:definition xml:lang="en">An instrument which distinguishes chemical species in terms of their different isotopic masses.</skos:definition>
    <skos:prefLabel xml:lang="en">Mass Spectrometer</skos:prefLabel>
    <skos:inScheme rdf:resource="http://isdc.gfz-potsdam.de/ontology/SPASE-allowed_values.skos.owl#Instrument_Type"/>
    <rdf:type rdf:resource="http://www.w3.org/2004/02/skos/core#Concept"/>
    <rdf:type rdf:resource="http://www.w3.org/2002/07/owl#NamedIndividual"/>
  </rdf:Description>
  <rdf:Description rdf:about="http://isdc.gfz-potsdam.de/ontology/SPASE-allowed_values.skos.owl#Ni-6768">
    <skos:topConceptOf rdf:resource="http://isdc.gfz-potsdam.de/ontology/SPASE-allowed_values.skos.owl#Spectral_Range"/>
    <rdf:type rdf:resource="http://www.w3.org/2004/02/skos/core#Concept"/>
    <rdf:type rdf:resource="http://www.w3.org/2002/07/owl#NamedIndividual"/>
    <skos:definition xml:lang="en">A spectrum with a wavelength range centered at 676.8 nm. VSO nickname: Ni-6768
dopplergram with a range of of 676.7 nm to 676.9 nm.</skos:definition>
    <skos:prefLabel xml:lang="en">Ni-6768</skos:prefLabel>
    <skos:inScheme rdf:resource="http://isdc.gfz-potsdam.de/ontology/SPASE-allowed_values.skos.owl#Spectral_Range"/>
  </rdf:Description>
  <rdf:Description rdf:about="http://isdc.gfz-potsdam.de/ontology/SPASE-allowed_values.skos.owl#Array">
    <skos:definition xml:lang="en">A sequence of values corresponding to the elements in a rectilinear, n-dimension matrix. Each
value can be referenced by a unique index.</skos:definition>
    <skos:topConceptOf rdf:resource="http://isdc.gfz-potsdam.de/ontology/SPASE-allowed_values.skos.owl#Qualifier"/>
    <skos:prefLabel xml:lang="en">Array</skos:prefLabel>
    <skos:inScheme rdf:resource="http://isdc.gfz-potsdam.de/ontology/SPASE-allowed_values.skos.owl#Qualifier"/>
    <rdf:type rdf:resource="http://www.w3.org/2002/07/owl#NamedIndividual"/>
    <rdf:type rdf:resource="http://www.w3.org/2004/02/skos/core#Concept"/>
  </rdf:Description>
  <rdf:Description rdf:about="http://isdc.gfz-potsdam.de/ontology/SPASE-allowed_values.skos.owl#Magnetogram">
    <rdf:type rdf:resource="http://www.w3.org/2004/02/skos/core#Concept"/>
    <skos:topConceptOf rdf:resource="http://isdc.gfz-potsdam.de/ontology/SPASE-allowed_values.skos.owl#Measurement_Type"/>
    <skos:inScheme rdf:resource="http://isdc.gfz-potsdam.de/ontology/SPASE-allowed_values.skos.owl#Measurement_Type"/>
    <skos:definition xml:lang="en">Measurements of the vector or line-of-sight magnetic field determined from remote sensing
measurements of the detailed structure of spectral lines, including their splitting and
polarization. ("Magnetogram.")</skos:definition>
    <skos:prefLabel xml:lang="en">Magnetogram</skos:prefLabel>
    <rdf:type rdf:resource="http://www.w3.org/2002/07/owl#NamedIndividual"/>
  </rdf:Description>
  <rdf:Description rdf:about="http://isdc.gfz-potsdam.de/ontology/SPASE-allowed_values.skos.owl#Rendering_Axis">
    <skos:hasTopConcept rdf:resource="http://isdc.gfz-potsdam.de/ontology/SPASE-allowed_values.skos.owl#Horizontal"/>
    <rdf:type rdf:resource="http://www.w3.org/2002/07/owl#NamedIndividual"/>
    <skos:hasTopConcept rdf:resource="http://isdc.gfz-potsdam.de/ontology/SPASE-allowed_values.skos.owl#Color_Bar"/>
    <rdf:type rdf:resource="http://www.w3.org/2004/02/skos/core#ConceptScheme"/>
    <skos:prefLabel xml:lang="en">Rendering Axis</skos:prefLabel>
    <skos:hasTopConcept rdf:resource="http://isdc.gfz-potsdam.de/ontology/SPASE-allowed_values.skos.owl#Vertical"/>
    <skos:definition xml:lang="en">A reference component of a plot or rendering of data. A plot typically is a 2-dimensional
rendering with a horizontal and verticle axis. A third dimension can be introduced with a color
coding of the rendered data.
Allowed Values:
Color Bar
Horizontal
Vertical</skos:definition>
  </rdf:Description>
  <rdf:Description rdf:about="http://isdc.gfz-potsdam.de/ontology/SPASE-allowed_values.skos.owl#Radiation_Belt">
    <skos:inScheme rdf:resource="http://isdc.gfz-potsdam.de/ontology/SPASE-allowed_values.skos.owl#Observatory_Region"/>
    <skos:inScheme rdf:resource="http://isdc.gfz-potsdam.de/ontology/SPASE-allowed_values.skos.owl#Observed_Region"/>
    <skos:broader rdf:resource="http://isdc.gfz-potsdam.de/ontology/SPASE-allowed_values.skos.owl#Magnetosphere"/>
    <rdf:type rdf:resource="http://www.w3.org/2004/02/skos/core#Concept"/>
    <rdf:type rdf:resource="http://www.w3.org/2002/07/owl#NamedIndividual"/>
    <skos:definition xml:lang="en">The region within a magnetosphere where high-energy particles could potentially be trapped in
a magnetic field.</skos:definition>
    <skos:prefLabel xml:lang="en">Radiation Belt</skos:prefLabel>
  </rdf:Description>
  <rdf:Description rdf:about="http://isdc.gfz-potsdam.de/ontology/SPASE-allowed_values.skos.owl#Coordinate_Representation">
    <skos:definition xml:lang="en">The method or form for specifying a given point or vector in a given coordinate system.
Allowed Values:
Cartesian
Cylindrical</skos:definition>
    <skos:prefLabel xml:lang="en">Coordinate Representation</skos:prefLabel>
    <rdf:type rdf:resource="http://www.w3.org/2002/07/owl#NamedIndividual"/>
    <skos:hasTopConcept rdf:resource="http://isdc.gfz-potsdam.de/ontology/SPASE-allowed_values.skos.owl#Cartesian"/>
    <skos:hasTopConcept rdf:resource="http://isdc.gfz-potsdam.de/ontology/SPASE-allowed_values.skos.owl#Cylindrical"/>
    <rdf:type rdf:resource="http://www.w3.org/2004/02/skos/core#ConceptScheme"/>
    <skos:hasTopConcept rdf:resource="http://isdc.gfz-potsdam.de/ontology/SPASE-allowed_values.skos.owl#Spherical"/>
  </rdf:Description>
  <rdf:Description rdf:about="http://isdc.gfz-potsdam.de/ontology/SPASE-allowed_values.skos.owl#Carrington">
    <skos:inScheme rdf:resource="http://isdc.gfz-potsdam.de/ontology/SPASE-allowed_values.skos.owl#Coordinate_System_Name"/>
    <skos:definition xml:lang="en">A coordinate system which is centered at the Sun and is "fixed" with respect to the synodic
rotation rate; the mean synodic value is about 27.2753 days. The Astronomical Almanac gives a
value for Carrington longitude of 349.03 degrees at 0000 UT on 1 January 1995.</skos:definition>
    <skos:topConceptOf rdf:resource="http://isdc.gfz-potsdam.de/ontology/SPASE-allowed_values.skos.owl#Coordinate_System_Name"/>
    <rdf:type rdf:resource="http://www.w3.org/2002/07/owl#NamedIndividual"/>
    <rdf:type rdf:resource="http://www.w3.org/2004/02/skos/core#Concept"/>
    <skos:prefLabel xml:lang="en">Carrington</skos:prefLabel>
  </rdf:Description>
  <rdf:Description rdf:about="http://isdc.gfz-potsdam.de/ontology/SPASE-allowed_values.skos.owl#Circular">
    <skos:inScheme rdf:resource="http://isdc.gfz-potsdam.de/ontology/SPASE-allowed_values.skos.owl#Qualifier"/>
    <rdf:type rdf:resource="http://www.w3.org/2002/07/owl#NamedIndividual"/>
    <skos:definition xml:lang="en">Relative to polarization, right-hand circularly polarized light is defined such that the electric
field is rotating clockwise as seen by an observer towards whom the wave is moving. Left-hand
circularly polarized light is defined such that the electric field is rotating counterclockwise as
seen by an observer towards whom the wave is moving. The polarization of
magnetohydrodynamic waves is specified with respect to the ambient mean magnetic field :
right-hand polarized waves have a transverse electric field component which turns in a
right-handed sense (that of the gyrating electrons) around the magnetic field.
-</skos:definition>
    <rdf:type rdf:resource="http://www.w3.org/2004/02/skos/core#Concept"/>
    <skos:topConceptOf rdf:resource="http://isdc.gfz-potsdam.de/ontology/SPASE-allowed_values.skos.owl#Qualifier"/>
    <skos:prefLabel xml:lang="en">Circular</skos:prefLabel>
  </rdf:Description>
  <rdf:Description rdf:about="http://isdc.gfz-potsdam.de/ontology/SPASE-allowed_values.skos.owl#Ultraviolet">
    <rdf:type rdf:resource="http://www.w3.org/2002/07/owl#NamedIndividual"/>
    <skos:definition xml:lang="en">Photons with a wavelength range: 10 to 400 nm.</skos:definition>
    <skos:topConceptOf rdf:resource="http://isdc.gfz-potsdam.de/ontology/SPASE-allowed_values.skos.owl#Spectral_Range"/>
    <rdf:type rdf:resource="http://www.w3.org/2004/02/skos/core#Concept"/>
    <skos:prefLabel xml:lang="en">Ultraviolet</skos:prefLabel>
    <skos:inScheme rdf:resource="http://isdc.gfz-potsdam.de/ontology/SPASE-allowed_values.skos.owl#Spectral_Range"/>
  </rdf:Description>
  <rdf:Description rdf:about="http://isdc.gfz-potsdam.de/ontology/SPASE-allowed_values.skos.owl#Magnetosheath">
    <skos:definition xml:lang="en">The region between the bow shock and the magnetopause, characterized by very turbulent
plasma.</skos:definition>
    <skos:inScheme rdf:resource="http://isdc.gfz-potsdam.de/ontology/SPASE-allowed_values.skos.owl#Observed_Region"/>
    <skos:prefLabel xml:lang="en">Magnetosheath</skos:prefLabel>
    <skos:broader rdf:resource="http://isdc.gfz-potsdam.de/ontology/SPASE-allowed_values.skos.owl#Earth"/>
    <skos:inScheme rdf:resource="http://isdc.gfz-potsdam.de/ontology/SPASE-allowed_values.skos.owl#Observatory_Region"/>
    <rdf:type rdf:resource="http://www.w3.org/2004/02/skos/core#Concept"/>
    <rdf:type rdf:resource="http://www.w3.org/2002/07/owl#NamedIndividual"/>
  </rdf:Description>
  <rdf:Description rdf:about="http://isdc.gfz-potsdam.de/ontology/SPASE-allowed_values.skos.owl#HCC">
    <rdf:type rdf:resource="http://www.w3.org/2004/02/skos/core#Concept"/>
    <skos:inScheme rdf:resource="http://isdc.gfz-potsdam.de/ontology/SPASE-allowed_values.skos.owl#Coordinate_System_Name"/>
    <skos:prefLabel xml:lang="en">HCC</skos:prefLabel>
    <rdf:type rdf:resource="http://www.w3.org/2002/07/owl#NamedIndividual"/>
    <skos:topConceptOf rdf:resource="http://isdc.gfz-potsdam.de/ontology/SPASE-allowed_values.skos.owl#Coordinate_System_Name"/>
    <skos:definition xml:lang="en">Heliocentric Cartesian - A 3-D orthonormal coordinate system that is primarily intended to
specify with two dimensions a point on the solar disk. The Z axis points toward the observer.
The Y axis lies in the plane defined by the solar spin vector and the Z axis, positive northward.
The X axis is perpendicular to the Y and Z axes, positive toward solar west. Standard
representation for this system is via the point's x and y values, expressed either as physical
distances or as fractions of the solar disk radius.</skos:definition>
  </rdf:Description>
  <rdf:Description rdf:about="http://isdc.gfz-potsdam.de/ontology/SPASE-allowed_values.skos.owl#Annotation_Type">
    <skos:prefLabel xml:lang="en">Annotation Type</skos:prefLabel>
    <skos:definition xml:lang="en">A classification for an annotation.
Allowed Values:
Anomaly
Event
Feature</skos:definition>
    <rdf:type rdf:resource="http://www.w3.org/2002/07/owl#NamedIndividual"/>
    <rdf:type rdf:resource="http://www.w3.org/2004/02/skos/core#ConceptScheme"/>
    <skos:hasTopConcept rdf:resource="http://isdc.gfz-potsdam.de/ontology/SPASE-allowed_values.skos.owl#Event"/>
    <skos:hasTopConcept rdf:resource="http://isdc.gfz-potsdam.de/ontology/SPASE-allowed_values.skos.owl#Feature"/>
    <skos:hasTopConcept rdf:resource="http://isdc.gfz-potsdam.de/ontology/SPASE-allowed_values.skos.owl#Anomaly"/>
  </rdf:Description>
  <rdf:Description rdf:about="http://isdc.gfz-potsdam.de/ontology/SPASE-allowed_values.skos.owl#Solar_Wind_Extreme">
    <rdf:type rdf:resource="http://www.w3.org/2002/07/owl#NamedIndividual"/>
    <rdf:type rdf:resource="http://www.w3.org/2004/02/skos/core#Concept"/>
    <skos:topConceptOf rdf:resource="http://isdc.gfz-potsdam.de/ontology/SPASE-allowed_values.skos.owl#Phenomenon_Type"/>
    <skos:definition xml:lang="en">Intervals of unusually large or small values of solar wind attributes such as flow speed and ion
density.</skos:definition>
    <skos:inScheme rdf:resource="http://isdc.gfz-potsdam.de/ontology/SPASE-allowed_values.skos.owl#Phenomenon_Type"/>
    <skos:prefLabel xml:lang="en">Solar Wind Extreme</skos:prefLabel>
  </rdf:Description>
  <rdf:Description rdf:about="http://isdc.gfz-potsdam.de/ontology/SPASE-allowed_values.skos.owl#Postscript">
    <skos:definition xml:lang="en">A page description programming language created by Adobe Systems Inc. that is a
device-independent industry standard for representing text and graphics.</skos:definition>
    <rdf:type rdf:resource="http://www.w3.org/2004/02/skos/core#Concept"/>
    <rdf:type rdf:resource="http://www.w3.org/2002/07/owl#NamedIndividual"/>
    <skos:inScheme rdf:resource="http://isdc.gfz-potsdam.de/ontology/SPASE-allowed_values.skos.owl#Format"/>
    <skos:topConceptOf rdf:resource="http://isdc.gfz-potsdam.de/ontology/SPASE-allowed_values.skos.owl#Format"/>
    <skos:prefLabel xml:lang="en">Postscript</skos:prefLabel>
  </rdf:Description>
  <rdf:Description rdf:about="http://isdc.gfz-potsdam.de/ontology/SPASE-allowed_values.skos.owl#Mass_Density">
    <skos:prefLabel xml:lang="en">Mass Density</skos:prefLabel>
    <skos:inScheme rdf:resource="http://isdc.gfz-potsdam.de/ontology/SPASE-allowed_values.skos.owl#Particle_Quantity"/>
    <rdf:type rdf:resource="http://www.w3.org/2002/07/owl#NamedIndividual"/>
    <rdf:type rdf:resource="http://www.w3.org/2004/02/skos/core#Concept"/>
    <skos:definition xml:lang="en">The mass of particles per unit volume.</skos:definition>
    <skos:topConceptOf rdf:resource="http://isdc.gfz-potsdam.de/ontology/SPASE-allowed_values.skos.owl#Particle_Quantity"/>
  </rdf:Description>
  <rdf:Description rdf:about="http://isdc.gfz-potsdam.de/ontology/SPASE-allowed_values.skos.owl#Interstellar">
    <skos:definition xml:lang="en">The region between stars outside of the star's heliopause.</skos:definition>
    <rdf:type rdf:resource="http://www.w3.org/2004/02/skos/core#Concept"/>
    <skos:inScheme rdf:resource="http://isdc.gfz-potsdam.de/ontology/SPASE-allowed_values.skos.owl#Observed_Region"/>
    <skos:topConceptOf rdf:resource="http://isdc.gfz-potsdam.de/ontology/SPASE-allowed_values.skos.owl#Observatory_Region"/>
    <skos:inScheme rdf:resource="http://isdc.gfz-potsdam.de/ontology/SPASE-allowed_values.skos.owl#Observatory_Region"/>
    <rdf:type rdf:resource="http://www.w3.org/2002/07/owl#NamedIndividual"/>
    <skos:prefLabel xml:lang="en">Interstellar</skos:prefLabel>
    <skos:topConceptOf rdf:resource="http://isdc.gfz-potsdam.de/ontology/SPASE-allowed_values.skos.owl#Observed_Region"/>
  </rdf:Description>
  <rdf:Description rdf:about="http://isdc.gfz-potsdam.de/ontology/SPASE-allowed_values.skos.owl#Feature">
    <skos:definition xml:lang="en">A prominent or distinctive characteristic that occurs at a location or persists over a period of
time.</skos:definition>
    <skos:topConceptOf rdf:resource="http://isdc.gfz-potsdam.de/ontology/SPASE-allowed_values.skos.owl#Annotation_Type"/>
    <rdf:type rdf:resource="http://www.w3.org/2004/02/skos/core#Concept"/>
    <rdf:type rdf:resource="http://www.w3.org/2002/07/owl#NamedIndividual"/>
    <skos:prefLabel xml:lang="en">Feature</skos:prefLabel>
    <skos:inScheme rdf:resource="http://isdc.gfz-potsdam.de/ontology/SPASE-allowed_values.skos.owl#Annotation_Type"/>
  </rdf:Description>
  <rdf:Description rdf:about="http://isdc.gfz-potsdam.de/ontology/SPASE-allowed_values.skos.owl#Print">
    <skos:prefLabel xml:lang="en">Print</skos:prefLabel>
    <skos:inScheme rdf:resource="http://isdc.gfz-potsdam.de/ontology/SPASE-allowed_values.skos.owl#Format"/>
    <rdf:type rdf:resource="http://www.w3.org/2002/07/owl#NamedIndividual"/>
    <rdf:type rdf:resource="http://www.w3.org/2004/02/skos/core#Concept"/>
    <skos:broader rdf:resource="http://isdc.gfz-potsdam.de/ontology/SPASE-allowed_values.skos.owl#Hardcopy"/>
    <skos:definition xml:lang="en">A sheet of any written or printed material which may include notes or graphics. Multiple
printed pages may be bound into a manuscript or book.</skos:definition>
  </rdf:Description>
  <rdf:Description rdf:about="http://isdc.gfz-potsdam.de/ontology/SPASE-allowed_values.skos.owl#WGS84">
    <rdf:type rdf:resource="http://www.w3.org/2004/02/skos/core#Concept"/>
    <rdf:type rdf:resource="http://www.w3.org/2002/07/owl#NamedIndividual"/>
    <skos:prefLabel xml:lang="en">WGS84</skos:prefLabel>
    <skos:topConceptOf rdf:resource="http://isdc.gfz-potsdam.de/ontology/SPASE-allowed_values.skos.owl#Coordinate_System_Name"/>
    <skos:definition xml:lang="en">The World Geodetic System (WGS) defines a reference frame for the earth, for use in geodesy
and navigation. The WGS84 uses the zero meridian as defined by the Bureau International de
l'Heure.</skos:definition>
    <skos:inScheme rdf:resource="http://isdc.gfz-potsdam.de/ontology/SPASE-allowed_values.skos.owl#Coordinate_System_Name"/>
  </rdf:Description>
  <rdf:Description rdf:about="http://isdc.gfz-potsdam.de/ontology/SPASE-allowed_values.skos.owl#Unicode">
    <rdf:type rdf:resource="http://www.w3.org/2004/02/skos/core#Concept"/>
    <skos:prefLabel xml:lang="en">Unicode</skos:prefLabel>
    <skos:inScheme rdf:resource="http://isdc.gfz-potsdam.de/ontology/SPASE-allowed_values.skos.owl#Encoding"/>
    <skos:inScheme rdf:resource="http://isdc.gfz-potsdam.de/ontology/SPASE-allowed_values.skos.owl#Format"/>
    <skos:definition xml:lang="en">Text in multi-byte Unicode format.</skos:definition>
    <skos:broader rdf:resource="http://isdc.gfz-potsdam.de/ontology/SPASE-allowed_values.skos.owl#Text"/>
    <rdf:type rdf:resource="http://www.w3.org/2002/07/owl#NamedIndividual"/>
  </rdf:Description>
  <rdf:Description rdf:about="http://isdc.gfz-potsdam.de/ontology/SPASE-allowed_values.skos.owl#White-Light">
    <skos:prefLabel xml:lang="en">White-Light</skos:prefLabel>
    <skos:definition xml:lang="en">Photons with a wavelength in the visible range for humans.</skos:definition>
    <skos:inScheme rdf:resource="http://isdc.gfz-potsdam.de/ontology/SPASE-allowed_values.skos.owl#Spectral_Range"/>
    <rdf:type rdf:resource="http://www.w3.org/2002/07/owl#NamedIndividual"/>
    <rdf:type rdf:resource="http://www.w3.org/2004/02/skos/core#Concept"/>
    <skos:topConceptOf rdf:resource="http://isdc.gfz-potsdam.de/ontology/SPASE-allowed_values.skos.owl#Spectral_Range"/>
  </rdf:Description>
  <rdf:Description rdf:about="http://isdc.gfz-potsdam.de/ontology/SPASE-allowed_values.skos.owl#UDF">
    <rdf:type rdf:resource="http://www.w3.org/2002/07/owl#NamedIndividual"/>
    <rdf:type rdf:resource="http://www.w3.org/2004/02/skos/core#Concept"/>
    <skos:prefLabel xml:lang="en">UDF</skos:prefLabel>
    <skos:inScheme rdf:resource="http://isdc.gfz-potsdam.de/ontology/SPASE-allowed_values.skos.owl#Format"/>
    <skos:definition xml:lang="en">Universal Data Format (UDF). The Optical Technology Storage Association's Universal Disk
Format, based on ISO 13346. See &lt;http://www.osta.org/specs/index.htm&gt;.</skos:definition>
    <skos:topConceptOf rdf:resource="http://isdc.gfz-potsdam.de/ontology/SPASE-allowed_values.skos.owl#Format"/>
  </rdf:Description>
  <rdf:Description rdf:about="http://isdc.gfz-potsdam.de/ontology/SPASE-allowed_values.skos.owl#HEEQ">
    <skos:topConceptOf rdf:resource="http://isdc.gfz-potsdam.de/ontology/SPASE-allowed_values.skos.owl#Coordinate_System_Name"/>
    <skos:definition xml:lang="en">Heliocentric Earth Equatorial - A coordinate system where the Z axis is normal to the solar
equatorial plane, positive northward. X axis is generally Earthward in the plane defined by the
Z axis and the Sun-Earth direction. See Hapgood, 1992.</skos:definition>
    <rdf:type rdf:resource="http://www.w3.org/2002/07/owl#NamedIndividual"/>
    <rdf:type rdf:resource="http://www.w3.org/2004/02/skos/core#Concept"/>
    <skos:inScheme rdf:resource="http://isdc.gfz-potsdam.de/ontology/SPASE-allowed_values.skos.owl#Coordinate_System_Name"/>
    <skos:prefLabel xml:lang="en">HEEQ</skos:prefLabel>
  </rdf:Description>
  <rdf:Description rdf:about="http://isdc.gfz-potsdam.de/ontology/SPASE-allowed_values.skos.owl#Coronograph">
    <skos:definition xml:lang="en">Coronograph</skos:definition>
    <skos:definition xml:lang="en">An instrument which can image things very close to the Sun by using a disk to block the Sun's
bright surface which reveals the faint solar corona and other celestial objects.</skos:definition>
    <skos:inScheme rdf:resource="http://isdc.gfz-potsdam.de/ontology/SPASE-allowed_values.skos.owl#Instrument_Type"/>
    <rdf:type rdf:resource="http://www.w3.org/2004/02/skos/core#Concept"/>
    <rdf:type rdf:resource="http://www.w3.org/2002/07/owl#NamedIndividual"/>
    <skos:topConceptOf rdf:resource="http://isdc.gfz-potsdam.de/ontology/SPASE-allowed_values.skos.owl#Instrument_Type"/>
  </rdf:Description>
  <rdf:Description rdf:about="http://isdc.gfz-potsdam.de/ontology/SPASE-allowed_values.skos.owl#Polar_Angle">
    <skos:inScheme rdf:resource="http://isdc.gfz-potsdam.de/ontology/SPASE-allowed_values.skos.owl#Qualifier"/>
    <skos:broader rdf:resource="http://isdc.gfz-potsdam.de/ontology/SPASE-allowed_values.skos.owl#Direction_Angle"/>
    <rdf:type rdf:resource="http://www.w3.org/2004/02/skos/core#Concept"/>
    <rdf:type rdf:resource="http://www.w3.org/2002/07/owl#NamedIndividual"/>
    <skos:definition xml:lang="en">The angle between the position or measured vector and the k-axis of the coordinate system.
Mathematically defined as arctan([SQRT(i^2+j^2)]/k).</skos:definition>
    <skos:prefLabel xml:lang="en">Polar Angle</skos:prefLabel>
  </rdf:Description>
  <rdf:Description rdf:about="http://isdc.gfz-potsdam.de/ontology/SPASE-allowed_values.skos.owl#Search_Coil">
    <rdf:type rdf:resource="http://www.w3.org/2002/07/owl#NamedIndividual"/>
    <rdf:type rdf:resource="http://www.w3.org/2004/02/skos/core#Concept"/>
    <skos:prefLabel xml:lang="en">Search Coil</skos:prefLabel>
    <skos:definition xml:lang="en">An instrument which measures the time variation of the magnetic flux threading a loop by
measurement of the electric potential difference induced between the ends of the wire.</skos:definition>
    <skos:topConceptOf rdf:resource="http://isdc.gfz-potsdam.de/ontology/SPASE-allowed_values.skos.owl#Instrument_Type"/>
    <skos:inScheme rdf:resource="http://isdc.gfz-potsdam.de/ontology/SPASE-allowed_values.skos.owl#Instrument_Type"/>
  </rdf:Description>
  <rdf:Description rdf:about="http://isdc.gfz-potsdam.de/ontology/SPASE-allowed_values.skos.owl#Main">
    <rdf:type rdf:resource="http://www.w3.org/2004/02/skos/core#Concept"/>
    <skos:prefLabel xml:lang="en">Main</skos:prefLabel>
    <skos:definition xml:lang="en">The region of the magnetosphere where the magnetic field lines are closed, but does not include
the gaseous region gravitationally bound to the body.</skos:definition>
    <skos:broader rdf:resource="http://isdc.gfz-potsdam.de/ontology/SPASE-allowed_values.skos.owl#Magnetosphere"/>
    <rdf:type rdf:resource="http://www.w3.org/2002/07/owl#NamedIndividual"/>
    <skos:inScheme rdf:resource="http://isdc.gfz-potsdam.de/ontology/SPASE-allowed_values.skos.owl#Observatory_Region"/>
    <skos:inScheme rdf:resource="http://isdc.gfz-potsdam.de/ontology/SPASE-allowed_values.skos.owl#Observed_Region"/>
  </rdf:Description>
  <rdf:Description rdf:about="http://isdc.gfz-potsdam.de/ontology/SPASE-allowed_values.skos.owl#Gamma_Rays">
    <skos:topConceptOf rdf:resource="http://isdc.gfz-potsdam.de/ontology/SPASE-allowed_values.skos.owl#Spectral_Range"/>
    <rdf:type rdf:resource="http://www.w3.org/2004/02/skos/core#Concept"/>
    <rdf:type rdf:resource="http://www.w3.org/2002/07/owl#NamedIndividual"/>
    <skos:prefLabel xml:lang="en">Gamma Rays</skos:prefLabel>
    <skos:definition xml:lang="en">Photons with a wavelength range: 0.00001 to 0.001 nm</skos:definition>
    <skos:inScheme rdf:resource="http://isdc.gfz-potsdam.de/ontology/SPASE-allowed_values.skos.owl#Spectral_Range"/>
  </rdf:Description>
  <rdf:Description rdf:about="http://isdc.gfz-potsdam.de/ontology/SPASE-allowed_values.skos.owl#Particle_Quantity">
    <skos:hasTopConcept rdf:resource="http://isdc.gfz-potsdam.de/ontology/SPASE-allowed_values.skos.owl#Plasma_Frequency"/>
    <skos:hasTopConcept rdf:resource="http://isdc.gfz-potsdam.de/ontology/SPASE-allowed_values.skos.owl#Counts"/>
    <skos:hasTopConcept rdf:resource="http://isdc.gfz-potsdam.de/ontology/SPASE-allowed_values.skos.owl#Pressure"/>
    <rdf:type rdf:resource="http://www.w3.org/2004/02/skos/core#ConceptScheme"/>
    <skos:hasTopConcept rdf:resource="http://isdc.gfz-potsdam.de/ontology/SPASE-allowed_values.skos.owl#Sound_Speed"/>
    <skos:hasTopConcept rdf:resource="http://isdc.gfz-potsdam.de/ontology/SPASE-allowed_values.skos.owl#Energy"/>
    <skos:hasTopConcept rdf:resource="http://isdc.gfz-potsdam.de/ontology/SPASE-allowed_values.skos.owl#Thermal_Speed"/>
    <skos:hasTopConcept rdf:resource="http://isdc.gfz-potsdam.de/ontology/SPASE-allowed_values.skos.owl#Number_Flux"/>
    <skos:hasTopConcept rdf:resource="http://isdc.gfz-potsdam.de/ontology/SPASE-allowed_values.skos.owl#Velocity"/>
    <skos:prefLabel xml:lang="en">Particle Quantity</skos:prefLabel>
    <skos:hasTopConcept rdf:resource="http://isdc.gfz-potsdam.de/ontology/SPASE-allowed_values.skos.owl#Average_Charge_State"/>
    <skos:hasTopConcept rdf:resource="http://isdc.gfz-potsdam.de/ontology/SPASE-allowed_values.skos.owl#Energy_Density"/>
    <skos:hasTopConcept rdf:resource="http://isdc.gfz-potsdam.de/ontology/SPASE-allowed_values.skos.owl#Mass"/>
    <skos:hasTopConcept rdf:resource="http://isdc.gfz-potsdam.de/ontology/SPASE-allowed_values.skos.owl#Sonic_Mach_Number"/>
    <skos:definition xml:lang="en">A characterization of the physical properties of the particle.
Allowed Values:
Arrival Direction
Atomic Number Detected
Average Charge State
Charge State
Count Rate
Counts
Energy
Energy Density
Energy Flux
Flow Speed
Flow Velocity
Fluence
Gyrofrequency
Heat Flux
Mass
Mass Density
Mass Number
Number Density
Number Flux
Particle Radius
Phase-Space Density
Plasma Frequency
Pressure
Sonic Mach Number
Sound Speed
Temperature</skos:definition>
    <skos:hasTopConcept rdf:resource="http://isdc.gfz-potsdam.de/ontology/SPASE-allowed_values.skos.owl#Charge_State"/>
    <skos:hasTopConcept rdf:resource="http://isdc.gfz-potsdam.de/ontology/SPASE-allowed_values.skos.owl#Heat_Flux"/>
    <skos:hasTopConcept rdf:resource="http://isdc.gfz-potsdam.de/ontology/SPASE-allowed_values.skos.owl#Atomic_Number_Detected"/>
    <skos:hasTopConcept rdf:resource="http://isdc.gfz-potsdam.de/ontology/SPASE-allowed_values.skos.owl#Temperature"/>
    <skos:hasTopConcept rdf:resource="http://isdc.gfz-potsdam.de/ontology/SPASE-allowed_values.skos.owl#Phase-Space_Density"/>
    <skos:hasTopConcept rdf:resource="http://isdc.gfz-potsdam.de/ontology/SPASE-allowed_values.skos.owl#Gyrofrequency"/>
    <skos:hasTopConcept rdf:resource="http://isdc.gfz-potsdam.de/ontology/SPASE-allowed_values.skos.owl#Count_Rate"/>
    <skos:hasTopConcept rdf:resource="http://isdc.gfz-potsdam.de/ontology/SPASE-allowed_values.skos.owl#Flow_Velocity"/>
    <skos:hasTopConcept rdf:resource="http://isdc.gfz-potsdam.de/ontology/SPASE-allowed_values.skos.owl#Fluence"/>
    <skos:hasTopConcept rdf:resource="http://isdc.gfz-potsdam.de/ontology/SPASE-allowed_values.skos.owl#Number_Density"/>
    <skos:hasTopConcept rdf:resource="http://isdc.gfz-potsdam.de/ontology/SPASE-allowed_values.skos.owl#Energy_Flux"/>
    <skos:hasTopConcept rdf:resource="http://isdc.gfz-potsdam.de/ontology/SPASE-allowed_values.skos.owl#Arrival_Direction"/>
    <skos:hasTopConcept rdf:resource="http://isdc.gfz-potsdam.de/ontology/SPASE-allowed_values.skos.owl#Mass_Density"/>
    <rdf:type rdf:resource="http://www.w3.org/2002/07/owl#NamedIndividual"/>
    <skos:hasTopConcept rdf:resource="http://isdc.gfz-potsdam.de/ontology/SPASE-allowed_values.skos.owl#Particle_Radius"/>
    <skos:hasTopConcept rdf:resource="http://isdc.gfz-potsdam.de/ontology/SPASE-allowed_values.skos.owl#Mass_Number"/>
    <skos:hasTopConcept rdf:resource="http://isdc.gfz-potsdam.de/ontology/SPASE-allowed_values.skos.owl#Flow_Speed"/>
  </rdf:Description>
  <rdf:Description rdf:about="http://isdc.gfz-potsdam.de/ontology/SPASE-allowed_values.skos.owl#Deputy-PI">
    <skos:topConceptOf rdf:resource="http://isdc.gfz-potsdam.de/ontology/SPASE-allowed_values.skos.owl#Role"/>
    <skos:definition xml:lang="en">An individual who is an administrative or scientific leader for an investigation operating under
the supervision of a Principal Investigator.</skos:definition>
    <rdf:type rdf:resource="http://www.w3.org/2002/07/owl#NamedIndividual"/>
    <rdf:type rdf:resource="http://www.w3.org/2004/02/skos/core#Concept"/>
    <skos:prefLabel xml:lang="en">Deputy-PI</skos:prefLabel>
    <skos:inScheme rdf:resource="http://isdc.gfz-potsdam.de/ontology/SPASE-allowed_values.skos.owl#Role"/>
  </rdf:Description>
  <rdf:Description rdf:about="http://isdc.gfz-potsdam.de/ontology/SPASE-allowed_values.skos.owl#Plasma_Waves">
    <skos:prefLabel>Plasma Waves</skos:prefLabel>
    <rdf:type rdf:resource="http://www.w3.org/2002/07/owl#NamedIndividual"/>
    <skos:inScheme rdf:resource="http://isdc.gfz-potsdam.de/ontology/SPASE-allowed_values.skos.owl#Wave_Type"/>
    <skos:topConceptOf rdf:resource="http://isdc.gfz-potsdam.de/ontology/SPASE-allowed_values.skos.owl#Wave_Type"/>
    <rdf:type rdf:resource="http://www.w3.org/2004/02/skos/core#Concept"/>
    <skos:definition xml:lang="en">Self-consistent collective oscillations of particles and fields (electric and magnetic) in a plasma.</skos:definition>
  </rdf:Description>
  <rdf:Description rdf:about="http://isdc.gfz-potsdam.de/ontology/SPASE-allowed_values.skos.owl#MATLAB_4">
    <skos:prefLabel xml:lang="en">MATLAB_4</skos:prefLabel>
    <rdf:type rdf:resource="http://www.w3.org/2004/02/skos/core#Concept"/>
    <rdf:type rdf:resource="http://www.w3.org/2002/07/owl#NamedIndividual"/>
    <skos:inScheme rdf:resource="http://isdc.gfz-potsdam.de/ontology/SPASE-allowed_values.skos.owl#Format"/>
    <skos:topConceptOf rdf:resource="http://isdc.gfz-potsdam.de/ontology/SPASE-allowed_values.skos.owl#Format"/>
    <skos:definition xml:lang="en">MATLAB Workspace save set, version 4. MAT-files are double-precision, binary, MATLAB
format files. MATLAB is a proprietary product of The MathWorks.</skos:definition>
  </rdf:Description>
  <rdf:Description rdf:about="http://isdc.gfz-potsdam.de/ontology/SPASE-allowed_values.skos.owl#Variance">
    <skos:prefLabel xml:lang="en">Variance</skos:prefLabel>
    <skos:inScheme rdf:resource="http://isdc.gfz-potsdam.de/ontology/SPASE-allowed_values.skos.owl#Qualifier"/>
    <rdf:type rdf:resource="http://www.w3.org/2004/02/skos/core#Concept"/>
    <rdf:type rdf:resource="http://www.w3.org/2002/07/owl#NamedIndividual"/>
    <skos:topConceptOf rdf:resource="http://isdc.gfz-potsdam.de/ontology/SPASE-allowed_values.skos.owl#Qualifier"/>
    <skos:definition xml:lang="en">A measure of dispersion of a set of data points around their mean value. The expectation value
of the squared deviations from the mean.</skos:definition>
  </rdf:Description>
  <rdf:Description rdf:about="http://isdc.gfz-potsdam.de/ontology/SPASE-allowed_values.skos.owl#Bow_Shock_Crossing">
    <skos:inScheme rdf:resource="http://isdc.gfz-potsdam.de/ontology/SPASE-allowed_values.skos.owl#Phenomenon_Type"/>
    <rdf:type rdf:resource="http://www.w3.org/2002/07/owl#NamedIndividual"/>
    <skos:prefLabel xml:lang="en">Bow Shock Crossing</skos:prefLabel>
    <skos:definition xml:lang="en">A crossing of the boundary between the undisturbed (except for foreshock effects) solar wind
and the shocked, decelerated solar wind of the magnetosheath.</skos:definition>
    <rdf:type rdf:resource="http://www.w3.org/2004/02/skos/core#Concept"/>
    <skos:topConceptOf rdf:resource="http://isdc.gfz-potsdam.de/ontology/SPASE-allowed_values.skos.owl#Phenomenon_Type"/>
  </rdf:Description>
  <rdf:Description rdf:about="http://isdc.gfz-potsdam.de/ontology/SPASE-allowed_values.skos.owl#SSE">
    <skos:inScheme rdf:resource="http://isdc.gfz-potsdam.de/ontology/SPASE-allowed_values.skos.owl#Coordinate_System_Name"/>
    <skos:definition xml:lang="en">Spacecraft Solar Ecliptic - A coordinate system used for deep space spacecraft, for example
Helios. - X axis from spacecraft to Sun. Z axis normal to ecliptic plane, positive northward.
Note: Angle between normals to ecliptic and to Helios orbit plane ~ 0.25 deg.</skos:definition>
    <skos:topConceptOf rdf:resource="http://isdc.gfz-potsdam.de/ontology/SPASE-allowed_values.skos.owl#Coordinate_System_Name"/>
    <rdf:type rdf:resource="http://www.w3.org/2004/02/skos/core#Concept"/>
    <rdf:type rdf:resource="http://www.w3.org/2002/07/owl#NamedIndividual"/>
    <skos:prefLabel xml:lang="en">SSE</skos:prefLabel>
  </rdf:Description>
  <rdf:Description rdf:about="http://isdc.gfz-potsdam.de/ontology/SPASE-allowed_values.skos.owl#Scintillation_Detector">
    <rdf:type rdf:resource="http://www.w3.org/2004/02/skos/core#Concept"/>
    <skos:prefLabel xml:lang="en">Scintillation Detector</skos:prefLabel>
    <skos:definition xml:lang="en">An instrument which detects flouresences of a material which is excited by high energy
(ionizing) electromagnetic or charged particle radiation.</skos:definition>
    <skos:topConceptOf rdf:resource="http://isdc.gfz-potsdam.de/ontology/SPASE-allowed_values.skos.owl#Instrument_Type"/>
    <skos:inScheme rdf:resource="http://isdc.gfz-potsdam.de/ontology/SPASE-allowed_values.skos.owl#Instrument_Type"/>
    <rdf:type rdf:resource="http://www.w3.org/2002/07/owl#NamedIndividual"/>
  </rdf:Description>
  <rdf:Description rdf:about="http://isdc.gfz-potsdam.de/ontology/SPASE-allowed_values.skos.owl#Median">
    <skos:inScheme rdf:resource="http://isdc.gfz-potsdam.de/ontology/SPASE-allowed_values.skos.owl#Qualifier"/>
    <rdf:type rdf:resource="http://www.w3.org/2004/02/skos/core#Concept"/>
    <rdf:type rdf:resource="http://www.w3.org/2002/07/owl#NamedIndividual"/>
    <skos:topConceptOf rdf:resource="http://isdc.gfz-potsdam.de/ontology/SPASE-allowed_values.skos.owl#Qualifier"/>
    <skos:definition xml:lang="en">The measure of central tendency of a set of n. values computed by ordering the values and
taking the value at position (n. + 1) / 2 when n. is odd or the arithmetic mean of the values at
positions n. / 2 and (n. / 2) + 1 when n. is even.</skos:definition>
    <skos:prefLabel xml:lang="en">Median</skos:prefLabel>
  </rdf:Description>
  <rdf:Description rdf:about="http://isdc.gfz-potsdam.de/ontology/SPASE-allowed_values.skos.owl#Retarding_Potential_Analyser">
    <skos:inScheme rdf:resource="http://isdc.gfz-potsdam.de/ontology/SPASE-allowed_values.skos.owl#Instrument_Type"/>
    <rdf:type rdf:resource="http://www.w3.org/2002/07/owl#NamedIndividual"/>
    <rdf:type rdf:resource="http://www.w3.org/2004/02/skos/core#Concept"/>
    <skos:prefLabel xml:lang="en">Retarding Potential Analyser</skos:prefLabel>
    <skos:definition xml:lang="en">An instrument which measures ion temperatures and ion concentrations using a planar ion trap.</skos:definition>
    <skos:topConceptOf rdf:resource="http://isdc.gfz-potsdam.de/ontology/SPASE-allowed_values.skos.owl#Instrument_Type"/>
  </rdf:Description>
  <rdf:Description rdf:about="http://www.w3.org/2004/02/skos/core#prefLabel">
    <rdfs:subPropertyOf rdf:resource="http://www.w3.org/2000/01/rdf-schema#label"/>
    <rdf:type rdf:resource="http://www.w3.org/2002/07/owl#AnnotationProperty"/>
  </rdf:Description>
  <rdf:Description rdf:about="http://isdc.gfz-potsdam.de/ontology/SPASE-allowed_values.skos.owl#Vertical">
    <skos:inScheme rdf:resource="http://isdc.gfz-potsdam.de/ontology/SPASE-allowed_values.skos.owl#Rendering_Axis"/>
    <rdf:type rdf:resource="http://www.w3.org/2002/07/owl#NamedIndividual"/>
    <skos:topConceptOf rdf:resource="http://isdc.gfz-potsdam.de/ontology/SPASE-allowed_values.skos.owl#Rendering_Axis"/>
    <skos:prefLabel xml:lang="en">Vertical</skos:prefLabel>
    <rdf:type rdf:resource="http://www.w3.org/2004/02/skos/core#Concept"/>
    <skos:definition xml:lang="en">Perpendicular to the plane of the horizon or a base line.</skos:definition>
  </rdf:Description>
  <rdf:Description rdf:about="http://isdc.gfz-potsdam.de/ontology/SPASE-allowed_values.skos.owl#Color_Bar">
    <skos:inScheme rdf:resource="http://isdc.gfz-potsdam.de/ontology/SPASE-allowed_values.skos.owl#Rendering_Axis"/>
    <rdf:type rdf:resource="http://www.w3.org/2004/02/skos/core#Concept"/>
    <skos:topConceptOf rdf:resource="http://isdc.gfz-potsdam.de/ontology/SPASE-allowed_values.skos.owl#Rendering_Axis"/>
    <skos:prefLabel xml:lang="en">Color Bar</skos:prefLabel>
    <skos:definition xml:lang="en">A spectrum or set of colors used to represent data values.</skos:definition>
    <rdf:type rdf:resource="http://www.w3.org/2002/07/owl#NamedIndividual"/>
  </rdf:Description>
  <rdf:Description rdf:about="http://isdc.gfz-potsdam.de/ontology/SPASE-allowed_values.skos.owl#Geomagnetic_Storm">
    <rdf:type rdf:resource="http://www.w3.org/2004/02/skos/core#Concept"/>
    <rdf:type rdf:resource="http://www.w3.org/2002/07/owl#NamedIndividual"/>
    <skos:topConceptOf rdf:resource="http://isdc.gfz-potsdam.de/ontology/SPASE-allowed_values.skos.owl#Phenomenon_Type"/>
    <skos:definition xml:lang="en">A magnetospheric disturbance typically defined by variations in the horizontal component of
the Earth's surface magnetic field. The variation typically starts with a field enhancement
associated with a solar wind pressure pulse and continues with a field depression associated
with an enhancement of the diamagnetic magnetospheric ring current.</skos:definition>
    <skos:inScheme rdf:resource="http://isdc.gfz-potsdam.de/ontology/SPASE-allowed_values.skos.owl#Phenomenon_Type"/>
    <skos:prefLabel xml:lang="en">Geomagnetic Storm</skos:prefLabel>
  </rdf:Description>
  <rdf:Description rdf:about="http://isdc.gfz-potsdam.de/ontology/SPASE-allowed_values.skos.owl#Neutral_Atom_Imager">
    <rdf:type rdf:resource="http://www.w3.org/2002/07/owl#NamedIndividual"/>
    <rdf:type rdf:resource="http://www.w3.org/2004/02/skos/core#Concept"/>
    <skos:prefLabel xml:lang="en">Neutral Atom Imager</skos:prefLabel>
    <skos:topConceptOf rdf:resource="http://isdc.gfz-potsdam.de/ontology/SPASE-allowed_values.skos.owl#Instrument_Type"/>
    <skos:definition xml:lang="en">An instrument which measures the quantity and properties of neutral particles over a range of
angles. Measured properties can include mass and energy.</skos:definition>
    <skos:inScheme rdf:resource="http://isdc.gfz-potsdam.de/ontology/SPASE-allowed_values.skos.owl#Instrument_Type"/>
  </rdf:Description>
  <rdf:Description rdf:about="http://isdc.gfz-potsdam.de/ontology/SPASE-allowed_values.skos.owl#Qualifier">
    <skos:hasTopConcept rdf:resource="http://isdc.gfz-potsdam.de/ontology/SPASE-allowed_values.skos.owl#Vector"/>
    <skos:hasTopConcept rdf:resource="http://isdc.gfz-potsdam.de/ontology/SPASE-allowed_values.skos.owl#Scalar"/>
    <skos:hasTopConcept rdf:resource="http://isdc.gfz-potsdam.de/ontology/SPASE-allowed_values.skos.owl#Maximum"/>
    <skos:hasTopConcept rdf:resource="http://isdc.gfz-potsdam.de/ontology/SPASE-allowed_values.skos.owl#Projection"/>
    <skos:hasTopConcept rdf:resource="http://isdc.gfz-potsdam.de/ontology/SPASE-allowed_values.skos.owl#Component"/>
    <skos:hasTopConcept rdf:resource="http://isdc.gfz-potsdam.de/ontology/SPASE-allowed_values.skos.owl#Uncertainty"/>
    <skos:definition xml:lang="en">Characterizes the refinement to apply to a type or attribute of a quantity.
Allowed Values:
Anisotropy
Array
Average
Characteristic
Circular
Column
Component
Component.I
Component.J
Component.K
Core
Cross Spectrum
Deviation
Differential
Direction
Direction Angle
Direction Angle.Azimuth Angle
Direction Angle.Elevation Angle
Direction Angle.Polar Angle
Directional
Field-Aligned
Fit
Group
Halo
Integral
Integral.Area
Integral.Bandwidth
Integral.Solid Angle
Line Of Sight
Linear
Magnitude
Maximum
Median
Minimum
Moment
Parallel
Peak
Perpendicular
Perturbation
Phase
Phase Angle
Projection
Projection.IJ
Projection.IK
Projection.JK
Pseudo
Ratio
Scalar
Spectral
Standard Deviation
Stoke's Parameters
Strahl
Superhalo
Symmetric
Tensor
Total
Trace
Uncertainty
Variance
Vector</skos:definition>
    <skos:hasTopConcept rdf:resource="http://isdc.gfz-potsdam.de/ontology/SPASE-allowed_values.skos.owl#Standard_Deviation"/>
    <skos:hasTopConcept rdf:resource="http://isdc.gfz-potsdam.de/ontology/SPASE-allowed_values.skos.owl#Field-Aligned"/>
    <skos:hasTopConcept rdf:resource="http://isdc.gfz-potsdam.de/ontology/SPASE-allowed_values.skos.owl#Stoke's_Parameters"/>
    <skos:hasTopConcept rdf:resource="http://isdc.gfz-potsdam.de/ontology/SPASE-allowed_values.skos.owl#Line_Of_Sight"/>
    <skos:hasTopConcept rdf:resource="http://isdc.gfz-potsdam.de/ontology/SPASE-allowed_values.skos.owl#Phase_Angle"/>
    <skos:hasTopConcept rdf:resource="http://isdc.gfz-potsdam.de/ontology/SPASE-allowed_values.skos.owl#Halo"/>
    <skos:hasTopConcept rdf:resource="http://isdc.gfz-potsdam.de/ontology/SPASE-allowed_values.skos.owl#Variance"/>
    <skos:hasTopConcept rdf:resource="http://isdc.gfz-potsdam.de/ontology/SPASE-allowed_values.skos.owl#Average"/>
    <skos:hasTopConcept rdf:resource="http://isdc.gfz-potsdam.de/ontology/SPASE-allowed_values.skos.owl#Group"/>
    <skos:hasTopConcept rdf:resource="http://isdc.gfz-potsdam.de/ontology/SPASE-allowed_values.skos.owl#Spectral"/>
    <skos:hasTopConcept rdf:resource="http://isdc.gfz-potsdam.de/ontology/SPASE-allowed_values.skos.owl#Median"/>
    <skos:hasTopConcept rdf:resource="http://isdc.gfz-potsdam.de/ontology/SPASE-allowed_values.skos.owl#Ratio"/>
    <skos:hasTopConcept rdf:resource="http://isdc.gfz-potsdam.de/ontology/SPASE-allowed_values.skos.owl#Circular"/>
    <skos:hasTopConcept rdf:resource="http://isdc.gfz-potsdam.de/ontology/SPASE-allowed_values.skos.owl#Magnitude"/>
    <skos:hasTopConcept rdf:resource="http://isdc.gfz-potsdam.de/ontology/SPASE-allowed_values.skos.owl#Array"/>
    <skos:hasTopConcept rdf:resource="http://isdc.gfz-potsdam.de/ontology/SPASE-allowed_values.skos.owl#Perturbation"/>
    <skos:hasTopConcept rdf:resource="http://isdc.gfz-potsdam.de/ontology/SPASE-allowed_values.skos.owl#Trace"/>
    <skos:hasTopConcept rdf:resource="http://isdc.gfz-potsdam.de/ontology/SPASE-allowed_values.skos.owl#Parallel"/>
    <skos:hasTopConcept rdf:resource="http://isdc.gfz-potsdam.de/ontology/SPASE-allowed_values.skos.owl#Peak"/>
    <skos:hasTopConcept rdf:resource="http://isdc.gfz-potsdam.de/ontology/SPASE-allowed_values.skos.owl#Minimum"/>
    <skos:prefLabel xml:lang="en">Qualifier</skos:prefLabel>
    <skos:hasTopConcept rdf:resource="http://isdc.gfz-potsdam.de/ontology/SPASE-allowed_values.skos.owl#Pseudo"/>
    <skos:hasTopConcept rdf:resource="http://isdc.gfz-potsdam.de/ontology/SPASE-allowed_values.skos.owl#Integral"/>
    <skos:hasTopConcept rdf:resource="http://isdc.gfz-potsdam.de/ontology/SPASE-allowed_values.skos.owl#Core"/>
    <skos:hasTopConcept rdf:resource="http://isdc.gfz-potsdam.de/ontology/SPASE-allowed_values.skos.owl#Phase"/>
    <skos:hasTopConcept rdf:resource="http://isdc.gfz-potsdam.de/ontology/SPASE-allowed_values.skos.owl#Column"/>
    <skos:hasTopConcept rdf:resource="http://isdc.gfz-potsdam.de/ontology/SPASE-allowed_values.skos.owl#Symmetric"/>
    <skos:hasTopConcept rdf:resource="http://isdc.gfz-potsdam.de/ontology/SPASE-allowed_values.skos.owl#Cross_Spectrum"/>
    <skos:hasTopConcept rdf:resource="http://isdc.gfz-potsdam.de/ontology/SPASE-allowed_values.skos.owl#Deviation"/>
    <skos:hasTopConcept rdf:resource="http://isdc.gfz-potsdam.de/ontology/SPASE-allowed_values.skos.owl#Strahl"/>
    <skos:hasTopConcept rdf:resource="http://isdc.gfz-potsdam.de/ontology/SPASE-allowed_values.skos.owl#Total"/>
    <skos:hasTopConcept rdf:resource="http://isdc.gfz-potsdam.de/ontology/SPASE-allowed_values.skos.owl#Differential"/>
    <skos:hasTopConcept rdf:resource="http://isdc.gfz-potsdam.de/ontology/SPASE-allowed_values.skos.owl#Characteristic"/>
    <skos:hasTopConcept rdf:resource="http://isdc.gfz-potsdam.de/ontology/SPASE-allowed_values.skos.owl#Directional"/>
    <skos:hasTopConcept rdf:resource="http://isdc.gfz-potsdam.de/ontology/SPASE-allowed_values.skos.owl#Tensor"/>
    <skos:hasTopConcept rdf:resource="http://isdc.gfz-potsdam.de/ontology/SPASE-allowed_values.skos.owl#Perpendicular"/>
    <skos:hasTopConcept rdf:resource="http://isdc.gfz-potsdam.de/ontology/SPASE-allowed_values.skos.owl#Fit"/>
    <skos:hasTopConcept rdf:resource="http://isdc.gfz-potsdam.de/ontology/SPASE-allowed_values.skos.owl#Anisotropy"/>
    <skos:hasTopConcept rdf:resource="http://isdc.gfz-potsdam.de/ontology/SPASE-allowed_values.skos.owl#Direction_Angle"/>
    <skos:hasTopConcept rdf:resource="http://isdc.gfz-potsdam.de/ontology/SPASE-allowed_values.skos.owl#Superhalo"/>
    <skos:hasTopConcept rdf:resource="http://isdc.gfz-potsdam.de/ontology/SPASE-allowed_values.skos.owl#Linear"/>
    <rdf:type rdf:resource="http://www.w3.org/2004/02/skos/core#ConceptScheme"/>
    <rdf:type rdf:resource="http://www.w3.org/2002/07/owl#NamedIndividual"/>
    <skos:hasTopConcept rdf:resource="http://isdc.gfz-potsdam.de/ontology/SPASE-allowed_values.skos.owl#Direction"/>
    <skos:hasTopConcept rdf:resource="http://isdc.gfz-potsdam.de/ontology/SPASE-allowed_values.skos.owl#Moment"/>
  </rdf:Description>
  <rdf:Description rdf:about="http://isdc.gfz-potsdam.de/ontology/SPASE-allowed_values.skos.owl#Scientist">
    <rdf:type rdf:resource="http://www.w3.org/2004/02/skos/core#Concept"/>
    <skos:definition xml:lang="en">An individual who is an expert in the phenomenon and related physics represented by the
resource.</skos:definition>
    <skos:topConceptOf rdf:resource="http://isdc.gfz-potsdam.de/ontology/SPASE-allowed_values.skos.owl#Role"/>
    <skos:inScheme rdf:resource="http://isdc.gfz-potsdam.de/ontology/SPASE-allowed_values.skos.owl#Role"/>
    <skos:prefLabel xml:lang="en">Scientist</skos:prefLabel>
    <rdf:type rdf:resource="http://www.w3.org/2002/07/owl#NamedIndividual"/>
  </rdf:Description>
  <rdf:Description rdf:about="http://isdc.gfz-potsdam.de/ontology/SPASE-allowed_values.skos.owl#Photographic_Plate">
    <rdf:type rdf:resource="http://www.w3.org/2004/02/skos/core#Concept"/>
    <rdf:type rdf:resource="http://www.w3.org/2002/07/owl#NamedIndividual"/>
    <skos:prefLabel xml:lang="en">Photographic Plate</skos:prefLabel>
    <skos:definition xml:lang="en">A rigid (typically glass) medium that functions like film. Its rigidity is for guarding against
image distortion due to medium deformation (caused by heat and humidity). Photographic
plates are often used for astronomical photography.</skos:definition>
    <skos:inScheme rdf:resource="http://isdc.gfz-potsdam.de/ontology/SPASE-allowed_values.skos.owl#Format"/>
    <skos:broader rdf:resource="http://isdc.gfz-potsdam.de/ontology/SPASE-allowed_values.skos.owl#Hardcopy"/>
  </rdf:Description>
  <rdf:Description rdf:about="http://isdc.gfz-potsdam.de/ontology/SPASE-allowed_values.skos.owl#Platform">
    <skos:inScheme rdf:resource="http://isdc.gfz-potsdam.de/ontology/SPASE-allowed_values.skos.owl#Instrument_Type"/>
    <rdf:type rdf:resource="http://www.w3.org/2004/02/skos/core#Concept"/>
    <rdf:type rdf:resource="http://www.w3.org/2002/07/owl#NamedIndividual"/>
    <skos:topConceptOf rdf:resource="http://isdc.gfz-potsdam.de/ontology/SPASE-allowed_values.skos.owl#Instrument_Type"/>
    <skos:definition xml:lang="en">A collection of components which can be positioned and oriented as a single unit. A platform
may contain other platforms. For example, a spacecraft is a platform which may have
components that can be articulated and are also considered platforms.</skos:definition>
    <skos:prefLabel xml:lang="en">Platform</skos:prefLabel>
  </rdf:Description>
  <rdf:Description rdf:about="http://isdc.gfz-potsdam.de/ontology/SPASE-allowed_values.skos.owl#Neptune">
    <skos:topConceptOf rdf:resource="http://isdc.gfz-potsdam.de/ontology/SPASE-allowed_values.skos.owl#Observatory_Region"/>
    <rdf:type rdf:resource="http://www.w3.org/2004/02/skos/core#Concept"/>
    <skos:prefLabel xml:lang="en">Neptune</skos:prefLabel>
    <skos:inScheme rdf:resource="http://isdc.gfz-potsdam.de/ontology/SPASE-allowed_values.skos.owl#Observed_Region"/>
    <rdf:type rdf:resource="http://www.w3.org/2002/07/owl#NamedIndividual"/>
    <skos:topConceptOf rdf:resource="http://isdc.gfz-potsdam.de/ontology/SPASE-allowed_values.skos.owl#Observed_Region"/>
    <skos:definition xml:lang="en">The seventh planet from the sun in our solar system.</skos:definition>
    <skos:inScheme rdf:resource="http://isdc.gfz-potsdam.de/ontology/SPASE-allowed_values.skos.owl#Observatory_Region"/>
  </rdf:Description>
  <rdf:Description rdf:about="http://isdc.gfz-potsdam.de/ontology/SPASE-allowed_values.skos.owl#Total_Pressure">
    <rdf:type rdf:resource="http://www.w3.org/2002/07/owl#NamedIndividual"/>
    <rdf:type rdf:resource="http://www.w3.org/2004/02/skos/core#Concept"/>
    <skos:prefLabel xml:lang="en">Total Pressure</skos:prefLabel>
    <skos:definition xml:lang="en">In an MHD fluid it is the number density (N) times Boltzmann constant times the temperature
in Kelvin.</skos:definition>
    <skos:topConceptOf rdf:resource="http://isdc.gfz-potsdam.de/ontology/SPASE-allowed_values.skos.owl#Mixed_Quantity"/>
    <skos:inScheme rdf:resource="http://isdc.gfz-potsdam.de/ontology/SPASE-allowed_values.skos.owl#Mixed_Quantity"/>
  </rdf:Description>
  <rdf:Description rdf:about="http://isdc.gfz-potsdam.de/ontology/SPASE-allowed_values.skos.owl#HDF_4">
    <skos:inScheme rdf:resource="http://isdc.gfz-potsdam.de/ontology/SPASE-allowed_values.skos.owl#Format"/>
    <rdf:type rdf:resource="http://www.w3.org/2004/02/skos/core#Concept"/>
    <rdf:type rdf:resource="http://www.w3.org/2002/07/owl#NamedIndividual"/>
    <skos:prefLabel xml:lang="en">HDF 4</skos:prefLabel>
    <skos:topConceptOf rdf:resource="http://isdc.gfz-potsdam.de/ontology/SPASE-allowed_values.skos.owl#Format"/>
    <skos:definition xml:lang="en">Hierarchical Data Format, Version 4</skos:definition>
  </rdf:Description>
  <rdf:Description rdf:about="http://isdc.gfz-potsdam.de/ontology/SPASE-allowed_values.skos.owl#Stack_Plot">
    <skos:prefLabel xml:lang="en">Stack Plot</skos:prefLabel>
    <skos:inScheme rdf:resource="http://isdc.gfz-potsdam.de/ontology/SPASE-allowed_values.skos.owl#Display_Type"/>
    <rdf:type rdf:resource="http://www.w3.org/2004/02/skos/core#Concept"/>
    <rdf:type rdf:resource="http://www.w3.org/2002/07/owl#NamedIndividual"/>
    <skos:topConceptOf rdf:resource="http://isdc.gfz-potsdam.de/ontology/SPASE-allowed_values.skos.owl#Display_Type"/>
    <skos:definition xml:lang="en">A representation of data showing multiple sets of observations on a single plot, possibly
offsetting each plot by some uniform amount.</skos:definition>
  </rdf:Description>
  <rdf:Description rdf:about="http://isdc.gfz-potsdam.de/ontology/SPASE-allowed_values.skos.owl#Uncalibrated">
    <rdf:type rdf:resource="http://www.w3.org/2002/07/owl#NamedIndividual"/>
    <skos:prefLabel xml:lang="en">Uncalibrated</skos:prefLabel>
    <skos:topConceptOf rdf:resource="http://isdc.gfz-potsdam.de/ontology/SPASE-allowed_values.skos.owl#Processing_Level"/>
    <skos:definition xml:lang="en">Duplicate data are removed from the data stream and data are time ordered. Values are not
adjusted for any potential biases or external factors.</skos:definition>
    <skos:inScheme rdf:resource="http://isdc.gfz-potsdam.de/ontology/SPASE-allowed_values.skos.owl#Processing_Level"/>
    <rdf:type rdf:resource="http://www.w3.org/2004/02/skos/core#Concept"/>
  </rdf:Description>
  <rdf:Description rdf:about="http://isdc.gfz-potsdam.de/ontology/SPASE-allowed_values.skos.owl#Time_Of_Flight">
    <skos:topConceptOf rdf:resource="http://isdc.gfz-potsdam.de/ontology/SPASE-allowed_values.skos.owl#Instrument_Type"/>
    <skos:definition xml:lang="en">An instrument which measures the time it takes for a particle to travel between two detectors.</skos:definition>
    <skos:inScheme rdf:resource="http://isdc.gfz-potsdam.de/ontology/SPASE-allowed_values.skos.owl#Instrument_Type"/>
    <skos:prefLabel xml:lang="en">Time Of Flight</skos:prefLabel>
    <rdf:type rdf:resource="http://www.w3.org/2002/07/owl#NamedIndividual"/>
    <rdf:type rdf:resource="http://www.w3.org/2004/02/skos/core#Concept"/>
  </rdf:Description>
  <rdf:Description rdf:about="http://isdc.gfz-potsdam.de/ontology/SPASE-allowed_values.skos.owl#Directional">
    <skos:topConceptOf rdf:resource="http://isdc.gfz-potsdam.de/ontology/SPASE-allowed_values.skos.owl#Qualifier"/>
    <skos:prefLabel xml:lang="en">Directional</skos:prefLabel>
    <skos:inScheme rdf:resource="http://isdc.gfz-potsdam.de/ontology/SPASE-allowed_values.skos.owl#Qualifier"/>
    <rdf:type rdf:resource="http://www.w3.org/2002/07/owl#NamedIndividual"/>
    <rdf:type rdf:resource="http://www.w3.org/2004/02/skos/core#Concept"/>
    <skos:definition xml:lang="en">A measurement within a narrow range of solid angle.</skos:definition>
  </rdf:Description>
  <rdf:Description rdf:about="http://isdc.gfz-potsdam.de/ontology/SPASE-allowed_values.skos.owl#Derived_From">
    <skos:definition xml:lang="en">A transformed or altered version of a resource instance.</skos:definition>
    <skos:inScheme rdf:resource="http://isdc.gfz-potsdam.de/ontology/SPASE-allowed_values.skos.owl#Association_Type"/>
    <skos:topConceptOf rdf:resource="http://isdc.gfz-potsdam.de/ontology/SPASE-allowed_values.skos.owl#Association_Type"/>
    <skos:prefLabel xml:lang="en">Derived From</skos:prefLabel>
    <rdf:type rdf:resource="http://www.w3.org/2004/02/skos/core#Concept"/>
    <rdf:type rdf:resource="http://www.w3.org/2002/07/owl#NamedIndividual"/>
  </rdf:Description>
  <rdf:Description rdf:about="http://isdc.gfz-potsdam.de/ontology/SPASE-allowed_values.skos.owl#Optical">
    <skos:prefLabel xml:lang="en">Optical</skos:prefLabel>
    <rdf:type rdf:resource="http://www.w3.org/2002/07/owl#NamedIndividual"/>
    <skos:inScheme rdf:resource="http://isdc.gfz-potsdam.de/ontology/SPASE-allowed_values.skos.owl#Spectral_Range"/>
    <skos:topConceptOf rdf:resource="http://isdc.gfz-potsdam.de/ontology/SPASE-allowed_values.skos.owl#Spectral_Range"/>
    <rdf:type rdf:resource="http://www.w3.org/2004/02/skos/core#Concept"/>
    <skos:altLabel xml:lang="en">Photons with a wavelength range: 380 to 760 nm.</skos:altLabel>
  </rdf:Description>
  <rdf:Description rdf:about="http://isdc.gfz-potsdam.de/ontology/SPASE-allowed_values.skos.owl#Proton">
    <skos:inScheme rdf:resource="http://isdc.gfz-potsdam.de/ontology/SPASE-allowed_values.skos.owl#Particle_Type"/>
    <skos:topConceptOf rdf:resource="http://isdc.gfz-potsdam.de/ontology/SPASE-allowed_values.skos.owl#Particle_Type"/>
    <skos:definition xml:lang="en">An elementary particle that is a constituent of all atomic nuclei, that carries a positive charge
numerically equal to the charge of an electron, and that has a mass of 1.673 x 10^(-24) gram.</skos:definition>
    <rdf:type rdf:resource="http://www.w3.org/2002/07/owl#NamedIndividual"/>
    <rdf:type rdf:resource="http://www.w3.org/2004/02/skos/core#Concept"/>
    <skos:prefLabel xml:lang="en">Proton</skos:prefLabel>
  </rdf:Description>
  <rdf:Description rdf:about="http://isdc.gfz-potsdam.de/ontology/SPASE-allowed_values.skos.owl#Magnetopause_Crossing">
    <rdf:type rdf:resource="http://www.w3.org/2002/07/owl#NamedIndividual"/>
    <rdf:type rdf:resource="http://www.w3.org/2004/02/skos/core#Concept"/>
    <skos:definition xml:lang="en">A crossing of the interface between the shocked solar wind in the magnetosheath and the
magnetic field and plasma in the magnetosphere.</skos:definition>
    <skos:prefLabel xml:lang="en">Magnetopause Crossing</skos:prefLabel>
    <skos:topConceptOf rdf:resource="http://isdc.gfz-potsdam.de/ontology/SPASE-allowed_values.skos.owl#Phenomenon_Type"/>
    <skos:inScheme rdf:resource="http://isdc.gfz-potsdam.de/ontology/SPASE-allowed_values.skos.owl#Phenomenon_Type"/>
  </rdf:Description>
  <rdf:Description rdf:about="http://isdc.gfz-potsdam.de/ontology/SPASE-allowed_values.skos.owl#Technical_Note">
    <skos:prefLabel xml:lang="en">Technical Note</skos:prefLabel>
    <skos:definition xml:lang="en">A document summarizing the performance and other technical characteristics of a product,
machine, component, subsystem or software in sufficient detail to be used by an engineer or
researcher.</skos:definition>
    <rdf:type rdf:resource="http://www.w3.org/2004/02/skos/core#Concept"/>
    <rdf:type rdf:resource="http://www.w3.org/2002/07/owl#NamedIndividual"/>
    <skos:topConceptOf rdf:resource="http://isdc.gfz-potsdam.de/ontology/SPASE-allowed_values.skos.owl#Document_Type"/>
    <skos:inScheme rdf:resource="http://isdc.gfz-potsdam.de/ontology/SPASE-allowed_values.skos.owl#Document_Type"/>
  </rdf:Description>
  <rdf:Description rdf:about="http://isdc.gfz-potsdam.de/ontology/SPASE-allowed_values.skos.owl#Absorption">
    <rdf:type rdf:resource="http://www.w3.org/2004/02/skos/core#Concept"/>
    <rdf:type rdf:resource="http://www.w3.org/2002/07/owl#NamedIndividual"/>
    <skos:prefLabel xml:lang="en">Absorption</skos:prefLabel>
    <skos:inScheme rdf:resource="http://isdc.gfz-potsdam.de/ontology/SPASE-allowed_values.skos.owl#Wave_Quantity"/>
    <skos:topConceptOf rdf:resource="http://isdc.gfz-potsdam.de/ontology/SPASE-allowed_values.skos.owl#Wave_Quantity"/>
    <skos:definition xml:lang="en">Decrease of radiant energy (relative to the background continuum spectrum).</skos:definition>
  </rdf:Description>
  <rdf:Description rdf:about="http://isdc.gfz-potsdam.de/ontology/SPASE-allowed_values.skos.owl#Earth">
    <skos:inScheme rdf:resource="http://isdc.gfz-potsdam.de/ontology/SPASE-allowed_values.skos.owl#Observed_Region"/>
    <rdf:type rdf:resource="http://www.w3.org/2004/02/skos/core#Concept"/>
    <skos:narrower rdf:resource="http://isdc.gfz-potsdam.de/ontology/SPASE-allowed_values.skos.owl#Near_Surface"/>
    <skos:narrower rdf:resource="http://isdc.gfz-potsdam.de/ontology/SPASE-allowed_values.skos.owl#Magnetosheath"/>
    <skos:narrower rdf:resource="http://isdc.gfz-potsdam.de/ontology/SPASE-allowed_values.skos.owl#Surface"/>
    <skos:prefLabel xml:lang="en">Earth</skos:prefLabel>
    <skos:inScheme rdf:resource="http://isdc.gfz-potsdam.de/ontology/SPASE-allowed_values.skos.owl#Observatory_Region"/>
    <rdf:type rdf:resource="http://www.w3.org/2002/07/owl#NamedIndividual"/>
    <skos:topConceptOf rdf:resource="http://isdc.gfz-potsdam.de/ontology/SPASE-allowed_values.skos.owl#Observed_Region"/>
    <skos:definition xml:lang="en">The third planet from the sun in our solar system.
Allowed Values:
Magnetosheath
Magnetosphere
Magnetosphere.Magnetotail
Magnetosphere.Main
Magnetosphere.Polar
Magnetosphere.Radiation Belt
Near Surface
Near Surface.Atmosphere
Near Surface.Auroral Region
Near Surface.Equatorial Region
Near Surface.Ionosphere
Near Surface.Ionosphere.D-Region
Near Surface.Ionosphere.E-Region
Near Surface.Ionosphere.F-Region
Near Surface.Ionosphere.Topside
Near Surface.Mesosphere
Near Surface.Plasmasphere
Near Surface.Polar Cap
Near Surface.South Atlantic Anomaly Region
Near Surface.Stratosphere
Near Surface.Thermosphere
Near Surface.Troposphere
Surface</skos:definition>
    <skos:topConceptOf rdf:resource="http://isdc.gfz-potsdam.de/ontology/SPASE-allowed_values.skos.owl#Observatory_Region"/>
    <skos:narrower rdf:resource="http://isdc.gfz-potsdam.de/ontology/SPASE-allowed_values.skos.owl#Magnetosphere"/>
  </rdf:Description>
  <rdf:Description rdf:about="http://isdc.gfz-potsdam.de/ontology/SPASE-allowed_values.skos.owl#Linear_Scale">
    <rdf:type rdf:resource="http://www.w3.org/2002/07/owl#NamedIndividual"/>
    <skos:prefLabel xml:lang="en">Linear Scale</skos:prefLabel>
    <skos:inScheme rdf:resource="http://isdc.gfz-potsdam.de/ontology/SPASE-allowed_values.skos.owl#Scale_Type"/>
    <skos:topConceptOf rdf:resource="http://isdc.gfz-potsdam.de/ontology/SPASE-allowed_values.skos.owl#Scale_Type"/>
    <skos:definition xml:lang="en">Intervals which are equally spaced.</skos:definition>
    <rdf:type rdf:resource="http://www.w3.org/2004/02/skos/core#Concept"/>
  </rdf:Description>
  <rdf:Description rdf:about="http://isdc.gfz-potsdam.de/ontology/SPASE-allowed_values.skos.owl#Ratio">
    <skos:topConceptOf rdf:resource="http://isdc.gfz-potsdam.de/ontology/SPASE-allowed_values.skos.owl#Qualifier"/>
    <skos:prefLabel xml:lang="en">Ratio</skos:prefLabel>
    <skos:altLabel xml:lang="en">The relative magnitudes of two quantities.</skos:altLabel>
    <skos:inScheme rdf:resource="http://isdc.gfz-potsdam.de/ontology/SPASE-allowed_values.skos.owl#Qualifier"/>
    <rdf:type rdf:resource="http://www.w3.org/2002/07/owl#NamedIndividual"/>
    <rdf:type rdf:resource="http://www.w3.org/2004/02/skos/core#Concept"/>
  </rdf:Description>
  <rdf:Description rdf:about="http://isdc.gfz-potsdam.de/ontology/SPASE-allowed_values.skos.owl#Magnitude">
    <skos:topConceptOf rdf:resource="http://isdc.gfz-potsdam.de/ontology/SPASE-allowed_values.skos.owl#Qualifier"/>
    <rdf:type rdf:resource="http://www.w3.org/2004/02/skos/core#Concept"/>
    <skos:inScheme rdf:resource="http://isdc.gfz-potsdam.de/ontology/SPASE-allowed_values.skos.owl#Qualifier"/>
    <skos:prefLabel xml:lang="en">Magnitude</skos:prefLabel>
    <rdf:type rdf:resource="http://www.w3.org/2002/07/owl#NamedIndividual"/>
    <skos:definition xml:lang="en">A measure of the strength of a vector quantity or length of its representational vector.</skos:definition>
  </rdf:Description>
  <rdf:Description rdf:about="http://isdc.gfz-potsdam.de/ontology/SPASE-allowed_values.skos.owl#PNG">
    <rdf:type rdf:resource="http://www.w3.org/2002/07/owl#NamedIndividual"/>
    <rdf:type rdf:resource="http://www.w3.org/2004/02/skos/core#Concept"/>
    <skos:topConceptOf rdf:resource="http://isdc.gfz-potsdam.de/ontology/SPASE-allowed_values.skos.owl#Format"/>
    <skos:definition xml:lang="en">A digital format for still images. Portable Network Graphics (PNG).</skos:definition>
    <skos:prefLabel xml:lang="en">PNG</skos:prefLabel>
    <skos:inScheme rdf:resource="http://isdc.gfz-potsdam.de/ontology/SPASE-allowed_values.skos.owl#Format"/>
  </rdf:Description>
  <rdf:Description rdf:about="http://isdc.gfz-potsdam.de/ontology/SPASE-allowed_values.skos.owl#Saturn">
    <skos:definition xml:lang="en">The sixth planet from the sun in our solar system.</skos:definition>
    <skos:topConceptOf rdf:resource="http://isdc.gfz-potsdam.de/ontology/SPASE-allowed_values.skos.owl#Observed_Region"/>
    <rdf:type rdf:resource="http://www.w3.org/2004/02/skos/core#Concept"/>
    <rdf:type rdf:resource="http://www.w3.org/2002/07/owl#NamedIndividual"/>
    <skos:prefLabel xml:lang="en">Saturn</skos:prefLabel>
    <skos:inScheme rdf:resource="http://isdc.gfz-potsdam.de/ontology/SPASE-allowed_values.skos.owl#Observatory_Region"/>
    <skos:topConceptOf rdf:resource="http://isdc.gfz-potsdam.de/ontology/SPASE-allowed_values.skos.owl#Observatory_Region"/>
    <skos:inScheme rdf:resource="http://isdc.gfz-potsdam.de/ontology/SPASE-allowed_values.skos.owl#Observed_Region"/>
  </rdf:Description>
  <rdf:Description rdf:about="http://isdc.gfz-potsdam.de/ontology/SPASE-allowed_values.skos.owl#Strahl">
    <skos:inScheme rdf:resource="http://isdc.gfz-potsdam.de/ontology/SPASE-allowed_values.skos.owl#Qualifier"/>
    <rdf:type rdf:resource="http://www.w3.org/2004/02/skos/core#Concept"/>
    <rdf:type rdf:resource="http://www.w3.org/2002/07/owl#NamedIndividual"/>
    <skos:prefLabel xml:lang="en">Strahl</skos:prefLabel>
    <skos:topConceptOf rdf:resource="http://isdc.gfz-potsdam.de/ontology/SPASE-allowed_values.skos.owl#Qualifier"/>
    <skos:definition xml:lang="en">A distribution of particles concentrated in a narrow energy band. The band may be may be
aligned with a secondary feature. For example, it may occur in a narrow cone aligned with the
mean magnetic field direction.</skos:definition>
  </rdf:Description>
  <rdf:Description rdf:about="http://isdc.gfz-potsdam.de/ontology/SPASE-allowed_values.skos.owl#SQ_Other">
    <skos:definition xml:lang="en">Not classified with more specific terms. The context of its usage may be described in related
text.</skos:definition>
    <skos:topConceptOf rdf:resource="http://isdc.gfz-potsdam.de/ontology/SPASE-allowed_values.skos.owl#Mixed_Quantity"/>
    <skos:inScheme rdf:resource="http://isdc.gfz-potsdam.de/ontology/SPASE-allowed_values.skos.owl#Association_Type"/>
    <rdf:type rdf:resource="http://www.w3.org/2004/02/skos/core#Concept"/>
    <skos:inScheme rdf:resource="http://isdc.gfz-potsdam.de/ontology/SPASE-allowed_values.skos.owl#Document_Type"/>
    <skos:topConceptOf rdf:resource="http://isdc.gfz-potsdam.de/ontology/SPASE-allowed_values.skos.owl#Support_Quantity"/>
    <skos:topConceptOf rdf:resource="http://isdc.gfz-potsdam.de/ontology/SPASE-allowed_values.skos.owl#Document_Type"/>
    <skos:inScheme rdf:resource="http://isdc.gfz-potsdam.de/ontology/SPASE-allowed_values.skos.owl#Mixed_Quantity"/>
    <rdf:type rdf:resource="http://www.w3.org/2002/07/owl#NamedIndividual"/>
    <skos:prefLabel xml:lang="en">Other</skos:prefLabel>
    <skos:topConceptOf rdf:resource="http://isdc.gfz-potsdam.de/ontology/SPASE-allowed_values.skos.owl#Association_Type"/>
    <skos:inScheme rdf:resource="http://isdc.gfz-potsdam.de/ontology/SPASE-allowed_values.skos.owl#Support_Quantity"/>
  </rdf:Description>
  <rdf:Description rdf:about="http://isdc.gfz-potsdam.de/ontology/SPASE-allowed_values.skos.owl#Mode_Amplitude">
    <skos:prefLabel xml:lang="en">Mode Amplitude</skos:prefLabel>
    <rdf:type rdf:resource="http://www.w3.org/2004/02/skos/core#Concept"/>
    <rdf:type rdf:resource="http://www.w3.org/2002/07/owl#NamedIndividual"/>
    <skos:inScheme rdf:resource="http://isdc.gfz-potsdam.de/ontology/SPASE-allowed_values.skos.owl#Wave_Quantity"/>
    <skos:topConceptOf rdf:resource="http://isdc.gfz-potsdam.de/ontology/SPASE-allowed_values.skos.owl#Wave_Quantity"/>
    <skos:definition xml:lang="en">In helioseismology the magnitude of oscillation of waves of a particular geometry.</skos:definition>
  </rdf:Description>
  <rdf:Description rdf:about="http://isdc.gfz-potsdam.de/ontology/SPASE-allowed_values.skos.owl#Spacecraft_Orbit_Plane">
    <skos:inScheme rdf:resource="http://isdc.gfz-potsdam.de/ontology/SPASE-allowed_values.skos.owl#Coordinate_System_Name"/>
    <rdf:type rdf:resource="http://www.w3.org/2002/07/owl#NamedIndividual"/>
    <skos:topConceptOf rdf:resource="http://isdc.gfz-potsdam.de/ontology/SPASE-allowed_values.skos.owl#Coordinate_System_Name"/>
    <skos:definition xml:lang="en">A coordinate system where X lies in the plane normal to and in the direction of motion of the
spacecraft, Z is normal to this plane and Y completes the triad in a right-handed coordinate
system.</skos:definition>
    <skos:prefLabel xml:lang="en">Spacecraft Orbit Plane</skos:prefLabel>
    <rdf:type rdf:resource="http://www.w3.org/2004/02/skos/core#Concept"/>
  </rdf:Description>
  <rdf:Description rdf:about="http://isdc.gfz-potsdam.de/ontology/SPASE-allowed_values.skos.owl#Symmetric">
    <skos:prefLabel xml:lang="en">Symmetric</skos:prefLabel>
    <skos:topConceptOf rdf:resource="http://isdc.gfz-potsdam.de/ontology/SPASE-allowed_values.skos.owl#Qualifier"/>
    <skos:altLabel xml:lang="en">Equal distribution about one or more axes.</skos:altLabel>
    <skos:inScheme rdf:resource="http://isdc.gfz-potsdam.de/ontology/SPASE-allowed_values.skos.owl#Qualifier"/>
    <rdf:type rdf:resource="http://www.w3.org/2004/02/skos/core#Concept"/>
    <rdf:type rdf:resource="http://www.w3.org/2002/07/owl#NamedIndividual"/>
  </rdf:Description>
  <rdf:Description rdf:about="http://isdc.gfz-potsdam.de/ontology/SPASE-allowed_values.skos.owl#Comet">
    <skos:topConceptOf rdf:resource="http://isdc.gfz-potsdam.de/ontology/SPASE-allowed_values.skos.owl#Observed_Region"/>
    <skos:definition xml:lang="en">A relatively small extraterrestrial body consisting of a frozen mass that travels around the sun in
a highly elliptical orbit.</skos:definition>
    <skos:inScheme rdf:resource="http://isdc.gfz-potsdam.de/ontology/SPASE-allowed_values.skos.owl#Observed_Region"/>
    <skos:topConceptOf rdf:resource="http://isdc.gfz-potsdam.de/ontology/SPASE-allowed_values.skos.owl#Observatory_Region"/>
    <skos:inScheme rdf:resource="http://isdc.gfz-potsdam.de/ontology/SPASE-allowed_values.skos.owl#Observatory_Region"/>
    <skos:prefLabel xml:lang="en">Comet</skos:prefLabel>
    <rdf:type rdf:resource="http://www.w3.org/2002/07/owl#NamedIndividual"/>
    <rdf:type rdf:resource="http://www.w3.org/2004/02/skos/core#Concept"/>
  </rdf:Description>
  <rdf:Description rdf:about="http://isdc.gfz-potsdam.de/ontology/SPASE-allowed_values.skos.owl#MATLAB_7">
    <skos:definition xml:lang="en">MATLAB Workspace save set, version 7. MAT-files are double-precision, binary, MATLAB
format files. Version 7 includes data compression and Unicode encoding. MATLAB is a
proprietary product of The MathWorks.</skos:definition>
    <skos:inScheme rdf:resource="http://isdc.gfz-potsdam.de/ontology/SPASE-allowed_values.skos.owl#Format"/>
    <skos:topConceptOf rdf:resource="http://isdc.gfz-potsdam.de/ontology/SPASE-allowed_values.skos.owl#Format"/>
    <rdf:type rdf:resource="http://www.w3.org/2002/07/owl#NamedIndividual"/>
    <rdf:type rdf:resource="http://www.w3.org/2004/02/skos/core#Concept"/>
    <skos:prefLabel xml:lang="en">MATLAB_7</skos:prefLabel>
  </rdf:Description>
  <rdf:Description rdf:about="http://isdc.gfz-potsdam.de/ontology/SPASE-allowed_values.skos.owl#FITS">
    <skos:definition xml:lang="en">Flexible Image Transport System (FITS) is a digital format primarily designed to store
scientific data sets consisting of multi-dimensional arrays (1-D spectra, 2-D images or 3-D data
cubes) and 2-dimensional tables containing rows and columns of data.</skos:definition>
    <skos:inScheme rdf:resource="http://isdc.gfz-potsdam.de/ontology/SPASE-allowed_values.skos.owl#Format"/>
    <rdf:type rdf:resource="http://www.w3.org/2004/02/skos/core#Concept"/>
    <rdf:type rdf:resource="http://www.w3.org/2002/07/owl#NamedIndividual"/>
    <skos:topConceptOf rdf:resource="http://isdc.gfz-potsdam.de/ontology/SPASE-allowed_values.skos.owl#Format"/>
    <skos:prefLabel xml:lang="en">FITS</skos:prefLabel>
  </rdf:Description>
  <rdf:Description rdf:about="http://isdc.gfz-potsdam.de/ontology/SPASE-allowed_values.skos.owl#GSM">
    <skos:prefLabel xml:lang="en">GSM</skos:prefLabel>
    <skos:definition xml:lang="en">Geocentric Solar Magnetospheric - A coordinate system where the X axis is from Earth to Sun,
Z axis is northward in a plane containing the X axis and the geomagnetic dipole axis. See
Russell, 1971.</skos:definition>
    <skos:inScheme rdf:resource="http://isdc.gfz-potsdam.de/ontology/SPASE-allowed_values.skos.owl#Coordinate_System_Name"/>
    <rdf:type rdf:resource="http://www.w3.org/2004/02/skos/core#Concept"/>
    <rdf:type rdf:resource="http://www.w3.org/2002/07/owl#NamedIndividual"/>
    <skos:topConceptOf rdf:resource="http://isdc.gfz-potsdam.de/ontology/SPASE-allowed_values.skos.owl#Coordinate_System_Name"/>
  </rdf:Description>
  <rdf:Description rdf:about="http://isdc.gfz-potsdam.de/ontology/SPASE-allowed_values.skos.owl#Presentation">
    <skos:topConceptOf rdf:resource="http://isdc.gfz-potsdam.de/ontology/SPASE-allowed_values.skos.owl#Document_Type"/>
    <skos:inScheme rdf:resource="http://isdc.gfz-potsdam.de/ontology/SPASE-allowed_values.skos.owl#Document_Type"/>
    <skos:definition xml:lang="en">A set of information that is used when communicating to an audience.</skos:definition>
    <skos:prefLabel xml:lang="en">Presentation</skos:prefLabel>
    <rdf:type rdf:resource="http://www.w3.org/2002/07/owl#NamedIndividual"/>
    <rdf:type rdf:resource="http://www.w3.org/2004/02/skos/core#Concept"/>
  </rdf:Description>
  <rdf:Description rdf:about="http://isdc.gfz-potsdam.de/ontology/SPASE-allowed_values.skos.owl#Photopolarimeter">
    <skos:topConceptOf rdf:resource="http://isdc.gfz-potsdam.de/ontology/SPASE-allowed_values.skos.owl#Instrument_Type"/>
    <skos:definition xml:lang="en">An instrument which measures the intensity and polarization or radiant energy. A
photopolarimeter is a combination of a photometer and a polarimeter.</skos:definition>
    <rdf:type rdf:resource="http://www.w3.org/2004/02/skos/core#Concept"/>
    <rdf:type rdf:resource="http://www.w3.org/2002/07/owl#NamedIndividual"/>
    <skos:prefLabel xml:lang="en">Photopolarimeter</skos:prefLabel>
    <skos:inScheme rdf:resource="http://isdc.gfz-potsdam.de/ontology/SPASE-allowed_values.skos.owl#Instrument_Type"/>
  </rdf:Description>
  <rdf:Description rdf:about="http://isdc.gfz-potsdam.de/ontology/SPASE-allowed_values.skos.owl#Event">
    <rdf:type rdf:resource="http://www.w3.org/2002/07/owl#NamedIndividual"/>
    <skos:inScheme rdf:resource="http://isdc.gfz-potsdam.de/ontology/SPASE-allowed_values.skos.owl#Annotation_Type"/>
    <skos:definition xml:lang="en">An action or observation which occurs at a point in time.</skos:definition>
    <skos:topConceptOf rdf:resource="http://isdc.gfz-potsdam.de/ontology/SPASE-allowed_values.skos.owl#Annotation_Type"/>
    <skos:prefLabel xml:lang="en">Event</skos:prefLabel>
    <rdf:type rdf:resource="http://www.w3.org/2004/02/skos/core#Concept"/>
  </rdf:Description>
  <rdf:Description rdf:about="http://isdc.gfz-potsdam.de/ontology/SPASE-allowed_values.skos.owl#Profile">
    <skos:prefLabel xml:lang="en">Profile</skos:prefLabel>
    <rdf:type rdf:resource="http://www.w3.org/2002/07/owl#NamedIndividual"/>
    <rdf:type rdf:resource="http://www.w3.org/2004/02/skos/core#Concept"/>
    <skos:topConceptOf rdf:resource="http://isdc.gfz-potsdam.de/ontology/SPASE-allowed_values.skos.owl#Measurement_Type"/>
    <skos:inScheme rdf:resource="http://isdc.gfz-potsdam.de/ontology/SPASE-allowed_values.skos.owl#Measurement_Type"/>
    <skos:definition xml:lang="en">Measurements of a quantity as a function of height above an object such as the limb of a body.</skos:definition>
  </rdf:Description>
  <rdf:Description rdf:about="http://isdc.gfz-potsdam.de/ontology/SPASE-allowed_values.skos.owl#Na-D">
    <skos:topConceptOf rdf:resource="http://isdc.gfz-potsdam.de/ontology/SPASE-allowed_values.skos.owl#Spectral_Range"/>
    <rdf:type rdf:resource="http://www.w3.org/2002/07/owl#NamedIndividual"/>
    <rdf:type rdf:resource="http://www.w3.org/2004/02/skos/core#Concept"/>
    <skos:prefLabel xml:lang="en">Na-D</skos:prefLabel>
    <skos:definition xml:lang="en">A spectrum with a wavelength range of centered at 589.3 nm. VSO nickname: Na-D image
with a range of 588.8 nm to 589.8 nm.</skos:definition>
    <skos:inScheme rdf:resource="http://isdc.gfz-potsdam.de/ontology/SPASE-allowed_values.skos.owl#Spectral_Range"/>
  </rdf:Description>
  <rdf:Description rdf:about="http://isdc.gfz-potsdam.de/ontology/SPASE-allowed_values.skos.owl#XML">
    <skos:definition xml:lang="en">eXtensible Mark-up Language (XML). A structured format for representing information. See
&lt;http://www.w3.org/XML/&gt;.</skos:definition>
    <skos:topConceptOf rdf:resource="http://isdc.gfz-potsdam.de/ontology/SPASE-allowed_values.skos.owl#Format"/>
    <rdf:type rdf:resource="http://www.w3.org/2004/02/skos/core#Concept"/>
    <rdf:type rdf:resource="http://www.w3.org/2002/07/owl#NamedIndividual"/>
    <skos:inScheme rdf:resource="http://isdc.gfz-potsdam.de/ontology/SPASE-allowed_values.skos.owl#Format"/>
    <skos:prefLabel xml:lang="en">XML</skos:prefLabel>
  </rdf:Description>
  <rdf:Description rdf:about="http://isdc.gfz-potsdam.de/ontology/SPASE-allowed_values.skos.owl#Propagation_Time">
    <skos:prefLabel xml:lang="en">Propagation Time</skos:prefLabel>
    <skos:inScheme rdf:resource="http://isdc.gfz-potsdam.de/ontology/SPASE-allowed_values.skos.owl#Wave_Quantity"/>
    <skos:definition xml:lang="en">Time difference between transmission and reception of a wave in an active wave experiment.</skos:definition>
    <rdf:type rdf:resource="http://www.w3.org/2002/07/owl#NamedIndividual"/>
    <rdf:type rdf:resource="http://www.w3.org/2004/02/skos/core#Concept"/>
    <skos:topConceptOf rdf:resource="http://isdc.gfz-potsdam.de/ontology/SPASE-allowed_values.skos.owl#Wave_Quantity"/>
  </rdf:Description>
  <rdf:Description rdf:about="http://isdc.gfz-potsdam.de/ontology/SPASE-allowed_values.skos.owl#Magnetosphere">
    <rdf:type rdf:resource="http://www.w3.org/2004/02/skos/core#Concept"/>
    <skos:definition xml:lang="en">The region of space above the atmosphere or surface of the planet, and bounded by the
magnetopause, that is under the direct influence of the planet's magnetic field.
Allowed Values:
Magnetotail
Main
Polar
Radiation Belt</skos:definition>
    <skos:narrower rdf:resource="http://isdc.gfz-potsdam.de/ontology/SPASE-allowed_values.skos.owl#Polar"/>
    <skos:narrower rdf:resource="http://isdc.gfz-potsdam.de/ontology/SPASE-allowed_values.skos.owl#Main"/>
    <skos:broader rdf:resource="http://isdc.gfz-potsdam.de/ontology/SPASE-allowed_values.skos.owl#Earth"/>
    <skos:inScheme rdf:resource="http://isdc.gfz-potsdam.de/ontology/SPASE-allowed_values.skos.owl#Observed_Region"/>
    <skos:prefLabel xml:lang="en">Magnetosphere</skos:prefLabel>
    <skos:narrower rdf:resource="http://isdc.gfz-potsdam.de/ontology/SPASE-allowed_values.skos.owl#Radiation_Belt"/>
    <skos:narrower rdf:resource="http://isdc.gfz-potsdam.de/ontology/SPASE-allowed_values.skos.owl#Magnetotail"/>
    <skos:inScheme rdf:resource="http://isdc.gfz-potsdam.de/ontology/SPASE-allowed_values.skos.owl#Observatory_Region"/>
    <rdf:type rdf:resource="http://www.w3.org/2002/07/owl#NamedIndividual"/>
  </rdf:Description>
  <rdf:Description rdf:about="http://isdc.gfz-potsdam.de/ontology/SPASE-allowed_values.skos.owl#Classification_Method">
    <skos:prefLabel xml:lang="en">Classification Method</skos:prefLabel>
    <skos:definition xml:lang="en">The technique used to determine the characteristics of an object.
Allowed Values:
Automatic
Inferred
Inspection</skos:definition>
    <skos:hasTopConcept rdf:resource="http://isdc.gfz-potsdam.de/ontology/SPASE-allowed_values.skos.owl#Inspection"/>
    <rdf:type rdf:resource="http://www.w3.org/2004/02/skos/core#ConceptScheme"/>
    <rdf:type rdf:resource="http://www.w3.org/2002/07/owl#NamedIndividual"/>
    <skos:hasTopConcept rdf:resource="http://isdc.gfz-potsdam.de/ontology/SPASE-allowed_values.skos.owl#Automatic"/>
    <skos:hasTopConcept rdf:resource="http://isdc.gfz-potsdam.de/ontology/SPASE-allowed_values.skos.owl#Inferred"/>
  </rdf:Description>
  <rdf:Description rdf:about="http://isdc.gfz-potsdam.de/ontology/SPASE-allowed_values.skos.owl#HCI">
    <rdf:type rdf:resource="http://www.w3.org/2004/02/skos/core#Concept"/>
    <rdf:type rdf:resource="http://www.w3.org/2002/07/owl#NamedIndividual"/>
    <skos:definition xml:lang="en">Heliographic Carrington Inertial.</skos:definition>
    <skos:topConceptOf rdf:resource="http://isdc.gfz-potsdam.de/ontology/SPASE-allowed_values.skos.owl#Coordinate_System_Name"/>
    <skos:prefLabel xml:lang="en">HCI</skos:prefLabel>
    <skos:inScheme rdf:resource="http://isdc.gfz-potsdam.de/ontology/SPASE-allowed_values.skos.owl#Coordinate_System_Name"/>
  </rdf:Description>
  <rdf:Description rdf:about="http://isdc.gfz-potsdam.de/ontology/SPASE-allowed_values.skos.owl#Observed_Region">
    <skos:prefLabel xml:lang="en">Observed Region</skos:prefLabel>
    <skos:hasTopConcept rdf:resource="http://isdc.gfz-potsdam.de/ontology/SPASE-allowed_values.skos.owl#Saturn"/>
    <rdf:type rdf:resource="http://www.w3.org/2002/07/owl#NamedIndividual"/>
    <skos:hasTopConcept rdf:resource="http://isdc.gfz-potsdam.de/ontology/SPASE-allowed_values.skos.owl#Heliosphere"/>
    <skos:hasTopConcept rdf:resource="http://isdc.gfz-potsdam.de/ontology/SPASE-allowed_values.skos.owl#Pluto"/>
    <skos:hasTopConcept rdf:resource="http://isdc.gfz-potsdam.de/ontology/SPASE-allowed_values.skos.owl#Interstellar"/>
    <skos:hasTopConcept rdf:resource="http://isdc.gfz-potsdam.de/ontology/SPASE-allowed_values.skos.owl#Neptune"/>
    <skos:hasTopConcept rdf:resource="http://isdc.gfz-potsdam.de/ontology/SPASE-allowed_values.skos.owl#Earth"/>
    <skos:hasTopConcept rdf:resource="http://isdc.gfz-potsdam.de/ontology/SPASE-allowed_values.skos.owl#Venus"/>
    <skos:hasTopConcept rdf:resource="http://isdc.gfz-potsdam.de/ontology/SPASE-allowed_values.skos.owl#Jupiter"/>
    <rdf:type rdf:resource="http://www.w3.org/2004/02/skos/core#ConceptScheme"/>
    <skos:hasTopConcept rdf:resource="http://isdc.gfz-potsdam.de/ontology/SPASE-allowed_values.skos.owl#Uranus"/>
    <skos:definition xml:lang="en">The portion of space measured by the instrument at the time of an observation. A region is
distinguished by certain natural features or physical characteristics. It is the location of the
observatory for in situ data, the location or region sensed by remote sensing observatories and
the location-of-relevance for parameters that are derived from observational data.
Allowed Values:
Asteroid
Comet
Earth
Earth.Magnetosheath
Earth.Magnetosphere
Earth.Magnetosphere.Magnetotail
Earth.Magnetosphere.Main
Earth.Magnetosphere.Polar
Earth.Magnetosphere.Radiation Belt
Earth.Near Surface
Earth.Near Surface.Atmosphere
Earth.Near Surface.Auroral Region
Earth.Near Surface.Equatorial Region
Earth.Near Surface.Ionosphere
Earth.Near Surface.Ionosphere.D-Region
Earth.Near Surface.Ionosphere.E-Region
Earth.Near Surface.Ionosphere.F-Region
Earth.Near Surface.Ionosphere.Topside
Earth.Near Surface.Mesosphere
Earth.Near Surface.Plasmasphere
Earth.Near Surface.Polar Cap
Earth.Near Surface.South Atlantic Anomaly Region
Earth.Near Surface.Stratosphere
Earth.Near Surface.Thermosphere
Earth.Near Surface.Troposphere
Earth.Surface
Heliosphere
Heliosphere.Heliosheath
Heliosphere.Inner
Heliosphere.Near Earth
Heliosphere.Outer
Heliosphere.Remote 1AU
Interstellar
Jupiter
Mars
Mercury
Neptune
Pluto
Saturn
Sun
Sun.Chromosphere
Sun.Corona
Sun.Interior
Sun.Photosphere
Sun.Transition Region
Uranus
Venus</skos:definition>
    <skos:hasTopConcept rdf:resource="http://isdc.gfz-potsdam.de/ontology/SPASE-allowed_values.skos.owl#Sun"/>
    <skos:hasTopConcept rdf:resource="http://isdc.gfz-potsdam.de/ontology/SPASE-allowed_values.skos.owl#Comet"/>
    <skos:hasTopConcept rdf:resource="http://isdc.gfz-potsdam.de/ontology/SPASE-allowed_values.skos.owl#Mars"/>
    <skos:hasTopConcept rdf:resource="http://isdc.gfz-potsdam.de/ontology/SPASE-allowed_values.skos.owl#Asteroid"/>
    <skos:hasTopConcept rdf:resource="http://isdc.gfz-potsdam.de/ontology/SPASE-allowed_values.skos.owl#Mercury"/>
  </rdf:Description>
  <rdf:Description rdf:about="http://isdc.gfz-potsdam.de/ontology/SPASE-allowed_values.skos.owl#Soft_X-Rays">
    <skos:inScheme rdf:resource="http://isdc.gfz-potsdam.de/ontology/SPASE-allowed_values.skos.owl#Spectral_Range"/>
    <rdf:type rdf:resource="http://www.w3.org/2002/07/owl#NamedIndividual"/>
    <rdf:type rdf:resource="http://www.w3.org/2004/02/skos/core#Concept"/>
    <skos:topConceptOf rdf:resource="http://isdc.gfz-potsdam.de/ontology/SPASE-allowed_values.skos.owl#Spectral_Range"/>
    <skos:prefLabel xml:lang="en">Soft X-Rays</skos:prefLabel>
    <skos:definition xml:lang="en">X-Rays with an energy range of 0.12 keV to 12 keV.</skos:definition>
  </rdf:Description>
  <rdf:Description rdf:about="http://isdc.gfz-potsdam.de/ontology/SPASE-allowed_values.skos.owl#Atmosphere">
    <skos:broader rdf:resource="http://isdc.gfz-potsdam.de/ontology/SPASE-allowed_values.skos.owl#Near_Surface"/>
    <skos:inScheme rdf:resource="http://isdc.gfz-potsdam.de/ontology/SPASE-allowed_values.skos.owl#Observed_Region"/>
    <skos:definition xml:lang="en">The neutral gases surrounding a body that extends from the surface and is bound to the body by
virtue of the gravitational attraction.</skos:definition>
    <skos:inScheme rdf:resource="http://isdc.gfz-potsdam.de/ontology/SPASE-allowed_values.skos.owl#Observatory_Region"/>
    <rdf:type rdf:resource="http://www.w3.org/2002/07/owl#NamedIndividual"/>
    <rdf:type rdf:resource="http://www.w3.org/2004/02/skos/core#Concept"/>
    <skos:prefLabel xml:lang="en">Atmosphere</skos:prefLabel>
  </rdf:Description>
  <rdf:Description rdf:about="http://isdc.gfz-potsdam.de/ontology/SPASE-allowed_values.skos.owl#Direction">
    <skos:prefLabel xml:lang="en">Direction</skos:prefLabel>
    <rdf:type rdf:resource="http://www.w3.org/2004/02/skos/core#Concept"/>
    <rdf:type rdf:resource="http://www.w3.org/2002/07/owl#NamedIndividual"/>
    <skos:definition xml:lang="en">The spatial relation between an object and another object, the orientation of the object or the
course along which the object points or moves.</skos:definition>
    <skos:inScheme rdf:resource="http://isdc.gfz-potsdam.de/ontology/SPASE-allowed_values.skos.owl#Qualifier"/>
    <skos:topConceptOf rdf:resource="http://isdc.gfz-potsdam.de/ontology/SPASE-allowed_values.skos.owl#Qualifier"/>
  </rdf:Description>
  <rdf:Description rdf:about="http://isdc.gfz-potsdam.de/ontology/SPASE-allowed_values.skos.owl#Potential">
    <rdf:type rdf:resource="http://www.w3.org/2002/07/owl#NamedIndividual"/>
    <rdf:type rdf:resource="http://www.w3.org/2004/02/skos/core#Concept"/>
    <skos:definition xml:lang="en">A field which obeys Laplace's Equation.</skos:definition>
    <skos:topConceptOf rdf:resource="http://isdc.gfz-potsdam.de/ontology/SPASE-allowed_values.skos.owl#Field_Quantity"/>
    <skos:prefLabel xml:lang="en">Potential</skos:prefLabel>
    <skos:inScheme rdf:resource="http://isdc.gfz-potsdam.de/ontology/SPASE-allowed_values.skos.owl#Field_Quantity"/>
  </rdf:Description>
  <rdf:Description rdf:about="http://isdc.gfz-potsdam.de/ontology/SPASE-allowed_values.skos.owl#DM">
    <skos:inScheme rdf:resource="http://isdc.gfz-potsdam.de/ontology/SPASE-allowed_values.skos.owl#Coordinate_System_Name"/>
    <skos:prefLabel xml:lang="en">DM</skos:prefLabel>
    <rdf:type rdf:resource="http://www.w3.org/2004/02/skos/core#Concept"/>
    <rdf:type rdf:resource="http://www.w3.org/2002/07/owl#NamedIndividual"/>
    <skos:topConceptOf rdf:resource="http://isdc.gfz-potsdam.de/ontology/SPASE-allowed_values.skos.owl#Coordinate_System_Name"/>
    <skos:definition xml:lang="en">Dipole Meridian - A coordinate system centered at the observation point. Z axis is parallel to
the Earth's dipole axis, positive northward. X is in the plane defined by Z and the line linking
the observation point with the Earth's center. Y is positive eastward. See
&lt;http://cdpp.cnes.fr/00428.pdf&gt;</skos:definition>
  </rdf:Description>
  <rdf:Description rdf:about="http://isdc.gfz-potsdam.de/ontology/SPASE-allowed_values.skos.owl#Venus">
    <skos:inScheme rdf:resource="http://isdc.gfz-potsdam.de/ontology/SPASE-allowed_values.skos.owl#Observed_Region"/>
    <skos:prefLabel xml:lang="en">Venus</skos:prefLabel>
    <skos:topConceptOf rdf:resource="http://isdc.gfz-potsdam.de/ontology/SPASE-allowed_values.skos.owl#Observatory_Region"/>
    <skos:definition xml:lang="en">The second planet from the sun in our solar system.</skos:definition>
    <skos:inScheme rdf:resource="http://isdc.gfz-potsdam.de/ontology/SPASE-allowed_values.skos.owl#Observatory_Region"/>
    <rdf:type rdf:resource="http://www.w3.org/2002/07/owl#NamedIndividual"/>
    <rdf:type rdf:resource="http://www.w3.org/2004/02/skos/core#Concept"/>
    <skos:topConceptOf rdf:resource="http://isdc.gfz-potsdam.de/ontology/SPASE-allowed_values.skos.owl#Observed_Region"/>
  </rdf:Description>
  <rdf:Description rdf:about="http://isdc.gfz-potsdam.de/ontology/SPASE-allowed_values.skos.owl#Surface">
    <rdf:type rdf:resource="http://www.w3.org/2002/07/owl#NamedIndividual"/>
    <rdf:type rdf:resource="http://www.w3.org/2004/02/skos/core#Concept"/>
    <skos:definition xml:lang="en">The outermost area of a solid object.</skos:definition>
    <skos:broader rdf:resource="http://isdc.gfz-potsdam.de/ontology/SPASE-allowed_values.skos.owl#Earth"/>
    <skos:inScheme rdf:resource="http://isdc.gfz-potsdam.de/ontology/SPASE-allowed_values.skos.owl#Observatory_Region"/>
    <skos:prefLabel xml:lang="en">Surface</skos:prefLabel>
    <skos:inScheme rdf:resource="http://isdc.gfz-potsdam.de/ontology/SPASE-allowed_values.skos.owl#Observed_Region"/>
  </rdf:Description>
  <rdf:Description rdf:about="http://isdc.gfz-potsdam.de/ontology/SPASE-allowed_values.skos.owl#GIF">
    <skos:inScheme rdf:resource="http://isdc.gfz-potsdam.de/ontology/SPASE-allowed_values.skos.owl#Format"/>
    <rdf:type rdf:resource="http://www.w3.org/2002/07/owl#NamedIndividual"/>
    <rdf:type rdf:resource="http://www.w3.org/2004/02/skos/core#Concept"/>
    <skos:topConceptOf rdf:resource="http://isdc.gfz-potsdam.de/ontology/SPASE-allowed_values.skos.owl#Format"/>
    <skos:definition xml:lang="en">Graphic Interchange Format (GIF) first introduced in 1987 by CompuServe. GIF uses LZW
compression and images are limited to 256 colours.</skos:definition>
    <skos:prefLabel xml:lang="en">GIF</skos:prefLabel>
  </rdf:Description>
  <rdf:Description rdf:about="http://isdc.gfz-potsdam.de/ontology/SPASE-allowed_values.skos.owl#Energy_Flux">
    <skos:topConceptOf rdf:resource="http://isdc.gfz-potsdam.de/ontology/SPASE-allowed_values.skos.owl#Wave_Quantity"/>
    <skos:prefLabel xml:lang="en">Energy Flux</skos:prefLabel>
    <rdf:type rdf:resource="http://www.w3.org/2004/02/skos/core#Concept"/>
    <skos:definition xml:lang="en">The amount of energy passing through a unit area in a unit time.</skos:definition>
    <skos:inScheme rdf:resource="http://isdc.gfz-potsdam.de/ontology/SPASE-allowed_values.skos.owl#Wave_Quantity"/>
    <skos:inScheme rdf:resource="http://isdc.gfz-potsdam.de/ontology/SPASE-allowed_values.skos.owl#Particle_Quantity"/>
    <rdf:type rdf:resource="http://www.w3.org/2002/07/owl#NamedIndividual"/>
    <skos:topConceptOf rdf:resource="http://isdc.gfz-potsdam.de/ontology/SPASE-allowed_values.skos.owl#Particle_Quantity"/>
  </rdf:Description>
  <rdf:Description rdf:about="http://isdc.gfz-potsdam.de/ontology/SPASE-allowed_values.skos.owl#Double_Sphere">
    <skos:inScheme rdf:resource="http://isdc.gfz-potsdam.de/ontology/SPASE-allowed_values.skos.owl#Instrument_Type"/>
    <rdf:type rdf:resource="http://www.w3.org/2002/07/owl#NamedIndividual"/>
    <rdf:type rdf:resource="http://www.w3.org/2004/02/skos/core#Concept"/>
    <skos:definition xml:lang="en">A dipole antenna of which the active (sensor) elements are small spheres located at the ends of
two wires deployed in the equatorial plane, on opposite sides of a spinning spacecraft.</skos:definition>
    <skos:topConceptOf rdf:resource="http://isdc.gfz-potsdam.de/ontology/SPASE-allowed_values.skos.owl#Instrument_Type"/>
    <skos:prefLabel xml:lang="en">Double Sphere</skos:prefLabel>
  </rdf:Description>
  <rdf:Description rdf:about="http://isdc.gfz-potsdam.de/ontology/SPASE-allowed_values.skos.owl#HCR">
    <skos:inScheme rdf:resource="http://isdc.gfz-potsdam.de/ontology/SPASE-allowed_values.skos.owl#Coordinate_System_Name"/>
    <skos:prefLabel xml:lang="en">HCR</skos:prefLabel>
    <skos:definition xml:lang="en">Heliocentric Radial - A 3-D orthonormal coordinate system that is primarily intended to specify
with two dimensions a point on the solar disk. The Z axis points toward the observer. The Y
axis lies in the plane defined by the solar spin vector and the Z axis, positive northward. The X
axis is perpendicular to the Y and Z axes, positive toward solar west. Standard representation
for this system is via the point's distance rho from the Z axis [Rho = SQRT(x**2 + y**2)] and
its phase angle psi measured counterclockwise from the +Y axis [psi = arctan (-y/x)].</skos:definition>
    <skos:topConceptOf rdf:resource="http://isdc.gfz-potsdam.de/ontology/SPASE-allowed_values.skos.owl#Coordinate_System_Name"/>
    <rdf:type rdf:resource="http://www.w3.org/2002/07/owl#NamedIndividual"/>
    <rdf:type rdf:resource="http://www.w3.org/2004/02/skos/core#Concept"/>
  </rdf:Description>
  <rdf:Description rdf:about="http://isdc.gfz-potsdam.de/ontology/SPASE-allowed_values.skos.owl#IDFS">
    <skos:definition xml:lang="en">Instrument Data File Set (IDFS) is a set of files written in a prescribed format which contain
data, timing data, and meta-data. IDFS was developed at Southwest Research Institute (SwRI).</skos:definition>
    <rdf:type rdf:resource="http://www.w3.org/2004/02/skos/core#Concept"/>
    <rdf:type rdf:resource="http://www.w3.org/2002/07/owl#NamedIndividual"/>
    <skos:topConceptOf rdf:resource="http://isdc.gfz-potsdam.de/ontology/SPASE-allowed_values.skos.owl#Format"/>
    <skos:prefLabel xml:lang="en">IDFS</skos:prefLabel>
    <skos:inScheme rdf:resource="http://isdc.gfz-potsdam.de/ontology/SPASE-allowed_values.skos.owl#Format"/>
  </rdf:Description>
  <rdf:Description rdf:about="http://isdc.gfz-potsdam.de/ontology/SPASE-allowed_values.skos.owl#Radio_Burst">
    <skos:definition xml:lang="en">Emissions of the sun in radio wavelengths from centimeters to dekameters, under both quiet
and disturbed conditions. Radio Bursts can be "Type I" consisting of many short, narrow-band
bursts in the metric range (300 - 50 MHz).; "Type II" consisting of narrow-band emission that
begins in the meter range (300 MHz) and sweeps slowly (tens of minutes) toward dekameter
wavelengths (10 MHz).; "Type III" consisting of narrow-band bursts that sweep rapidly
(seconds) from decimeter to dekameter wavelengths (500 - 0.5 MHz); and "Type IV" consisting
of a smooth continuum of broad-band bursts primarily in the meter range (300 - 30 MHz).</skos:definition>
    <rdf:type rdf:resource="http://www.w3.org/2004/02/skos/core#Concept"/>
    <rdf:type rdf:resource="http://www.w3.org/2002/07/owl#NamedIndividual"/>
    <skos:inScheme rdf:resource="http://isdc.gfz-potsdam.de/ontology/SPASE-allowed_values.skos.owl#Phenomenon_Type"/>
    <skos:topConceptOf rdf:resource="http://isdc.gfz-potsdam.de/ontology/SPASE-allowed_values.skos.owl#Phenomenon_Type"/>
    <skos:prefLabel xml:lang="en">Radio Burst</skos:prefLabel>
  </rdf:Description>
  <rdf:Description rdf:about="http://isdc.gfz-potsdam.de/ontology/SPASE-allowed_values.skos.owl#Intensity">
    <skos:inScheme rdf:resource="http://isdc.gfz-potsdam.de/ontology/SPASE-allowed_values.skos.owl#Wave_Quantity"/>
    <skos:definition xml:lang="en">The measurement of radiant or wave energy per unit detector area per unit bandwidth per unit
solid angle per unit time.</skos:definition>
    <skos:prefLabel xml:lang="en">Intensity</skos:prefLabel>
    <rdf:type rdf:resource="http://www.w3.org/2002/07/owl#NamedIndividual"/>
    <rdf:type rdf:resource="http://www.w3.org/2004/02/skos/core#Concept"/>
    <skos:topConceptOf rdf:resource="http://isdc.gfz-potsdam.de/ontology/SPASE-allowed_values.skos.owl#Wave_Quantity"/>
  </rdf:Description>
  <rdf:Description rdf:about="http://isdc.gfz-potsdam.de/ontology/SPASE-allowed_values.skos.owl#Publisher">
    <rdf:type rdf:resource="http://www.w3.org/2004/02/skos/core#Concept"/>
    <rdf:type rdf:resource="http://www.w3.org/2002/07/owl#NamedIndividual"/>
    <skos:definition xml:lang="en">An individual, organization, institution or government department responsible for the
production and dissemination of a document.</skos:definition>
    <skos:inScheme rdf:resource="http://isdc.gfz-potsdam.de/ontology/SPASE-allowed_values.skos.owl#Role"/>
    <skos:topConceptOf rdf:resource="http://isdc.gfz-potsdam.de/ontology/SPASE-allowed_values.skos.owl#Role"/>
    <skos:prefLabel xml:lang="en">Publisher</skos:prefLabel>
  </rdf:Description>
  <rdf:Description rdf:about="http://isdc.gfz-potsdam.de/ontology/SPASE-allowed_values.skos.owl#Atomic_Number_Detected">
    <rdf:type rdf:resource="http://www.w3.org/2004/02/skos/core#Concept"/>
    <skos:prefLabel xml:lang="en">Atomic Number Detected</skos:prefLabel>
    <skos:topConceptOf rdf:resource="http://isdc.gfz-potsdam.de/ontology/SPASE-allowed_values.skos.owl#Particle_Quantity"/>
    <skos:definition xml:lang="en">The number of protons in the nucleus of an atom as determined by a detector.</skos:definition>
    <skos:inScheme rdf:resource="http://isdc.gfz-potsdam.de/ontology/SPASE-allowed_values.skos.owl#Particle_Quantity"/>
    <rdf:type rdf:resource="http://www.w3.org/2002/07/owl#NamedIndividual"/>
  </rdf:Description>
  <rdf:Description rdf:about="http://isdc.gfz-potsdam.de/ontology/SPASE-allowed_values.skos.owl#Thumbnail">
    <skos:topConceptOf rdf:resource="http://isdc.gfz-potsdam.de/ontology/SPASE-allowed_values.skos.owl#Source_Type"/>
    <skos:definition xml:lang="en">A small representation of an image which is suitable to infer what the full-sized imaged is like.</skos:definition>
    <rdf:type rdf:resource="http://www.w3.org/2004/02/skos/core#Concept"/>
    <rdf:type rdf:resource="http://www.w3.org/2002/07/owl#NamedIndividual"/>
    <skos:prefLabel xml:lang="en">Thumbnail</skos:prefLabel>
    <skos:inScheme rdf:resource="http://isdc.gfz-potsdam.de/ontology/SPASE-allowed_values.skos.owl#Source_Type"/>
  </rdf:Description>
  <rdf:Description rdf:about="http://isdc.gfz-potsdam.de/ontology/SPASE-allowed_values.skos.owl#Magnetometer">
    <skos:inScheme rdf:resource="http://isdc.gfz-potsdam.de/ontology/SPASE-allowed_values.skos.owl#Instrument_Type"/>
    <rdf:type rdf:resource="http://www.w3.org/2004/02/skos/core#Concept"/>
    <rdf:type rdf:resource="http://www.w3.org/2002/07/owl#NamedIndividual"/>
    <skos:topConceptOf rdf:resource="http://isdc.gfz-potsdam.de/ontology/SPASE-allowed_values.skos.owl#Instrument_Type"/>
    <skos:prefLabel xml:lang="en">Magnetometer</skos:prefLabel>
    <skos:definition xml:lang="en">An instrument which measures the ambient magnetic field.</skos:definition>
  </rdf:Description>
  <rdf:Description rdf:about="http://isdc.gfz-potsdam.de/ontology/SPASE-allowed_values.skos.owl#E-Region">
    <skos:inScheme rdf:resource="http://isdc.gfz-potsdam.de/ontology/SPASE-allowed_values.skos.owl#Observatory_Region"/>
    <rdf:type rdf:resource="http://www.w3.org/2004/02/skos/core#Concept"/>
    <skos:definition xml:lang="en">A layer of ionised gas occurring at 90-150km above the ground. One of several layers in the
ionosphere. Also called the The Kennelly-Heaviside layer.</skos:definition>
    <skos:broader rdf:resource="http://isdc.gfz-potsdam.de/ontology/SPASE-allowed_values.skos.owl#Ionosphere"/>
    <rdf:type rdf:resource="http://www.w3.org/2002/07/owl#NamedIndividual"/>
    <skos:inScheme rdf:resource="http://isdc.gfz-potsdam.de/ontology/SPASE-allowed_values.skos.owl#Observed_Region"/>
    <skos:prefLabel xml:lang="en">E-Region</skos:prefLabel>
  </rdf:Description>
  <rdf:Description rdf:about="http://isdc.gfz-potsdam.de/ontology/SPASE-allowed_values.skos.owl#Spectrogram">
    <rdf:type rdf:resource="http://www.w3.org/2002/07/owl#NamedIndividual"/>
    <skos:definition xml:lang="en">The characterization of signal strengths as a function of frequency (or energy) and time.</skos:definition>
    <skos:prefLabel xml:lang="en">Spectrogram</skos:prefLabel>
    <skos:inScheme rdf:resource="http://isdc.gfz-potsdam.de/ontology/SPASE-allowed_values.skos.owl#Display_Type"/>
    <skos:topConceptOf rdf:resource="http://isdc.gfz-potsdam.de/ontology/SPASE-allowed_values.skos.owl#Display_Type"/>
    <rdf:type rdf:resource="http://www.w3.org/2004/02/skos/core#Concept"/>
  </rdf:Description>
  <rdf:Description rdf:about="http://isdc.gfz-potsdam.de/ontology/SPASE-allowed_values.skos.owl#Instrument_Type">
    <skos:hasTopConcept rdf:resource="http://isdc.gfz-potsdam.de/ontology/SPASE-allowed_values.skos.owl#Antenna"/>
    <skos:hasTopConcept rdf:resource="http://isdc.gfz-potsdam.de/ontology/SPASE-allowed_values.skos.owl#Radar"/>
    <skos:definition xml:lang="en">A characterization of an integrated collection of software and hardware containing one or more
sensors and associated controls used to produce data on an environment.
Allowed Values:
Antenna
Channeltron
Coronograph
Double Sphere
Dust Detector
Electron Drift Instrument
Electrostatic Analyser
Energetic Particle Instrument
Faraday Cup
Flux Feedback
Fourier Transform Spectrograph
Geiger-Mueller Tube
Imager
Imaging Spectrometer
Interferometer
Ion Chamber
Ion Drift
Langmuir Probe
Long Wire
Magnetometer
Mass Spectrometer
Microchannel Plate
Multispectral Imager
Neutral Atom Imager
Neutral Particle Detector
Particle Correlator
Particle Detector
Photometer
Photopolarimeter
Platform
Proportional Counter
Quadrispherical Analyser
Radar
Radiometer
Resonance Sounder
Retarding Potential Analyser
Riometer
Scintillation Detector
Search Coil
Sounder
Spacecraft Potential Control
Spectral Power Receiver
Spectrometer
Time Of Flight
Unspecified
Waveform Receiver</skos:definition>
    <skos:hasTopConcept rdf:resource="http://isdc.gfz-potsdam.de/ontology/SPASE-allowed_values.skos.owl#Ion_Chamber"/>
    <skos:hasTopConcept rdf:resource="http://isdc.gfz-potsdam.de/ontology/SPASE-allowed_values.skos.owl#Waveform_Receiver"/>
    <skos:hasTopConcept rdf:resource="http://isdc.gfz-potsdam.de/ontology/SPASE-allowed_values.skos.owl#Microchannel_Plate"/>
    <skos:hasTopConcept rdf:resource="http://isdc.gfz-potsdam.de/ontology/SPASE-allowed_values.skos.owl#Channeltron"/>
    <skos:hasTopConcept rdf:resource="http://isdc.gfz-potsdam.de/ontology/SPASE-allowed_values.skos.owl#Magnetometer"/>
    <skos:hasTopConcept rdf:resource="http://isdc.gfz-potsdam.de/ontology/SPASE-allowed_values.skos.owl#Spectrometer"/>
    <skos:hasTopConcept rdf:resource="http://isdc.gfz-potsdam.de/ontology/SPASE-allowed_values.skos.owl#Time_Of_Flight"/>
    <skos:hasTopConcept rdf:resource="http://isdc.gfz-potsdam.de/ontology/SPASE-allowed_values.skos.owl#Proportional_Counter"/>
    <skos:hasTopConcept rdf:resource="http://isdc.gfz-potsdam.de/ontology/SPASE-allowed_values.skos.owl#Particle_Correlator"/>
    <skos:hasTopConcept rdf:resource="http://isdc.gfz-potsdam.de/ontology/SPASE-allowed_values.skos.owl#Faraday_Cup"/>
    <skos:hasTopConcept rdf:resource="http://isdc.gfz-potsdam.de/ontology/SPASE-allowed_values.skos.owl#Geiger-Mueller_Tube"/>
    <skos:prefLabel xml:lang="en">Instrument Type</skos:prefLabel>
    <skos:hasTopConcept rdf:resource="http://isdc.gfz-potsdam.de/ontology/SPASE-allowed_values.skos.owl#Electrostatic_Analyser"/>
    <skos:hasTopConcept rdf:resource="http://isdc.gfz-potsdam.de/ontology/SPASE-allowed_values.skos.owl#Multispectral_Imager"/>
    <skos:hasTopConcept rdf:resource="http://isdc.gfz-potsdam.de/ontology/SPASE-allowed_values.skos.owl#Double_Sphere"/>
    <skos:hasTopConcept rdf:resource="http://isdc.gfz-potsdam.de/ontology/SPASE-allowed_values.skos.owl#Neutral_Atom_Imager"/>
    <skos:hasTopConcept rdf:resource="http://isdc.gfz-potsdam.de/ontology/SPASE-allowed_values.skos.owl#Sounder"/>
    <skos:hasTopConcept rdf:resource="http://isdc.gfz-potsdam.de/ontology/SPASE-allowed_values.skos.owl#Long_Wire"/>
    <skos:hasTopConcept rdf:resource="http://isdc.gfz-potsdam.de/ontology/SPASE-allowed_values.skos.owl#Radiometer"/>
    <skos:hasTopConcept rdf:resource="http://isdc.gfz-potsdam.de/ontology/SPASE-allowed_values.skos.owl#Energetic_Particle_Instrument"/>
    <skos:hasTopConcept rdf:resource="http://isdc.gfz-potsdam.de/ontology/SPASE-allowed_values.skos.owl#Interferometer"/>
    <skos:hasTopConcept rdf:resource="http://isdc.gfz-potsdam.de/ontology/SPASE-allowed_values.skos.owl#Photometer"/>
    <skos:hasTopConcept rdf:resource="http://isdc.gfz-potsdam.de/ontology/SPASE-allowed_values.skos.owl#Unspecified"/>
    <skos:hasTopConcept rdf:resource="http://isdc.gfz-potsdam.de/ontology/SPASE-allowed_values.skos.owl#Imager"/>
    <skos:hasTopConcept rdf:resource="http://isdc.gfz-potsdam.de/ontology/SPASE-allowed_values.skos.owl#Ion_Drift"/>
    <skos:hasTopConcept rdf:resource="http://isdc.gfz-potsdam.de/ontology/SPASE-allowed_values.skos.owl#Retarding_Potential_Analyser"/>
    <rdf:type rdf:resource="http://www.w3.org/2004/02/skos/core#ConceptScheme"/>
    <skos:hasTopConcept rdf:resource="http://isdc.gfz-potsdam.de/ontology/SPASE-allowed_values.skos.owl#Photopolarimeter"/>
    <skos:hasTopConcept rdf:resource="http://isdc.gfz-potsdam.de/ontology/SPASE-allowed_values.skos.owl#Coronograph"/>
    <skos:hasTopConcept rdf:resource="http://isdc.gfz-potsdam.de/ontology/SPASE-allowed_values.skos.owl#Langmuir_Probe"/>
    <skos:hasTopConcept rdf:resource="http://isdc.gfz-potsdam.de/ontology/SPASE-allowed_values.skos.owl#Spectral_Power_Receiver"/>
    <skos:hasTopConcept rdf:resource="http://isdc.gfz-potsdam.de/ontology/SPASE-allowed_values.skos.owl#Particle_Detector"/>
    <skos:hasTopConcept rdf:resource="http://isdc.gfz-potsdam.de/ontology/SPASE-allowed_values.skos.owl#Scintillation_Detector"/>
    <skos:hasTopConcept rdf:resource="http://isdc.gfz-potsdam.de/ontology/SPASE-allowed_values.skos.owl#Imaging_Spectrometer"/>
    <skos:hasTopConcept rdf:resource="http://isdc.gfz-potsdam.de/ontology/SPASE-allowed_values.skos.owl#Mass_Spectrometer"/>
    <skos:hasTopConcept rdf:resource="http://isdc.gfz-potsdam.de/ontology/SPASE-allowed_values.skos.owl#Search_Coil"/>
    <skos:hasTopConcept rdf:resource="http://isdc.gfz-potsdam.de/ontology/SPASE-allowed_values.skos.owl#Resonance_Sounder"/>
    <skos:hasTopConcept rdf:resource="http://isdc.gfz-potsdam.de/ontology/SPASE-allowed_values.skos.owl#Quadrispherical_Analyser"/>
    <skos:hasTopConcept rdf:resource="http://isdc.gfz-potsdam.de/ontology/SPASE-allowed_values.skos.owl#Flux_Feedback"/>
    <skos:hasTopConcept rdf:resource="http://isdc.gfz-potsdam.de/ontology/SPASE-allowed_values.skos.owl#Spacecraft_Potential_Control"/>
    <skos:hasTopConcept rdf:resource="http://isdc.gfz-potsdam.de/ontology/SPASE-allowed_values.skos.owl#Fourier_Transform_Spectrograph"/>
    <skos:hasTopConcept rdf:resource="http://isdc.gfz-potsdam.de/ontology/SPASE-allowed_values.skos.owl#Electron_Drift_Instrument"/>
    <skos:hasTopConcept rdf:resource="http://isdc.gfz-potsdam.de/ontology/SPASE-allowed_values.skos.owl#Riometer"/>
    <rdf:type rdf:resource="http://www.w3.org/2002/07/owl#NamedIndividual"/>
    <skos:hasTopConcept rdf:resource="http://isdc.gfz-potsdam.de/ontology/SPASE-allowed_values.skos.owl#Platform"/>
    <skos:hasTopConcept rdf:resource="http://isdc.gfz-potsdam.de/ontology/SPASE-allowed_values.skos.owl#Neutral_Particle_Detector"/>
    <skos:hasTopConcept rdf:resource="http://isdc.gfz-potsdam.de/ontology/SPASE-allowed_values.skos.owl#Dust_Detector"/>
  </rdf:Description>
  <rdf:Description rdf:about="http://isdc.gfz-potsdam.de/ontology/SPASE-allowed_values.skos.owl#Time_Series">
    <skos:topConceptOf rdf:resource="http://isdc.gfz-potsdam.de/ontology/SPASE-allowed_values.skos.owl#Display_Type"/>
    <skos:definition xml:lang="en">A representation of data showing a set of observations taken at different points in time and
charted as a time series.</skos:definition>
    <skos:inScheme rdf:resource="http://isdc.gfz-potsdam.de/ontology/SPASE-allowed_values.skos.owl#Display_Type"/>
    <rdf:type rdf:resource="http://www.w3.org/2004/02/skos/core#Concept"/>
    <rdf:type rdf:resource="http://www.w3.org/2002/07/owl#NamedIndividual"/>
    <skos:prefLabel xml:lang="en">Time Series</skos:prefLabel>
  </rdf:Description>
  <rdf:Description rdf:about="http://isdc.gfz-potsdam.de/ontology/SPASE-allowed_values.skos.owl#Mercury">
    <rdf:type rdf:resource="http://www.w3.org/2004/02/skos/core#Concept"/>
    <skos:inScheme rdf:resource="http://isdc.gfz-potsdam.de/ontology/SPASE-allowed_values.skos.owl#Observed_Region"/>
    <skos:definition xml:lang="en">The first planet from the sun in our solar system.</skos:definition>
    <skos:topConceptOf rdf:resource="http://isdc.gfz-potsdam.de/ontology/SPASE-allowed_values.skos.owl#Observed_Region"/>
    <skos:prefLabel xml:lang="en">Mercury</skos:prefLabel>
    <rdf:type rdf:resource="http://www.w3.org/2002/07/owl#NamedIndividual"/>
    <skos:inScheme rdf:resource="http://isdc.gfz-potsdam.de/ontology/SPASE-allowed_values.skos.owl#Observatory_Region"/>
    <skos:topConceptOf rdf:resource="http://isdc.gfz-potsdam.de/ontology/SPASE-allowed_values.skos.owl#Observatory_Region"/>
  </rdf:Description>
  <rdf:Description rdf:about="http://isdc.gfz-potsdam.de/ontology/SPASE-allowed_values.skos.owl#Infrared">
    <skos:prefLabel xml:lang="en">Infrared</skos:prefLabel>
    <skos:topConceptOf rdf:resource="http://isdc.gfz-potsdam.de/ontology/SPASE-allowed_values.skos.owl#Spectral_Range"/>
    <rdf:type rdf:resource="http://www.w3.org/2004/02/skos/core#Concept"/>
    <rdf:type rdf:resource="http://www.w3.org/2002/07/owl#NamedIndividual"/>
    <skos:inScheme rdf:resource="http://isdc.gfz-potsdam.de/ontology/SPASE-allowed_values.skos.owl#Spectral_Range"/>
    <skos:definition xml:lang="en">Photons with a wavelength range: 760 to 1.00x10^6 nm.</skos:definition>
  </rdf:Description>
  <rdf:Description rdf:about="http://isdc.gfz-potsdam.de/ontology/SPASE-allowed_values.skos.owl#Frequency">
    <rdf:type rdf:resource="http://www.w3.org/2002/07/owl#NamedIndividual"/>
    <skos:topConceptOf rdf:resource="http://isdc.gfz-potsdam.de/ontology/SPASE-allowed_values.skos.owl#Wave_Quantity"/>
    <skos:prefLabel xml:lang="en">Frequency</skos:prefLabel>
    <skos:inScheme rdf:resource="http://isdc.gfz-potsdam.de/ontology/SPASE-allowed_values.skos.owl#Wave_Quantity"/>
    <skos:definition xml:lang="en">The number of occurrences of a repeating event per unit time.</skos:definition>
    <rdf:type rdf:resource="http://www.w3.org/2004/02/skos/core#Concept"/>
  </rdf:Description>
  <rdf:Description rdf:about="http://isdc.gfz-potsdam.de/ontology/SPASE-allowed_values.skos.owl#Photograph">
    <skos:prefLabel xml:lang="en">Photograph</skos:prefLabel>
    <skos:definition xml:lang="en">An image (positive or negative) registered on a piece of photo-sensitive paper.</skos:definition>
    <skos:broader rdf:resource="http://isdc.gfz-potsdam.de/ontology/SPASE-allowed_values.skos.owl#Hardcopy"/>
    <skos:inScheme rdf:resource="http://isdc.gfz-potsdam.de/ontology/SPASE-allowed_values.skos.owl#Format"/>
    <rdf:type rdf:resource="http://www.w3.org/2002/07/owl#NamedIndividual"/>
    <rdf:type rdf:resource="http://www.w3.org/2004/02/skos/core#Concept"/>
  </rdf:Description>
  <rdf:Description rdf:about="http://isdc.gfz-potsdam.de/ontology/SPASE-allowed_values.skos.owl#Average">
    <rdf:type rdf:resource="http://www.w3.org/2004/02/skos/core#Concept"/>
    <rdf:type rdf:resource="http://www.w3.org/2002/07/owl#NamedIndividual"/>
    <skos:definition xml:lang="en">The statistical mean; the sum of a set of values divided by the number of values in the set.</skos:definition>
    <skos:inScheme rdf:resource="http://isdc.gfz-potsdam.de/ontology/SPASE-allowed_values.skos.owl#Qualifier"/>
    <skos:prefLabel xml:lang="en">Average</skos:prefLabel>
    <skos:topConceptOf rdf:resource="http://isdc.gfz-potsdam.de/ontology/SPASE-allowed_values.skos.owl#Qualifier"/>
  </rdf:Description>
  <rdf:Description rdf:about="http://isdc.gfz-potsdam.de/ontology/SPASE-allowed_values.skos.owl#Spectral">
    <skos:prefLabel xml:lang="en">Spectral</skos:prefLabel>
    <skos:inScheme rdf:resource="http://isdc.gfz-potsdam.de/ontology/SPASE-allowed_values.skos.owl#Qualifier"/>
    <rdf:type rdf:resource="http://www.w3.org/2002/07/owl#NamedIndividual"/>
    <rdf:type rdf:resource="http://www.w3.org/2004/02/skos/core#Concept"/>
    <skos:topConceptOf rdf:resource="http://isdc.gfz-potsdam.de/ontology/SPASE-allowed_values.skos.owl#Qualifier"/>
    <skos:definition xml:lang="en">Characterized as a range or continuum of frequencies.</skos:definition>
  </rdf:Description>
  <rdf:Description rdf:about="http://isdc.gfz-potsdam.de/ontology/SPASE-allowed_values.skos.owl#Heliosphere">
    <rdf:type rdf:resource="http://www.w3.org/2002/07/owl#NamedIndividual"/>
    <rdf:type rdf:resource="http://www.w3.org/2004/02/skos/core#Concept"/>
    <skos:topConceptOf rdf:resource="http://isdc.gfz-potsdam.de/ontology/SPASE-allowed_values.skos.owl#Observed_Region"/>
    <skos:narrower rdf:resource="http://isdc.gfz-potsdam.de/ontology/SPASE-allowed_values.skos.owl#Heliosheath"/>
    <skos:narrower rdf:resource="http://isdc.gfz-potsdam.de/ontology/SPASE-allowed_values.skos.owl#Outer"/>
    <skos:inScheme rdf:resource="http://isdc.gfz-potsdam.de/ontology/SPASE-allowed_values.skos.owl#Observed_Region"/>
    <skos:prefLabel xml:lang="en">Heliosphere</skos:prefLabel>
    <skos:narrower rdf:resource="http://isdc.gfz-potsdam.de/ontology/SPASE-allowed_values.skos.owl#Inner"/>
    <skos:narrower rdf:resource="http://isdc.gfz-potsdam.de/ontology/SPASE-allowed_values.skos.owl#Near_Earth"/>
    <skos:topConceptOf rdf:resource="http://isdc.gfz-potsdam.de/ontology/SPASE-allowed_values.skos.owl#Observatory_Region"/>
    <skos:definition xml:lang="en">The solar atmosphere extending roughly from the outer corona to the edge of the solar plasma
at the heliopause separating primarily solar plasma from interstellar plasma.
Allowed Values:
Heliosheath
Inner
Near Earth
Outer
Remote 1AU</skos:definition>
    <skos:narrower rdf:resource="http://isdc.gfz-potsdam.de/ontology/SPASE-allowed_values.skos.owl#Remote_1AU"/>
    <skos:inScheme rdf:resource="http://isdc.gfz-potsdam.de/ontology/SPASE-allowed_values.skos.owl#Observatory_Region"/>
  </rdf:Description>
  <rdf:Description rdf:about="http://isdc.gfz-potsdam.de/ontology/SPASE-allowed_values.skos.owl#MD5">
    <skos:topConceptOf rdf:resource="http://isdc.gfz-potsdam.de/ontology/SPASE-allowed_values.skos.owl#Hash_Function"/>
    <rdf:type rdf:resource="http://www.w3.org/2004/02/skos/core#Concept"/>
    <rdf:type rdf:resource="http://www.w3.org/2002/07/owl#NamedIndividual"/>
    <skos:inScheme rdf:resource="http://isdc.gfz-potsdam.de/ontology/SPASE-allowed_values.skos.owl#Hash_Function"/>
    <skos:prefLabel xml:lang="en">MD5</skos:prefLabel>
    <skos:definition xml:lang="en">Message Digest 5 (MD5) is a 128-bit message digest algorithm created in 1991 by Professor
Ronald Rivest.</skos:definition>
  </rdf:Description>
  <rdf:Description rdf:about="http://isdc.gfz-potsdam.de/ontology/SPASE-allowed_values.skos.owl#Spacecraft_Potential_Control">
    <rdf:type rdf:resource="http://www.w3.org/2004/02/skos/core#Concept"/>
    <skos:topConceptOf rdf:resource="http://isdc.gfz-potsdam.de/ontology/SPASE-allowed_values.skos.owl#Instrument_Type"/>
    <rdf:type rdf:resource="http://www.w3.org/2002/07/owl#NamedIndividual"/>
    <skos:inScheme rdf:resource="http://isdc.gfz-potsdam.de/ontology/SPASE-allowed_values.skos.owl#Instrument_Type"/>
    <skos:prefLabel xml:lang="en">Spacecraft Potential Control</skos:prefLabel>
    <skos:definition xml:lang="en">An instrument to control the electric potential of a spacecraft with respect to the ambient
plasma by emitting a variable current of positive ions.</skos:definition>
  </rdf:Description>
  <rdf:Description rdf:about="http://isdc.gfz-potsdam.de/ontology/SPASE-allowed_values.skos.owl#Current">
    <rdf:type rdf:resource="http://www.w3.org/2002/07/owl#NamedIndividual"/>
    <skos:definition xml:lang="en">The flow of electrons through a conductor caused by a potential difference.</skos:definition>
    <skos:topConceptOf rdf:resource="http://isdc.gfz-potsdam.de/ontology/SPASE-allowed_values.skos.owl#Field_Quantity"/>
    <skos:prefLabel xml:lang="en">Current</skos:prefLabel>
    <skos:inScheme rdf:resource="http://isdc.gfz-potsdam.de/ontology/SPASE-allowed_values.skos.owl#Field_Quantity"/>
    <rdf:type rdf:resource="http://www.w3.org/2004/02/skos/core#Concept"/>
  </rdf:Description>
  <rdf:Description rdf:about="http://isdc.gfz-potsdam.de/ontology/SPASE-allowed_values.skos.owl#Browse">
    <skos:topConceptOf rdf:resource="http://isdc.gfz-potsdam.de/ontology/SPASE-allowed_values.skos.owl#Source_Type"/>
    <rdf:type rdf:resource="http://www.w3.org/2004/02/skos/core#Concept"/>
    <rdf:type rdf:resource="http://www.w3.org/2002/07/owl#NamedIndividual"/>
    <skos:prefLabel xml:lang="en">Browse</skos:prefLabel>
    <skos:inScheme rdf:resource="http://isdc.gfz-potsdam.de/ontology/SPASE-allowed_values.skos.owl#Source_Type"/>
    <skos:definition xml:lang="en">A representation of an image which is suitable to reveal most or all of the details of the image.</skos:definition>
  </rdf:Description>
  <rdf:Description rdf:about="http://isdc.gfz-potsdam.de/ontology/SPASE-allowed_values.skos.owl#Solar_Flare">
    <skos:definition xml:lang="en">An explosive event in the Sun's atmosphere which produces electromagnetic radiation across
the electromagnetic spectrum at multiple wavelengths from long-wave radio to the shortest
wavelength gamma rays.</skos:definition>
    <skos:prefLabel xml:lang="en">Solar Flare</skos:prefLabel>
    <skos:topConceptOf rdf:resource="http://isdc.gfz-potsdam.de/ontology/SPASE-allowed_values.skos.owl#Phenomenon_Type"/>
    <rdf:type rdf:resource="http://www.w3.org/2002/07/owl#NamedIndividual"/>
    <rdf:type rdf:resource="http://www.w3.org/2004/02/skos/core#Concept"/>
    <skos:inScheme rdf:resource="http://isdc.gfz-potsdam.de/ontology/SPASE-allowed_values.skos.owl#Phenomenon_Type"/>
  </rdf:Description>
  <rdf:Description rdf:about="http://isdc.gfz-potsdam.de/ontology/SPASE-allowed_values.skos.owl#Moment">
    <skos:definition xml:lang="en">Parameters determined by integration over a distribution function convolved with a power of
velocity.</skos:definition>
    <skos:topConceptOf rdf:resource="http://isdc.gfz-potsdam.de/ontology/SPASE-allowed_values.skos.owl#Qualifier"/>
    <rdf:type rdf:resource="http://www.w3.org/2004/02/skos/core#Concept"/>
    <rdf:type rdf:resource="http://www.w3.org/2002/07/owl#NamedIndividual"/>
    <skos:prefLabel xml:lang="en">Moment</skos:prefLabel>
    <skos:inScheme rdf:resource="http://isdc.gfz-potsdam.de/ontology/SPASE-allowed_values.skos.owl#Qualifier"/>
  </rdf:Description>
</rdf:RDF>
